
{
    "@context": {
        "unece": "https://service.unece.org/trade/uncefact/vocabulary/unece#",
        "rdf": "http://www.w3.org/1999/02/22-rdf-syntax-ns#",
        "rdfs": "http://www.w3.org/2000/01/rdf-schema#",
        "schema": "http://schema.org/",
        "agriculture": "https://service.unece.org/trade/uncefact/vocabulary/unece/agriculture#",
        "cefact": "https://service.unece.org/trade/uncefact/vocabulary/cefact#",
        "xsd": "http://www.w3.org/2001/XMLSchema#"
    },
    "@graph": [
        {
            "@id": "agriculture:Address",
            "@type": "rdfs:Class",
            "rdfs:comment": "A location, using an unstructured address format, at which a particular organization or person may be found or reached in relation to Sanitary and Phytosanitary (SPS) measures.",
            "rdfs:label": "Address",
            "unece:cefactElementMetadata": [
                {
                    "@id": "cefact:SPS_Address.Details",
                    "@type": "unece:AggregateBIE",
                    "unece:cefactUNId": "UN03000019",
                    "rdfs:comment": "A location, using an unstructured address format, at which a particular organization or person may be found or reached in relation to Sanitary and Phytosanitary (SPS) measures."
                }
            ]
        },
        {
            "@id": "agriculture:AgriculturalApplication",
            "@type": "rdfs:Class",
            "rdfs:comment": "Any substance such as seed, fertilizer, water, gas or chemical applied to an agricultural field, substrate, construction, plant, animal or product.",
            "rdfs:label": "AgriculturalApplication",
            "unece:cefactElementMetadata": [
                {
                    "@id": "cefact:Specified_AgriculturalApplication.Details",
                    "@type": "unece:AggregateBIE",
                    "unece:cefactUNId": "UN01012422",
                    "rdfs:comment": "Any substance such as seed, fertilizer, water, gas or chemical applied to an agricultural field, substrate, construction, plant, animal or product."
                }
            ]
        },
        {
            "@id": "agriculture:AgriculturalDevice",
            "@type": "rdfs:Class",
            "rdfs:comment": "An object specified to be used to perform an agricultural activity.",
            "rdfs:label": "AgriculturalDevice",
            "unece:cefactElementMetadata": [
                {
                    "@id": "cefact:Specified_AgriculturalDevice.Details",
                    "@type": "unece:AggregateBIE",
                    "unece:cefactUNId": "UN01002736",
                    "rdfs:comment": "An object specified to be used to perform an agricultural activity."
                }
            ]
        },
        {
            "@id": "agriculture:AgriculturalProcess",
            "@type": "rdfs:Class",
            "rdfs:comment": [
                "A practice of cultivating land, raising crops, or treatment of the agricultural produce.",
                "A practice of cultivating land, raising crops, and feeding, breeding and raising livestock, that is applied to a plot."
            ],
            "rdfs:label": "AgriculturalProcess",
            "unece:cefactElementMetadata": [
                {
                    "@id": "cefact:Plot_AgriculturalProcess.Details",
                    "@type": "unece:AggregateBIE",
                    "unece:cefactUNId": "UN01002783",
                    "rdfs:comment": "A practice of cultivating land, raising crops, and feeding, breeding and raising livestock, that is applied to a plot."
                },
                {
                    "@id": "cefact:CropProduction_AgriculturalProcess.Details",
                    "@type": "unece:AggregateBIE",
                    "unece:cefactUNId": "UN01012408",
                    "rdfs:comment": "A practice of cultivating land, raising crops, or treatment of the agricultural produce."
                }
            ]
        },
        {
            "@id": "agriculture:AgronomicalObservation",
            "@type": "rdfs:Class",
            "rdfs:comment": "A single collection of diagnostic data, visual or technical, for agronomical purposes.",
            "rdfs:label": "AgronomicalObservation",
            "unece:cefactElementMetadata": [
                {
                    "@id": "cefact:Single_AgronomicalObservation.Details",
                    "@type": "unece:AggregateBIE",
                    "unece:cefactUNId": "UN01009309",
                    "rdfs:comment": "A single collection of diagnostic data, visual or technical, for agronomical purposes."
                }
            ]
        },
        {
            "@id": "agriculture:Analysis",
            "@type": "rdfs:Class",
            "rdfs:comment": "A detailed examination of agricultural elements and structure.",
            "rdfs:label": "Analysis",
            "unece:cefactElementMetadata": [
                {
                    "@id": "cefact:Agricultural_Analysis.Details",
                    "@type": "unece:AggregateBIE",
                    "unece:cefactUNId": "UN01002664",
                    "rdfs:comment": "A detailed examination of agricultural elements and structure."
                }
            ]
        },
        {
            "@id": "agriculture:Animal",
            "@type": "rdfs:Class",
            "rdfs:comment": "A domesticated creature kept or raised on a farm or ranch.",
            "rdfs:label": "Animal",
            "unece:cefactElementMetadata": [
                {
                    "@id": "cefact:Livestock_Animal.Details",
                    "@type": "unece:AggregateBIE",
                    "unece:cefactUNId": "UN01007642",
                    "rdfs:comment": "A domesticated creature kept or raised on a farm or ranch."
                }
            ]
        },
        {
            "@id": "agriculture:Area",
            "@type": "rdfs:Class",
            "rdfs:comment": [
                "A named, delimited and identified part of a land and or water surface of the globe subject to dedicated uniform agricultural treatment.",
                "A part of a land surface used in agriculture."
            ],
            "rdfs:label": "Area",
            "unece:cefactElementMetadata": [
                {
                    "@id": "cefact:Agricultural_Area.Details",
                    "@type": "unece:AggregateBIE",
                    "unece:cefactUNId": "UN01002671",
                    "rdfs:comment": "A part of a land surface used in agriculture."
                },
                {
                    "@id": "cefact:AgriculturalZone_Area.Details",
                    "@type": "unece:AggregateBIE",
                    "unece:cefactUNId": "UN01012213",
                    "rdfs:comment": "A named, delimited and identified part of a land and or water surface of the globe subject to dedicated uniform agricultural treatment."
                }
            ]
        },
        {
            "@id": "agriculture:Authentication",
            "@type": "rdfs:Class",
            "rdfs:comment": "A proof that a Sanitary and Phytosanitary (SPS) certificate document is genuine.",
            "rdfs:label": "Authentication",
            "unece:cefactElementMetadata": [
                {
                    "@id": "cefact:SPS_Authentication.Details",
                    "@type": "unece:AggregateBIE",
                    "unece:cefactUNId": "UN03000033",
                    "rdfs:comment": "A proof that a Sanitary and Phytosanitary (SPS) certificate document is genuine."
                }
            ]
        },
        {
            "@id": "agriculture:Autopsy",
            "@type": "rdfs:Class",
            "rdfs:comment": "Characteristics of a post-mortem examination of an agricultural sample.",
            "rdfs:label": "Autopsy",
            "unece:cefactElementMetadata": [
                {
                    "@id": "cefact:AgriculturalSample_Autopsy.Details",
                    "@type": "unece:AggregateBIE",
                    "unece:cefactUNId": "UN01009572",
                    "rdfs:comment": "Characteristics of a post-mortem examination of an agricultural sample."
                }
            ]
        },
        {
            "@id": "agriculture:Batch",
            "@type": "rdfs:Class",
            "rdfs:comment": [
                "A group of products considered or dealt with together.",
                "A group of crop produce considered or dealt with together.",
                "A group of animals dealt with together.",
                "A group of organic or inorganic substances, applied to soil or a crop to improve crop quality."
            ],
            "rdfs:label": "Batch",
            "unece:cefactElementMetadata": [
                {
                    "@id": "cefact:CropProduce_Batch.Details",
                    "@type": "unece:AggregateBIE",
                    "unece:cefactUNId": "UN01012331",
                    "rdfs:comment": "A group of crop produce considered or dealt with together."
                },
                {
                    "@id": "cefact:CropInput_Batch.Details",
                    "@type": "unece:AggregateBIE",
                    "unece:cefactUNId": "UN01002709",
                    "rdfs:comment": "A group of organic or inorganic substances, applied to soil or a crop to improve crop quality."
                },
                {
                    "@id": "cefact:Product_Batch.Details",
                    "@type": "unece:AggregateBIE",
                    "unece:cefactUNId": "UN01012346",
                    "rdfs:comment": "A group of products considered or dealt with together."
                },
                {
                    "@id": "cefact:Animal_Batch.Details",
                    "@type": "unece:AggregateBIE",
                    "unece:cefactUNId": "UN01011244",
                    "rdfs:comment": "A group of animals dealt with together."
                }
            ]
        },
        {
            "@id": "agriculture:Cargo",
            "@type": "rdfs:Class",
            "rdfs:comment": "Goods being transported that are subject to Sanitary and Phytosanitary (SPS) measures.",
            "rdfs:label": "Cargo",
            "unece:cefactElementMetadata": [
                {
                    "@id": "cefact:SPS_Cargo.Details",
                    "@type": "unece:AggregateBIE",
                    "unece:cefactUNId": "UN03000040",
                    "rdfs:comment": "Goods being transported that are subject to Sanitary and Phytosanitary (SPS) measures."
                }
            ]
        },
        {
            "@id": "agriculture:Certificate",
            "@type": "rdfs:Class",
            "rdfs:comment": [
                "A legal proof of ownership, worthiness or qualification to operate an agricultural item.",
                "A collection of data for a piece of written, printed or electronic matter that provides information or evidence about the identity of an animal or a batch of animals."
            ],
            "rdfs:label": "Certificate",
            "unece:cefactElementMetadata": [
                {
                    "@id": "cefact:Agricultural_Certificate.Details",
                    "@type": "unece:AggregateBIE",
                    "unece:cefactUNId": "UN01012277",
                    "rdfs:comment": "A legal proof of ownership, worthiness or qualification to operate an agricultural item."
                },
                {
                    "@id": "cefact:Animal_Certificate.Details",
                    "@type": "unece:AggregateBIE",
                    "unece:cefactUNId": "UN01011237",
                    "rdfs:comment": "A collection of data for a piece of written, printed or electronic matter that provides information or evidence about the identity of an animal or a batch of animals."
                }
            ]
        },
        {
            "@id": "agriculture:Certification",
            "@type": "rdfs:Class",
            "rdfs:comment": "The process of certifying that a certain animal has met performance and quality assurance requirements, or qualification requirements as stipulated in regulations.",
            "rdfs:label": "Certification",
            "unece:cefactElementMetadata": [
                {
                    "@id": "cefact:Animal_Certification.Details",
                    "@type": "unece:AggregateBIE",
                    "unece:cefactUNId": "UN01013720",
                    "rdfs:comment": "The process of certifying that a certain animal has met performance and quality assurance requirements, or qualification requirements as stipulated in regulations."
                }
            ]
        },
        {
            "@id": "agriculture:Characteristic",
            "@type": "rdfs:Class",
            "rdfs:comment": [
                "A prominent attribute or aspect of Sanitary and Phytosanitary (SPS) measures.",
                "A prominent attribute or aspect of an agricultural object."
            ],
            "rdfs:label": "Characteristic",
            "unece:cefactElementMetadata": [
                {
                    "@id": "cefact:Agricultural_Characteristic.Details",
                    "@type": "unece:AggregateBIE",
                    "unece:cefactUNId": "UN01012359",
                    "rdfs:comment": "A prominent attribute or aspect of an agricultural object."
                },
                {
                    "@id": "cefact:SPSProcess_Characteristic.Details",
                    "@type": "unece:AggregateBIE",
                    "unece:cefactUNId": "UN03000176",
                    "rdfs:comment": "A prominent attribute or aspect of Sanitary and Phytosanitary (SPS) measures."
                }
            ]
        },
        {
            "@id": "agriculture:Chemical",
            "@type": "rdfs:Class",
            "rdfs:comment": [
                "A substance used on a crop, such as a mineral element.",
                "A chemical used as input in an agricultural process."
            ],
            "rdfs:label": "Chemical",
            "unece:cefactElementMetadata": [
                {
                    "@id": "cefact:CropInput_Chemical.Details",
                    "@type": "unece:AggregateBIE",
                    "unece:cefactUNId": "UN01002746",
                    "rdfs:comment": "A substance used on a crop, such as a mineral element."
                },
                {
                    "@id": "cefact:AgriculturalInput_Chemical.Details",
                    "@type": "unece:AggregateBIE",
                    "unece:cefactUNId": "UN01012401",
                    "rdfs:comment": "A chemical used as input in an agricultural process."
                }
            ]
        },
        {
            "@id": "agriculture:Classification",
            "@type": "rdfs:Class",
            "rdfs:comment": [
                "A systematic arrangement of products in classes or categories in relation to Sanitary and Phytosanitary Standards (SPS) measures.",
                "A specified systematic arrangement in classes or categories according to established criteria."
            ],
            "rdfs:label": "Classification",
            "unece:cefactElementMetadata": [
                {
                    "@id": "cefact:SPS_Classification.Details",
                    "@type": "unece:AggregateBIE",
                    "unece:cefactUNId": "UN03000042",
                    "rdfs:comment": "A systematic arrangement of products in classes or categories in relation to Sanitary and Phytosanitary Standards (SPS) measures."
                },
                {
                    "@id": "cefact:Specified_Classification.Details",
                    "@type": "unece:AggregateBIE",
                    "unece:cefactUNId": "UN01007617",
                    "rdfs:comment": "A specified systematic arrangement in classes or categories according to established criteria."
                }
            ]
        },
        {
            "@id": "agriculture:Clause",
            "@type": "rdfs:Class",
            "rdfs:comment": "A distinct article or provision in a Sanitary and Phytosanitary (SPS) certificate document, which requires compliance.",
            "rdfs:label": "Clause",
            "unece:cefactElementMetadata": [
                {
                    "@id": "cefact:SPS_Clause.Details",
                    "@type": "unece:AggregateBIE",
                    "unece:cefactUNId": "UN03000047",
                    "rdfs:comment": "A distinct article or provision in a Sanitary and Phytosanitary (SPS) certificate document, which requires compliance."
                }
            ]
        },
        {
            "@id": "agriculture:Condition",
            "@type": "rdfs:Class",
            "rdfs:comment": "A physical state within which an agricultural process takes place, such as weather conditions.",
            "rdfs:label": "Condition",
            "unece:cefactElementMetadata": [
                {
                    "@id": "cefact:AgriculturalProcess_Condition.Details",
                    "@type": "unece:AggregateBIE",
                    "unece:cefactUNId": "UN01002681",
                    "rdfs:comment": "A physical state within which an agricultural process takes place, such as weather conditions."
                }
            ]
        },
        {
            "@id": "agriculture:Consignment",
            "@type": "rdfs:Class",
            "rdfs:comment": "A separately identifiable collection of goods items subject to Sanitary and Phytosanitary (SPS) measures to be transported from one consignor to one consignee via one or more modes of transport where each consignment is the subject of one single transport contract.",
            "rdfs:label": "Consignment",
            "unece:cefactElementMetadata": [
                {
                    "@id": "cefact:SPS_Consignment.Details",
                    "@type": "unece:AggregateBIE",
                    "unece:cefactUNId": "UN03000053",
                    "rdfs:comment": "A separately identifiable collection of goods items subject to Sanitary and Phytosanitary (SPS) measures to be transported from one consignor to one consignee via one or more modes of transport where each consignment is the subject of one single transport contract."
                }
            ]
        },
        {
            "@id": "agriculture:ConsignmentItem",
            "@type": "rdfs:Class",
            "rdfs:comment": "An item within a consignment of goods subject to Sanitary and Phytosanitary (SPS) measures that is separately identified for transport and customs purposes.",
            "rdfs:label": "ConsignmentItem",
            "unece:cefactElementMetadata": [
                {
                    "@id": "cefact:SPS_ConsignmentItem.Details",
                    "@type": "unece:AggregateBIE",
                    "unece:cefactUNId": "UN03000050",
                    "rdfs:comment": "An item within a consignment of goods subject to Sanitary and Phytosanitary (SPS) measures that is separately identified for transport and customs purposes."
                }
            ]
        },
        {
            "@id": "agriculture:Construction",
            "@type": "rdfs:Class",
            "rdfs:comment": "A man made agricultural physical structure, such as a building, greenhouse, installation, storage.",
            "rdfs:label": "Construction",
            "unece:cefactElementMetadata": [
                {
                    "@id": "cefact:Agricultural_Construction.Details",
                    "@type": "unece:AggregateBIE",
                    "unece:cefactUNId": "UN01012225",
                    "rdfs:comment": "A man made agricultural physical structure, such as a building, greenhouse, installation, storage."
                }
            ]
        },
        {
            "@id": "agriculture:Contact",
            "@type": "rdfs:Class",
            "rdfs:comment": "A person or department involved in Sanitary and Phytosanitary (SPS) measures that acts as a point of contact with another person or department.",
            "rdfs:label": "Contact",
            "unece:cefactElementMetadata": [
                {
                    "@id": "cefact:SPS_Contact.Details",
                    "@type": "unece:AggregateBIE",
                    "unece:cefactUNId": "UN03000077",
                    "rdfs:comment": "A person or department involved in Sanitary and Phytosanitary (SPS) measures that acts as a point of contact with another person or department."
                }
            ]
        },
        {
            "@id": "agriculture:Contract",
            "@type": "rdfs:Class",
            "rdfs:comment": [
                "The written or spoken contract between two or more parties for the expressed purpose of specifying the required agricultural produce, products or services.",
                "An agreement between a farm and its trading partner specifying a use of soil."
            ],
            "rdfs:label": "Contract",
            "unece:cefactElementMetadata": [
                {
                    "@id": "cefact:SoilOccupation_Contract.Details",
                    "@type": "unece:AggregateBIE",
                    "unece:cefactUNId": "UN01002821",
                    "rdfs:comment": "An agreement between a farm and its trading partner specifying a use of soil."
                },
                {
                    "@id": "cefact:Agricultural_Contract.Details",
                    "@type": "unece:AggregateBIE",
                    "unece:cefactUNId": "UN01012444",
                    "rdfs:comment": "The written or spoken contract between two or more parties for the expressed purpose of specifying the required agricultural produce, products or services."
                }
            ]
        },
        {
            "@id": "agriculture:CoordinateReferenceSystem",
            "@type": "rdfs:Class",
            "rdfs:comment": "A coordinate reference system that is used in a contextually local sense to describe the relative locations of objects in which coordinates of points are recorded in a Coordinate System (CS) (reference ISO 19111).",
            "rdfs:label": "CoordinateReferenceSystem",
            "unece:cefactElementMetadata": [
                {
                    "@id": "cefact:CSEngineering_CoordinateReferenceSystem.Details",
                    "@type": "unece:AggregateBIE",
                    "unece:cefactUNId": "UN01012162",
                    "rdfs:comment": "A coordinate reference system that is used in a contextually local sense to describe the relative locations of objects in which coordinates of points are recorded in a Coordinate System (CS) (reference ISO 19111)."
                }
            ]
        },
        {
            "@id": "agriculture:Country",
            "@type": "rdfs:Class",
            "rdfs:comment": [
                "A country that is referenced.",
                "The area of land that belongs to a nation together with its properties, such as population, political organization, etc. relevant to Sanitary and Phytosanitary (SPS) measures."
            ],
            "rdfs:label": "Country",
            "unece:cefactElementMetadata": [
                {
                    "@id": "cefact:SPS_Country.Details",
                    "@type": "unece:AggregateBIE",
                    "unece:cefactUNId": "UN03000087",
                    "rdfs:comment": "The area of land that belongs to a nation together with its properties, such as population, political organization, etc. relevant to Sanitary and Phytosanitary (SPS) measures."
                },
                {
                    "@id": "cefact:Referenced_Country.Details",
                    "@type": "unece:AggregateBIE",
                    "unece:cefactUNId": "UN01007614",
                    "rdfs:comment": "A country that is referenced."
                }
            ]
        },
        {
            "@id": "agriculture:CountrySubDivision",
            "@type": "rdfs:Class",
            "rdfs:comment": [
                "A political or physical area or region within the political boundaries of a country relevant to Sanitary and Phytosanitary (SPS) measures.",
                "An area of land within a country which has specific agricultural characteristics."
            ],
            "rdfs:label": "CountrySubDivision",
            "unece:cefactElementMetadata": [
                {
                    "@id": "cefact:Agricultural_CountrySub-Division.Details",
                    "@type": "unece:AggregateBIE",
                    "unece:cefactUNId": "UN01002776",
                    "rdfs:comment": "An area of land within a country which has specific agricultural characteristics."
                },
                {
                    "@id": "cefact:SPS_CountrySub-Division.Details",
                    "@type": "unece:AggregateBIE",
                    "unece:cefactUNId": "UN03000079",
                    "rdfs:comment": "A political or physical area or region within the political boundaries of a country relevant to Sanitary and Phytosanitary (SPS) measures."
                }
            ]
        },
        {
            "@id": "agriculture:Crop",
            "@type": "rdfs:Class",
            "rdfs:comment": [
                "Plants or produce cultivated from a single botanical species or variety.",
                "The produce from agriculturally cultivated plants.",
                "A field with one or more cultivated plants or produce from one or more botanical species or varieties."
            ],
            "rdfs:label": "Crop",
            "unece:cefactElementMetadata": [
                {
                    "@id": "cefact:Agricultural_Crop.Details",
                    "@type": "unece:AggregateBIE",
                    "unece:cefactUNId": "UN01002685",
                    "rdfs:comment": "The produce from agriculturally cultivated plants."
                },
                {
                    "@id": "cefact:Botanical_Crop.Details",
                    "@type": "unece:AggregateBIE",
                    "unece:cefactUNId": "UN01012289",
                    "rdfs:comment": "Plants or produce cultivated from a single botanical species or variety."
                },
                {
                    "@id": "cefact:Field_Crop.Details",
                    "@type": "unece:AggregateBIE",
                    "unece:cefactUNId": "UN01012296",
                    "rdfs:comment": "A field with one or more cultivated plants or produce from one or more botanical species or varieties."
                }
            ]
        },
        {
            "@id": "agriculture:CropInput",
            "@type": "rdfs:Class",
            "rdfs:comment": "An organic or inorganic substance supporting an agricultural process, applied to soil or crop to improve crop quality.",
            "rdfs:label": "CropInput",
            "unece:cefactElementMetadata": [
                {
                    "@id": "cefact:AgriculturalProcess_CropInput.Details",
                    "@type": "unece:AggregateBIE",
                    "unece:cefactUNId": "UN01002723",
                    "rdfs:comment": "An organic or inorganic substance supporting an agricultural process, applied to soil or crop to improve crop quality."
                }
            ]
        },
        {
            "@id": "agriculture:CropMixtureConstituent",
            "@type": "rdfs:Class",
            "rdfs:comment": "A plant species or variety constituting part of a field crop mixture.",
            "rdfs:label": "CropMixtureConstituent",
            "unece:cefactElementMetadata": [
                {
                    "@id": "cefact:Field_CropMixtureConstituent.Details",
                    "@type": "unece:AggregateBIE",
                    "unece:cefactUNId": "UN01012321",
                    "rdfs:comment": "A plant species or variety constituting part of a field crop mixture."
                }
            ]
        },
        {
            "@id": "agriculture:CropProductionCycle",
            "@type": "rdfs:Class",
            "rdfs:comment": "A series of agricultural events in the production of a crop.",
            "rdfs:label": "CropProductionCycle",
            "unece:cefactElementMetadata": [
                {
                    "@id": "cefact:Agricultural_CropProductionCycle.Details",
                    "@type": "unece:AggregateBIE",
                    "unece:cefactUNId": "UN01002762",
                    "rdfs:comment": "A series of agricultural events in the production of a crop."
                }
            ]
        },
        {
            "@id": "agriculture:CropProtectionTreatment",
            "@type": "rdfs:Class",
            "rdfs:comment": "A method or substance, such as chemical fertilizers and crop protection products, applied to plant growth whilst managing and controlling diseases and pests.",
            "rdfs:label": "CropProtectionTreatment",
            "unece:cefactElementMetadata": [
                {
                    "@id": "cefact:Specified_CropProtectionTreatment.Details",
                    "@type": "unece:AggregateBIE",
                    "unece:cefactUNId": "UN01014285",
                    "rdfs:comment": "A method or substance, such as chemical fertilizers and crop protection products, applied to plant growth whilst managing and controlling diseases and pests."
                }
            ]
        },
        {
            "@id": "agriculture:CropResidue",
            "@type": "rdfs:Class",
            "rdfs:comment": "The material from soil occupation that is left after a crop has been harvested or processed.",
            "rdfs:label": "CropResidue",
            "unece:cefactElementMetadata": [
                {
                    "@id": "cefact:SoilOccupation_CropResidue.Details",
                    "@type": "unece:AggregateBIE",
                    "unece:cefactUNId": "UN01002692",
                    "rdfs:comment": "The material from soil occupation that is left after a crop has been harvested or processed."
                }
            ]
        },
        {
            "@id": "agriculture:CropStage",
            "@type": "rdfs:Class",
            "rdfs:comment": "A point or step in a process or development of a crop in an agricultural process.",
            "rdfs:label": "CropStage",
            "unece:cefactElementMetadata": [
                {
                    "@id": "cefact:AgriculturalProcess_CropStage.Details",
                    "@type": "unece:AggregateBIE",
                    "unece:cefactUNId": "UN01002695",
                    "rdfs:comment": "A point or step in a process or development of a crop in an agricultural process."
                }
            ]
        },
        {
            "@id": "agriculture:DirectPositionList",
            "@type": "rdfs:Class",
            "rdfs:comment": "The specified list of coordinates for a physical location, expressed as a sequence of direct positions.",
            "rdfs:label": "DirectPositionList",
            "unece:cefactElementMetadata": [
                {
                    "@id": "cefact:Specified_DirectPositionList.Details",
                    "@type": "unece:AggregateBIE",
                    "unece:cefactUNId": "UN01012471",
                    "rdfs:comment": "The specified list of coordinates for a physical location, expressed as a sequence of direct positions."
                }
            ]
        },
        {
            "@id": "agriculture:Document",
            "@type": "rdfs:Class",
            "rdfs:comment": [
                "A reference to a collection of data for a piece of written, printed or electronic matter that provides information or evidence about Sanitary and Phytosanitary (SPS) measures.",
                "A detailed description of a crop, used for administrative or traceability purposes.",
                "A collection of data for a piece of written, printed or electronic matter that is exchanged between two or more parties for crop reporting purposes.",
                "A collection of data for a piece of written, printed or electronic matter that provides information or evidence of the transfer of agronomical data from the field to one or more parties, such as to set up a network of epidemiological monitoring of crops.",
                "A collection of data for a piece of written, printed or electronic matter that is exchanged between two or more parties pertaining to Sanitary and Phytosanitary (SPS) measures.",
                "A collection of data for a piece of written, printed or electronic matter that is exchanged between two or more parties in a Livestock Animal (LA) document exchange.",
                "A collection of data for a piece of written, printed or electronic matter that is exchanged between two or more parties in a Sanitary and Phytosanitary (SPS) certificate document exchange.",
                "A collection of data for a piece of written, printed or electronic matter that provides information or evidence about the identity of an animal for domestic or cross border movement purposes."
            ],
            "rdfs:label": "Document",
            "unece:cefactElementMetadata": [
                {
                    "@id": "cefact:SPSAcknowledgement_Document.Details",
                    "@type": "unece:AggregateBIE",
                    "unece:cefactUNId": "UN03000182",
                    "rdfs:comment": "A collection of data for a piece of written, printed or electronic matter that is exchanged between two or more parties pertaining to Sanitary and Phytosanitary (SPS) measures."
                },
                {
                    "@id": "cefact:SPSReferenced_Document.Details",
                    "@type": "unece:AggregateBIE",
                    "unece:cefactUNId": "UN03000014",
                    "rdfs:comment": "A reference to a collection of data for a piece of written, printed or electronic matter that provides information or evidence about Sanitary and Phytosanitary (SPS) measures."
                },
                {
                    "@id": "cefact:SPSExchanged_Document.Details",
                    "@type": "unece:AggregateBIE",
                    "unece:cefactUNId": "UN03000001",
                    "rdfs:comment": "A collection of data for a piece of written, printed or electronic matter that is exchanged between two or more parties in a Sanitary and Phytosanitary (SPS) certificate document exchange."
                },
                {
                    "@id": "cefact:CropReport_Document.Details",
                    "@type": "unece:AggregateBIE",
                    "unece:cefactUNId": "UN01012429",
                    "rdfs:comment": "A collection of data for a piece of written, printed or electronic matter that is exchanged between two or more parties for crop reporting purposes."
                },
                {
                    "@id": "cefact:AgronomicalObservation_Document.Details",
                    "@type": "unece:AggregateBIE",
                    "unece:cefactUNId": "UN01009294",
                    "rdfs:comment": "A collection of data for a piece of written, printed or electronic matter that provides information or evidence of the transfer of agronomical data from the field to one or more parties, such as to set up a network of epidemiological monitoring of crops."
                },
                {
                    "@id": "cefact:CropDataSheet_Document.Details",
                    "@type": "unece:AggregateBIE",
                    "unece:cefactUNId": "UN01002813",
                    "rdfs:comment": "A detailed description of a crop, used for administrative or traceability purposes."
                },
                {
                    "@id": "cefact:AnimalPassport_Document.Details",
                    "@type": "unece:AggregateBIE",
                    "unece:cefactUNId": "UN01007670",
                    "rdfs:comment": "A collection of data for a piece of written, printed or electronic matter that provides information or evidence about the identity of an animal for domestic or cross border movement purposes."
                },
                {
                    "@id": "cefact:LAExchanged_Document.Details",
                    "@type": "unece:AggregateBIE",
                    "unece:cefactUNId": "UN01007697",
                    "rdfs:comment": "A collection of data for a piece of written, printed or electronic matter that is exchanged between two or more parties in a Livestock Animal (LA) document exchange."
                }
            ]
        },
        {
            "@id": "agriculture:Event",
            "@type": "rdfs:Class",
            "rdfs:comment": [
                "A conveyance of an animal or animals from place to place.",
                "A conveyance of an animal or animals from country to country.",
                "A veterinarian occurrence, such as the treatment of an animal or an inspection.",
                "A significant occurrence or happening relevant to Sanitary and Phytosanitary (SPS) measures.",
                "The keeping of an animal in a particular location."
            ],
            "rdfs:label": "Event",
            "unece:cefactElementMetadata": [
                {
                    "@id": "cefact:AnimalMovement_Event.Details",
                    "@type": "unece:AggregateBIE",
                    "unece:cefactUNId": "UN01007638",
                    "rdfs:comment": "A conveyance of an animal or animals from place to place."
                },
                {
                    "@id": "cefact:CrossBorderAnimalMovement_Event.Details",
                    "@type": "unece:AggregateBIE",
                    "unece:cefactUNId": "UN01007660",
                    "rdfs:comment": "A conveyance of an animal or animals from country to country."
                },
                {
                    "@id": "cefact:Veterinarian_Event.Details",
                    "@type": "unece:AggregateBIE",
                    "unece:cefactUNId": "UN01007631",
                    "rdfs:comment": "A veterinarian occurrence, such as the treatment of an animal or an inspection."
                },
                {
                    "@id": "cefact:AnimalHolding_Event.Details",
                    "@type": "unece:AggregateBIE",
                    "unece:cefactUNId": "UN01007634",
                    "rdfs:comment": "The keeping of an animal in a particular location."
                },
                {
                    "@id": "cefact:SPS_Event.Details",
                    "@type": "unece:AggregateBIE",
                    "unece:cefactUNId": "UN03000091",
                    "rdfs:comment": "A significant occurrence or happening relevant to Sanitary and Phytosanitary (SPS) measures."
                }
            ]
        },
        {
            "@id": "agriculture:ExaminationResult",
            "@type": "rdfs:Class",
            "rdfs:comment": "Results obtained from the process of performing an in-depth assessment or test on an animal.",
            "rdfs:label": "ExaminationResult",
            "unece:cefactElementMetadata": [
                {
                    "@id": "cefact:Animal_ExaminationResult.Details",
                    "@type": "unece:AggregateBIE",
                    "unece:cefactUNId": "UN01007681",
                    "rdfs:comment": "Results obtained from the process of performing an in-depth assessment or test on an animal."
                }
            ]
        },
        {
            "@id": "agriculture:GeographicalFeature",
            "@type": "rdfs:Class",
            "rdfs:comment": "Representation of real world phenomenon associated with a location relative to the Earth, such as cities, buildings, roads, rivers, forests and lakes.",
            "rdfs:label": "GeographicalFeature",
            "unece:cefactElementMetadata": [
                {
                    "@id": "cefact:Specified_GeographicalFeature.Details",
                    "@type": "unece:AggregateBIE",
                    "unece:cefactUNId": "UN01012168",
                    "rdfs:comment": "Representation of real world phenomenon associated with a location relative to the Earth, such as cities, buildings, roads, rivers, forests and lakes."
                }
            ]
        },
        {
            "@id": "agriculture:GeographicalGrid",
            "@type": "rdfs:Class",
            "rdfs:comment": "The combination of the latitude and longitude forming a graticule, used for specifying the position of any location on the surface of the Earth, without consideration of altitude or depth (reference ISO 19136).",
            "rdfs:label": "GeographicalGrid",
            "unece:cefactElementMetadata": [
                {
                    "@id": "cefact:Specified_GeographicalGrid.Details",
                    "@type": "unece:AggregateBIE",
                    "unece:cefactUNId": "UN01012202",
                    "rdfs:comment": "The combination of the latitude and longitude forming a graticule, used for specifying the position of any location on the surface of the Earth, without consideration of altitude or depth (reference ISO 19136)."
                }
            ]
        },
        {
            "@id": "agriculture:GeographicalLine",
            "@type": "rdfs:Class",
            "rdfs:comment": "A connection between two points on the surface of the Earth (reference ISO 19136).",
            "rdfs:label": "GeographicalLine",
            "unece:cefactElementMetadata": [
                {
                    "@id": "cefact:Specified_GeographicalLine.Details",
                    "@type": "unece:AggregateBIE",
                    "unece:cefactUNId": "UN01012187",
                    "rdfs:comment": "A connection between two points on the surface of the Earth (reference ISO 19136)."
                }
            ]
        },
        {
            "@id": "agriculture:GeographicalMultiCurve",
            "@type": "rdfs:Class",
            "rdfs:comment": "A collection of curves on the surface of the Earth (reference ISO 19136).",
            "rdfs:label": "GeographicalMultiCurve",
            "unece:cefactElementMetadata": [
                {
                    "@id": "cefact:Specified_GeographicalMulti-Curve.Details",
                    "@type": "unece:AggregateBIE",
                    "unece:cefactUNId": "UN01012190",
                    "rdfs:comment": "A collection of curves on the surface of the Earth (reference ISO 19136)."
                }
            ]
        },
        {
            "@id": "agriculture:GeographicalMultiPoint",
            "@type": "rdfs:Class",
            "rdfs:comment": "A collection of points, on the surface of the Earth (reference ISO 19136).",
            "rdfs:label": "GeographicalMultiPoint",
            "unece:cefactElementMetadata": [
                {
                    "@id": "cefact:Specified_GeographicalMulti-Point.Details",
                    "@type": "unece:AggregateBIE",
                    "unece:cefactUNId": "UN01012183",
                    "rdfs:comment": "A collection of points, on the surface of the Earth (reference ISO 19136)."
                }
            ]
        },
        {
            "@id": "agriculture:GeographicalMultiSurface",
            "@type": "rdfs:Class",
            "rdfs:comment": "A collection of surfaces on the Earth (reference ISO 19136).",
            "rdfs:label": "GeographicalMultiSurface",
            "unece:cefactElementMetadata": [
                {
                    "@id": "cefact:Specified_GeographicalMulti-Surface.Details",
                    "@type": "unece:AggregateBIE",
                    "unece:cefactUNId": "UN01012196",
                    "rdfs:comment": "A collection of surfaces on the Earth (reference ISO 19136)."
                }
            ]
        },
        {
            "@id": "agriculture:GeographicalObjectCharacteristic",
            "@type": "rdfs:Class",
            "rdfs:comment": "An attribute of a geographical object.",
            "rdfs:label": "GeographicalObjectCharacteristic",
            "unece:cefactElementMetadata": [
                {
                    "@id": "cefact:Specified_GeographicalObjectCharacteristic.Details",
                    "@type": "unece:AggregateBIE",
                    "unece:cefactUNId": "UN01012368",
                    "rdfs:comment": "An attribute of a geographical object."
                }
            ]
        },
        {
            "@id": "agriculture:GeographicalPoint",
            "@type": "rdfs:Class",
            "rdfs:comment": "A point on the surface of the Earth (reference ISO 19136).",
            "rdfs:label": "GeographicalPoint",
            "unece:cefactElementMetadata": [
                {
                    "@id": "cefact:Specified_GeographicalPoint.Details",
                    "@type": "unece:AggregateBIE",
                    "unece:cefactUNId": "UN01012180",
                    "rdfs:comment": "A point on the surface of the Earth (reference ISO 19136)."
                }
            ]
        },
        {
            "@id": "agriculture:GeographicalSurface",
            "@type": "rdfs:Class",
            "rdfs:comment": "A figure on the Earth having only two dimensions (reference ISO 19136).",
            "rdfs:label": "GeographicalSurface",
            "unece:cefactElementMetadata": [
                {
                    "@id": "cefact:Specified_GeographicalSurface.Details",
                    "@type": "unece:AggregateBIE",
                    "unece:cefactUNId": "UN01012199",
                    "rdfs:comment": "A figure on the Earth having only two dimensions (reference ISO 19136)."
                }
            ]
        },
        {
            "@id": "agriculture:Grant",
            "@type": "rdfs:Class",
            "rdfs:comment": "An allocation of funds for an animal related purpose.",
            "rdfs:label": "Grant",
            "unece:cefactElementMetadata": [
                {
                    "@id": "cefact:Animal_Grant.Details",
                    "@type": "unece:AggregateBIE",
                    "unece:cefactUNId": "UN01007676",
                    "rdfs:comment": "An allocation of funds for an animal related purpose."
                }
            ]
        },
        {
            "@id": "agriculture:Identity",
            "@type": "rdfs:Class",
            "rdfs:comment": "Information about an animal which uniquely identifies it.",
            "rdfs:label": "Identity",
            "unece:cefactElementMetadata": [
                {
                    "@id": "cefact:Animal_Identity.Details",
                    "@type": "unece:AggregateBIE",
                    "unece:cefactUNId": "UN01007624",
                    "rdfs:comment": "Information about an animal which uniquely identifies it."
                }
            ]
        },
        {
            "@id": "agriculture:Inspection",
            "@type": "rdfs:Class",
            "rdfs:comment": "The process of performing documented checks, with a focus on spotting deviations, such as illnesses, related to animals.",
            "rdfs:label": "Inspection",
            "unece:cefactElementMetadata": [
                {
                    "@id": "cefact:Animal_Inspection.Details",
                    "@type": "unece:AggregateBIE",
                    "unece:cefactUNId": "UN01007692",
                    "rdfs:comment": "The process of performing documented checks, with a focus on spotting deviations, such as illnesses, related to animals."
                }
            ]
        },
        {
            "@id": "agriculture:Issue",
            "@type": "rdfs:Class",
            "rdfs:comment": [
                "A topic for debate or resolution arising from cross border animal movement.",
                "A topic for debate or resolution, expressed as a dissatisfaction."
            ],
            "rdfs:label": "Issue",
            "unece:cefactElementMetadata": [
                {
                    "@id": "cefact:CrossBorderAnimalMovement_Issue.Details",
                    "@type": "unece:AggregateBIE",
                    "unece:cefactUNId": "UN01007667",
                    "rdfs:comment": "A topic for debate or resolution arising from cross border animal movement."
                },
                {
                    "@id": "cefact:Complaint_Issue.Details",
                    "@type": "unece:AggregateBIE",
                    "unece:cefactUNId": "UN01012266",
                    "rdfs:comment": "A topic for debate or resolution, expressed as a dissatisfaction."
                }
            ]
        },
        {
            "@id": "agriculture:Label",
            "@type": "rdfs:Class",
            "rdfs:comment": "Information about an attachment to an animal which uniquely identifies the animal.",
            "rdfs:label": "Label",
            "unece:cefactElementMetadata": [
                {
                    "@id": "cefact:Animal_Label.Details",
                    "@type": "unece:AggregateBIE",
                    "unece:cefactUNId": "UN01007621",
                    "rdfs:comment": "Information about an attachment to an animal which uniquely identifies the animal."
                }
            ]
        },
        {
            "@id": "agriculture:Location",
            "@type": "rdfs:Class",
            "rdfs:comment": "A physical location or place relevant to Sanitary and Phytosanitary (SPS) measures.",
            "rdfs:label": "Location",
            "unece:cefactElementMetadata": [
                {
                    "@id": "cefact:SPS_Location.Details",
                    "@type": "unece:AggregateBIE",
                    "unece:cefactUNId": "UN03000093",
                    "rdfs:comment": "A physical location or place relevant to Sanitary and Phytosanitary (SPS) measures."
                }
            ]
        },
        {
            "@id": "agriculture:ManMachineSystem",
            "@type": "rdfs:Class",
            "rdfs:comment": "A combination of man and farm machinery which can be combined and operated as one independently controllable unit to perform an agricultural process.",
            "rdfs:label": "ManMachineSystem",
            "unece:cefactElementMetadata": [
                {
                    "@id": "cefact:Agricultural_ManMachineSystem.Details",
                    "@type": "unece:AggregateBIE",
                    "unece:cefactUNId": "UN01012457",
                    "rdfs:comment": "A combination of man and farm machinery which can be combined and operated as one independently controllable unit to perform an agricultural process."
                }
            ]
        },
        {
            "@id": "agriculture:Material",
            "@type": "rdfs:Class",
            "rdfs:comment": "A substance out of which something is or could be made to be used as agricultural input.",
            "rdfs:label": "Material",
            "unece:cefactElementMetadata": [
                {
                    "@id": "cefact:AgriculturalInput_Material.Details",
                    "@type": "unece:AggregateBIE",
                    "unece:cefactUNId": "UN01012386",
                    "rdfs:comment": "A substance out of which something is or could be made to be used as agricultural input."
                }
            ]
        },
        {
            "@id": "agriculture:Note",
            "@type": "rdfs:Class",
            "rdfs:comment": [
                "A textual or coded description, such as a remark or additional information relevant to Sanitary and Phytosanitary (SPS) measures.",
                "A basic textual or coded description, such as a remark or additional information."
            ],
            "rdfs:label": "Note",
            "unece:cefactElementMetadata": [
                {
                    "@id": "cefact:Basic_Note.Details",
                    "@type": "unece:AggregateBIE",
                    "unece:cefactUNId": "UN01007714",
                    "rdfs:comment": "A basic textual or coded description, such as a remark or additional information."
                },
                {
                    "@id": "cefact:SPS_Note.Details",
                    "@type": "unece:AggregateBIE",
                    "unece:cefactUNId": "UN03000096",
                    "rdfs:comment": "A textual or coded description, such as a remark or additional information relevant to Sanitary and Phytosanitary (SPS) measures."
                }
            ]
        },
        {
            "@id": "agriculture:ObservationResult",
            "@type": "rdfs:Class",
            "rdfs:comment": "A reference to a collection of diagnostic data, visual or technical, and processing data, performed on a sample by a laboratory.",
            "rdfs:label": "ObservationResult",
            "unece:cefactElementMetadata": [
                {
                    "@id": "cefact:Referenced_ObservationResult.Details",
                    "@type": "unece:AggregateBIE",
                    "unece:cefactUNId": "UN01012454",
                    "rdfs:comment": "A reference to a collection of diagnostic data, visual or technical, and processing data, performed on a sample by a laboratory."
                }
            ]
        },
        {
            "@id": "agriculture:Package",
            "@type": "rdfs:Class",
            "rdfs:comment": "Any self-contained wrapping or container within which goods that are subject to Sanitary and Phytosanitary (SPS) measures can be contained, such as a box or a barrel which can be filled, partially filled or empty.",
            "rdfs:label": "Package",
            "unece:cefactElementMetadata": [
                {
                    "@id": "cefact:SPS_Package.Details",
                    "@type": "unece:AggregateBIE",
                    "unece:cefactUNId": "UN03000104",
                    "rdfs:comment": "Any self-contained wrapping or container within which goods that are subject to Sanitary and Phytosanitary (SPS) measures can be contained, such as a box or a barrel which can be filled, partially filled or empty."
                }
            ]
        },
        {
            "@id": "agriculture:Party",
            "@type": "rdfs:Class",
            "rdfs:comment": [
                "An individual, a group, or a body having a role in the production of crops such as vegetables, flowers, plants.",
                "A reference to an individual, a group, or a body having a role in Sanitary and Phytosanitary (SPS) measures.",
                "A specified individual, group, or body having a role in a business function.",
                "An individual, a group, or a body referenced on an agronomical observation report document.",
                "An individual, a group, or a body referenced on a crop data sheet."
            ],
            "rdfs:label": "Party",
            "unece:cefactElementMetadata": [
                {
                    "@id": "cefact:AgronomicalObservation_Party.Details",
                    "@type": "unece:AggregateBIE",
                    "unece:cefactUNId": "UN01009301",
                    "rdfs:comment": "An individual, a group, or a body referenced on an agronomical observation report document."
                },
                {
                    "@id": "cefact:Specified_Party.Details",
                    "@type": "unece:AggregateBIE",
                    "unece:cefactUNId": "UN01007608",
                    "rdfs:comment": "A specified individual, group, or body having a role in a business function."
                },
                {
                    "@id": "cefact:CropDataSheet_Party.Details",
                    "@type": "unece:AggregateBIE",
                    "unece:cefactUNId": "UN01002807",
                    "rdfs:comment": "An individual, a group, or a body referenced on a crop data sheet."
                },
                {
                    "@id": "cefact:AgriculturalProducer_Party.Details",
                    "@type": "unece:AggregateBIE",
                    "unece:cefactUNId": "UN01012258",
                    "rdfs:comment": "An individual, a group, or a body having a role in the production of crops such as vegetables, flowers, plants."
                },
                {
                    "@id": "cefact:SPS_Party.Details",
                    "@type": "unece:AggregateBIE",
                    "unece:cefactUNId": "UN03000111",
                    "rdfs:comment": "A reference to an individual, a group, or a body having a role in Sanitary and Phytosanitary (SPS) measures."
                }
            ]
        },
        {
            "@id": "agriculture:Period",
            "@type": "rdfs:Class",
            "rdfs:comment": "A period of time from a start date time up to an end date time in which activities took place that are subject to Sanitary and Phytosanitary (SPS) measures.",
            "rdfs:label": "Period",
            "unece:cefactElementMetadata": [
                {
                    "@id": "cefact:SPS_Period.Details",
                    "@type": "unece:AggregateBIE",
                    "unece:cefactUNId": "UN03000119",
                    "rdfs:comment": "A period of time from a start date time up to an end date time in which activities took place that are subject to Sanitary and Phytosanitary (SPS) measures."
                }
            ]
        },
        {
            "@id": "agriculture:Person",
            "@type": "rdfs:Class",
            "rdfs:comment": [
                "A person acting as an operator.",
                "A person who is involved in Sanitary and Phytosanitary (SPS) measures, such as a government official.",
                "An individual human being who conducts an inspection."
            ],
            "rdfs:label": "Person",
            "unece:cefactElementMetadata": [
                {
                    "@id": "cefact:SPS_Person.Details",
                    "@type": "unece:AggregateBIE",
                    "unece:cefactUNId": "UN03000123",
                    "rdfs:comment": "A person who is involved in Sanitary and Phytosanitary (SPS) measures, such as a government official."
                },
                {
                    "@id": "cefact:Inspection_Person.Details",
                    "@type": "unece:AggregateBIE",
                    "unece:cefactUNId": "UN01007689",
                    "rdfs:comment": "An individual human being who conducts an inspection."
                },
                {
                    "@id": "cefact:Operator_Person.Details",
                    "@type": "unece:AggregateBIE",
                    "unece:cefactUNId": "UN01012272",
                    "rdfs:comment": "A person acting as an operator."
                }
            ]
        },
        {
            "@id": "agriculture:Plot",
            "@type": "rdfs:Class",
            "rdfs:comment": [
                "A small piece of land used in agriculture.",
                "A piece of land, used in agriculture, on which observations are conducted.",
                "A mobile platform covered with soil, substrate or water used in agriculture or aquaculture to grow organisms.",
                "A small piece of land or water used for a crop such as an agricultural or aquacultural crop."
            ],
            "rdfs:label": "Plot",
            "unece:cefactElementMetadata": [
                {
                    "@id": "cefact:Agricultural_Plot.Details",
                    "@type": "unece:AggregateBIE",
                    "unece:cefactUNId": "UN01002651",
                    "rdfs:comment": "A small piece of land used in agriculture."
                },
                {
                    "@id": "cefact:AgronomicalObservation_Plot.Details",
                    "@type": "unece:AggregateBIE",
                    "unece:cefactUNId": "UN01009365",
                    "rdfs:comment": "A piece of land, used in agriculture, on which observations are conducted."
                },
                {
                    "@id": "cefact:Crop_Plot.Details",
                    "@type": "unece:AggregateBIE",
                    "unece:cefactUNId": "UN01012138",
                    "rdfs:comment": "A small piece of land or water used for a crop such as an agricultural or aquacultural crop."
                },
                {
                    "@id": "cefact:Mobile_Plot.Details",
                    "@type": "unece:AggregateBIE",
                    "unece:cefactUNId": "UN01012154",
                    "rdfs:comment": "A mobile platform covered with soil, substrate or water used in agriculture or aquaculture to grow organisms."
                }
            ]
        },
        {
            "@id": "agriculture:Process",
            "@type": "rdfs:Class",
            "rdfs:comment": "A naturally occurring or designed sequence of operations or events that that are subject to Sanitary and Phytosanitary (SPS) measures, such as manufacturing, treating, packaging, and storing.",
            "rdfs:label": "Process",
            "unece:cefactElementMetadata": [
                {
                    "@id": "cefact:SPS_Process.Details",
                    "@type": "unece:AggregateBIE",
                    "unece:cefactUNId": "UN03000126",
                    "rdfs:comment": "A naturally occurring or designed sequence of operations or events that that are subject to Sanitary and Phytosanitary (SPS) measures, such as manufacturing, treating, packaging, and storing."
                }
            ]
        },
        {
            "@id": "agriculture:Produce",
            "@type": "rdfs:Class",
            "rdfs:comment": [
                "Agricultural plants or plant products grown and harvested, such as grain, fruit, vegetables, silage.",
                "Agricultural products, such as grain, fruits, vegetables, poultry and livestock."
            ],
            "rdfs:label": "Produce",
            "unece:cefactElementMetadata": [
                {
                    "@id": "cefact:Agricultural_Produce.Details",
                    "@type": "unece:AggregateBIE",
                    "unece:cefactUNId": "UN01002699",
                    "rdfs:comment": "Agricultural products, such as grain, fruits, vegetables, poultry and livestock."
                },
                {
                    "@id": "cefact:Crop_Produce.Details",
                    "@type": "unece:AggregateBIE",
                    "unece:cefactUNId": "UN01012324",
                    "rdfs:comment": "Agricultural plants or plant products grown and harvested, such as grain, fruit, vegetables, silage."
                }
            ]
        },
        {
            "@id": "agriculture:Product",
            "@type": "rdfs:Class",
            "rdfs:comment": [
                "A class of domesticated creatures raised on a farm or ranch.",
                "Any product used as an input for an agricultural process."
            ],
            "rdfs:label": "Product",
            "unece:cefactElementMetadata": [
                {
                    "@id": "cefact:AgriculturalInput_Product.Details",
                    "@type": "unece:AggregateBIE",
                    "unece:cefactUNId": "UN01012373",
                    "rdfs:comment": "Any product used as an input for an agricultural process."
                },
                {
                    "@id": "cefact:LivestockAnimal_Product.Details",
                    "@type": "unece:AggregateBIE",
                    "unece:cefactUNId": "UN01007705",
                    "rdfs:comment": "A class of domesticated creatures raised on a farm or ranch."
                }
            ]
        },
        {
            "@id": "agriculture:ProductInstance",
            "@type": "rdfs:Class",
            "rdfs:comment": "An individual domesticated creature kept or raised on a farm or ranch.",
            "rdfs:label": "ProductInstance",
            "unece:cefactElementMetadata": [
                {
                    "@id": "cefact:LivestockAnimal_ProductInstance.Details",
                    "@type": "unece:AggregateBIE",
                    "unece:cefactUNId": "UN01007710",
                    "rdfs:comment": "An individual domesticated creature kept or raised on a farm or ranch."
                }
            ]
        },
        {
            "@id": "agriculture:ProductionUnit",
            "@type": "rdfs:Class",
            "rdfs:comment": "A defined set of agricultural production utilities under a single management.",
            "rdfs:label": "ProductionUnit",
            "unece:cefactElementMetadata": [
                {
                    "@id": "cefact:Agricultural_ProductionUnit.Details",
                    "@type": "unece:AggregateBIE",
                    "unece:cefactUNId": "UN01012244",
                    "rdfs:comment": "A defined set of agricultural production utilities under a single management."
                }
            ]
        },
        {
            "@id": "agriculture:ProtectionMeans",
            "@type": "rdfs:Class",
            "rdfs:comment": "A way to protect something, such as human beings, animals or environment, from getting infected or becoming ill.",
            "rdfs:label": "ProtectionMeans",
            "unece:cefactElementMetadata": [
                {
                    "@id": "cefact:Disease_ProtectionMeans.Details",
                    "@type": "unece:AggregateBIE",
                    "unece:cefactUNId": "UN01015109",
                    "rdfs:comment": "A way to protect something, such as human beings, animals or environment, from getting infected or becoming ill."
                }
            ]
        },
        {
            "@id": "agriculture:Qualification",
            "@type": "rdfs:Class",
            "rdfs:comment": [
                "An academic achievement relevant to Sanitary and Phytosanitary (SPS) measures.",
                "A specified condition that must be fulfilled."
            ],
            "rdfs:label": "Qualification",
            "unece:cefactElementMetadata": [
                {
                    "@id": "cefact:SPS_Qualification.Details",
                    "@type": "unece:AggregateBIE",
                    "unece:cefactUNId": "UN03000132",
                    "rdfs:comment": "An academic achievement relevant to Sanitary and Phytosanitary (SPS) measures."
                },
                {
                    "@id": "cefact:Specified_Qualification.Details",
                    "@type": "unece:AggregateBIE",
                    "unece:cefactUNId": "UN01007687",
                    "rdfs:comment": "A specified condition that must be fulfilled."
                }
            ]
        },
        {
            "@id": "agriculture:Reason",
            "@type": "rdfs:Class",
            "rdfs:comment": "A motive, cause or justification for an agricultural process.",
            "rdfs:label": "Reason",
            "unece:cefactElementMetadata": [
                {
                    "@id": "cefact:AgriculturalProcess_Reason.Details",
                    "@type": "unece:AggregateBIE",
                    "unece:cefactUNId": "UN01002741",
                    "rdfs:comment": "A motive, cause or justification for an agricultural process."
                }
            ]
        },
        {
            "@id": "agriculture:Sample",
            "@type": "rdfs:Class",
            "rdfs:comment": "An agricultural specimen (small part of the whole) taken for testing or analysis.",
            "rdfs:label": "Sample",
            "unece:cefactElementMetadata": [
                {
                    "@id": "cefact:Agricultural_Sample.Details",
                    "@type": "unece:AggregateBIE",
                    "unece:cefactUNId": "UN01009584",
                    "rdfs:comment": "An agricultural specimen (small part of the whole) taken for testing or analysis."
                }
            ]
        },
        {
            "@id": "agriculture:SampleType",
            "@type": "rdfs:Class",
            "rdfs:comment": "The type of material, such as animal or plant, an agricultural sample contains.",
            "rdfs:label": "SampleType",
            "unece:cefactElementMetadata": [
                {
                    "@id": "cefact:Agricultural_SampleType.Details",
                    "@type": "unece:AggregateBIE",
                    "unece:cefactUNId": "UN01009578",
                    "rdfs:comment": "The type of material, such as animal or plant, an agricultural sample contains."
                }
            ]
        },
        {
            "@id": "agriculture:SampledObject",
            "@type": "rdfs:Class",
            "rdfs:comment": "The physical agricultural object from which a sample has been taken.",
            "rdfs:label": "SampledObject",
            "unece:cefactElementMetadata": [
                {
                    "@id": "cefact:Agricultural_SampledObject.Details",
                    "@type": "unece:AggregateBIE",
                    "unece:cefactUNId": "UN01009609",
                    "rdfs:comment": "The physical agricultural object from which a sample has been taken."
                }
            ]
        },
        {
            "@id": "agriculture:Scope",
            "@type": "rdfs:Class",
            "rdfs:comment": "The area over which an agronomical observation operates.",
            "rdfs:label": "Scope",
            "unece:cefactElementMetadata": [
                {
                    "@id": "cefact:AgronomicalObservation_Scope.Details",
                    "@type": "unece:AggregateBIE",
                    "unece:cefactUNId": "UN01009325",
                    "rdfs:comment": "The area over which an agronomical observation operates."
                }
            ]
        },
        {
            "@id": "agriculture:Seal",
            "@type": "rdfs:Class",
            "rdfs:comment": "A device used to secure an object and protect from unauthorized entry or tampering as part of Sanitary and Phytosanitary (SPS) measures, such as a seal affixed to a piece of transport equipment.",
            "rdfs:label": "Seal",
            "unece:cefactElementMetadata": [
                {
                    "@id": "cefact:SPS_Seal.Details",
                    "@type": "unece:AggregateBIE",
                    "unece:cefactUNId": "UN03000135",
                    "rdfs:comment": "A device used to secure an object and protect from unauthorized entry or tampering as part of Sanitary and Phytosanitary (SPS) measures, such as a seal affixed to a piece of transport equipment."
                }
            ]
        },
        {
            "@id": "agriculture:ShippingMarks",
            "@type": "rdfs:Class",
            "rdfs:comment": "Physical markings or labels on individual packages or transport units relevant to Sanitary and Phytosanitary (SPS) measures.",
            "rdfs:label": "ShippingMarks",
            "unece:cefactElementMetadata": [
                {
                    "@id": "cefact:SPS_ShippingMarks.Details",
                    "@type": "unece:AggregateBIE",
                    "unece:cefactUNId": "UN03000139",
                    "rdfs:comment": "Physical markings or labels on individual packages or transport units relevant to Sanitary and Phytosanitary (SPS) measures."
                }
            ]
        },
        {
            "@id": "agriculture:SoilOccupation",
            "@type": "rdfs:Class",
            "rdfs:comment": "The use or occupation of soil to grow a crop on a plot.",
            "rdfs:label": "SoilOccupation",
            "unece:cefactElementMetadata": [
                {
                    "@id": "cefact:Plot_SoilOccupation.Details",
                    "@type": "unece:AggregateBIE",
                    "unece:cefactUNId": "UN01002749",
                    "rdfs:comment": "The use or occupation of soil to grow a crop on a plot."
                }
            ]
        },
        {
            "@id": "agriculture:SoilSupplement",
            "@type": "rdfs:Class",
            "rdfs:comment": "A material specified to be added to soil to improve its quality.",
            "rdfs:label": "SoilSupplement",
            "unece:cefactElementMetadata": [
                {
                    "@id": "cefact:Specified_SoilSupplement.Details",
                    "@type": "unece:AggregateBIE",
                    "unece:cefactUNId": "UN01002718",
                    "rdfs:comment": "A material specified to be added to soil to improve its quality."
                }
            ]
        },
        {
            "@id": "agriculture:SpeciesVariety",
            "@type": "rdfs:Class",
            "rdfs:comment": "A sub-division of cultivated plants within a species.",
            "rdfs:label": "SpeciesVariety",
            "unece:cefactElementMetadata": [
                {
                    "@id": "cefact:Crop_SpeciesVariety.Details",
                    "@type": "unece:AggregateBIE",
                    "unece:cefactUNId": "UN01002774",
                    "rdfs:comment": "A sub-division of cultivated plants within a species."
                }
            ]
        },
        {
            "@id": "agriculture:Tank",
            "@type": "rdfs:Class",
            "rdfs:comment": "A bulk storage on a farm for collecting and storage of fresh raw milk.",
            "rdfs:label": "Tank",
            "unece:cefactElementMetadata": [
                {
                    "@id": "cefact:Milk_Tank.Details",
                    "@type": "unece:AggregateBIE",
                    "unece:cefactUNId": "UN01009834",
                    "rdfs:comment": "A bulk storage on a farm for collecting and storage of fresh raw milk."
                }
            ]
        },
        {
            "@id": "agriculture:TargetObject",
            "@type": "rdfs:Class",
            "rdfs:comment": [
                "An entity at which agronomical observation efforts are aimed, such as a pest, a disease or weed.",
                "An entity at which agricultural process efforts are aimed."
            ],
            "rdfs:label": "TargetObject",
            "unece:cefactElementMetadata": [
                {
                    "@id": "cefact:AgriculturalProcess_TargetObject.Details",
                    "@type": "unece:AggregateBIE",
                    "unece:cefactUNId": "UN01002770",
                    "rdfs:comment": "An entity at which agricultural process efforts are aimed."
                },
                {
                    "@id": "cefact:AgronomicalObservation_TargetObject.Details",
                    "@type": "unece:AggregateBIE",
                    "unece:cefactUNId": "UN01009318",
                    "rdfs:comment": "An entity at which agronomical observation efforts are aimed, such as a pest, a disease or weed."
                }
            ]
        },
        {
            "@id": "agriculture:Temperature",
            "@type": "rdfs:Class",
            "rdfs:comment": "Temperature settings for goods that are subject to Sanitary and Phytosanitary (SPS) measures, such as a required storage temperature range.",
            "rdfs:label": "Temperature",
            "unece:cefactElementMetadata": [
                {
                    "@id": "cefact:SPS_Temperature.Details",
                    "@type": "unece:AggregateBIE",
                    "unece:cefactUNId": "UN03000141",
                    "rdfs:comment": "Temperature settings for goods that are subject to Sanitary and Phytosanitary (SPS) measures, such as a required storage temperature range."
                }
            ]
        },
        {
            "@id": "agriculture:Tissue",
            "@type": "rdfs:Class",
            "rdfs:comment": "An aggregate of similar cells and cell products forming a definite kind of structural material with a specific function, in a multicellular organism of an agricultural sample.",
            "rdfs:label": "Tissue",
            "unece:cefactElementMetadata": [
                {
                    "@id": "cefact:AgriculturalSample_Tissue.Details",
                    "@type": "unece:AggregateBIE",
                    "unece:cefactUNId": "UN01009575",
                    "rdfs:comment": "An aggregate of similar cells and cell products forming a definite kind of structural material with a specific function, in a multicellular organism of an agricultural sample."
                }
            ]
        },
        {
            "@id": "agriculture:TradeDelivery",
            "@type": "rdfs:Class",
            "rdfs:comment": "The shipping arrangements and movement of animals including despatch and delivery.",
            "rdfs:label": "TradeDelivery",
            "unece:cefactElementMetadata": [
                {
                    "@id": "cefact:Animal_TradeDelivery.Details",
                    "@type": "unece:AggregateBIE",
                    "unece:cefactUNId": "UN01011261",
                    "rdfs:comment": "The shipping arrangements and movement of animals including despatch and delivery."
                }
            ]
        },
        {
            "@id": "agriculture:TradeLineItem",
            "@type": "rdfs:Class",
            "rdfs:comment": "A collection of information specific to an item that is subject to Sanitary and Phytosanitary (SPS) measures.",
            "rdfs:label": "TradeLineItem",
            "unece:cefactElementMetadata": [
                {
                    "@id": "cefact:SPS_TradeLineItem.Details",
                    "@type": "unece:AggregateBIE",
                    "unece:cefactUNId": "UN03000146",
                    "rdfs:comment": "A collection of information specific to an item that is subject to Sanitary and Phytosanitary (SPS) measures."
                }
            ]
        },
        {
            "@id": "agriculture:TransportEquipment",
            "@type": "rdfs:Class",
            "rdfs:comment": "A piece of equipment used to hold, protect or secure cargo that is subject to Sanitary and Phytosanitary (SPS) measures for transportation purposes.",
            "rdfs:label": "TransportEquipment",
            "unece:cefactElementMetadata": [
                {
                    "@id": "cefact:SPS_TransportEquipment.Details",
                    "@type": "unece:AggregateBIE",
                    "unece:cefactUNId": "UN03000166",
                    "rdfs:comment": "A piece of equipment used to hold, protect or secure cargo that is subject to Sanitary and Phytosanitary (SPS) measures for transportation purposes."
                }
            ]
        },
        {
            "@id": "agriculture:TransportMeans",
            "@type": "rdfs:Class",
            "rdfs:comment": "A device used to convey goods or other objects such as animals that are subject to Sanitary and Phytosanitary (SPS) measures from place to place.",
            "rdfs:label": "TransportMeans",
            "unece:cefactElementMetadata": [
                {
                    "@id": "cefact:SPS_TransportMeans.Details",
                    "@type": "unece:AggregateBIE",
                    "unece:cefactUNId": "UN03000170",
                    "rdfs:comment": "A device used to convey goods or other objects such as animals that are subject to Sanitary and Phytosanitary (SPS) measures from place to place."
                }
            ]
        },
        {
            "@id": "agriculture:TransportMovement",
            "@type": "rdfs:Class",
            "rdfs:comment": "The conveyance (physical carriage) of goods that are subject to Sanitary and Phytosanitary (SPS) measures.",
            "rdfs:label": "TransportMovement",
            "unece:cefactElementMetadata": [
                {
                    "@id": "cefact:SPS_TransportMovement.Details",
                    "@type": "unece:AggregateBIE",
                    "unece:cefactUNId": "UN03000172",
                    "rdfs:comment": "The conveyance (physical carriage) of goods that are subject to Sanitary and Phytosanitary (SPS) measures."
                }
            ]
        },
        {
            "@id": "agriculture:WeatherCondition",
            "@type": "rdfs:Class",
            "rdfs:comment": "A weather condition regarded as extreme in agriculture.",
            "rdfs:label": "WeatherCondition",
            "unece:cefactElementMetadata": [
                {
                    "@id": "cefact:AgriculturalExtreme_WeatherCondition.Details",
                    "@type": "unece:AggregateBIE",
                    "unece:cefactUNId": "UN01012451",
                    "rdfs:comment": "A weather condition regarded as extreme in agriculture."
                }
            ]
        },
        {
            "@id": "agriculture:WorkItem",
            "@type": "rdfs:Class",
            "rdfs:comment": "A specific task or a set of tasks to be undertaken for an agricultural process.",
            "rdfs:label": "WorkItem",
            "unece:cefactElementMetadata": [
                {
                    "@id": "cefact:AgriculturalProcess_WorkItem.Details",
                    "@type": "unece:AggregateBIE",
                    "unece:cefactUNId": "UN01002804",
                    "rdfs:comment": "A specific task or a set of tasks to be undertaken for an agricultural process."
                }
            ]
        },
        {
            "@id": "agriculture:abbreviatedName",
            "@type": "rdf:Property",
            "schema:rangeIncludes": {
                "@id": "xsd:string"
            },
            "schema:domainIncludes": {
                "@id": "agriculture:Qualification"
            },
            "rdfs:comment": "The abbreviated name, expressed as text, of this SPS qualification.",
            "rdfs:label": "abbreviatedName",
            "unece:cefactElementMetadata": [
                {
                    "@id": "cefact:SPS_Qualification.AbbreviatedName.Text",
                    "@type": "unece:BasicBIE",
                    "unece:TDED": "9006",
                    "unece:cefactUNId": "UN03000134",
                    "unece:cefactBieDomainClass": "cefact:SPS_Qualification.Details",
                    "rdfs:comment": "The abbreviated name, expressed as text, of this SPS qualification."
                }
            ]
        },
        {
            "@id": "agriculture:acceptedIndicator",
            "@type": "rdf:Property",
            "schema:rangeIncludes": {
                "@id": "xsd:boolean"
            },
            "schema:domainIncludes": {
                "@id": "agriculture:ProtectionMeans"
            },
            "rdfs:comment": "The indication of whether or not this disease protection means is accepted.",
            "rdfs:label": "acceptedIndicator",
            "unece:cefactElementMetadata": [
                {
                    "@id": "cefact:Disease_ProtectionMeans.Accepted.Indicator",
                    "@type": "unece:BasicBIE",
                    "unece:cefactUNId": "UN01015113",
                    "unece:cefactBieDomainClass": "cefact:Disease_ProtectionMeans.Details",
                    "rdfs:comment": "The indication of whether or not this disease protection means is accepted."
                }
            ]
        },
        {
            "@id": "agriculture:activeIngredientIndicator",
            "@type": "rdf:Property",
            "schema:rangeIncludes": {
                "@id": "xsd:boolean"
            },
            "schema:domainIncludes": {
                "@id": "agriculture:Material"
            },
            "rdfs:comment": "The indication of whether or not this agricultural input material is an active ingredient.",
            "rdfs:label": "activeIngredientIndicator",
            "unece:cefactElementMetadata": [
                {
                    "@id": "cefact:AgriculturalInput_Material.ActiveIngredient.Indicator",
                    "@type": "unece:BasicBIE",
                    "unece:cefactUNId": "UN01012398",
                    "unece:cefactBieDomainClass": "cefact:AgriculturalInput_Material.Details",
                    "rdfs:comment": "The indication of whether or not this agricultural input material is an active ingredient."
                }
            ]
        },
        {
            "@id": "agriculture:activityAuthorizedParty",
            "@type": "rdf:Property",
            "schema:rangeIncludes": {
                "@id": "agriculture:Party"
            },
            "schema:domainIncludes": {
                "@id": "agriculture:CountrySubDivision"
            },
            "rdfs:comment": "A party that is authorized to perform an activity in this SPS country sub-division.",
            "rdfs:label": "activityAuthorizedParty",
            "unece:cefactElementMetadata": [
                {
                    "@id": "cefact:SPS_CountrySub-Division.Activity_Authorized.SPS_Party",
                    "@type": "unece:AssociationBIE",
                    "unece:cefactUNId": "UN03000086",
                    "unece:cefactBieDomainClass": "cefact:SPS_CountrySubDivision.Details",
                    "rdfs:comment": "A party that is authorized to perform an activity in this SPS country sub-division."
                }
            ]
        },
        {
            "@id": "agriculture:actualDateTime",
            "@type": "rdf:Property",
            "schema:rangeIncludes": {
                "@id": "xsd:dateTime"
            },
            "schema:domainIncludes": {
                "@id": "agriculture:Authentication"
            },
            "rdfs:comment": "The actual date, time, date time, or other date time value of this SPS authentication.",
            "rdfs:label": "actualDateTime",
            "unece:cefactElementMetadata": [
                {
                    "@id": "cefact:SPS_Authentication.Actual.DateTime",
                    "@type": "unece:BasicBIE",
                    "unece:TDED": "2007",
                    "unece:cefactUNId": "UN03000035",
                    "unece:cefactBieDomainClass": "cefact:SPS_Authentication.Details",
                    "rdfs:comment": "The actual date, time, date time, or other date time value of this SPS authentication."
                }
            ]
        },
        {
            "@id": "agriculture:actualEffectiveDateTime",
            "@type": "rdf:Property",
            "schema:rangeIncludes": {
                "@id": "xsd:dateTime"
            },
            "schema:domainIncludes": {
                "@id": "agriculture:Certificate"
            },
            "rdfs:comment": "The actual effective date, time, date time or other date time value for this agricultural certificate.",
            "rdfs:label": "actualEffectiveDateTime",
            "unece:cefactElementMetadata": [
                {
                    "@id": "cefact:Agricultural_Certificate.ActualEffective.DateTime",
                    "@type": "unece:BasicBIE",
                    "unece:cefactUNId": "UN01012284",
                    "unece:cefactBieDomainClass": "cefact:Agricultural_Certificate.Details",
                    "rdfs:comment": "The actual effective date, time, date time or other date time value for this agricultural certificate."
                }
            ]
        },
        {
            "@id": "agriculture:actualEndDateTime",
            "@type": "rdf:Property",
            "schema:rangeIncludes": {
                "@id": "xsd:dateTime"
            },
            "schema:domainIncludes": {
                "@id": "agriculture:AgriculturalProcess"
            },
            "rdfs:comment": "The date, time, date time or other date time value of the actual end for the crop production in this agricultural process.",
            "rdfs:label": "actualEndDateTime",
            "unece:cefactElementMetadata": [
                {
                    "@id": "cefact:CropProduction_AgriculturalProcess.Actual_End.DateTime",
                    "@type": "unece:BasicBIE",
                    "unece:cefactUNId": "UN01012414",
                    "unece:cefactBieDomainClass": "cefact:CropProduction_AgriculturalProcess.Details",
                    "rdfs:comment": "The date, time, date time or other date time value of the actual end for the crop production in this agricultural process."
                }
            ]
        },
        {
            "@id": "agriculture:actualMeasure",
            "@type": "rdf:Property",
            "schema:rangeIncludes": {
                "@id": "xsd:decimal"
            },
            "schema:domainIncludes": {
                "@id": "agriculture:Area"
            },
            "rdfs:comment": "The actual measure of this agricultural area.",
            "rdfs:label": "actualMeasure",
            "unece:cefactElementMetadata": [
                {
                    "@id": "cefact:Agricultural_Area.Actual.Measure",
                    "@type": "unece:BasicBIE",
                    "unece:cefactUNId": "UN01002673",
                    "unece:cefactBieDomainClass": "cefact:Agricultural_Area.Details",
                    "rdfs:comment": "The actual measure of this agricultural area."
                }
            ]
        },
        {
            "@id": "agriculture:actualStartDateTime",
            "@type": "rdf:Property",
            "schema:rangeIncludes": {
                "@id": "xsd:dateTime"
            },
            "schema:domainIncludes": {
                "@id": "agriculture:AgriculturalProcess"
            },
            "rdfs:comment": "The date, time, date time or other date time value for the actual start of the crop production in this agricultural process.",
            "rdfs:label": "actualStartDateTime",
            "unece:cefactElementMetadata": [
                {
                    "@id": "cefact:CropProduction_AgriculturalProcess.Actual_Start.DateTime",
                    "@type": "unece:BasicBIE",
                    "unece:cefactUNId": "UN01012412",
                    "unece:cefactBieDomainClass": "cefact:CropProduction_AgriculturalProcess.Details",
                    "rdfs:comment": "The date, time, date time or other date time value for the actual start of the crop production in this agricultural process."
                }
            ]
        },
        {
            "@id": "agriculture:additionalIdentifiedParty",
            "@type": "rdf:Property",
            "schema:rangeIncludes": {
                "@id": "agriculture:Party"
            },
            "schema:domainIncludes": {
                "@id": "agriculture:Contract"
            },
            "rdfs:comment": "An additional party identified for this agricultural contract.",
            "rdfs:label": "additionalIdentifiedParty",
            "unece:cefactElementMetadata": [
                {
                    "@id": "cefact:Agricultural_Contract.Additional_Identified.Specified_Party",
                    "@type": "unece:AssociationBIE",
                    "unece:cefactUNId": "UN01012450",
                    "unece:cefactBieDomainClass": "cefact:Agricultural_Contract.Details",
                    "rdfs:comment": "An additional party identified for this agricultural contract."
                }
            ]
        },
        {
            "@id": "agriculture:additionalInformationNote",
            "@type": "rdf:Property",
            "schema:rangeIncludes": {
                "@id": "agriculture:Note"
            },
            "schema:domainIncludes": [
                {
                    "@id": "agriculture:ProductInstance"
                },
                {
                    "@id": "agriculture:TradeLineItem"
                }
            ],
            "rdfs:comment": [
                "A note providing additional information for this SPS trade line item.",
                "The basic note that provides additional information for this livestock animal product instance."
            ],
            "rdfs:label": "additionalInformationNote",
            "unece:cefactElementMetadata": [
                {
                    "@id": "cefact:LivestockAnimal_ProductInstance.AdditionalInformation.Basic_Note",
                    "@type": "unece:AssociationBIE",
                    "unece:cefactUNId": "UN01007713",
                    "unece:cefactBieDomainClass": "cefact:LivestockAnimal_ProductInstance.Details",
                    "rdfs:comment": "The basic note that provides additional information for this livestock animal product instance."
                },
                {
                    "@id": "cefact:SPS_TradeLineItem.AdditionalInformation.SPS_Note",
                    "@type": "unece:AssociationBIE",
                    "unece:cefactUNId": "UN03000158",
                    "unece:cefactBieDomainClass": "cefact:SPS_TradeLineItem.Details",
                    "rdfs:comment": "A note providing additional information for this SPS trade line item."
                }
            ]
        },
        {
            "@id": "agriculture:additionalInformationSpecifiedNote",
            "@type": "rdf:Property",
            "schema:rangeIncludes": {
                "@id": "agriculture:Note"
            },
            "schema:domainIncludes": {
                "@id": "agriculture:SampledObject"
            },
            "rdfs:comment": "The note, containing additional information, specified for this sampled agricultural object.",
            "rdfs:label": "additionalInformationSpecifiedNote",
            "unece:cefactElementMetadata": [
                {
                    "@id": "cefact:Agricultural_SampledObject.AdditionalInformation_Specified.LaboratoryObservation_Note",
                    "@type": "unece:AssociationBIE",
                    "unece:cefactUNId": "UN01009626",
                    "unece:cefactBieDomainClass": "cefact:Agricultural_SampledObject.Details",
                    "rdfs:comment": "The note, containing additional information, specified for this sampled agricultural object."
                }
            ]
        },
        {
            "@id": "agriculture:addressTypeCode",
            "@type": "rdf:Property",
            "schema:rangeIncludes": {
                "@id": "unece:UNECECL3131Code"
            },
            "schema:domainIncludes": {
                "@id": "agriculture:Address"
            },
            "rdfs:comment": "The code specifying the type of SPS address.",
            "rdfs:label": "addressTypeCode",
            "unece:cefactElementMetadata": [
                {
                    "@id": "cefact:SPS_Address.Type.Code",
                    "@type": "unece:BasicBIE",
                    "unece:TDED": "3131",
                    "unece:cefactUNId": "UN03000028",
                    "unece:cefactBieDomainClass": "cefact:SPS_Address.Details",
                    "rdfs:comment": "The code specifying the type of SPS address."
                }
            ]
        },
        {
            "@id": "agriculture:affixedSeal",
            "@type": "rdf:Property",
            "schema:rangeIncludes": {
                "@id": "agriculture:Seal"
            },
            "schema:domainIncludes": {
                "@id": "agriculture:TransportEquipment"
            },
            "rdfs:comment": "A seal affixed to this piece of SPS transport equipment.",
            "rdfs:label": "affixedSeal",
            "unece:cefactElementMetadata": [
                {
                    "@id": "cefact:SPS_TransportEquipment.Affixed.SPS_Seal",
                    "@type": "unece:AssociationBIE",
                    "unece:cefactUNId": "UN03000168",
                    "unece:cefactBieDomainClass": "cefact:SPS_TransportEquipment.Details",
                    "rdfs:comment": "A seal affixed to this piece of SPS transport equipment."
                }
            ]
        },
        {
            "@id": "agriculture:aggregatedSpecifiedBatchHistoryRecord",
            "@type": "rdf:Property",
            "schema:rangeIncludes": {
                "@id": "agriculture:BatchHistoryRecord"
            },
            "schema:domainIncludes": {
                "@id": "agriculture:Batch"
            },
            "rdfs:comment": "An aggregated Track and Trace (TT) batch history record specified for this animal batch.",
            "rdfs:label": "aggregatedSpecifiedBatchHistoryRecord",
            "unece:cefactElementMetadata": [
                {
                    "@id": "cefact:Animal_Batch.Aggregated_Specified.TT_BatchHistoryRecord",
                    "@type": "unece:AssociationBIE",
                    "unece:cefactUNId": "UN01011257",
                    "unece:cefactBieDomainClass": "cefact:Animal_Batch.Details",
                    "rdfs:comment": "An aggregated Track and Trace (TT) batch history record specified for this animal batch."
                }
            ]
        },
        {
            "@id": "agriculture:agriculturalCharacteristicValueCode",
            "@type": "rdf:Property",
            "schema:rangeIncludes": {
                "@id": "unece:UNECECL7111Code"
            },
            "schema:domainIncludes": {
                "@id": "agriculture:Characteristic"
            },
            "rdfs:comment": "The code specifying the value of this agricultural characteristic.",
            "rdfs:label": "agriculturalCharacteristicValueCode",
            "unece:cefactElementMetadata": [
                {
                    "@id": "cefact:Agricultural_Characteristic.Value.Code",
                    "@type": "unece:BasicBIE",
                    "unece:TDED": "7111",
                    "unece:cefactUNId": "UN01012365",
                    "unece:cefactBieDomainClass": "cefact:Agricultural_Characteristic.Details",
                    "rdfs:comment": "The code specifying the value of this agricultural characteristic."
                }
            ]
        },
        {
            "@id": "agriculture:agriculturalSampleProcessingStatusCode",
            "@type": "rdf:Property",
            "schema:rangeIncludes": {
                "@id": "unece:UNECECL7045Code"
            },
            "schema:domainIncludes": {
                "@id": "agriculture:Sample"
            },
            "rdfs:comment": "The code specifying the processing status for this agricultural sample, such as taking sample, processing intake sample, performing observations, preparing report observations and conclusions.",
            "rdfs:label": "agriculturalSampleProcessingStatusCode",
            "unece:cefactElementMetadata": [
                {
                    "@id": "cefact:Agricultural_Sample.ProcessingStatus.Code",
                    "@type": "unece:BasicBIE",
                    "unece:TDED": "7045",
                    "unece:cefactUNId": "UN01010563",
                    "unece:cefactBieDomainClass": "cefact:Agricultural_Sample.Details",
                    "rdfs:comment": "The code specifying the processing status for this agricultural sample, such as taking sample, processing intake sample, performing observations, preparing report observations and conclusions."
                }
            ]
        },
        {
            "@id": "agriculture:agronomicalObservationDocumentStatusCode",
            "@type": "rdf:Property",
            "schema:rangeIncludes": {
                "@id": "unece:UNECECL1373Code"
            },
            "schema:domainIncludes": {
                "@id": "agriculture:Document"
            },
            "rdfs:comment": "The code specifying the status of this agronomical observation document.",
            "rdfs:label": "agronomicalObservationDocumentStatusCode",
            "unece:cefactElementMetadata": [
                {
                    "@id": "cefact:AgronomicalObservation_Document.Status.Code",
                    "@type": "unece:BasicBIE",
                    "unece:TDED": "1373",
                    "unece:cefactUNId": "UN01009297",
                    "unece:cefactBieDomainClass": "cefact:AgronomicalObservation_Document.Details",
                    "rdfs:comment": "The code specifying the status of this agronomical observation document."
                }
            ]
        },
        {
            "@id": "agriculture:allocatedManMachineSystem",
            "@type": "rdf:Property",
            "schema:rangeIncludes": {
                "@id": "agriculture:ManMachineSystem"
            },
            "schema:domainIncludes": {
                "@id": "agriculture:AgriculturalProcess"
            },
            "rdfs:comment": "A man machine system allocated to this crop production agricultural process.",
            "rdfs:label": "allocatedManMachineSystem",
            "unece:cefactElementMetadata": [
                {
                    "@id": "cefact:CropProduction_AgriculturalProcess.Allocated.Agricultural_ManMachineSystem",
                    "@type": "unece:AssociationBIE",
                    "unece:cefactUNId": "UN01012419",
                    "unece:cefactBieDomainClass": "cefact:CropProduction_AgriculturalProcess.Details",
                    "rdfs:comment": "A man machine system allocated to this crop production agricultural process."
                }
            ]
        },
        {
            "@id": "agriculture:allocationDateTime",
            "@type": "rdf:Property",
            "schema:rangeIncludes": {
                "@id": "xsd:dateTime"
            },
            "schema:domainIncludes": {
                "@id": "agriculture:Grant"
            },
            "rdfs:comment": "The date for the allocation of this animal grant.",
            "rdfs:label": "allocationDateTime",
            "unece:cefactElementMetadata": [
                {
                    "@id": "cefact:Animal_Grant.Allocation.DateTime",
                    "@type": "unece:BasicBIE",
                    "unece:cefactUNId": "UN01007677",
                    "unece:cefactBieDomainClass": "cefact:Animal_Grant.Details",
                    "rdfs:comment": "The date for the allocation of this animal grant."
                }
            ]
        },
        {
            "@id": "agriculture:anatomicalLocation",
            "@type": "rdf:Property",
            "schema:rangeIncludes": {
                "@id": "xsd:string"
            },
            "schema:domainIncludes": {
                "@id": "agriculture:Tissue"
            },
            "rdfs:comment": "The area or part of the body or plant, expressed as text, from which this agricultural sample tissue has been taken.",
            "rdfs:label": "anatomicalLocation",
            "unece:cefactElementMetadata": [
                {
                    "@id": "cefact:AgriculturalSample_Tissue.AnatomicalLocation.Text",
                    "@type": "unece:BasicBIE",
                    "unece:cefactUNId": "UN01009577",
                    "unece:cefactBieDomainClass": "cefact:AgriculturalSample_Tissue.Details",
                    "rdfs:comment": "The area or part of the body or plant, expressed as text, from which this agricultural sample tissue has been taken."
                }
            ]
        },
        {
            "@id": "agriculture:anatomicalName",
            "@type": "rdf:Property",
            "schema:rangeIncludes": {
                "@id": "xsd:string"
            },
            "schema:domainIncludes": {
                "@id": "agriculture:Tissue"
            },
            "rdfs:comment": "The anatomical name, expressed as text, of the organ or part of the organism from which this agricultural sample tissue has been taken.",
            "rdfs:label": "anatomicalName",
            "unece:cefactElementMetadata": [
                {
                    "@id": "cefact:AgriculturalSample_Tissue.AnatomicalName.Text",
                    "@type": "unece:BasicBIE",
                    "unece:cefactUNId": "UN01009576",
                    "unece:cefactBieDomainClass": "cefact:AgriculturalSample_Tissue.Details",
                    "rdfs:comment": "The anatomical name, expressed as text, of the organ or part of the organism from which this agricultural sample tissue has been taken."
                }
            ]
        },
        {
            "@id": "agriculture:applicableAgriculturalProcess",
            "@type": "rdf:Property",
            "schema:rangeIncludes": {
                "@id": "agriculture:AgriculturalProcess"
            },
            "schema:domainIncludes": [
                {
                    "@id": "agriculture:Crop"
                },
                {
                    "@id": "agriculture:CropProductionCycle"
                },
                {
                    "@id": "agriculture:Plot"
                }
            ],
            "rdfs:comment": [
                "A plot agricultural process applicable to this agricultural crop production cycle.",
                "An agricultural process crop production applicable for this field crop.",
                "An agricultural process crop production specified for this crop plot."
            ],
            "rdfs:label": "applicableAgriculturalProcess",
            "unece:cefactElementMetadata": [
                {
                    "@id": "cefact:Agricultural_CropProductionCycle.Applicable.Plot_AgriculturalProcess",
                    "@type": "unece:AssociationBIE",
                    "unece:cefactUNId": "UN01002767",
                    "unece:cefactBieDomainClass": "cefact:Agricultural_CropProductionCycle.Details",
                    "rdfs:comment": "A plot agricultural process applicable to this agricultural crop production cycle."
                },
                {
                    "@id": "cefact:Field_Crop.Applicable.CropProduction_AgriculturalProcess",
                    "@type": "unece:AssociationBIE",
                    "unece:cefactUNId": "UN01012316",
                    "unece:cefactBieDomainClass": "cefact:Field_Crop.Details",
                    "rdfs:comment": "An agricultural process crop production applicable for this field crop."
                },
                {
                    "@id": "cefact:Crop_Plot.Applicable.CropProduction_AgriculturalProcess",
                    "@type": "unece:AssociationBIE",
                    "unece:cefactUNId": "UN01012152",
                    "unece:cefactBieDomainClass": "cefact:Crop_Plot.Details",
                    "rdfs:comment": "An agricultural process crop production specified for this crop plot."
                }
            ]
        },
        {
            "@id": "agriculture:applicableAssertion",
            "@type": "rdf:Property",
            "schema:rangeIncludes": {
                "@id": "agriculture:Assertion"
            },
            "schema:domainIncludes": {
                "@id": "agriculture:Certificate"
            },
            "rdfs:comment": [
                "A sustainability assertion applicable to this agricultural certificate.",
                "A sustainability assertion applicable to this animal certificate."
            ],
            "rdfs:label": "applicableAssertion",
            "unece:cefactElementMetadata": [
                {
                    "@id": "cefact:Animal_Certificate.Applicable.Sustainability_Assertion",
                    "@type": "unece:AssociationBIE",
                    "unece:cefactUNId": "UN01013717",
                    "unece:cefactBieDomainClass": "cefact:Animal_Certificate.Details",
                    "rdfs:comment": "A sustainability assertion applicable to this animal certificate."
                },
                {
                    "@id": "cefact:Agricultural_Certificate.Applicable.Sustainability_Assertion",
                    "@type": "unece:AssociationBIE",
                    "unece:cefactUNId": "UN01013707",
                    "unece:cefactBieDomainClass": "cefact:Agricultural_Certificate.Details",
                    "rdfs:comment": "A sustainability assertion applicable to this agricultural certificate."
                }
            ]
        },
        {
            "@id": "agriculture:applicableCertificate",
            "@type": "rdf:Property",
            "schema:rangeIncludes": {
                "@id": "agriculture:Certificate"
            },
            "schema:domainIncludes": {
                "@id": "agriculture:CropProtectionTreatment"
            },
            "rdfs:comment": "A process certificate applicable to this specified crop protection treatment.",
            "rdfs:label": "applicableCertificate",
            "unece:cefactElementMetadata": [
                {
                    "@id": "cefact:Specified_CropProtectionTreatment.Applicable.Process_Certificate",
                    "@type": "unece:AssociationBIE",
                    "unece:cefactUNId": "UN01014291",
                    "unece:cefactBieDomainClass": "cefact:Specified_CropProtectionTreatment.Details",
                    "rdfs:comment": "A process certificate applicable to this specified crop protection treatment."
                }
            ]
        },
        {
            "@id": "agriculture:applicableCertification",
            "@type": "rdf:Property",
            "schema:rangeIncludes": {
                "@id": "agriculture:Certification"
            },
            "schema:domainIncludes": {
                "@id": "agriculture:Certificate"
            },
            "rdfs:comment": "An animal certification applicable to this animal certificate.",
            "rdfs:label": "applicableCertification",
            "unece:cefactElementMetadata": [
                {
                    "@id": "cefact:Animal_Certificate.Applicable.Animal_Certification",
                    "@type": "unece:AssociationBIE",
                    "unece:cefactUNId": "UN01013718",
                    "unece:cefactBieDomainClass": "cefact:Animal_Certificate.Details",
                    "rdfs:comment": "An animal certification applicable to this animal certificate."
                }
            ]
        },
        {
            "@id": "agriculture:applicableCharacteristic",
            "@type": "rdf:Property",
            "schema:rangeIncludes": {
                "@id": "agriculture:Characteristic"
            },
            "schema:domainIncludes": [
                {
                    "@id": "agriculture:AgriculturalApplication"
                },
                {
                    "@id": "agriculture:AgriculturalProcess"
                },
                {
                    "@id": "agriculture:Area"
                },
                {
                    "@id": "agriculture:Batch"
                },
                {
                    "@id": "agriculture:Certificate"
                },
                {
                    "@id": "agriculture:CountrySubDivision"
                },
                {
                    "@id": "agriculture:CropInput"
                },
                {
                    "@id": "agriculture:CropProductionCycle"
                },
                {
                    "@id": "agriculture:CropProtectionTreatment"
                },
                {
                    "@id": "agriculture:Material"
                },
                {
                    "@id": "agriculture:Plot"
                },
                {
                    "@id": "agriculture:Process"
                },
                {
                    "@id": "agriculture:Produce"
                },
                {
                    "@id": "agriculture:Product"
                },
                {
                    "@id": "agriculture:SoilOccupation"
                }
            ],
            "rdfs:comment": [
                "A sustainability characteristic applicable to this agricultural application.",
                "A sustainability characteristic applicable to this agricultural certificate.",
                "A sustainability characteristic applicable to this animal certificate.",
                "A sustainability characteristic applicable to this specified crop protection treatment.",
                "A technical characteristic applicable to this agricultural area.",
                "A technical characteristic applicable to this agricultural country sub-division.",
                "A technical characteristic applicable to this agricultural crop production cycle.",
                "A technical characteristic applicable to this agricultural plot, such as soil acidity or type of soil.",
                "A technical characteristic applicable to this agricultural process crop input.",
                "A technical characteristic applicable to this agricultural produce.",
                "A technical characteristic applicable to this agronomical observation plot.",
                "A technical characteristic applicable to this crop input batch.",
                "A technical characteristic applicable to this plot agricultural process.",
                "A technical characteristic applicable to this plot soil occupation.",
                "An SPS process characteristic applicable to this SPS process.",
                "An agricultural characteristic applicable to this agricultural input material.",
                "An agricultural characteristic applicable to this agricultural input product.",
                "An agricultural characteristic applicable to this agricultural zone area."
            ],
            "rdfs:label": "applicableCharacteristic",
            "unece:cefactElementMetadata": [
                {
                    "@id": "cefact:AgriculturalProcess_CropInput.Applicable.Technical_Characteristic",
                    "@type": "unece:AssociationBIE",
                    "unece:cefactUNId": "UN01002734",
                    "unece:cefactBieDomainClass": "cefact:AgriculturalProcess_CropInput.Details",
                    "rdfs:comment": "A technical characteristic applicable to this agricultural process crop input."
                },
                {
                    "@id": "cefact:Agricultural_Area.Applicable.Technical_Characteristic",
                    "@type": "unece:AssociationBIE",
                    "unece:cefactUNId": "UN01009348",
                    "unece:cefactBieDomainClass": "cefact:Agricultural_Area.Details",
                    "rdfs:comment": "A technical characteristic applicable to this agricultural area."
                },
                {
                    "@id": "cefact:Agricultural_Produce.Applicable.Technical_Characteristic",
                    "@type": "unece:AssociationBIE",
                    "unece:cefactUNId": "UN01002707",
                    "unece:cefactBieDomainClass": "cefact:Agricultural_Produce.Details",
                    "rdfs:comment": "A technical characteristic applicable to this agricultural produce."
                },
                {
                    "@id": "cefact:Agricultural_CountrySub-Division.Applicable.Technical_Characteristic",
                    "@type": "unece:AssociationBIE",
                    "unece:cefactUNId": "UN01002780",
                    "unece:cefactBieDomainClass": "cefact:Agricultural_CountrySubDivision.Details",
                    "rdfs:comment": "A technical characteristic applicable to this agricultural country sub-division."
                },
                {
                    "@id": "cefact:AgriculturalZone_Area.Applicable.Agricultural_Characteristic",
                    "@type": "unece:AssociationBIE",
                    "unece:cefactUNId": "UN01012219",
                    "unece:cefactBieDomainClass": "cefact:AgriculturalZone_Area.Details",
                    "rdfs:comment": "An agricultural characteristic applicable to this agricultural zone area."
                },
                {
                    "@id": "cefact:Agricultural_CropProductionCycle.Applicable.Technical_Characteristic",
                    "@type": "unece:AssociationBIE",
                    "unece:cefactUNId": "UN01002768",
                    "unece:cefactBieDomainClass": "cefact:Agricultural_CropProductionCycle.Details",
                    "rdfs:comment": "A technical characteristic applicable to this agricultural crop production cycle."
                },
                {
                    "@id": "cefact:SPS_Process.Applicable.SPSProcess_Characteristic",
                    "@type": "unece:AssociationBIE",
                    "unece:cefactUNId": "UN03000129",
                    "unece:cefactBieDomainClass": "cefact:SPS_Process.Details",
                    "rdfs:comment": "An SPS process characteristic applicable to this SPS process."
                },
                {
                    "@id": "cefact:Specified_CropProtectionTreatment.Applicable.Sustainability_Characteristic",
                    "@type": "unece:AssociationBIE",
                    "unece:cefactUNId": "UN01014290",
                    "unece:cefactBieDomainClass": "cefact:Specified_CropProtectionTreatment.Details",
                    "rdfs:comment": "A sustainability characteristic applicable to this specified crop protection treatment."
                },
                {
                    "@id": "cefact:AgriculturalInput_Material.Applicable.Agricultural_Characteristic",
                    "@type": "unece:AssociationBIE",
                    "unece:cefactUNId": "UN01012400",
                    "unece:cefactBieDomainClass": "cefact:AgriculturalInput_Material.Details",
                    "rdfs:comment": "An agricultural characteristic applicable to this agricultural input material."
                },
                {
                    "@id": "cefact:Specified_AgriculturalApplication.Applicable.Sustainability_Characteristic",
                    "@type": "unece:AssociationBIE",
                    "unece:cefactUNId": "UN01014276",
                    "unece:cefactBieDomainClass": "cefact:Specified_AgriculturalApplication.Details",
                    "rdfs:comment": "A sustainability characteristic applicable to this agricultural application."
                },
                {
                    "@id": "cefact:CropInput_Batch.Applicable.Technical_Characteristic",
                    "@type": "unece:AssociationBIE",
                    "unece:cefactUNId": "UN01002712",
                    "unece:cefactBieDomainClass": "cefact:CropInput_Batch.Details",
                    "rdfs:comment": "A technical characteristic applicable to this crop input batch."
                },
                {
                    "@id": "cefact:Agricultural_Plot.Applicable.Technical_Characteristic",
                    "@type": "unece:AssociationBIE",
                    "unece:cefactUNId": "UN01002660",
                    "unece:cefactBieDomainClass": "cefact:Agricultural_Plot.Details",
                    "rdfs:comment": "A technical characteristic applicable to this agricultural plot, such as soil acidity or type of soil."
                },
                {
                    "@id": "cefact:AgriculturalInput_Product.Applicable.Agricultural_Characteristic",
                    "@type": "unece:AssociationBIE",
                    "unece:cefactUNId": "UN01012382",
                    "unece:cefactBieDomainClass": "cefact:AgriculturalInput_Product.Details",
                    "rdfs:comment": "An agricultural characteristic applicable to this agricultural input product."
                },
                {
                    "@id": "cefact:Animal_Certificate.Applicable.Sustainability_Characteristic",
                    "@type": "unece:AssociationBIE",
                    "unece:cefactUNId": "UN01013716",
                    "unece:cefactBieDomainClass": "cefact:Animal_Certificate.Details",
                    "rdfs:comment": "A sustainability characteristic applicable to this animal certificate."
                },
                {
                    "@id": "cefact:Plot_SoilOccupation.Applicable.Technical_Characteristic",
                    "@type": "unece:AssociationBIE",
                    "unece:cefactUNId": "UN01002761",
                    "unece:cefactBieDomainClass": "cefact:Plot_SoilOccupation.Details",
                    "rdfs:comment": "A technical characteristic applicable to this plot soil occupation."
                },
                {
                    "@id": "cefact:Plot_AgriculturalProcess.Applicable.Technical_Characteristic",
                    "@type": "unece:AssociationBIE",
                    "unece:cefactUNId": "UN01002796",
                    "unece:cefactBieDomainClass": "cefact:Plot_AgriculturalProcess.Details",
                    "rdfs:comment": "A technical characteristic applicable to this plot agricultural process."
                },
                {
                    "@id": "cefact:Agricultural_Certificate.Applicable.Sustainability_Characteristic",
                    "@type": "unece:AssociationBIE",
                    "unece:cefactUNId": "UN01013706",
                    "unece:cefactBieDomainClass": "cefact:Agricultural_Certificate.Details",
                    "rdfs:comment": "A sustainability characteristic applicable to this agricultural certificate."
                },
                {
                    "@id": "cefact:AgronomicalObservation_Plot.Applicable.Technical_Characteristic",
                    "@type": "unece:AssociationBIE",
                    "unece:cefactUNId": "UN01009375",
                    "unece:cefactBieDomainClass": "cefact:AgronomicalObservation_Plot.Details",
                    "rdfs:comment": "A technical characteristic applicable to this agronomical observation plot."
                }
            ]
        },
        {
            "@id": "agriculture:applicableClassification",
            "@type": "rdf:Property",
            "schema:rangeIncludes": {
                "@id": "agriculture:Classification"
            },
            "schema:domainIncludes": {
                "@id": "agriculture:TradeLineItem"
            },
            "rdfs:comment": "A classification applicable to this SPS trade line item.",
            "rdfs:label": "applicableClassification",
            "unece:cefactElementMetadata": [
                {
                    "@id": "cefact:SPS_TradeLineItem.Applicable.SPS_Classification",
                    "@type": "unece:AssociationBIE",
                    "unece:cefactUNId": "UN03000159",
                    "unece:cefactBieDomainClass": "cefact:SPS_TradeLineItem.Details",
                    "rdfs:comment": "A classification applicable to this SPS trade line item."
                }
            ]
        },
        {
            "@id": "agriculture:applicableContract",
            "@type": "rdf:Property",
            "schema:rangeIncludes": {
                "@id": "agriculture:Contract"
            },
            "schema:domainIncludes": {
                "@id": "agriculture:SoilOccupation"
            },
            "rdfs:comment": "A soil occupation contract applicable to this plot soil occupation.",
            "rdfs:label": "applicableContract",
            "unece:cefactElementMetadata": [
                {
                    "@id": "cefact:Plot_SoilOccupation.Applicable.SoilOccupation_Contract",
                    "@type": "unece:AssociationBIE",
                    "unece:cefactUNId": "UN01002758",
                    "unece:cefactBieDomainClass": "cefact:Plot_SoilOccupation.Details",
                    "rdfs:comment": "A soil occupation contract applicable to this plot soil occupation."
                }
            ]
        },
        {
            "@id": "agriculture:applicableObjectCode",
            "@type": "rdf:Property",
            "schema:rangeIncludes": {
                "@id": "xsd:token"
            },
            "schema:domainIncludes": {
                "@id": "agriculture:Certificate"
            },
            "rdfs:comment": "A code specifying an applicable object, such as item, animal, person or organization, for this agricultural certificate.",
            "rdfs:label": "applicableObjectCode",
            "unece:cefactElementMetadata": [
                {
                    "@id": "cefact:Agricultural_Certificate.Applicable_Object.Code",
                    "@type": "unece:BasicBIE",
                    "unece:cefactUNId": "UN01012286",
                    "unece:cefactBieDomainClass": "cefact:Agricultural_Certificate.Details",
                    "rdfs:comment": "A code specifying an applicable object, such as item, animal, person or organization, for this agricultural certificate."
                }
            ]
        },
        {
            "@id": "agriculture:applicableStandard",
            "@type": "rdf:Property",
            "schema:rangeIncludes": {
                "@id": "agriculture:Standard"
            },
            "schema:domainIncludes": {
                "@id": "agriculture:Certificate"
            },
            "rdfs:comment": [
                "A referenced standard applicable to this agricultural certificate.",
                "A referenced standard applicable to this animal certificate."
            ],
            "rdfs:label": "applicableStandard",
            "unece:cefactElementMetadata": [
                {
                    "@id": "cefact:Agricultural_Certificate.Applicable.Referenced_Standard",
                    "@type": "unece:AssociationBIE",
                    "unece:cefactUNId": "UN01013708",
                    "unece:cefactBieDomainClass": "cefact:Agricultural_Certificate.Details",
                    "rdfs:comment": "A referenced standard applicable to this agricultural certificate."
                },
                {
                    "@id": "cefact:Animal_Certificate.Applicable.Referenced_Standard",
                    "@type": "unece:AssociationBIE",
                    "unece:cefactUNId": "UN01013719",
                    "unece:cefactBieDomainClass": "cefact:Animal_Certificate.Details",
                    "rdfs:comment": "A referenced standard applicable to this animal certificate."
                }
            ]
        },
        {
            "@id": "agriculture:applicationDateTime",
            "@type": "rdf:Property",
            "schema:rangeIncludes": {
                "@id": "xsd:dateTime"
            },
            "schema:domainIncludes": {
                "@id": "agriculture:SoilSupplement"
            },
            "rdfs:comment": "The date or date time value of the application of this specified soil supplement.",
            "rdfs:label": "applicationDateTime",
            "unece:cefactElementMetadata": [
                {
                    "@id": "cefact:Specified_SoilSupplement.Application.DateTime",
                    "@type": "unece:BasicBIE",
                    "unece:cefactUNId": "UN01002720",
                    "unece:cefactBieDomainClass": "cefact:Specified_SoilSupplement.Details",
                    "rdfs:comment": "The date or date time value of the application of this specified soil supplement."
                }
            ]
        },
        {
            "@id": "agriculture:applicationType",
            "@type": "rdf:Property",
            "schema:rangeIncludes": {
                "@id": "xsd:string"
            },
            "schema:domainIncludes": {
                "@id": "agriculture:Grant"
            },
            "rdfs:comment": "The application type, expressed as text, for this animal grant, such as for a bull, heifer or steer.",
            "rdfs:label": "applicationType",
            "unece:cefactElementMetadata": [
                {
                    "@id": "cefact:Animal_Grant.Application_Type.Text",
                    "@type": "unece:BasicBIE",
                    "unece:cefactUNId": "UN01007678",
                    "unece:cefactBieDomainClass": "cefact:Animal_Grant.Details",
                    "rdfs:comment": "The application type, expressed as text, for this animal grant, such as for a bull, heifer or steer."
                }
            ]
        },
        {
            "@id": "agriculture:appliedAdditive",
            "@type": "rdf:Property",
            "schema:rangeIncludes": {
                "@id": "agriculture:Additive"
            },
            "schema:domainIncludes": {
                "@id": "agriculture:SampledObject"
            },
            "rdfs:comment": "An additive applied to this sampled agricultural object.",
            "rdfs:label": "appliedAdditive",
            "unece:cefactElementMetadata": [
                {
                    "@id": "cefact:Agricultural_SampledObject.Applied.SampledObject_Additive",
                    "@type": "unece:AssociationBIE",
                    "unece:cefactUNId": "UN01009635",
                    "unece:cefactBieDomainClass": "cefact:Agricultural_SampledObject.Details",
                    "rdfs:comment": "An additive applied to this sampled agricultural object."
                }
            ]
        },
        {
            "@id": "agriculture:appliedAgriculturalApplication",
            "@type": "rdf:Property",
            "schema:rangeIncludes": {
                "@id": "agriculture:AgriculturalApplication"
            },
            "schema:domainIncludes": [
                {
                    "@id": "agriculture:AgriculturalProcess"
                },
                {
                    "@id": "agriculture:Area"
                },
                {
                    "@id": "agriculture:Batch"
                },
                {
                    "@id": "agriculture:Crop"
                },
                {
                    "@id": "agriculture:Location"
                },
                {
                    "@id": "agriculture:Plot"
                }
            ],
            "rdfs:comment": [
                "A specified agricultural application applied to this agricultural zone area.",
                "A specified agricultural application applied to this crop plot.",
                "A specified agricultural application applied to this product batch.",
                "A specified agricultural application applied to this referenced location.",
                "An agricultural application applied to a crop production agricultural process.",
                "An agricultural application applied to this field crop."
            ],
            "rdfs:label": "appliedAgriculturalApplication",
            "unece:cefactElementMetadata": [
                {
                    "@id": "cefact:Product_Batch.Applied.Specified_AgriculturalApplication",
                    "@type": "unece:AssociationBIE",
                    "unece:cefactUNId": "UN01012358",
                    "unece:cefactBieDomainClass": "cefact:Product_Batch.Details",
                    "rdfs:comment": "A specified agricultural application applied to this product batch."
                },
                {
                    "@id": "cefact:CropProduction_AgriculturalProcess.Applied.Specified_AgriculturalApplication",
                    "@type": "unece:AssociationBIE",
                    "unece:cefactUNId": "UN01012420",
                    "unece:cefactBieDomainClass": "cefact:CropProduction_AgriculturalProcess.Details",
                    "rdfs:comment": "An agricultural application applied to a crop production agricultural process."
                },
                {
                    "@id": "cefact:AgriculturalZone_Area.Applied.Specified_AgriculturalApplication",
                    "@type": "unece:AssociationBIE",
                    "unece:cefactUNId": "UN01012223",
                    "unece:cefactBieDomainClass": "cefact:AgriculturalZone_Area.Details",
                    "rdfs:comment": "A specified agricultural application applied to this agricultural zone area."
                },
                {
                    "@id": "cefact:Crop_Plot.Applied.Specified_AgriculturalApplication",
                    "@type": "unece:AssociationBIE",
                    "unece:cefactUNId": "UN01012153",
                    "unece:cefactBieDomainClass": "cefact:Crop_Plot.Details",
                    "rdfs:comment": "A specified agricultural application applied to this crop plot."
                },
                {
                    "@id": "cefact:Field_Crop.Applied.Specified_AgriculturalApplication",
                    "@type": "unece:AssociationBIE",
                    "unece:cefactUNId": "UN01012319",
                    "unece:cefactBieDomainClass": "cefact:Field_Crop.Details",
                    "rdfs:comment": "An agricultural application applied to this field crop."
                },
                {
                    "@id": "cefact:Referenced_Location.Applied.Specified_AgriculturalApplication",
                    "@type": "unece:AssociationBIE",
                    "unece:cefactUNId": "UN01012161",
                    "unece:cefactBieDomainClass": "cefact:Referenced_Location.Details",
                    "rdfs:comment": "A specified agricultural application applied to this referenced location."
                }
            ]
        },
        {
            "@id": "agriculture:appliedArea",
            "@type": "rdf:Property",
            "schema:rangeIncludes": {
                "@id": "agriculture:Area"
            },
            "schema:domainIncludes": {
                "@id": "agriculture:AgriculturalApplication"
            },
            "rdfs:comment": "A specified agricultural application applied to this agricultural zone area.",
            "rdfs:label": "appliedArea",
            "unece:cefactElementMetadata": [
                {
                    "@id": "cefact:Specified_AgriculturalApplication.Applied.AgriculturalZone_Area",
                    "@type": "unece:AssociationBIE",
                    "unece:cefactUNId": "UN01012425",
                    "unece:cefactBieDomainClass": "cefact:Specified_AgriculturalApplication.Details",
                    "rdfs:comment": "A specified agricultural application applied to this agricultural zone area."
                }
            ]
        },
        {
            "@id": "agriculture:appliedCertificate",
            "@type": "rdf:Property",
            "schema:rangeIncludes": {
                "@id": "agriculture:Certificate"
            },
            "schema:domainIncludes": {
                "@id": "agriculture:AgriculturalApplication"
            },
            "rdfs:comment": "An agricultural certificate applied to this specified agricultural application.",
            "rdfs:label": "appliedCertificate",
            "unece:cefactElementMetadata": [
                {
                    "@id": "cefact:Specified_AgriculturalApplication.Applied.Agricultural_Certificate",
                    "@type": "unece:AssociationBIE",
                    "unece:cefactUNId": "UN01012427",
                    "unece:cefactBieDomainClass": "cefact:Specified_AgriculturalApplication.Details",
                    "rdfs:comment": "An agricultural certificate applied to this specified agricultural application."
                }
            ]
        },
        {
            "@id": "agriculture:appliedChemicalTreatment",
            "@type": "rdf:Property",
            "schema:rangeIncludes": {
                "@id": "agriculture:ChemicalTreatment"
            },
            "schema:domainIncludes": {
                "@id": "agriculture:AgriculturalApplication"
            },
            "rdfs:comment": "A specified chemical treatment applied to this agricultural application.",
            "rdfs:label": "appliedChemicalTreatment",
            "unece:cefactElementMetadata": [
                {
                    "@id": "cefact:Specified_AgriculturalApplication.Applied.Specified_ChemicalTreatment",
                    "@type": "unece:AssociationBIE",
                    "unece:cefactUNId": "UN01014275",
                    "unece:cefactBieDomainClass": "cefact:Specified_AgriculturalApplication.Details",
                    "rdfs:comment": "A specified chemical treatment applied to this agricultural application."
                }
            ]
        },
        {
            "@id": "agriculture:appliedMaterial",
            "@type": "rdf:Property",
            "schema:rangeIncludes": {
                "@id": "agriculture:Material"
            },
            "schema:domainIncludes": {
                "@id": "agriculture:AgriculturalApplication"
            },
            "rdfs:comment": "Specified material applied to this agricultural application.",
            "rdfs:label": "appliedMaterial",
            "unece:cefactElementMetadata": [
                {
                    "@id": "cefact:Specified_AgriculturalApplication.Applied.Specified_Material",
                    "@type": "unece:AssociationBIE",
                    "unece:cefactUNId": "UN01014274",
                    "unece:cefactBieDomainClass": "cefact:Specified_AgriculturalApplication.Details",
                    "rdfs:comment": "Specified material applied to this agricultural application."
                }
            ]
        },
        {
            "@id": "agriculture:appliedProcess",
            "@type": "rdf:Property",
            "schema:rangeIncludes": {
                "@id": "agriculture:Process"
            },
            "schema:domainIncludes": {
                "@id": "agriculture:TradeLineItem"
            },
            "rdfs:comment": "A process applied to this SPS trade line item, such as manufacturing or storage.",
            "rdfs:label": "appliedProcess",
            "unece:cefactElementMetadata": [
                {
                    "@id": "cefact:SPS_TradeLineItem.Applied.SPS_Process",
                    "@type": "unece:AssociationBIE",
                    "unece:cefactUNId": "UN03000164",
                    "unece:cefactBieDomainClass": "cefact:SPS_TradeLineItem.Details",
                    "rdfs:comment": "A process applied to this SPS trade line item, such as manufacturing or storage."
                }
            ]
        },
        {
            "@id": "agriculture:appliedSoilOccupation",
            "@type": "rdf:Property",
            "schema:rangeIncludes": {
                "@id": "agriculture:SoilOccupation"
            },
            "schema:domainIncludes": {
                "@id": "agriculture:Plot"
            },
            "rdfs:comment": "A plot soil occupation applied to this agricultural plot.",
            "rdfs:label": "appliedSoilOccupation",
            "unece:cefactElementMetadata": [
                {
                    "@id": "cefact:Agricultural_Plot.Applied.Plot_SoilOccupation",
                    "@type": "unece:AssociationBIE",
                    "unece:cefactUNId": "UN01002661",
                    "unece:cefactBieDomainClass": "cefact:Agricultural_Plot.Details",
                    "rdfs:comment": "A plot soil occupation applied to this agricultural plot."
                }
            ]
        },
        {
            "@id": "agriculture:appliedSoilSupplement",
            "@type": "rdf:Property",
            "schema:rangeIncludes": {
                "@id": "agriculture:SoilSupplement"
            },
            "schema:domainIncludes": {
                "@id": "agriculture:SoilOccupation"
            },
            "rdfs:comment": "A specified soil supplement applied to this plot soil occupation.",
            "rdfs:label": "appliedSoilSupplement",
            "unece:cefactElementMetadata": [
                {
                    "@id": "cefact:Plot_SoilOccupation.Applied.Specified_SoilSupplement",
                    "@type": "unece:AssociationBIE",
                    "unece:cefactUNId": "UN01002760",
                    "unece:cefactBieDomainClass": "cefact:Plot_SoilOccupation.Details",
                    "rdfs:comment": "A specified soil supplement applied to this plot soil occupation."
                }
            ]
        },
        {
            "@id": "agriculture:appliedSurfaceUnitVolumeMeasure",
            "@type": "rdf:Property",
            "schema:rangeIncludes": {
                "@id": "xsd:decimal"
            },
            "schema:domainIncludes": {
                "@id": "agriculture:CropInput"
            },
            "rdfs:comment": "The measure of the applied per surface unit volume of this agricultural process crop input.",
            "rdfs:label": "appliedSurfaceUnitVolumeMeasure",
            "unece:cefactElementMetadata": [
                {
                    "@id": "cefact:AgriculturalProcess_CropInput.AppliedSurfaceUnit_Volume.Measure",
                    "@type": "unece:BasicBIE",
                    "unece:cefactUNId": "UN01002731",
                    "unece:cefactBieDomainClass": "cefact:AgriculturalProcess_CropInput.Details",
                    "rdfs:comment": "The measure of the applied per surface unit volume of this agricultural process crop input."
                }
            ]
        },
        {
            "@id": "agriculture:appliedTreatment",
            "@type": "rdf:Property",
            "schema:rangeIncludes": {
                "@id": "xsd:string"
            },
            "schema:domainIncludes": {
                "@id": "agriculture:Batch"
            },
            "rdfs:comment": [
                "A treatment, expressed as text, applied to this crop produce batch.",
                "A treatment, expressed as text, applied to this product batch."
            ],
            "rdfs:label": "appliedTreatment",
            "unece:cefactElementMetadata": [
                {
                    "@id": "cefact:Product_Batch.AppliedTreatment.Text",
                    "@type": "unece:BasicBIE",
                    "unece:cefactUNId": "UN01012354",
                    "unece:cefactBieDomainClass": "cefact:Product_Batch.Details",
                    "rdfs:comment": "A treatment, expressed as text, applied to this product batch."
                },
                {
                    "@id": "cefact:CropProduce_Batch.AppliedTreatment.Text",
                    "@type": "unece:BasicBIE",
                    "unece:cefactUNId": "UN01012341",
                    "unece:cefactBieDomainClass": "cefact:CropProduce_Batch.Details",
                    "rdfs:comment": "A treatment, expressed as text, applied to this crop produce batch."
                }
            ]
        },
        {
            "@id": "agriculture:approvalDateTime",
            "@type": "rdf:Property",
            "schema:rangeIncludes": {
                "@id": "xsd:dateTime"
            },
            "schema:domainIncludes": {
                "@id": "agriculture:ExaminationResult"
            },
            "rdfs:comment": "The date for the approval of this animal examination result.",
            "rdfs:label": "approvalDateTime",
            "unece:cefactElementMetadata": [
                {
                    "@id": "cefact:Animal_ExaminationResult.Approval.DateTime",
                    "@type": "unece:BasicBIE",
                    "unece:cefactUNId": "UN01007682",
                    "unece:cefactBieDomainClass": "cefact:Animal_ExaminationResult.Details",
                    "rdfs:comment": "The date for the approval of this animal examination result."
                }
            ]
        },
        {
            "@id": "agriculture:areaMeasure",
            "@type": "rdf:Property",
            "schema:rangeIncludes": {
                "@id": "xsd:decimal"
            },
            "schema:domainIncludes": {
                "@id": "agriculture:Plot"
            },
            "rdfs:comment": "The area measure for this crop plot.",
            "rdfs:label": "areaMeasure",
            "unece:cefactElementMetadata": [
                {
                    "@id": "cefact:Crop_Plot.Area.Measure",
                    "@type": "unece:BasicBIE",
                    "unece:cefactUNId": "UN01012142",
                    "unece:cefactBieDomainClass": "cefact:Crop_Plot.Details",
                    "rdfs:comment": "The area measure for this crop plot."
                }
            ]
        },
        {
            "@id": "agriculture:arrivalLocationId",
            "@type": "rdf:Property",
            "schema:rangeIncludes": {
                "@id": "xsd:token"
            },
            "schema:domainIncludes": {
                "@id": "agriculture:Event"
            },
            "rdfs:comment": "The identifier of the arrival location for this cross border animal movement event.",
            "rdfs:label": "arrivalLocationId",
            "unece:cefactElementMetadata": [
                {
                    "@id": "cefact:CrossBorderAnimalMovement_Event.Arrival_Location.Identifier",
                    "@type": "unece:BasicBIE",
                    "unece:cefactUNId": "UN01007664",
                    "unece:cefactBieDomainClass": "cefact:CrossBorderAnimalMovement_Event.Details",
                    "rdfs:comment": "The identifier of the arrival location for this cross border animal movement event."
                }
            ]
        },
        {
            "@id": "agriculture:arrivalSpecifiedEvent",
            "@type": "rdf:Property",
            "schema:rangeIncludes": {
                "@id": "agriculture:Event"
            },
            "schema:domainIncludes": {
                "@id": "agriculture:Event"
            },
            "rdfs:comment": "The arrival movement event specified for this animal holding event.",
            "rdfs:label": "arrivalSpecifiedEvent",
            "unece:cefactElementMetadata": [
                {
                    "@id": "cefact:AnimalHolding_Event.Arrival_Specified.AnimalMovement_Event",
                    "@type": "unece:AssociationBIE",
                    "unece:cefactUNId": "UN01007636",
                    "unece:cefactBieDomainClass": "cefact:AnimalHolding_Event.Details",
                    "rdfs:comment": "The arrival movement event specified for this animal holding event."
                }
            ]
        },
        {
            "@id": "agriculture:assertedAuthentication",
            "@type": "rdf:Property",
            "schema:rangeIncludes": {
                "@id": "agriculture:Authentication"
            },
            "schema:domainIncludes": {
                "@id": "agriculture:TradeLineItem"
            },
            "rdfs:comment": "An authentication asserted for this SPS trade line item.",
            "rdfs:label": "assertedAuthentication",
            "unece:cefactElementMetadata": [
                {
                    "@id": "cefact:SPS_TradeLineItem.Asserted.SPS_Authentication",
                    "@type": "unece:AssociationBIE",
                    "unece:cefactUNId": "UN03000165",
                    "unece:cefactBieDomainClass": "cefact:SPS_TradeLineItem.Details",
                    "rdfs:comment": "An authentication asserted for this SPS trade line item."
                }
            ]
        },
        {
            "@id": "agriculture:assertion",
            "@type": "rdf:Property",
            "schema:rangeIncludes": {
                "@id": "xsd:string"
            },
            "schema:domainIncludes": {
                "@id": "agriculture:Certification"
            },
            "rdfs:comment": "An assertion, expressed as text, for this animal certification.",
            "rdfs:label": "assertion",
            "unece:cefactElementMetadata": [
                {
                    "@id": "cefact:Animal_Certification.Assertion.Text",
                    "@type": "unece:BasicBIE",
                    "unece:cefactUNId": "UN01013722",
                    "unece:cefactBieDomainClass": "cefact:Animal_Certification.Details",
                    "rdfs:comment": "An assertion, expressed as text, for this animal certification."
                }
            ]
        },
        {
            "@id": "agriculture:assertionCode",
            "@type": "rdf:Property",
            "schema:rangeIncludes": {
                "@id": "xsd:token"
            },
            "schema:domainIncludes": {
                "@id": "agriculture:Certification"
            },
            "rdfs:comment": "The code specifying the assertion, such as a claim that the process is free from child labour, for this animal certification.",
            "rdfs:label": "assertionCode",
            "unece:cefactElementMetadata": [
                {
                    "@id": "cefact:Animal_Certification.Assertion.Code",
                    "@type": "unece:BasicBIE",
                    "unece:cefactUNId": "UN01013721",
                    "unece:cefactBieDomainClass": "cefact:Animal_Certification.Details",
                    "rdfs:comment": "The code specifying the assertion, such as a claim that the process is free from child labour, for this animal certification."
                }
            ]
        },
        {
            "@id": "agriculture:associatedDirectPositionList",
            "@type": "rdf:Property",
            "schema:rangeIncludes": {
                "@id": "agriculture:DirectPositionList"
            },
            "schema:domainIncludes": [
                {
                    "@id": "agriculture:GeographicalLine"
                },
                {
                    "@id": "agriculture:GeographicalMultiCurve"
                },
                {
                    "@id": "agriculture:GeographicalMultiPoint"
                },
                {
                    "@id": "agriculture:GeographicalPoint"
                }
            ],
            "rdfs:comment": [
                "The direct position list associated with this geographical line.",
                "The direct position list associated with this geographical multi-curve.",
                "The direct position list associated with this geographical multi-point.",
                "The direct position list associated with this geographical point."
            ],
            "rdfs:label": "associatedDirectPositionList",
            "unece:cefactElementMetadata": [
                {
                    "@id": "cefact:Specified_GeographicalMulti-Curve.Associated.Specified_DirectPositionList",
                    "@type": "unece:AssociationBIE",
                    "unece:cefactUNId": "UN01012191",
                    "unece:cefactBieDomainClass": "cefact:Specified_GeographicalMultiCurve.Details",
                    "rdfs:comment": "The direct position list associated with this geographical multi-curve."
                },
                {
                    "@id": "cefact:Specified_GeographicalLine.Associated.Specified_DirectPositionList",
                    "@type": "unece:AssociationBIE",
                    "unece:cefactUNId": "UN01012188",
                    "unece:cefactBieDomainClass": "cefact:Specified_GeographicalLine.Details",
                    "rdfs:comment": "The direct position list associated with this geographical line."
                },
                {
                    "@id": "cefact:Specified_GeographicalMulti-Point.Associated.Specified_DirectPositionList",
                    "@type": "unece:AssociationBIE",
                    "unece:cefactUNId": "UN01012184",
                    "unece:cefactBieDomainClass": "cefact:Specified_GeographicalMultiPoint.Details",
                    "rdfs:comment": "The direct position list associated with this geographical multi-point."
                },
                {
                    "@id": "cefact:Specified_GeographicalPoint.Associated.Specified_DirectPositionList",
                    "@type": "unece:AssociationBIE",
                    "unece:cefactUNId": "UN01012181",
                    "unece:cefactBieDomainClass": "cefact:Specified_GeographicalPoint.Details",
                    "rdfs:comment": "The direct position list associated with this geographical point."
                }
            ]
        },
        {
            "@id": "agriculture:associatedDocument",
            "@type": "rdf:Property",
            "schema:rangeIncludes": {
                "@id": "agriculture:Document"
            },
            "schema:domainIncludes": {
                "@id": "agriculture:Animal"
            },
            "rdfs:comment": "An animal passport associated with this livestock animal.",
            "rdfs:label": "associatedDocument",
            "unece:cefactElementMetadata": [
                {
                    "@id": "cefact:Livestock_Animal.Associated.AnimalPassport_Document",
                    "@type": "unece:AssociationBIE",
                    "unece:cefactUNId": "UN01007659",
                    "unece:cefactBieDomainClass": "cefact:Livestock_Animal.Details",
                    "rdfs:comment": "An animal passport associated with this livestock animal."
                }
            ]
        },
        {
            "@id": "agriculture:associatedGeographicalObjectCharacteristic",
            "@type": "rdf:Property",
            "schema:rangeIncludes": {
                "@id": "agriculture:GeographicalObjectCharacteristic"
            },
            "schema:domainIncludes": [
                {
                    "@id": "agriculture:GeographicalGrid"
                },
                {
                    "@id": "agriculture:GeographicalLine"
                },
                {
                    "@id": "agriculture:GeographicalMultiCurve"
                },
                {
                    "@id": "agriculture:GeographicalMultiPoint"
                },
                {
                    "@id": "agriculture:GeographicalMultiSurface"
                },
                {
                    "@id": "agriculture:GeographicalPoint"
                },
                {
                    "@id": "agriculture:GeographicalSurface"
                },
                {
                    "@id": "agriculture:LinearRing"
                },
                {
                    "@id": "agriculture:Polygon"
                }
            ],
            "rdfs:comment": [
                "The geographical object characteristic associated with this geographical grid.",
                "The geographical object characteristic associated with this geographical line.",
                "The geographical object characteristic associated with this geographical multi-curve.",
                "The geographical object characteristic associated with this geographical multi-point.",
                "The geographical object characteristic associated with this geographical multi-surface.",
                "The geographical object characteristic associated with this geographical point.",
                "The geographical object characteristic associated with this geographical surface.",
                "The geographical object characteristic associated with this linear ring.",
                "The geographical object characteristic associated with this specified polygon."
            ],
            "rdfs:label": "associatedGeographicalObjectCharacteristic",
            "unece:cefactElementMetadata": [
                {
                    "@id": "cefact:Specified_GeographicalMulti-Curve.Associated.Specified_GeographicalObjectCharacteristic",
                    "@type": "unece:AssociationBIE",
                    "unece:cefactUNId": "UN01012192",
                    "unece:cefactBieDomainClass": "cefact:Specified_GeographicalMultiCurve.Details",
                    "rdfs:comment": "The geographical object characteristic associated with this geographical multi-curve."
                },
                {
                    "@id": "cefact:Specified_Polygon.Associated.Specified_GeographicalObjectCharacteristic",
                    "@type": "unece:AssociationBIE",
                    "unece:cefactUNId": "UN01012195",
                    "unece:cefactBieDomainClass": "cefact:Specified_Polygon.Details",
                    "rdfs:comment": "The geographical object characteristic associated with this specified polygon."
                },
                {
                    "@id": "cefact:Specified_GeographicalSurface.Associated.Specified_GeographicalObjectCharacteristic",
                    "@type": "unece:AssociationBIE",
                    "unece:cefactUNId": "UN01012200",
                    "unece:cefactBieDomainClass": "cefact:Specified_GeographicalSurface.Details",
                    "rdfs:comment": "The geographical object characteristic associated with this geographical surface."
                },
                {
                    "@id": "cefact:Specified_GeographicalGrid.Associated.Specified_GeographicalObjectCharacteristic",
                    "@type": "unece:AssociationBIE",
                    "unece:cefactUNId": "UN01012211",
                    "unece:cefactBieDomainClass": "cefact:Specified_GeographicalGrid.Details",
                    "rdfs:comment": "The geographical object characteristic associated with this geographical grid."
                },
                {
                    "@id": "cefact:Specified_GeographicalMulti-Point.Associated.Specified_GeographicalObjectCharacteristic",
                    "@type": "unece:AssociationBIE",
                    "unece:cefactUNId": "UN01012185",
                    "unece:cefactBieDomainClass": "cefact:Specified_GeographicalMultiPoint.Details",
                    "rdfs:comment": "The geographical object characteristic associated with this geographical multi-point."
                },
                {
                    "@id": "cefact:Specified_GeographicalMulti-Surface.Associated.Specified_GeographicalObjectCharacteristic",
                    "@type": "unece:AssociationBIE",
                    "unece:cefactUNId": "UN01012197",
                    "unece:cefactBieDomainClass": "cefact:Specified_GeographicalMultiSurface.Details",
                    "rdfs:comment": "The geographical object characteristic associated with this geographical multi-surface."
                },
                {
                    "@id": "cefact:Specified_GeographicalLine.Associated.Specified_GeographicalObjectCharacteristic",
                    "@type": "unece:AssociationBIE",
                    "unece:cefactUNId": "UN01012189",
                    "unece:cefactBieDomainClass": "cefact:Specified_GeographicalLine.Details",
                    "rdfs:comment": "The geographical object characteristic associated with this geographical line."
                },
                {
                    "@id": "cefact:Specified_GeographicalPoint.Associated.Specified_GeographicalObjectCharacteristic",
                    "@type": "unece:AssociationBIE",
                    "unece:cefactUNId": "UN01012182",
                    "unece:cefactBieDomainClass": "cefact:Specified_GeographicalPoint.Details",
                    "rdfs:comment": "The geographical object characteristic associated with this geographical point."
                },
                {
                    "@id": "cefact:Specified_LinearRing.Associated.Specified_GeographicalObjectCharacteristic",
                    "@type": "unece:AssociationBIE",
                    "unece:cefactUNId": "UN01012194",
                    "unece:cefactBieDomainClass": "cefact:Specified_LinearRing.Details",
                    "rdfs:comment": "The geographical object characteristic associated with this linear ring."
                }
            ]
        },
        {
            "@id": "agriculture:associatedTransportEquipment",
            "@type": "rdf:Property",
            "schema:rangeIncludes": {
                "@id": "agriculture:TransportEquipment"
            },
            "schema:domainIncludes": {
                "@id": "agriculture:TradeLineItem"
            },
            "rdfs:comment": "Transport equipment associated with this SPS trade line item.",
            "rdfs:label": "associatedTransportEquipment",
            "unece:cefactElementMetadata": [
                {
                    "@id": "cefact:SPS_TradeLineItem.Associated.SPS_TransportEquipment",
                    "@type": "unece:AssociationBIE",
                    "unece:cefactUNId": "UN03000161",
                    "unece:cefactBieDomainClass": "cefact:SPS_TradeLineItem.Details",
                    "rdfs:comment": "Transport equipment associated with this SPS trade line item."
                }
            ]
        },
        {
            "@id": "agriculture:attachedBinaryFile",
            "@type": "rdf:Property",
            "schema:rangeIncludes": {
                "@id": "agriculture:BinaryFile"
            },
            "schema:domainIncludes": [
                {
                    "@id": "agriculture:Certificate"
                },
                {
                    "@id": "agriculture:Sample"
                }
            ],
            "rdfs:comment": [
                "A binary file attached to this agricultural certificate.",
                "An attached binary file of this agricultural sample."
            ],
            "rdfs:label": "attachedBinaryFile",
            "unece:cefactElementMetadata": [
                {
                    "@id": "cefact:Agricultural_Sample.Attached.Specified_BinaryFile",
                    "@type": "unece:AssociationBIE",
                    "unece:cefactUNId": "UN01010482",
                    "unece:cefactBieDomainClass": "cefact:Agricultural_Sample.Details",
                    "rdfs:comment": "An attached binary file of this agricultural sample."
                },
                {
                    "@id": "cefact:Agricultural_Certificate.Attached.Specified_BinaryFile",
                    "@type": "unece:AssociationBIE",
                    "unece:cefactUNId": "UN01013709",
                    "unece:cefactBieDomainClass": "cefact:Agricultural_Certificate.Details",
                    "rdfs:comment": "A binary file attached to this agricultural certificate."
                }
            ]
        },
        {
            "@id": "agriculture:attachedPicture",
            "@type": "rdf:Property",
            "schema:rangeIncludes": {
                "@id": "agriculture:Picture"
            },
            "schema:domainIncludes": {
                "@id": "agriculture:Sample"
            },
            "rdfs:comment": "An attached photographic picture of this agricultural sample.",
            "rdfs:label": "attachedPicture",
            "unece:cefactElementMetadata": [
                {
                    "@id": "cefact:Agricultural_Sample.Attached.Photographic_Picture",
                    "@type": "unece:AssociationBIE",
                    "unece:cefactUNId": "UN01010481",
                    "unece:cefactBieDomainClass": "cefact:Agricultural_Sample.Details",
                    "rdfs:comment": "An attached photographic picture of this agricultural sample."
                }
            ]
        },
        {
            "@id": "agriculture:attachmentBinaryObject",
            "@type": "rdf:Property",
            "schema:rangeIncludes": {
                "@id": "xsd:base64Binary"
            },
            "schema:domainIncludes": {
                "@id": "agriculture:Document"
            },
            "rdfs:comment": "A binary object that is attached or otherwise appended to this referenced SPS document.",
            "rdfs:label": "attachmentBinaryObject",
            "unece:cefactElementMetadata": [
                {
                    "@id": "cefact:SPSReferenced_Document.Attachment.BinaryObject",
                    "@type": "unece:BasicBIE",
                    "unece:cefactUNId": "UN01007574",
                    "unece:cefactBieDomainClass": "cefact:SPSReferenced_Document.Details",
                    "rdfs:comment": "A binary object that is attached or otherwise appended to this referenced SPS document."
                }
            ]
        },
        {
            "@id": "agriculture:attachmentDateTime",
            "@type": "rdf:Property",
            "schema:rangeIncludes": {
                "@id": "xsd:dateTime"
            },
            "schema:domainIncludes": {
                "@id": "agriculture:Label"
            },
            "rdfs:comment": "The date of attachment of this animal label.",
            "rdfs:label": "attachmentDateTime",
            "unece:cefactElementMetadata": [
                {
                    "@id": "cefact:Animal_Label.Attachment.DateTime",
                    "@type": "unece:BasicBIE",
                    "unece:cefactUNId": "UN01007622",
                    "unece:cefactBieDomainClass": "cefact:Animal_Label.Details",
                    "rdfs:comment": "The date of attachment of this animal label."
                }
            ]
        },
        {
            "@id": "agriculture:attainedQualification",
            "@type": "rdf:Property",
            "schema:rangeIncludes": {
                "@id": "agriculture:Qualification"
            },
            "schema:domainIncludes": {
                "@id": "agriculture:Person"
            },
            "rdfs:comment": [
                "An academic qualification attained by this SPS person.",
                "The specified qualification attained by this inspection person."
            ],
            "rdfs:label": "attainedQualification",
            "unece:cefactElementMetadata": [
                {
                    "@id": "cefact:SPS_Person.Attained.SPS_Qualification",
                    "@type": "unece:AssociationBIE",
                    "unece:cefactUNId": "UN03000125",
                    "unece:cefactBieDomainClass": "cefact:SPS_Person.Details",
                    "rdfs:comment": "An academic qualification attained by this SPS person."
                },
                {
                    "@id": "cefact:Inspection_Person.Attained.Specified_Qualification",
                    "@type": "unece:AssociationBIE",
                    "unece:cefactUNId": "UN01007691",
                    "unece:cefactBieDomainClass": "cefact:Inspection_Person.Details",
                    "rdfs:comment": "The specified qualification attained by this inspection person."
                }
            ]
        },
        {
            "@id": "agriculture:authorizedParty",
            "@type": "rdf:Property",
            "schema:rangeIncludes": {
                "@id": "agriculture:Party"
            },
            "schema:domainIncludes": {
                "@id": "agriculture:SampledObject"
            },
            "rdfs:comment": "A party authorized to do something concerning this sampled agricultural object.",
            "rdfs:label": "authorizedParty",
            "unece:cefactElementMetadata": [
                {
                    "@id": "cefact:Agricultural_SampledObject.Authorized.LaboratoryObservation_Party",
                    "@type": "unece:AssociationBIE",
                    "unece:cefactUNId": "UN01009627",
                    "unece:cefactBieDomainClass": "cefact:Agricultural_SampledObject.Details",
                    "rdfs:comment": "A party authorized to do something concerning this sampled agricultural object."
                }
            ]
        },
        {
            "@id": "agriculture:availabilityDueDateTime",
            "@type": "rdf:Property",
            "schema:rangeIncludes": {
                "@id": "xsd:dateTime"
            },
            "schema:domainIncludes": {
                "@id": "agriculture:Consignment"
            },
            "rdfs:comment": "The date, time, date time, or other date time value when this SPS consignment is due to be available.",
            "rdfs:label": "availabilityDueDateTime",
            "unece:cefactElementMetadata": [
                {
                    "@id": "cefact:SPS_Consignment.AvailabilityDue.DateTime",
                    "@type": "unece:BasicBIE",
                    "unece:TDED": "2111",
                    "unece:cefactUNId": "UN03000055",
                    "unece:cefactBieDomainClass": "cefact:SPS_Consignment.Details",
                    "rdfs:comment": "The date, time, date time, or other date time value when this SPS consignment is due to be available."
                }
            ]
        },
        {
            "@id": "agriculture:awardedGrant",
            "@type": "rdf:Property",
            "schema:rangeIncludes": {
                "@id": "agriculture:Grant"
            },
            "schema:domainIncludes": {
                "@id": "agriculture:Animal"
            },
            "rdfs:comment": "A grant awarded for this livestock animal.",
            "rdfs:label": "awardedGrant",
            "unece:cefactElementMetadata": [
                {
                    "@id": "cefact:Livestock_Animal.Awarded.Animal_Grant",
                    "@type": "unece:AssociationBIE",
                    "unece:cefactUNId": "UN01007658",
                    "unece:cefactBieDomainClass": "cefact:Livestock_Animal.Details",
                    "rdfs:comment": "A grant awarded for this livestock animal."
                }
            ]
        },
        {
            "@id": "agriculture:awardingParty",
            "@type": "rdf:Property",
            "schema:rangeIncludes": {
                "@id": "agriculture:Party"
            },
            "schema:domainIncludes": {
                "@id": "agriculture:Grant"
            },
            "rdfs:comment": "The party that awards this animal grant.",
            "rdfs:label": "awardingParty",
            "unece:cefactElementMetadata": [
                {
                    "@id": "cefact:Animal_Grant.Awarding.Specified_Party",
                    "@type": "unece:AssociationBIE",
                    "unece:cefactUNId": "UN01007679",
                    "unece:cefactBieDomainClass": "cefact:Animal_Grant.Details",
                    "rdfs:comment": "The party that awards this animal grant."
                }
            ]
        },
        {
            "@id": "agriculture:axisLabelList",
            "@type": "rdf:Property",
            "schema:rangeIncludes": {
                "@id": "xsd:string"
            },
            "schema:domainIncludes": {
                "@id": "agriculture:DirectPositionList"
            },
            "rdfs:comment": "An ordered list of axis labels, expressed as text, for this specified direct position list.",
            "rdfs:label": "axisLabelList",
            "unece:cefactElementMetadata": [
                {
                    "@id": "cefact:Specified_DirectPositionList.Axis_LabelList.Text",
                    "@type": "unece:BasicBIE",
                    "unece:cefactUNId": "UN01012475",
                    "unece:cefactBieDomainClass": "cefact:Specified_DirectPositionList.Details",
                    "rdfs:comment": "An ordered list of axis labels, expressed as text, for this specified direct position list."
                }
            ]
        },
        {
            "@id": "agriculture:axisName",
            "@type": "rdf:Property",
            "schema:rangeIncludes": {
                "@id": "xsd:string"
            },
            "schema:domainIncludes": {
                "@id": "agriculture:GeographicalGrid"
            },
            "rdfs:comment": "An axis name, expressed as text, for this geographical grid.",
            "rdfs:label": "axisName",
            "unece:cefactElementMetadata": [
                {
                    "@id": "cefact:Specified_GeographicalGrid.Axis_Name.Text",
                    "@type": "unece:BasicBIE",
                    "unece:cefactUNId": "UN01012209",
                    "unece:cefactBieDomainClass": "cefact:Specified_GeographicalGrid.Details",
                    "rdfs:comment": "An axis name, expressed as text, for this geographical grid."
                }
            ]
        },
        {
            "@id": "agriculture:batchIdentificationId",
            "@type": "rdf:Property",
            "schema:rangeIncludes": {
                "@id": "xsd:token"
            },
            "schema:domainIncludes": {
                "@id": "agriculture:SampledObject"
            },
            "rdfs:comment": "The identifier of this sampled agricultural object batch.",
            "rdfs:label": "batchIdentificationId",
            "unece:cefactElementMetadata": [
                {
                    "@id": "cefact:Agricultural_SampledObject.BatchIdentification.Identifier",
                    "@type": "unece:BasicBIE",
                    "unece:cefactUNId": "UN01009624",
                    "unece:cefactBieDomainClass": "cefact:Agricultural_SampledObject.Details",
                    "rdfs:comment": "The identifier of this sampled agricultural object batch."
                }
            ]
        },
        {
            "@id": "agriculture:batchPopulationSizeMeasure",
            "@type": "rdf:Property",
            "schema:rangeIncludes": {
                "@id": "xsd:decimal"
            },
            "schema:domainIncludes": {
                "@id": "agriculture:SampledObject"
            },
            "rdfs:comment": "The measure of the population size of this sampled agricultural object.",
            "rdfs:label": "batchPopulationSizeMeasure",
            "unece:cefactElementMetadata": [
                {
                    "@id": "cefact:Agricultural_SampledObject.Batch_PopulationSize.Measure",
                    "@type": "unece:BasicBIE",
                    "unece:cefactUNId": "UN01009622",
                    "unece:cefactBieDomainClass": "cefact:Agricultural_SampledObject.Details",
                    "rdfs:comment": "The measure of the population size of this sampled agricultural object."
                }
            ]
        },
        {
            "@id": "agriculture:batchQuantity",
            "@type": "rdf:Property",
            "schema:rangeIncludes": {
                "@id": "xsd:decimal"
            },
            "schema:domainIncludes": {
                "@id": "agriculture:SampledObject"
            },
            "rdfs:comment": "The batch quantity for this sampled agricultural object.",
            "rdfs:label": "batchQuantity",
            "unece:cefactElementMetadata": [
                {
                    "@id": "cefact:Agricultural_SampledObject.Batch.Quantity",
                    "@type": "unece:BasicBIE",
                    "unece:cefactUNId": "UN01009621",
                    "unece:cefactBieDomainClass": "cefact:Agricultural_SampledObject.Details",
                    "rdfs:comment": "The batch quantity for this sampled agricultural object."
                }
            ]
        },
        {
            "@id": "agriculture:birthDateTime",
            "@type": "rdf:Property",
            "schema:rangeIncludes": {
                "@id": "xsd:dateTime"
            },
            "schema:domainIncludes": {
                "@id": "agriculture:Animal"
            },
            "rdfs:comment": "The date of birth for this livestock animal.",
            "rdfs:label": "birthDateTime",
            "unece:cefactElementMetadata": [
                {
                    "@id": "cefact:Livestock_Animal.Birth.DateTime",
                    "@type": "unece:BasicBIE",
                    "unece:cefactUNId": "UN01007644",
                    "unece:cefactBieDomainClass": "cefact:Livestock_Animal.Details",
                    "rdfs:comment": "The date of birth for this livestock animal."
                }
            ]
        },
        {
            "@id": "agriculture:botanicalGenusCode",
            "@type": "rdf:Property",
            "schema:rangeIncludes": {
                "@id": "xsd:token"
            },
            "schema:domainIncludes": {
                "@id": "agriculture:Crop"
            },
            "rdfs:comment": "The code specifying the genus for this botanical crop.",
            "rdfs:label": "botanicalGenusCode",
            "unece:cefactElementMetadata": [
                {
                    "@id": "cefact:Botanical_Crop.BotanicalGenus.Code",
                    "@type": "unece:BasicBIE",
                    "unece:cefactUNId": "UN01012293",
                    "unece:cefactBieDomainClass": "cefact:Botanical_Crop.Details",
                    "rdfs:comment": "The code specifying the genus for this botanical crop."
                }
            ]
        },
        {
            "@id": "agriculture:botanicalIdentificationId",
            "@type": "rdf:Property",
            "schema:rangeIncludes": {
                "@id": "xsd:token"
            },
            "schema:domainIncludes": {
                "@id": "agriculture:Crop"
            },
            "rdfs:comment": "The identifier for this botanical crop.",
            "rdfs:label": "botanicalIdentificationId",
            "unece:cefactElementMetadata": [
                {
                    "@id": "cefact:Botanical_Crop.BotanicalIdentification.Identifier",
                    "@type": "unece:BasicBIE",
                    "unece:cefactUNId": "UN01012290",
                    "unece:cefactBieDomainClass": "cefact:Botanical_Crop.Details",
                    "rdfs:comment": "The identifier for this botanical crop."
                }
            ]
        },
        {
            "@id": "agriculture:botanicalName",
            "@type": "rdf:Property",
            "schema:rangeIncludes": {
                "@id": "xsd:string"
            },
            "schema:domainIncludes": {
                "@id": "agriculture:Crop"
            },
            "rdfs:comment": "The botanical name, expressed as text, for this botanical crop.",
            "rdfs:label": "botanicalName",
            "unece:cefactElementMetadata": [
                {
                    "@id": "cefact:Botanical_Crop.BotanicalName.Text",
                    "@type": "unece:BasicBIE",
                    "unece:cefactUNId": "UN01012294",
                    "unece:cefactBieDomainClass": "cefact:Botanical_Crop.Details",
                    "rdfs:comment": "The botanical name, expressed as text, for this botanical crop."
                }
            ]
        },
        {
            "@id": "agriculture:botanicalSpeciesCode",
            "@type": "rdf:Property",
            "schema:rangeIncludes": {
                "@id": "xsd:token"
            },
            "schema:domainIncludes": {
                "@id": "agriculture:Crop"
            },
            "rdfs:comment": [
                "The code specifying the botanical species for this agricultural crop.",
                "The code specifying the species for this botanical crop."
            ],
            "rdfs:label": "botanicalSpeciesCode",
            "unece:cefactElementMetadata": [
                {
                    "@id": "cefact:Agricultural_Crop.BotanicalSpecies.Code",
                    "@type": "unece:BasicBIE",
                    "unece:cefactUNId": "UN01002686",
                    "unece:cefactBieDomainClass": "cefact:Agricultural_Crop.Details",
                    "rdfs:comment": "The code specifying the botanical species for this agricultural crop."
                },
                {
                    "@id": "cefact:Botanical_Crop.BotanicalSpecies.Code",
                    "@type": "unece:BasicBIE",
                    "unece:cefactUNId": "UN01012291",
                    "unece:cefactBieDomainClass": "cefact:Botanical_Crop.Details",
                    "rdfs:comment": "The code specifying the species for this botanical crop."
                }
            ]
        },
        {
            "@id": "agriculture:boundaryGeographicalCoordinate",
            "@type": "rdf:Property",
            "schema:rangeIncludes": {
                "@id": "agriculture:GeographicalCoordinate"
            },
            "schema:domainIncludes": {
                "@id": "agriculture:Area"
            },
            "rdfs:comment": "A specified geographical coordinate of the boundary for this agricultural area.",
            "rdfs:label": "boundaryGeographicalCoordinate",
            "unece:cefactElementMetadata": [
                {
                    "@id": "cefact:Agricultural_Area.Boundary.Specified_GeographicalCoordinate",
                    "@type": "unece:AssociationBIE",
                    "unece:cefactUNId": "UN01002674",
                    "unece:cefactBieDomainClass": "cefact:Agricultural_Area.Details",
                    "rdfs:comment": "A specified geographical coordinate of the boundary for this agricultural area."
                }
            ]
        },
        {
            "@id": "agriculture:breakUpDateTime",
            "@type": "rdf:Property",
            "schema:rangeIncludes": {
                "@id": "xsd:dateTime"
            },
            "schema:domainIncludes": {
                "@id": "agriculture:Batch"
            },
            "rdfs:comment": [
                "The date, time, date time, or other date time value of the break up of this animal batch.",
                "The date, time, date time, or other date time value of the break up of this crop produce batch."
            ],
            "rdfs:label": "breakUpDateTime",
            "unece:cefactElementMetadata": [
                {
                    "@id": "cefact:Animal_Batch.BreakUp.DateTime",
                    "@type": "unece:BasicBIE",
                    "unece:cefactUNId": "UN01011247",
                    "unece:cefactBieDomainClass": "cefact:Animal_Batch.Details",
                    "rdfs:comment": "The date, time, date time, or other date time value of the break up of this animal batch."
                },
                {
                    "@id": "cefact:CropProduce_Batch.BreakUp.DateTime",
                    "@type": "unece:BasicBIE",
                    "unece:cefactUNId": "UN01012334",
                    "unece:cefactBieDomainClass": "cefact:CropProduce_Batch.Details",
                    "rdfs:comment": "The date, time, date time, or other date time value of the break up of this crop produce batch."
                }
            ]
        },
        {
            "@id": "agriculture:bufferCapacityMeasure",
            "@type": "rdf:Property",
            "schema:rangeIncludes": {
                "@id": "xsd:decimal"
            },
            "schema:domainIncludes": {
                "@id": "agriculture:Construction"
            },
            "rdfs:comment": "The measure of the buffer capacity for this agricultural construction.",
            "rdfs:label": "bufferCapacityMeasure",
            "unece:cefactElementMetadata": [
                {
                    "@id": "cefact:Agricultural_Construction.Buffer_Capacity.Measure",
                    "@type": "unece:BasicBIE",
                    "unece:cefactUNId": "UN01012240",
                    "unece:cefactBieDomainClass": "cefact:Agricultural_Construction.Details",
                    "rdfs:comment": "The measure of the buffer capacity for this agricultural construction."
                }
            ]
        },
        {
            "@id": "agriculture:buyerParty",
            "@type": "rdf:Property",
            "schema:rangeIncludes": {
                "@id": "agriculture:Party"
            },
            "schema:domainIncludes": {
                "@id": "agriculture:Contract"
            },
            "rdfs:comment": "The buyer party for this agricultural contract.",
            "rdfs:label": "buyerParty",
            "unece:cefactElementMetadata": [
                {
                    "@id": "cefact:Agricultural_Contract.Buyer.Specified_Party",
                    "@type": "unece:AssociationBIE",
                    "unece:cefactUNId": "UN01012448",
                    "unece:cefactBieDomainClass": "cefact:Agricultural_Contract.Details",
                    "rdfs:comment": "The buyer party for this agricultural contract."
                }
            ]
        },
        {
            "@id": "agriculture:cAPId",
            "@type": "rdf:Property",
            "schema:rangeIncludes": {
                "@id": "xsd:token"
            },
            "schema:domainIncludes": {
                "@id": "agriculture:Plot"
            },
            "rdfs:comment": "The Common Agricultural Policy (CAP) identifier for this agricultural plot.",
            "rdfs:label": "cAPId",
            "unece:cefactElementMetadata": [
                {
                    "@id": "cefact:Agricultural_Plot.CAP_Identification.Identifier",
                    "@type": "unece:BasicBIE",
                    "unece:cefactUNId": "UN01009352",
                    "unece:cefactBieDomainClass": "cefact:Agricultural_Plot.Details",
                    "rdfs:comment": "The Common Agricultural Policy (CAP) identifier for this agricultural plot."
                }
            ]
        },
        {
            "@id": "agriculture:calculatedYieldMeasure",
            "@type": "rdf:Property",
            "schema:rangeIncludes": {
                "@id": "xsd:decimal"
            },
            "schema:domainIncludes": {
                "@id": "agriculture:Produce"
            },
            "rdfs:comment": [
                "A measure of the calculated yield, such as weight per surface area unit, of this crop produce.",
                "The measure of the calculated yield of this agricultural produce, such as weight per surface area unit."
            ],
            "rdfs:label": "calculatedYieldMeasure",
            "unece:cefactElementMetadata": [
                {
                    "@id": "cefact:Crop_Produce.Calculated_Yield.Measure",
                    "@type": "unece:BasicBIE",
                    "unece:cefactUNId": "UN01013743",
                    "unece:cefactBieDomainClass": "cefact:Crop_Produce.Details",
                    "rdfs:comment": "A measure of the calculated yield, such as weight per surface area unit, of this crop produce."
                },
                {
                    "@id": "cefact:Agricultural_Produce.Calculated_Yield.Measure",
                    "@type": "unece:BasicBIE",
                    "unece:cefactUNId": "UN01002705",
                    "unece:cefactBieDomainClass": "cefact:Agricultural_Produce.Details",
                    "rdfs:comment": "The measure of the calculated yield of this agricultural produce, such as weight per surface area unit."
                }
            ]
        },
        {
            "@id": "agriculture:capacityMeasure",
            "@type": "rdf:Property",
            "schema:rangeIncludes": {
                "@id": "xsd:decimal"
            },
            "schema:domainIncludes": {
                "@id": "agriculture:Construction"
            },
            "rdfs:comment": "A measure of the capacity of this agricultural construction, such as the number of horses in a stable or the quantity of grain in a silo.",
            "rdfs:label": "capacityMeasure",
            "unece:cefactElementMetadata": [
                {
                    "@id": "cefact:Agricultural_Construction.Capacity.Measure",
                    "@type": "unece:BasicBIE",
                    "unece:cefactUNId": "UN01012237",
                    "unece:cefactBieDomainClass": "cefact:Agricultural_Construction.Details",
                    "rdfs:comment": "A measure of the capacity of this agricultural construction, such as the number of horses in a stable or the quantity of grain in a silo."
                }
            ]
        },
        {
            "@id": "agriculture:cargoTypeClassificationCode",
            "@type": "rdf:Property",
            "schema:rangeIncludes": {
                "@id": "unece:UNECECL7085Code"
            },
            "schema:domainIncludes": {
                "@id": "agriculture:Cargo"
            },
            "rdfs:comment": "The code specifying the type of SPS cargo, such as a UNECE Recommendation 21 single digit code.",
            "rdfs:label": "cargoTypeClassificationCode",
            "unece:cefactElementMetadata": [
                {
                    "@id": "cefact:SPS_Cargo.Type.Code",
                    "@type": "unece:BasicBIE",
                    "unece:TDED": "7085",
                    "unece:cefactUNId": "UN03000041",
                    "unece:cefactBieDomainClass": "cefact:SPS_Cargo.Details",
                    "rdfs:comment": "The code specifying the type of SPS cargo, such as a UNECE Recommendation 21 single digit code."
                }
            ]
        },
        {
            "@id": "agriculture:carrierParty",
            "@type": "rdf:Property",
            "schema:rangeIncludes": {
                "@id": "agriculture:Party"
            },
            "schema:domainIncludes": [
                {
                    "@id": "agriculture:Consignment"
                },
                {
                    "@id": "agriculture:SampledObject"
                }
            ],
            "rdfs:comment": [
                "The carrier party for this sampled agricultural object.",
                "The carrier party of this SPS consignment."
            ],
            "rdfs:label": "carrierParty",
            "unece:cefactElementMetadata": [
                {
                    "@id": "cefact:SPS_Consignment.Carrier.SPS_Party",
                    "@type": "unece:AssociationBIE",
                    "unece:cefactUNId": "UN03000070",
                    "unece:cefactBieDomainClass": "cefact:SPS_Consignment.Details",
                    "rdfs:comment": "The carrier party of this SPS consignment."
                },
                {
                    "@id": "cefact:Agricultural_SampledObject.Carrier.LaboratoryObservation_Party",
                    "@type": "unece:AssociationBIE",
                    "unece:cefactUNId": "UN01009629",
                    "unece:cefactBieDomainClass": "cefact:Agricultural_SampledObject.Details",
                    "rdfs:comment": "The carrier party for this sampled agricultural object."
                }
            ]
        },
        {
            "@id": "agriculture:categoryCode",
            "@type": "rdf:Property",
            "schema:rangeIncludes": {
                "@id": "xsd:token"
            },
            "schema:domainIncludes": {
                "@id": "agriculture:ProtectionMeans"
            },
            "rdfs:comment": "The code specifying the category of disease protection means.",
            "rdfs:label": "categoryCode",
            "unece:cefactElementMetadata": [
                {
                    "@id": "cefact:Disease_ProtectionMeans.Category.Code",
                    "@type": "unece:BasicBIE",
                    "unece:cefactUNId": "UN01015110",
                    "unece:cefactBieDomainClass": "cefact:Disease_ProtectionMeans.Details",
                    "rdfs:comment": "The code specifying the category of disease protection means."
                }
            ]
        },
        {
            "@id": "agriculture:cell",
            "@type": "rdf:Property",
            "schema:rangeIncludes": {
                "@id": "xsd:string"
            },
            "schema:domainIncludes": {
                "@id": "agriculture:GeographicalGrid"
            },
            "rdfs:comment": "The cell value, expressed as text, for this geographical grid.",
            "rdfs:label": "cell",
            "unece:cefactElementMetadata": [
                {
                    "@id": "cefact:Specified_GeographicalGrid.Cell.Text",
                    "@type": "unece:BasicBIE",
                    "unece:cefactUNId": "UN01012203",
                    "unece:cefactBieDomainClass": "cefact:Specified_GeographicalGrid.Details",
                    "rdfs:comment": "The cell value, expressed as text, for this geographical grid."
                }
            ]
        },
        {
            "@id": "agriculture:certificationCode",
            "@type": "rdf:Property",
            "schema:rangeIncludes": {
                "@id": "xsd:token"
            },
            "schema:domainIncludes": {
                "@id": "agriculture:Construction"
            },
            "rdfs:comment": "A code specifying a certification for this agricultural construction.",
            "rdfs:label": "certificationCode",
            "unece:cefactElementMetadata": [
                {
                    "@id": "cefact:Agricultural_Construction.Certification.Code",
                    "@type": "unece:BasicBIE",
                    "unece:cefactUNId": "UN01012232",
                    "unece:cefactBieDomainClass": "cefact:Agricultural_Construction.Details",
                    "rdfs:comment": "A code specifying a certification for this agricultural construction."
                }
            ]
        },
        {
            "@id": "agriculture:characteristicValue",
            "@type": "rdf:Property",
            "schema:rangeIncludes": {
                "@id": "xsd:string"
            },
            "schema:domainIncludes": {
                "@id": "agriculture:WeatherCondition"
            },
            "rdfs:comment": "A characteristic value, expressed as text, for this agricultural extreme weather condition.",
            "rdfs:label": "characteristicValue",
            "unece:cefactElementMetadata": [
                {
                    "@id": "cefact:AgriculturalExtreme_WeatherCondition.Characteristic_Value.Text",
                    "@type": "unece:BasicBIE",
                    "unece:cefactUNId": "UN01012453",
                    "unece:cefactBieDomainClass": "cefact:AgriculturalExtreme_WeatherCondition.Details",
                    "rdfs:comment": "A characteristic value, expressed as text, for this agricultural extreme weather condition."
                }
            ]
        },
        {
            "@id": "agriculture:characteristicValueCode",
            "@type": "rdf:Property",
            "schema:rangeIncludes": {
                "@id": "xsd:token"
            },
            "schema:domainIncludes": {
                "@id": "agriculture:WeatherCondition"
            },
            "rdfs:comment": "A code specifying a characteristic value for this agricultural extreme weather condition.",
            "rdfs:label": "characteristicValueCode",
            "unece:cefactElementMetadata": [
                {
                    "@id": "cefact:AgriculturalExtreme_WeatherCondition.Characteristic_Value.Code",
                    "@type": "unece:BasicBIE",
                    "unece:cefactUNId": "UN01012452",
                    "unece:cefactBieDomainClass": "cefact:AgriculturalExtreme_WeatherCondition.Details",
                    "rdfs:comment": "A code specifying a characteristic value for this agricultural extreme weather condition."
                }
            ]
        },
        {
            "@id": "agriculture:cityId",
            "@type": "rdf:Property",
            "schema:rangeIncludes": {
                "@id": "xsd:token"
            },
            "schema:domainIncludes": {
                "@id": "agriculture:Address"
            },
            "rdfs:comment": "The identifier of the city for this SPS address, such as a United Nations Location Code (UNLOCODE) or GS1 Global Location Number (GLN).",
            "rdfs:label": "cityId",
            "unece:cefactElementMetadata": [
                {
                    "@id": "cefact:SPS_Address.City.Identifier",
                    "@type": "unece:BasicBIE",
                    "unece:cefactUNId": "UN03000032",
                    "unece:cefactBieDomainClass": "cefact:SPS_Address.Details",
                    "rdfs:comment": "The identifier of the city for this SPS address, such as a United Nations Location Code (UNLOCODE) or GS1 Global Location Number (GLN)."
                }
            ]
        },
        {
            "@id": "agriculture:cityName",
            "@type": "rdf:Property",
            "schema:rangeIncludes": {
                "@id": "xsd:string"
            },
            "schema:domainIncludes": {
                "@id": "agriculture:Address"
            },
            "rdfs:comment": "The name, expressed as text, of the city, town or village in this SPS address.",
            "rdfs:label": "cityName",
            "unece:cefactElementMetadata": [
                {
                    "@id": "cefact:SPS_Address.CityName.Text",
                    "@type": "unece:BasicBIE",
                    "unece:TDED": "3164",
                    "unece:cefactUNId": "UN03000026",
                    "unece:cefactBieDomainClass": "cefact:SPS_Address.Details",
                    "rdfs:comment": "The name, expressed as text, of the city, town or village in this SPS address."
                }
            ]
        },
        {
            "@id": "agriculture:classCode",
            "@type": "rdf:Property",
            "schema:rangeIncludes": {
                "@id": "xsd:token"
            },
            "schema:domainIncludes": {
                "@id": "agriculture:Classification"
            },
            "rdfs:comment": [
                "The code specifying the class for this SPS classification.",
                "The code specifying the class for this specified classification."
            ],
            "rdfs:label": "classCode",
            "unece:cefactElementMetadata": [
                {
                    "@id": "cefact:SPS_Classification.Class.Code",
                    "@type": "unece:BasicBIE",
                    "unece:TDED": "9021",
                    "unece:cefactUNId": "UN03000045",
                    "unece:cefactBieDomainClass": "cefact:SPS_Classification.Details",
                    "rdfs:comment": "The code specifying the class for this SPS classification."
                },
                {
                    "@id": "cefact:Specified_Classification.Class.Code",
                    "@type": "unece:BasicBIE",
                    "unece:cefactUNId": "UN01007618",
                    "unece:cefactBieDomainClass": "cefact:Specified_Classification.Details",
                    "rdfs:comment": "The code specifying the class for this specified classification."
                }
            ]
        },
        {
            "@id": "agriculture:className",
            "@type": "rdf:Property",
            "schema:rangeIncludes": {
                "@id": "xsd:string"
            },
            "schema:domainIncludes": [
                {
                    "@id": "agriculture:Classification"
                },
                {
                    "@id": "agriculture:Crop"
                }
            ],
            "rdfs:comment": [
                "A class name, expressed as text, for this SPS classification.",
                "The class name, expressed as a text, for this field crop.",
                "The class name, expressed as text, for this specified classification."
            ],
            "rdfs:label": "className",
            "unece:cefactElementMetadata": [
                {
                    "@id": "cefact:SPS_Classification.ClassName.Text",
                    "@type": "unece:BasicBIE",
                    "unece:TDED": "9020",
                    "unece:cefactUNId": "UN03000046",
                    "unece:cefactBieDomainClass": "cefact:SPS_Classification.Details",
                    "rdfs:comment": "A class name, expressed as text, for this SPS classification."
                },
                {
                    "@id": "cefact:Specified_Classification.ClassName.Text",
                    "@type": "unece:BasicBIE",
                    "unece:cefactUNId": "UN01007619",
                    "unece:cefactBieDomainClass": "cefact:Specified_Classification.Details",
                    "rdfs:comment": "The class name, expressed as text, for this specified classification."
                },
                {
                    "@id": "cefact:Field_Crop.ClassName.Text",
                    "@type": "unece:BasicBIE",
                    "unece:cefactUNId": "UN01012308",
                    "unece:cefactBieDomainClass": "cefact:Field_Crop.Details",
                    "rdfs:comment": "The class name, expressed as a text, for this field crop."
                }
            ]
        },
        {
            "@id": "agriculture:classificationCode",
            "@type": "rdf:Property",
            "schema:rangeIncludes": {
                "@id": "xsd:token"
            },
            "schema:domainIncludes": [
                {
                    "@id": "agriculture:Crop"
                },
                {
                    "@id": "agriculture:Party"
                }
            ],
            "rdfs:comment": [
                "A code specifying a classification for this agricultural producer party.",
                "A code specifying a classification for this field crop."
            ],
            "rdfs:label": "classificationCode",
            "unece:cefactElementMetadata": [
                {
                    "@id": "cefact:AgriculturalProducer_Party.Classification.Code",
                    "@type": "unece:BasicBIE",
                    "unece:cefactUNId": "UN01012262",
                    "unece:cefactBieDomainClass": "cefact:AgriculturalProducer_Party.Details",
                    "rdfs:comment": "A code specifying a classification for this agricultural producer party."
                },
                {
                    "@id": "cefact:Field_Crop.Classification.Code",
                    "@type": "unece:BasicBIE",
                    "unece:cefactUNId": "UN01012301",
                    "unece:cefactBieDomainClass": "cefact:Field_Crop.Details",
                    "rdfs:comment": "A code specifying a classification for this field crop."
                }
            ]
        },
        {
            "@id": "agriculture:classificationId",
            "@type": "rdf:Property",
            "schema:rangeIncludes": {
                "@id": "xsd:token"
            },
            "schema:domainIncludes": {
                "@id": "agriculture:Material"
            },
            "rdfs:comment": "An identifier for the classification of this agricultural input material.",
            "rdfs:label": "classificationId",
            "unece:cefactElementMetadata": [
                {
                    "@id": "cefact:AgriculturalInput_Material.Classification.Identifier",
                    "@type": "unece:BasicBIE",
                    "unece:cefactUNId": "UN01012394",
                    "unece:cefactBieDomainClass": "cefact:AgriculturalInput_Material.Details",
                    "rdfs:comment": "An identifier for the classification of this agricultural input material."
                }
            ]
        },
        {
            "@id": "agriculture:closedIndicator",
            "@type": "rdf:Property",
            "schema:rangeIncludes": {
                "@id": "xsd:boolean"
            },
            "schema:domainIncludes": {
                "@id": "agriculture:Issue"
            },
            "rdfs:comment": "The indication of whether or not this complaint issue has been closed.",
            "rdfs:label": "closedIndicator",
            "unece:cefactElementMetadata": [
                {
                    "@id": "cefact:Complaint_Issue.Closed.Indicator",
                    "@type": "unece:BasicBIE",
                    "unece:cefactUNId": "UN01012271",
                    "unece:cefactBieDomainClass": "cefact:Complaint_Issue.Details",
                    "rdfs:comment": "The indication of whether or not this complaint issue has been closed."
                }
            ]
        },
        {
            "@id": "agriculture:collectionDateTime",
            "@type": "rdf:Property",
            "schema:rangeIncludes": {
                "@id": "xsd:dateTime"
            },
            "schema:domainIncludes": {
                "@id": "agriculture:AgronomicalObservation"
            },
            "rdfs:comment": "The date, time, date time, or other date time value when this single agronomical observation is collected.",
            "rdfs:label": "collectionDateTime",
            "unece:cefactElementMetadata": [
                {
                    "@id": "cefact:Single_AgronomicalObservation.Collection.DateTime",
                    "@type": "unece:BasicBIE",
                    "unece:cefactUNId": "UN01009311",
                    "unece:cefactBieDomainClass": "cefact:Single_AgronomicalObservation.Details",
                    "rdfs:comment": "The date, time, date time, or other date time value when this single agronomical observation is collected."
                }
            ]
        },
        {
            "@id": "agriculture:combinedAgriculturalDevice",
            "@type": "rdf:Property",
            "schema:rangeIncludes": {
                "@id": "agriculture:AgriculturalDevice"
            },
            "schema:domainIncludes": {
                "@id": "agriculture:AgriculturalDevice"
            },
            "rdfs:comment": "An agricultural device combined with this specified agricultural device into a single (temporary) working unit.",
            "rdfs:label": "combinedAgriculturalDevice",
            "unece:cefactElementMetadata": [
                {
                    "@id": "cefact:Specified_AgriculturalDevice.Combined.Specified_AgriculturalDevice",
                    "@type": "unece:AssociationBIE",
                    "unece:cefactUNId": "UN01012463",
                    "unece:cefactBieDomainClass": "cefact:Specified_AgriculturalDevice.Details",
                    "rdfs:comment": "An agricultural device combined with this specified agricultural device into a single (temporary) working unit."
                }
            ]
        },
        {
            "@id": "agriculture:comment",
            "@type": "rdf:Property",
            "schema:rangeIncludes": {
                "@id": "xsd:string"
            },
            "schema:domainIncludes": {
                "@id": "agriculture:AgronomicalObservation"
            },
            "rdfs:comment": "The comment, expressed as text, for this single agronomical observation.",
            "rdfs:label": "comment",
            "unece:cefactElementMetadata": [
                {
                    "@id": "cefact:Single_AgronomicalObservation.Comment.Text",
                    "@type": "unece:BasicBIE",
                    "unece:cefactUNId": "UN01009312",
                    "unece:cefactBieDomainClass": "cefact:Single_AgronomicalObservation.Details",
                    "rdfs:comment": "The comment, expressed as text, for this single agronomical observation."
                }
            ]
        },
        {
            "@id": "agriculture:commonName",
            "@type": "rdf:Property",
            "schema:rangeIncludes": {
                "@id": "xsd:string"
            },
            "schema:domainIncludes": {
                "@id": "agriculture:TradeLineItem"
            },
            "rdfs:comment": "A common name, expressed as text, of this SPS trade line item.",
            "rdfs:label": "commonName",
            "unece:cefactElementMetadata": [
                {
                    "@id": "cefact:SPS_TradeLineItem.Common_Name.Text",
                    "@type": "unece:BasicBIE",
                    "unece:TDED": "7036",
                    "unece:cefactUNId": "UN03000149",
                    "unece:cefactBieDomainClass": "cefact:SPS_TradeLineItem.Details",
                    "rdfs:comment": "A common name, expressed as text, of this SPS trade line item."
                }
            ]
        },
        {
            "@id": "agriculture:commonSpeciesName",
            "@type": "rdf:Property",
            "schema:rangeIncludes": {
                "@id": "xsd:string"
            },
            "schema:domainIncludes": {
                "@id": "agriculture:Product"
            },
            "rdfs:comment": "The common species name, expressed as text, for this livestock animal product.",
            "rdfs:label": "commonSpeciesName",
            "unece:cefactElementMetadata": [
                {
                    "@id": "cefact:LivestockAnimal_Product.CommonSpecies_Name.Text",
                    "@type": "unece:BasicBIE",
                    "unece:TDED": "7134",
                    "unece:cefactUNId": "UN01007706",
                    "unece:cefactBieDomainClass": "cefact:LivestockAnimal_Product.Details",
                    "rdfs:comment": "The common species name, expressed as text, for this livestock animal product."
                }
            ]
        },
        {
            "@id": "agriculture:completionDateTime",
            "@type": "rdf:Property",
            "schema:rangeIncludes": {
                "@id": "xsd:dateTime"
            },
            "schema:domainIncludes": {
                "@id": "agriculture:Construction"
            },
            "rdfs:comment": "The date of the completion of this agricultural construction.",
            "rdfs:label": "completionDateTime",
            "unece:cefactElementMetadata": [
                {
                    "@id": "cefact:Agricultural_Construction.Completion.DateTime",
                    "@type": "unece:BasicBIE",
                    "unece:cefactUNId": "UN01012235",
                    "unece:cefactBieDomainClass": "cefact:Agricultural_Construction.Details",
                    "rdfs:comment": "The date of the completion of this agricultural construction."
                }
            ]
        },
        {
            "@id": "agriculture:completionPeriod",
            "@type": "rdf:Property",
            "schema:rangeIncludes": {
                "@id": "agriculture:Period"
            },
            "schema:domainIncludes": {
                "@id": "agriculture:Process"
            },
            "rdfs:comment": "The completion period for this SPS process.",
            "rdfs:label": "completionPeriod",
            "unece:cefactElementMetadata": [
                {
                    "@id": "cefact:SPS_Process.Completion.SPS_Period",
                    "@type": "unece:AssociationBIE",
                    "unece:cefactUNId": "UN03000128",
                    "unece:cefactBieDomainClass": "cefact:SPS_Process.Details",
                    "rdfs:comment": "The completion period for this SPS process."
                }
            ]
        },
        {
            "@id": "agriculture:componentChemical",
            "@type": "rdf:Property",
            "schema:rangeIncludes": {
                "@id": "agriculture:Chemical"
            },
            "schema:domainIncludes": {
                "@id": "agriculture:CropInput"
            },
            "rdfs:comment": "A crop input chemical, such as a mineral element, which is a component of this agricultural process crop input.",
            "rdfs:label": "componentChemical",
            "unece:cefactElementMetadata": [
                {
                    "@id": "cefact:AgriculturalProcess_CropInput.Component.CropInput_Chemical",
                    "@type": "unece:AssociationBIE",
                    "unece:cefactUNId": "UN01002733",
                    "unece:cefactBieDomainClass": "cefact:AgriculturalProcess_CropInput.Details",
                    "rdfs:comment": "A crop input chemical, such as a mineral element, which is a component of this agricultural process crop input."
                }
            ]
        },
        {
            "@id": "agriculture:compositionDescription",
            "@type": "rdf:Property",
            "schema:rangeIncludes": {
                "@id": "xsd:string"
            },
            "schema:domainIncludes": {
                "@id": "agriculture:Material"
            },
            "rdfs:comment": "The textual description of the composition of this agricultural input material.",
            "rdfs:label": "compositionDescription",
            "unece:cefactElementMetadata": [
                {
                    "@id": "cefact:AgriculturalInput_Material.CompositionDescription.Text",
                    "@type": "unece:BasicBIE",
                    "unece:cefactUNId": "UN01012389",
                    "unece:cefactBieDomainClass": "cefact:AgriculturalInput_Material.Details",
                    "rdfs:comment": "The textual description of the composition of this agricultural input material."
                }
            ]
        },
        {
            "@id": "agriculture:compositionMaterial",
            "@type": "rdf:Property",
            "schema:rangeIncludes": {
                "@id": "agriculture:Material"
            },
            "schema:domainIncludes": {
                "@id": "agriculture:Product"
            },
            "rdfs:comment": "A composition of agricultural input material for this agricultural input product.",
            "rdfs:label": "compositionMaterial",
            "unece:cefactElementMetadata": [
                {
                    "@id": "cefact:AgriculturalInput_Product.Composition.AgriculturalInput_Material",
                    "@type": "unece:AssociationBIE",
                    "unece:cefactUNId": "UN01012383",
                    "unece:cefactBieDomainClass": "cefact:AgriculturalInput_Product.Details",
                    "rdfs:comment": "A composition of agricultural input material for this agricultural input product."
                }
            ]
        },
        {
            "@id": "agriculture:conclusionRelatedBinaryFile",
            "@type": "rdf:Property",
            "schema:rangeIncludes": {
                "@id": "agriculture:BinaryFile"
            },
            "schema:domainIncludes": {
                "@id": "agriculture:SampledObject"
            },
            "rdfs:comment": "A binary file containing conclusions such as additional laboratory observations related to this sampled agricultural object.",
            "rdfs:label": "conclusionRelatedBinaryFile",
            "unece:cefactElementMetadata": [
                {
                    "@id": "cefact:Agricultural_SampledObject.Conclusion_Related.Specified_BinaryFile",
                    "@type": "unece:AssociationBIE",
                    "unece:cefactUNId": "UN01011947",
                    "unece:cefactBieDomainClass": "cefact:Agricultural_SampledObject.Details",
                    "rdfs:comment": "A binary file containing conclusions such as additional laboratory observations related to this sampled agricultural object."
                }
            ]
        },
        {
            "@id": "agriculture:conclusionRelatedPicture",
            "@type": "rdf:Property",
            "schema:rangeIncludes": {
                "@id": "agriculture:Picture"
            },
            "schema:domainIncludes": {
                "@id": "agriculture:SampledObject"
            },
            "rdfs:comment": "A photographic picture showing conclusions such as laboratory observations related to this sampled agricultural object.",
            "rdfs:label": "conclusionRelatedPicture",
            "unece:cefactElementMetadata": [
                {
                    "@id": "cefact:Agricultural_SampledObject.Conclusion_Related.Photographic_Picture",
                    "@type": "unece:AssociationBIE",
                    "unece:cefactUNId": "UN01011946",
                    "unece:cefactBieDomainClass": "cefact:Agricultural_SampledObject.Details",
                    "rdfs:comment": "A photographic picture showing conclusions such as laboratory observations related to this sampled agricultural object."
                }
            ]
        },
        {
            "@id": "agriculture:conclusionSpecifiedNote",
            "@type": "rdf:Property",
            "schema:rangeIncludes": {
                "@id": "agriculture:Note"
            },
            "schema:domainIncludes": {
                "@id": "agriculture:SampledObject"
            },
            "rdfs:comment": "The note, containing additional laboratory observations and or conclusions, specified for this sampled agricultural object.",
            "rdfs:label": "conclusionSpecifiedNote",
            "unece:cefactElementMetadata": [
                {
                    "@id": "cefact:Agricultural_SampledObject.Conclusion_Specified.LaboratoryObservation_Note",
                    "@type": "unece:AssociationBIE",
                    "unece:cefactUNId": "UN01009625",
                    "unece:cefactBieDomainClass": "cefact:Agricultural_SampledObject.Details",
                    "rdfs:comment": "The note, containing additional laboratory observations and or conclusions, specified for this sampled agricultural object."
                }
            ]
        },
        {
            "@id": "agriculture:consigneeParty",
            "@type": "rdf:Property",
            "schema:rangeIncludes": {
                "@id": "agriculture:Party"
            },
            "schema:domainIncludes": {
                "@id": "agriculture:Consignment"
            },
            "rdfs:comment": "The consignee party for this SPS consignment.",
            "rdfs:label": "consigneeParty",
            "unece:cefactElementMetadata": [
                {
                    "@id": "cefact:SPS_Consignment.Consignee.SPS_Party",
                    "@type": "unece:AssociationBIE",
                    "unece:cefactUNId": "UN03000059",
                    "unece:cefactBieDomainClass": "cefact:SPS_Consignment.Details",
                    "rdfs:comment": "The consignee party for this SPS consignment."
                }
            ]
        },
        {
            "@id": "agriculture:consigneeReceiptLocation",
            "@type": "rdf:Property",
            "schema:rangeIncludes": {
                "@id": "agriculture:Location"
            },
            "schema:domainIncludes": {
                "@id": "agriculture:Consignment"
            },
            "rdfs:comment": "The location where the consignee receives this SPS consignment.",
            "rdfs:label": "consigneeReceiptLocation",
            "unece:cefactElementMetadata": [
                {
                    "@id": "cefact:SPS_Consignment.ConsigneeReceipt.SPS_Location",
                    "@type": "unece:AssociationBIE",
                    "unece:cefactUNId": "UN03000065",
                    "unece:cefactBieDomainClass": "cefact:SPS_Consignment.Details",
                    "rdfs:comment": "The location where the consignee receives this SPS consignment."
                }
            ]
        },
        {
            "@id": "agriculture:consignorParty",
            "@type": "rdf:Property",
            "schema:rangeIncludes": {
                "@id": "agriculture:Party"
            },
            "schema:domainIncludes": {
                "@id": "agriculture:Consignment"
            },
            "rdfs:comment": "The consignor party for this SPS consignment.",
            "rdfs:label": "consignorParty",
            "unece:cefactElementMetadata": [
                {
                    "@id": "cefact:SPS_Consignment.Consignor.SPS_Party",
                    "@type": "unece:AssociationBIE",
                    "unece:cefactUNId": "UN03000058",
                    "unece:cefactBieDomainClass": "cefact:SPS_Consignment.Details",
                    "rdfs:comment": "The consignor party for this SPS consignment."
                }
            ]
        },
        {
            "@id": "agriculture:containingTank",
            "@type": "rdf:Property",
            "schema:rangeIncludes": {
                "@id": "agriculture:Tank"
            },
            "schema:domainIncludes": {
                "@id": "agriculture:SampledObject"
            },
            "rdfs:comment": "The milk tank containing this sampled agricultural object.",
            "rdfs:label": "containingTank",
            "unece:cefactElementMetadata": [
                {
                    "@id": "cefact:Agricultural_SampledObject.Containing.Milk_Tank",
                    "@type": "unece:AssociationBIE",
                    "unece:cefactUNId": "UN01009639",
                    "unece:cefactBieDomainClass": "cefact:Agricultural_SampledObject.Details",
                    "rdfs:comment": "The milk tank containing this sampled agricultural object."
                }
            ]
        },
        {
            "@id": "agriculture:content",
            "@type": "rdf:Property",
            "schema:rangeIncludes": {
                "@id": "xsd:string"
            },
            "schema:domainIncludes": [
                {
                    "@id": "agriculture:Clause"
                },
                {
                    "@id": "agriculture:Note"
                }
            ],
            "rdfs:comment": [
                "Content, expressed as text, in this SPS note.",
                "Content, expressed as text, of this SPS clause.",
                "Content, expressed as text, of this basic note."
            ],
            "rdfs:label": "content",
            "unece:cefactElementMetadata": [
                {
                    "@id": "cefact:SPS_Note.Content.Text",
                    "@type": "unece:BasicBIE",
                    "unece:TDED": "4150",
                    "unece:cefactUNId": "UN03000099",
                    "unece:cefactBieDomainClass": "cefact:SPS_Note.Details",
                    "rdfs:comment": "Content, expressed as text, in this SPS note."
                },
                {
                    "@id": "cefact:Basic_Note.Content.Text",
                    "@type": "unece:BasicBIE",
                    "unece:TDED": "4440",
                    "unece:cefactUNId": "UN01007715",
                    "unece:cefactBieDomainClass": "cefact:Basic_Note.Details",
                    "rdfs:comment": "Content, expressed as text, of this basic note."
                },
                {
                    "@id": "cefact:SPS_Clause.Content.Text",
                    "@type": "unece:BasicBIE",
                    "unece:TDED": "4180",
                    "unece:cefactUNId": "UN03000049",
                    "unece:cefactBieDomainClass": "cefact:SPS_Clause.Details",
                    "rdfs:comment": "Content, expressed as text, of this SPS clause."
                }
            ]
        },
        {
            "@id": "agriculture:contentCode",
            "@type": "rdf:Property",
            "schema:rangeIncludes": {
                "@id": "xsd:token"
            },
            "schema:domainIncludes": {
                "@id": "agriculture:Note"
            },
            "rdfs:comment": "A code specifying the content of this SPS note.",
            "rdfs:label": "contentCode",
            "unece:cefactElementMetadata": [
                {
                    "@id": "cefact:SPS_Note.Content.Code",
                    "@type": "unece:BasicBIE",
                    "unece:TDED": "4151",
                    "unece:cefactUNId": "UN03000098",
                    "unece:cefactBieDomainClass": "cefact:SPS_Note.Details",
                    "rdfs:comment": "A code specifying the content of this SPS note."
                }
            ]
        },
        {
            "@id": "agriculture:controlRequirementIndicator",
            "@type": "rdf:Property",
            "schema:rangeIncludes": {
                "@id": "xsd:boolean"
            },
            "schema:domainIncludes": {
                "@id": "agriculture:Document"
            },
            "rdfs:comment": "The indication of whether or not this crop report document has specific control requirements.",
            "rdfs:label": "controlRequirementIndicator",
            "unece:cefactElementMetadata": [
                {
                    "@id": "cefact:CropReport_Document.ControlRequirement.Indicator",
                    "@type": "unece:BasicBIE",
                    "unece:cefactUNId": "UN01012436",
                    "unece:cefactBieDomainClass": "cefact:CropReport_Document.Details",
                    "rdfs:comment": "The indication of whether or not this crop report document has specific control requirements."
                }
            ]
        },
        {
            "@id": "agriculture:coordinate",
            "@type": "rdf:Property",
            "schema:rangeIncludes": {
                "@id": "xsd:string"
            },
            "schema:domainIncludes": {
                "@id": "agriculture:DirectPositionList"
            },
            "rdfs:comment": "The coordinate, expressed as text, for this specified direct position list.",
            "rdfs:label": "coordinate",
            "unece:cefactElementMetadata": [
                {
                    "@id": "cefact:Specified_DirectPositionList.Coordinate.Text",
                    "@type": "unece:BasicBIE",
                    "unece:cefactUNId": "UN01012472",
                    "unece:cefactBieDomainClass": "cefact:Specified_DirectPositionList.Details",
                    "rdfs:comment": "The coordinate, expressed as text, for this specified direct position list."
                }
            ]
        },
        {
            "@id": "agriculture:coordinateReferenceDimension",
            "@type": "rdf:Property",
            "schema:rangeIncludes": {
                "@id": "xsd:string"
            },
            "schema:domainIncludes": {
                "@id": "agriculture:DirectPositionList"
            },
            "rdfs:comment": "A coordinate reference dimension, expressed as text, for this specified direct position list.",
            "rdfs:label": "coordinateReferenceDimension",
            "unece:cefactElementMetadata": [
                {
                    "@id": "cefact:Specified_DirectPositionList.CoordinateReferenceDimension.Text",
                    "@type": "unece:BasicBIE",
                    "unece:cefactUNId": "UN01012474",
                    "unece:cefactBieDomainClass": "cefact:Specified_DirectPositionList.Details",
                    "rdfs:comment": "A coordinate reference dimension, expressed as text, for this specified direct position list."
                }
            ]
        },
        {
            "@id": "agriculture:coordinateReferenceSystemId",
            "@type": "rdf:Property",
            "schema:rangeIncludes": {
                "@id": "xsd:token"
            },
            "schema:domainIncludes": {
                "@id": "agriculture:GeographicalFeature"
            },
            "rdfs:comment": "The identifier of the coordinate reference system for this geographical feature.",
            "rdfs:label": "coordinateReferenceSystemId",
            "unece:cefactElementMetadata": [
                {
                    "@id": "cefact:Specified_GeographicalFeature.CoordinateReferenceSystem.Identifier",
                    "@type": "unece:BasicBIE",
                    "unece:cefactUNId": "UN01012171",
                    "unece:cefactBieDomainClass": "cefact:Specified_GeographicalFeature.Details",
                    "rdfs:comment": "The identifier of the coordinate reference system for this geographical feature."
                }
            ]
        },
        {
            "@id": "agriculture:copyIndicator",
            "@type": "rdf:Property",
            "schema:rangeIncludes": {
                "@id": "xsd:boolean"
            },
            "schema:domainIncludes": {
                "@id": "agriculture:Document"
            },
            "rdfs:comment": [
                "The indication of whether or not this crop data sheet document is a copy.",
                "The indication of whether or not this crop report document is a copy.",
                "The indication of whether or not this exchanged SPS document is a copy."
            ],
            "rdfs:label": "copyIndicator",
            "unece:cefactElementMetadata": [
                {
                    "@id": "cefact:SPSExchanged_Document.Copy.Indicator",
                    "@type": "unece:BasicBIE",
                    "unece:TDED": "4366",
                    "unece:cefactUNId": "UN03000008",
                    "unece:cefactBieDomainClass": "cefact:SPSExchanged_Document.Details",
                    "rdfs:comment": "The indication of whether or not this exchanged SPS document is a copy."
                },
                {
                    "@id": "cefact:CropReport_Document.Copy.Indicator",
                    "@type": "unece:BasicBIE",
                    "unece:cefactUNId": "UN01012435",
                    "unece:cefactBieDomainClass": "cefact:CropReport_Document.Details",
                    "rdfs:comment": "The indication of whether or not this crop report document is a copy."
                },
                {
                    "@id": "cefact:CropDataSheet_Document.Copy.Indicator",
                    "@type": "unece:BasicBIE",
                    "unece:cefactUNId": "UN01002817",
                    "unece:cefactBieDomainClass": "cefact:CropDataSheet_Document.Details",
                    "rdfs:comment": "The indication of whether or not this crop data sheet document is a copy."
                }
            ]
        },
        {
            "@id": "agriculture:countNumeric",
            "@type": "rdf:Property",
            "schema:rangeIncludes": {
                "@id": "xsd:decimal"
            },
            "schema:domainIncludes": {
                "@id": "agriculture:DirectPositionList"
            },
            "rdfs:comment": "A count for this specified direct position list.",
            "rdfs:label": "countNumeric",
            "unece:cefactElementMetadata": [
                {
                    "@id": "cefact:Specified_DirectPositionList.Count.Numeric",
                    "@type": "unece:BasicBIE",
                    "unece:cefactUNId": "UN01012477",
                    "unece:cefactBieDomainClass": "cefact:Specified_DirectPositionList.Details",
                    "rdfs:comment": "A count for this specified direct position list."
                }
            ]
        },
        {
            "@id": "agriculture:countryId",
            "@type": "rdf:Property",
            "schema:rangeIncludes": {
                "@id": "xsd:token"
            },
            "schema:domainIncludes": [
                {
                    "@id": "agriculture:Address"
                },
                {
                    "@id": "agriculture:Classification"
                },
                {
                    "@id": "agriculture:Party"
                }
            ],
            "rdfs:comment": [
                "The country identifier for this specified classification.",
                "The country identifier for this specified party.",
                "The unique identifier of a country in the SPS address (Reference ISO 3166 and UN/ECE Rec 3)."
            ],
            "rdfs:label": "countryId",
            "unece:cefactElementMetadata": [
                {
                    "@id": "cefact:Specified_Party.Country.Identifier",
                    "@type": "unece:BasicBIE",
                    "unece:cefactUNId": "UN01007611",
                    "unece:cefactBieDomainClass": "cefact:Specified_Party.Details",
                    "rdfs:comment": "The country identifier for this specified party."
                },
                {
                    "@id": "cefact:Specified_Classification.Country.Identifier",
                    "@type": "unece:BasicBIE",
                    "unece:cefactUNId": "UN01007620",
                    "unece:cefactBieDomainClass": "cefact:Specified_Classification.Details",
                    "rdfs:comment": "The country identifier for this specified classification."
                },
                {
                    "@id": "cefact:SPS_Address.Country.Identifier",
                    "@type": "unece:BasicBIE",
                    "unece:TDED": "3207",
                    "unece:cefactUNId": "UN03000027",
                    "unece:cefactBieDomainClass": "cefact:SPS_Address.Details",
                    "rdfs:comment": "The unique identifier of a country in the SPS address (Reference ISO 3166 and UN/ECE Rec 3)."
                }
            ]
        },
        {
            "@id": "agriculture:countryName",
            "@type": "rdf:Property",
            "schema:rangeIncludes": {
                "@id": "xsd:string"
            },
            "schema:domainIncludes": {
                "@id": "agriculture:Address"
            },
            "rdfs:comment": "The name, expressed as text, of the country in this SPS address.",
            "rdfs:label": "countryName",
            "unece:cefactElementMetadata": [
                {
                    "@id": "cefact:SPS_Address.CountryName.Text",
                    "@type": "unece:BasicBIE",
                    "unece:TDED": "3206",
                    "unece:cefactUNId": "UN03000029",
                    "unece:cefactBieDomainClass": "cefact:SPS_Address.Details",
                    "rdfs:comment": "The name, expressed as text, of the country in this SPS address."
                }
            ]
        },
        {
            "@id": "agriculture:countryOfOriginId",
            "@type": "rdf:Property",
            "schema:rangeIncludes": {
                "@id": "xsd:token"
            },
            "schema:domainIncludes": {
                "@id": "agriculture:SampledObject"
            },
            "rdfs:comment": "The identifier for the country of origin for this sampled agricultural object.",
            "rdfs:label": "countryOfOriginId",
            "unece:cefactElementMetadata": [
                {
                    "@id": "cefact:Agricultural_SampledObject.CountryOfOrigin_Identification.Identifier",
                    "@type": "unece:BasicBIE",
                    "unece:cefactUNId": "UN01009618",
                    "unece:cefactBieDomainClass": "cefact:Agricultural_SampledObject.Details",
                    "rdfs:comment": "The identifier for the country of origin for this sampled agricultural object."
                }
            ]
        },
        {
            "@id": "agriculture:countryOfOriginSubDivisionName",
            "@type": "rdf:Property",
            "schema:rangeIncludes": {
                "@id": "xsd:string"
            },
            "schema:domainIncludes": {
                "@id": "agriculture:SampledObject"
            },
            "rdfs:comment": "The name, expressed as text, for the country of origin subdivision for this sampled agricultural object.",
            "rdfs:label": "countryOfOriginSubDivisionName",
            "unece:cefactElementMetadata": [
                {
                    "@id": "cefact:Agricultural_SampledObject.CountryOfOriginSubDivision_Name.Text",
                    "@type": "unece:BasicBIE",
                    "unece:cefactUNId": "UN01009619",
                    "unece:cefactBieDomainClass": "cefact:Agricultural_SampledObject.Details",
                    "rdfs:comment": "The name, expressed as text, for the country of origin subdivision for this sampled agricultural object."
                }
            ]
        },
        {
            "@id": "agriculture:countrySubDivisionId",
            "@type": "rdf:Property",
            "schema:rangeIncludes": {
                "@id": "xsd:token"
            },
            "schema:domainIncludes": {
                "@id": "agriculture:Address"
            },
            "rdfs:comment": "The unique identifier in this country sub-division in this SPS address.",
            "rdfs:label": "countrySubDivisionId",
            "unece:cefactElementMetadata": [
                {
                    "@id": "cefact:SPS_Address.CountrySub-Division.Identifier",
                    "@type": "unece:BasicBIE",
                    "unece:TDED": "3229",
                    "unece:cefactUNId": "UN03000030",
                    "unece:cefactBieDomainClass": "cefact:SPS_Address.Details",
                    "rdfs:comment": "The unique identifier in this country sub-division in this SPS address."
                }
            ]
        },
        {
            "@id": "agriculture:countrySubDivisionName",
            "@type": "rdf:Property",
            "schema:rangeIncludes": {
                "@id": "xsd:string"
            },
            "schema:domainIncludes": {
                "@id": "agriculture:Address"
            },
            "rdfs:comment": "The name, expressed as text, of the sub-division of a country in this SPS address.",
            "rdfs:label": "countrySubDivisionName",
            "unece:cefactElementMetadata": [
                {
                    "@id": "cefact:SPS_Address.CountrySub-DivisionName.Text",
                    "@type": "unece:BasicBIE",
                    "unece:TDED": "3228",
                    "unece:cefactUNId": "UN03000031",
                    "unece:cefactBieDomainClass": "cefact:SPS_Address.Details",
                    "rdfs:comment": "The name, expressed as text, of the sub-division of a country in this SPS address."
                }
            ]
        },
        {
            "@id": "agriculture:coverageTypeCode",
            "@type": "rdf:Property",
            "schema:rangeIncludes": {
                "@id": "xsd:token"
            },
            "schema:domainIncludes": {
                "@id": "agriculture:Construction"
            },
            "rdfs:comment": "The code specifying the type of coverage, such as a glass roof, for this agricultural construction.",
            "rdfs:label": "coverageTypeCode",
            "unece:cefactElementMetadata": [
                {
                    "@id": "cefact:Agricultural_Construction.Coverage_Type.Code",
                    "@type": "unece:BasicBIE",
                    "unece:cefactUNId": "UN01012231",
                    "unece:cefactBieDomainClass": "cefact:Agricultural_Construction.Details",
                    "rdfs:comment": "The code specifying the type of coverage, such as a glass roof, for this agricultural construction."
                }
            ]
        },
        {
            "@id": "agriculture:creationDateTime",
            "@type": "rdf:Property",
            "schema:rangeIncludes": {
                "@id": "xsd:dateTime"
            },
            "schema:domainIncludes": [
                {
                    "@id": "agriculture:Batch"
                },
                {
                    "@id": "agriculture:Document"
                }
            ],
            "rdfs:comment": [
                "The date or date time value of the creation of this crop data sheet document.",
                "The date, time, date time or other date time value of the creation of this agronomical observation document.",
                "The date, time, date time or other date time value of the creation of this product batch.",
                "The date, time, date time, or other date time value of the creation of this animal batch.",
                "The date, time, date time, or other date time value of the creation of this crop produce batch."
            ],
            "rdfs:label": "creationDateTime",
            "unece:cefactElementMetadata": [
                {
                    "@id": "cefact:AgronomicalObservation_Document.Creation.DateTime",
                    "@type": "unece:BasicBIE",
                    "unece:cefactUNId": "UN01009296",
                    "unece:cefactBieDomainClass": "cefact:AgronomicalObservation_Document.Details",
                    "rdfs:comment": "The date, time, date time or other date time value of the creation of this agronomical observation document."
                },
                {
                    "@id": "cefact:Product_Batch.Creation.DateTime",
                    "@type": "unece:BasicBIE",
                    "unece:cefactUNId": "UN01012348",
                    "unece:cefactBieDomainClass": "cefact:Product_Batch.Details",
                    "rdfs:comment": "The date, time, date time or other date time value of the creation of this product batch."
                },
                {
                    "@id": "cefact:CropDataSheet_Document.Creation.DateTime",
                    "@type": "unece:BasicBIE",
                    "unece:cefactUNId": "UN01002816",
                    "unece:cefactBieDomainClass": "cefact:CropDataSheet_Document.Details",
                    "rdfs:comment": "The date or date time value of the creation of this crop data sheet document."
                },
                {
                    "@id": "cefact:Animal_Batch.Creation.DateTime",
                    "@type": "unece:BasicBIE",
                    "unece:cefactUNId": "UN01011246",
                    "unece:cefactBieDomainClass": "cefact:Animal_Batch.Details",
                    "rdfs:comment": "The date, time, date time, or other date time value of the creation of this animal batch."
                },
                {
                    "@id": "cefact:CropProduce_Batch.Creation.DateTime",
                    "@type": "unece:BasicBIE",
                    "unece:cefactUNId": "UN01012333",
                    "unece:cefactBieDomainClass": "cefact:CropProduce_Batch.Details",
                    "rdfs:comment": "The date, time, date time, or other date time value of the creation of this crop produce batch."
                }
            ]
        },
        {
            "@id": "agriculture:cropDataSheetDocumentTypeCode",
            "@type": "rdf:Property",
            "schema:rangeIncludes": {
                "@id": "unece:UNECECL1001Code"
            },
            "schema:domainIncludes": {
                "@id": "agriculture:Document"
            },
            "rdfs:comment": "The code specifying the type of crop data sheet document.",
            "rdfs:label": "cropDataSheetDocumentTypeCode",
            "unece:cefactElementMetadata": [
                {
                    "@id": "cefact:CropDataSheet_Document.Type.Code",
                    "@type": "unece:BasicBIE",
                    "unece:TDED": "1001",
                    "unece:cefactUNId": "UN01002815",
                    "unece:cefactBieDomainClass": "cefact:CropDataSheet_Document.Details",
                    "rdfs:comment": "The code specifying the type of crop data sheet document."
                }
            ]
        },
        {
            "@id": "agriculture:cropProportionPercent",
            "@type": "rdf:Property",
            "schema:rangeIncludes": {
                "@id": "xsd:decimal"
            },
            "schema:domainIncludes": {
                "@id": "agriculture:CropMixtureConstituent"
            },
            "rdfs:comment": "The percent of the crop proportion of this field crop mixture constituent.",
            "rdfs:label": "cropProportionPercent",
            "unece:cefactElementMetadata": [
                {
                    "@id": "cefact:Field_CropMixtureConstituent.Crop_Proportion.Percent",
                    "@type": "unece:BasicBIE",
                    "unece:cefactUNId": "UN01012322",
                    "unece:cefactBieDomainClass": "cefact:Field_CropMixtureConstituent.Details",
                    "rdfs:comment": "The percent of the crop proportion of this field crop mixture constituent."
                }
            ]
        },
        {
            "@id": "agriculture:cropReportDocumentPurposeCode",
            "@type": "rdf:Property",
            "schema:rangeIncludes": {
                "@id": "unece:UNECECL1225Code"
            },
            "schema:domainIncludes": {
                "@id": "agriculture:Document"
            },
            "rdfs:comment": "The code specifying the purpose of this crop report document.",
            "rdfs:label": "cropReportDocumentPurposeCode",
            "unece:cefactElementMetadata": [
                {
                    "@id": "cefact:CropReport_Document.Purpose.Code",
                    "@type": "unece:BasicBIE",
                    "unece:TDED": "1225",
                    "unece:cefactUNId": "UN01012437",
                    "unece:cefactBieDomainClass": "cefact:CropReport_Document.Details",
                    "rdfs:comment": "The code specifying the purpose of this crop report document."
                }
            ]
        },
        {
            "@id": "agriculture:cropReportDocumentStatusCode",
            "@type": "rdf:Property",
            "schema:rangeIncludes": {
                "@id": "unece:UNECECL1373Code"
            },
            "schema:domainIncludes": {
                "@id": "agriculture:Document"
            },
            "rdfs:comment": "The code specifying the status of this crop report document.",
            "rdfs:label": "cropReportDocumentStatusCode",
            "unece:cefactElementMetadata": [
                {
                    "@id": "cefact:CropReport_Document.Status.Code",
                    "@type": "unece:BasicBIE",
                    "unece:TDED": "1373",
                    "unece:cefactUNId": "UN01012440",
                    "unece:cefactBieDomainClass": "cefact:CropReport_Document.Details",
                    "rdfs:comment": "The code specifying the status of this crop report document."
                }
            ]
        },
        {
            "@id": "agriculture:cropReportDocumentTypeCode",
            "@type": "rdf:Property",
            "schema:rangeIncludes": {
                "@id": "unece:UNECECL1001Code"
            },
            "schema:domainIncludes": {
                "@id": "agriculture:Document"
            },
            "rdfs:comment": "The code specifying the type of crop report document.",
            "rdfs:label": "cropReportDocumentTypeCode",
            "unece:cefactElementMetadata": [
                {
                    "@id": "cefact:CropReport_Document.Type.Code",
                    "@type": "unece:BasicBIE",
                    "unece:TDED": "1001",
                    "unece:cefactUNId": "UN01012434",
                    "unece:cefactBieDomainClass": "cefact:CropReport_Document.Details",
                    "rdfs:comment": "The code specifying the type of crop report document."
                }
            ]
        },
        {
            "@id": "agriculture:cultivationContainerCode",
            "@type": "rdf:Property",
            "schema:rangeIncludes": {
                "@id": "xsd:token"
            },
            "schema:domainIncludes": {
                "@id": "agriculture:Crop"
            },
            "rdfs:comment": "The code specifying the type of cultivation container, such as a pot or an iron cabinet, for this field crop.",
            "rdfs:label": "cultivationContainerCode",
            "unece:cefactElementMetadata": [
                {
                    "@id": "cefact:Field_Crop.CultivationContainer.Code",
                    "@type": "unece:BasicBIE",
                    "unece:cefactUNId": "UN01012306",
                    "unece:cefactBieDomainClass": "cefact:Field_Crop.Details",
                    "rdfs:comment": "The code specifying the type of cultivation container, such as a pot or an iron cabinet, for this field crop."
                }
            ]
        },
        {
            "@id": "agriculture:cultivationCoverageCode",
            "@type": "rdf:Property",
            "schema:rangeIncludes": {
                "@id": "xsd:token"
            },
            "schema:domainIncludes": {
                "@id": "agriculture:Crop"
            },
            "rdfs:comment": "A code specifying a type of cultivation coverage, such as glass, for this field crop.",
            "rdfs:label": "cultivationCoverageCode",
            "unece:cefactElementMetadata": [
                {
                    "@id": "cefact:Field_Crop.CultivationCoverage.Code",
                    "@type": "unece:BasicBIE",
                    "unece:cefactUNId": "UN01012304",
                    "unece:cefactBieDomainClass": "cefact:Field_Crop.Details",
                    "rdfs:comment": "A code specifying a type of cultivation coverage, such as glass, for this field crop."
                }
            ]
        },
        {
            "@id": "agriculture:cultivationMediumCode",
            "@type": "rdf:Property",
            "schema:rangeIncludes": {
                "@id": "xsd:token"
            },
            "schema:domainIncludes": {
                "@id": "agriculture:Crop"
            },
            "rdfs:comment": "The code specifying the type of cultivation medium, such as substrate, for this field crop.",
            "rdfs:label": "cultivationMediumCode",
            "unece:cefactElementMetadata": [
                {
                    "@id": "cefact:Field_Crop.CultivationMedium.Code",
                    "@type": "unece:BasicBIE",
                    "unece:cefactUNId": "UN01012305",
                    "unece:cefactBieDomainClass": "cefact:Field_Crop.Details",
                    "rdfs:comment": "The code specifying the type of cultivation medium, such as substrate, for this field crop."
                }
            ]
        },
        {
            "@id": "agriculture:cultivationTypeCode",
            "@type": "rdf:Property",
            "schema:rangeIncludes": {
                "@id": "xsd:token"
            },
            "schema:domainIncludes": {
                "@id": "agriculture:Crop"
            },
            "rdfs:comment": "The code specifying the type of cultivation for this field crop.",
            "rdfs:label": "cultivationTypeCode",
            "unece:cefactElementMetadata": [
                {
                    "@id": "cefact:Field_Crop.CultivationType.Code",
                    "@type": "unece:BasicBIE",
                    "unece:cefactUNId": "UN01012302",
                    "unece:cefactBieDomainClass": "cefact:Field_Crop.Details",
                    "rdfs:comment": "The code specifying the type of cultivation for this field crop."
                }
            ]
        },
        {
            "@id": "agriculture:customerParty",
            "@type": "rdf:Property",
            "schema:rangeIncludes": {
                "@id": "agriculture:Party"
            },
            "schema:domainIncludes": {
                "@id": "agriculture:SampledObject"
            },
            "rdfs:comment": "The customer party for this sampled agricultural object.",
            "rdfs:label": "customerParty",
            "unece:cefactElementMetadata": [
                {
                    "@id": "cefact:Agricultural_SampledObject.Customer.LaboratoryObservation_Party",
                    "@type": "unece:AssociationBIE",
                    "unece:cefactUNId": "UN01009630",
                    "unece:cefactBieDomainClass": "cefact:Agricultural_SampledObject.Details",
                    "rdfs:comment": "The customer party for this sampled agricultural object."
                }
            ]
        },
        {
            "@id": "agriculture:customsTransitAgentParty",
            "@type": "rdf:Property",
            "schema:rangeIncludes": {
                "@id": "agriculture:Party"
            },
            "schema:domainIncludes": {
                "@id": "agriculture:Consignment"
            },
            "rdfs:comment": "The party acting as an agent for, or on behalf of, the consignor with respect to customs transit procedures for this SPS consignment.",
            "rdfs:label": "customsTransitAgentParty",
            "unece:cefactElementMetadata": [
                {
                    "@id": "cefact:SPS_Consignment.CustomsTransitAgent.SPS_Party",
                    "@type": "unece:AssociationBIE",
                    "unece:cefactUNId": "UN03000073",
                    "unece:cefactBieDomainClass": "cefact:SPS_Consignment.Details",
                    "rdfs:comment": "The party acting as an agent for, or on behalf of, the consignor with respect to customs transit procedures for this SPS consignment."
                }
            ]
        },
        {
            "@id": "agriculture:dataSheetEndDateTime",
            "@type": "rdf:Property",
            "schema:rangeIncludes": {
                "@id": "xsd:dateTime"
            },
            "schema:domainIncludes": {
                "@id": "agriculture:Plot"
            },
            "rdfs:comment": [
                "The date or date time value for the end of the period covered by the data sheet for this agricultural plot.",
                "The date or date time value for the end of the period covered by the data sheet for this agronomical observation plot."
            ],
            "rdfs:label": "dataSheetEndDateTime",
            "unece:cefactElementMetadata": [
                {
                    "@id": "cefact:Agricultural_Plot.DataSheetEnd.DateTime",
                    "@type": "unece:BasicBIE",
                    "unece:cefactUNId": "UN01002656",
                    "unece:cefactBieDomainClass": "cefact:Agricultural_Plot.Details",
                    "rdfs:comment": "The date or date time value for the end of the period covered by the data sheet for this agricultural plot."
                },
                {
                    "@id": "cefact:AgronomicalObservation_Plot.DataSheetEnd.DateTime",
                    "@type": "unece:BasicBIE",
                    "unece:cefactUNId": "UN01009370",
                    "unece:cefactBieDomainClass": "cefact:AgronomicalObservation_Plot.Details",
                    "rdfs:comment": "The date or date time value for the end of the period covered by the data sheet for this agronomical observation plot."
                }
            ]
        },
        {
            "@id": "agriculture:dataSheetStartDateTime",
            "@type": "rdf:Property",
            "schema:rangeIncludes": {
                "@id": "xsd:dateTime"
            },
            "schema:domainIncludes": {
                "@id": "agriculture:Plot"
            },
            "rdfs:comment": [
                "The date or date time value for the start of the period covered by the data sheet for this agricultural plot.",
                "The date or date time value for the start of the period covered by the data sheet for this agronomical observation plot."
            ],
            "rdfs:label": "dataSheetStartDateTime",
            "unece:cefactElementMetadata": [
                {
                    "@id": "cefact:Agricultural_Plot.DataSheetStart.DateTime",
                    "@type": "unece:BasicBIE",
                    "unece:cefactUNId": "UN01002655",
                    "unece:cefactBieDomainClass": "cefact:Agricultural_Plot.Details",
                    "rdfs:comment": "The date or date time value for the start of the period covered by the data sheet for this agricultural plot."
                },
                {
                    "@id": "cefact:AgronomicalObservation_Plot.DataSheetStart.DateTime",
                    "@type": "unece:BasicBIE",
                    "unece:cefactUNId": "UN01009369",
                    "unece:cefactBieDomainClass": "cefact:AgronomicalObservation_Plot.Details",
                    "rdfs:comment": "The date or date time value for the start of the period covered by the data sheet for this agronomical observation plot."
                }
            ]
        },
        {
            "@id": "agriculture:deathDateTime",
            "@type": "rdf:Property",
            "schema:rangeIncludes": {
                "@id": "xsd:dateTime"
            },
            "schema:domainIncludes": {
                "@id": "agriculture:Animal"
            },
            "rdfs:comment": "The date of death for this livestock animal.",
            "rdfs:label": "deathDateTime",
            "unece:cefactElementMetadata": [
                {
                    "@id": "cefact:Livestock_Animal.Death.DateTime",
                    "@type": "unece:BasicBIE",
                    "unece:cefactUNId": "UN01007645",
                    "unece:cefactBieDomainClass": "cefact:Livestock_Animal.Details",
                    "rdfs:comment": "The date of death for this livestock animal."
                }
            ]
        },
        {
            "@id": "agriculture:declaredIssue",
            "@type": "rdf:Property",
            "schema:rangeIncludes": {
                "@id": "agriculture:Issue"
            },
            "schema:domainIncludes": {
                "@id": "agriculture:ProductionUnit"
            },
            "rdfs:comment": "A complaint issue declared for this agricultural production unit.",
            "rdfs:label": "declaredIssue",
            "unece:cefactElementMetadata": [
                {
                    "@id": "cefact:Agricultural_ProductionUnit.Declared.Complaint_Issue",
                    "@type": "unece:AssociationBIE",
                    "unece:cefactUNId": "UN01012250",
                    "unece:cefactBieDomainClass": "cefact:Agricultural_ProductionUnit.Details",
                    "rdfs:comment": "A complaint issue declared for this agricultural production unit."
                }
            ]
        },
        {
            "@id": "agriculture:dedicatedConstruction",
            "@type": "rdf:Property",
            "schema:rangeIncludes": {
                "@id": "agriculture:Construction"
            },
            "schema:domainIncludes": {
                "@id": "agriculture:ProductionUnit"
            },
            "rdfs:comment": "An agricultural construction dedicated to this agricultural production unit.",
            "rdfs:label": "dedicatedConstruction",
            "unece:cefactElementMetadata": [
                {
                    "@id": "cefact:Agricultural_ProductionUnit.Dedicated.Agricultural_Construction",
                    "@type": "unece:AssociationBIE",
                    "unece:cefactUNId": "UN01012248",
                    "unece:cefactBieDomainClass": "cefact:Agricultural_ProductionUnit.Details",
                    "rdfs:comment": "An agricultural construction dedicated to this agricultural production unit."
                }
            ]
        },
        {
            "@id": "agriculture:definedContact",
            "@type": "rdf:Property",
            "schema:rangeIncludes": {
                "@id": "agriculture:Contact"
            },
            "schema:domainIncludes": {
                "@id": "agriculture:Party"
            },
            "rdfs:comment": [
                "A contact defined for this SPS party.",
                "The defined contact for this specified party.",
                "The defined party contact for this agronomical observation party.",
                "The defined party contact for this crop data sheet party."
            ],
            "rdfs:label": "definedContact",
            "unece:cefactElementMetadata": [
                {
                    "@id": "cefact:AgronomicalObservation_Party.Defined.Party_Contact",
                    "@type": "unece:AssociationBIE",
                    "unece:cefactUNId": "UN01009305",
                    "unece:cefactBieDomainClass": "cefact:AgronomicalObservation_Party.Details",
                    "rdfs:comment": "The defined party contact for this agronomical observation party."
                },
                {
                    "@id": "cefact:Specified_Party.Defined.Party_Contact",
                    "@type": "unece:AssociationBIE",
                    "unece:cefactUNId": "UN01007612",
                    "unece:cefactBieDomainClass": "cefact:Specified_Party.Details",
                    "rdfs:comment": "The defined contact for this specified party."
                },
                {
                    "@id": "cefact:CropDataSheet_Party.Defined.Party_Contact",
                    "@type": "unece:AssociationBIE",
                    "unece:cefactUNId": "UN01002811",
                    "unece:cefactBieDomainClass": "cefact:CropDataSheet_Party.Details",
                    "rdfs:comment": "The defined party contact for this crop data sheet party."
                },
                {
                    "@id": "cefact:SPS_Party.Defined.SPS_Contact",
                    "@type": "unece:AssociationBIE",
                    "unece:cefactUNId": "UN03000117",
                    "unece:cefactBieDomainClass": "cefact:SPS_Party.Details",
                    "rdfs:comment": "A contact defined for this SPS party."
                }
            ]
        },
        {
            "@id": "agriculture:definedCoordinateReferenceSystem",
            "@type": "rdf:Property",
            "schema:rangeIncludes": {
                "@id": "agriculture:CoordinateReferenceSystem"
            },
            "schema:domainIncludes": {
                "@id": "agriculture:Location"
            },
            "rdfs:comment": "The Coordinate System (CS) engineering coordinate reference system defined for this referenced location.",
            "rdfs:label": "definedCoordinateReferenceSystem",
            "unece:cefactElementMetadata": [
                {
                    "@id": "cefact:Referenced_Location.Defined.CSEngineering_CoordinateReferenceSystem",
                    "@type": "unece:AssociationBIE",
                    "unece:cefactUNId": "UN01012159",
                    "unece:cefactBieDomainClass": "cefact:Referenced_Location.Details",
                    "rdfs:comment": "The Coordinate System (CS) engineering coordinate reference system defined for this referenced location."
                }
            ]
        },
        {
            "@id": "agriculture:deliveryEvent",
            "@type": "rdf:Property",
            "schema:rangeIncludes": {
                "@id": "agriculture:Event"
            },
            "schema:domainIncludes": {
                "@id": "agriculture:TradeDelivery"
            },
            "rdfs:comment": "A Track and Trace (TT) delivery event for this animal trade delivery.",
            "rdfs:label": "deliveryEvent",
            "unece:cefactElementMetadata": [
                {
                    "@id": "cefact:Animal_TradeDelivery.Delivery.TT_Event",
                    "@type": "unece:AssociationBIE",
                    "unece:cefactUNId": "UN01011266",
                    "unece:cefactBieDomainClass": "cefact:Animal_TradeDelivery.Details",
                    "rdfs:comment": "A Track and Trace (TT) delivery event for this animal trade delivery."
                }
            ]
        },
        {
            "@id": "agriculture:deliveryParty",
            "@type": "rdf:Property",
            "schema:rangeIncludes": {
                "@id": "agriculture:Party"
            },
            "schema:domainIncludes": {
                "@id": "agriculture:Consignment"
            },
            "rdfs:comment": "The party to whom this SPS consignment will be, or has been, delivered.",
            "rdfs:label": "deliveryParty",
            "unece:cefactElementMetadata": [
                {
                    "@id": "cefact:SPS_Consignment.Delivery.SPS_Party",
                    "@type": "unece:AssociationBIE",
                    "unece:cefactUNId": "UN03000072",
                    "unece:cefactBieDomainClass": "cefact:SPS_Consignment.Details",
                    "rdfs:comment": "The party to whom this SPS consignment will be, or has been, delivered."
                }
            ]
        },
        {
            "@id": "agriculture:departureLocationId",
            "@type": "rdf:Property",
            "schema:rangeIncludes": {
                "@id": "xsd:token"
            },
            "schema:domainIncludes": {
                "@id": "agriculture:Event"
            },
            "rdfs:comment": "The identifier of the departure location for this cross border animal movement event.",
            "rdfs:label": "departureLocationId",
            "unece:cefactElementMetadata": [
                {
                    "@id": "cefact:CrossBorderAnimalMovement_Event.Departure_Location.Identifier",
                    "@type": "unece:BasicBIE",
                    "unece:cefactUNId": "UN01007663",
                    "unece:cefactBieDomainClass": "cefact:CrossBorderAnimalMovement_Event.Details",
                    "rdfs:comment": "The identifier of the departure location for this cross border animal movement event."
                }
            ]
        },
        {
            "@id": "agriculture:departureSpecifiedEvent",
            "@type": "rdf:Property",
            "schema:rangeIncludes": {
                "@id": "agriculture:Event"
            },
            "schema:domainIncludes": {
                "@id": "agriculture:Event"
            },
            "rdfs:comment": "The departure movement event specified for this animal holding event.",
            "rdfs:label": "departureSpecifiedEvent",
            "unece:cefactElementMetadata": [
                {
                    "@id": "cefact:AnimalHolding_Event.Departure_Specified.AnimalMovement_Event",
                    "@type": "unece:AssociationBIE",
                    "unece:cefactUNId": "UN01007637",
                    "unece:cefactBieDomainClass": "cefact:AnimalHolding_Event.Details",
                    "rdfs:comment": "The departure movement event specified for this animal holding event."
                }
            ]
        },
        {
            "@id": "agriculture:description",
            "@type": "rdf:Property",
            "schema:rangeIncludes": {
                "@id": "xsd:string"
            },
            "schema:domainIncludes": [
                {
                    "@id": "agriculture:AgriculturalProcess"
                },
                {
                    "@id": "agriculture:Certificate"
                },
                {
                    "@id": "agriculture:Characteristic"
                },
                {
                    "@id": "agriculture:Chemical"
                },
                {
                    "@id": "agriculture:Contract"
                },
                {
                    "@id": "agriculture:CountrySubDivision"
                },
                {
                    "@id": "agriculture:Crop"
                },
                {
                    "@id": "agriculture:CropInput"
                },
                {
                    "@id": "agriculture:CropProtectionTreatment"
                },
                {
                    "@id": "agriculture:CropStage"
                },
                {
                    "@id": "agriculture:Document"
                },
                {
                    "@id": "agriculture:GeographicalFeature"
                },
                {
                    "@id": "agriculture:GeographicalObjectCharacteristic"
                },
                {
                    "@id": "agriculture:Issue"
                },
                {
                    "@id": "agriculture:Material"
                },
                {
                    "@id": "agriculture:Party"
                },
                {
                    "@id": "agriculture:Plot"
                },
                {
                    "@id": "agriculture:Product"
                },
                {
                    "@id": "agriculture:ProtectionMeans"
                },
                {
                    "@id": "agriculture:SpeciesVariety"
                },
                {
                    "@id": "agriculture:TargetObject"
                },
                {
                    "@id": "agriculture:TradeLineItem"
                },
                {
                    "@id": "agriculture:WorkItem"
                }
            ],
            "rdfs:comment": [
                "A textual description of this SPS process characteristic.",
                "A textual description of this SPS trade line item.",
                "A textual description of this disease protection means.",
                "A textual description of this exchanged SPS document.",
                "A textual description of this specified crop protection treatment.",
                "The textual description for this agricultural crop.",
                "The textual description for this agronomical observation party.",
                "The textual description for this crop data sheet party.",
                "The textual description for this crop species variety.",
                "The textual description for this field crop.",
                "The textual description for this geographical object characteristic.",
                "The textual description of the agricultural process for this crop production.",
                "The textual description of this agricultural certificate.",
                "The textual description of this agricultural characteristic.",
                "The textual description of this agricultural country sub-division.",
                "The textual description of this agricultural input chemical.",
                "The textual description of this agricultural input material.",
                "The textual description of this agricultural input product.",
                "The textual description of this agricultural plot.",
                "The textual description of this agricultural process crop input.",
                "The textual description of this agricultural process crop stage.",
                "The textual description of this agricultural process work item.",
                "The textual description of this agricultural producer party.",
                "The textual description of this agronomical observation plot.",
                "The textual description of this agronomical observation target object.",
                "The textual description of this complaint issue.",
                "The textual description of this crop report document.",
                "The textual description of this cross border animal movement issue.",
                "The textual description of this livestock animal product.",
                "The textual description of this plot agricultural process.",
                "The textual description of this soil occupation contract.",
                "The textual description of this specified geographical feature."
            ],
            "rdfs:label": "description",
            "unece:cefactElementMetadata": [
                {
                    "@id": "cefact:AgronomicalObservation_TargetObject.Description.Text",
                    "@type": "unece:BasicBIE",
                    "unece:cefactUNId": "UN01009322",
                    "unece:cefactBieDomainClass": "cefact:AgronomicalObservation_TargetObject.Details",
                    "rdfs:comment": "The textual description of this agronomical observation target object."
                },
                {
                    "@id": "cefact:SPSProcess_Characteristic.Description.Text",
                    "@type": "unece:BasicBIE",
                    "unece:TDED": "9018",
                    "unece:cefactUNId": "UN03000179",
                    "unece:cefactBieDomainClass": "cefact:SPSProcess_Characteristic.Details",
                    "rdfs:comment": "A textual description of this SPS process characteristic."
                },
                {
                    "@id": "cefact:LivestockAnimal_Product.Description.Text",
                    "@type": "unece:BasicBIE",
                    "unece:cefactUNId": "UN01007708",
                    "unece:cefactBieDomainClass": "cefact:LivestockAnimal_Product.Details",
                    "rdfs:comment": "The textual description of this livestock animal product."
                },
                {
                    "@id": "cefact:AgriculturalProducer_Party.Description.Text",
                    "@type": "unece:BasicBIE",
                    "unece:cefactUNId": "UN01012261",
                    "unece:cefactBieDomainClass": "cefact:AgriculturalProducer_Party.Details",
                    "rdfs:comment": "The textual description of this agricultural producer party."
                },
                {
                    "@id": "cefact:CropReport_Document.Description.Text",
                    "@type": "unece:BasicBIE",
                    "unece:cefactUNId": "UN01012432",
                    "unece:cefactBieDomainClass": "cefact:CropReport_Document.Details",
                    "rdfs:comment": "The textual description of this crop report document."
                },
                {
                    "@id": "cefact:AgriculturalInput_Chemical.Description.Text",
                    "@type": "unece:BasicBIE",
                    "unece:cefactUNId": "UN01012406",
                    "unece:cefactBieDomainClass": "cefact:AgriculturalInput_Chemical.Details",
                    "rdfs:comment": "The textual description of this agricultural input chemical."
                },
                {
                    "@id": "cefact:Plot_AgriculturalProcess.Description.Text",
                    "@type": "unece:BasicBIE",
                    "unece:cefactUNId": "UN01002786",
                    "unece:cefactBieDomainClass": "cefact:Plot_AgriculturalProcess.Details",
                    "rdfs:comment": "The textual description of this plot agricultural process."
                },
                {
                    "@id": "cefact:AgriculturalProcess_CropStage.Description.Text",
                    "@type": "unece:BasicBIE",
                    "unece:cefactUNId": "UN01002698",
                    "unece:cefactBieDomainClass": "cefact:AgriculturalProcess_CropStage.Details",
                    "rdfs:comment": "The textual description of this agricultural process crop stage."
                },
                {
                    "@id": "cefact:CrossBorderAnimalMovement_Issue.Description.Text",
                    "@type": "unece:BasicBIE",
                    "unece:cefactUNId": "UN01007668",
                    "unece:cefactBieDomainClass": "cefact:CrossBorderAnimalMovement_Issue.Details",
                    "rdfs:comment": "The textual description of this cross border animal movement issue."
                },
                {
                    "@id": "cefact:Complaint_Issue.Description.Text",
                    "@type": "unece:BasicBIE",
                    "unece:cefactUNId": "UN01012270",
                    "unece:cefactBieDomainClass": "cefact:Complaint_Issue.Details",
                    "rdfs:comment": "The textual description of this complaint issue."
                },
                {
                    "@id": "cefact:Field_Crop.Description.Text",
                    "@type": "unece:BasicBIE",
                    "unece:cefactUNId": "UN01012300",
                    "unece:cefactBieDomainClass": "cefact:Field_Crop.Details",
                    "rdfs:comment": "The textual description for this field crop."
                },
                {
                    "@id": "cefact:SPSExchanged_Document.Description.Text",
                    "@type": "unece:BasicBIE",
                    "unece:TDED": "4142",
                    "unece:cefactUNId": "UN03000004",
                    "unece:cefactBieDomainClass": "cefact:SPSExchanged_Document.Details",
                    "rdfs:comment": "A textual description of this exchanged SPS document."
                },
                {
                    "@id": "cefact:AgriculturalProcess_WorkItem.Description.Text",
                    "@type": "unece:BasicBIE",
                    "unece:cefactUNId": "UN01002806",
                    "unece:cefactBieDomainClass": "cefact:AgriculturalProcess_WorkItem.Details",
                    "rdfs:comment": "The textual description of this agricultural process work item."
                },
                {
                    "@id": "cefact:Agricultural_CountrySub-Division.Description.Text",
                    "@type": "unece:BasicBIE",
                    "unece:cefactUNId": "UN01002779",
                    "unece:cefactBieDomainClass": "cefact:Agricultural_CountrySubDivision.Details",
                    "rdfs:comment": "The textual description of this agricultural country sub-division."
                },
                {
                    "@id": "cefact:AgriculturalInput_Material.Description.Text",
                    "@type": "unece:BasicBIE",
                    "unece:cefactUNId": "UN01012399",
                    "unece:cefactBieDomainClass": "cefact:AgriculturalInput_Material.Details",
                    "rdfs:comment": "The textual description of this agricultural input material."
                },
                {
                    "@id": "cefact:AgriculturalProcess_CropInput.Description.Text",
                    "@type": "unece:BasicBIE",
                    "unece:cefactUNId": "UN01002726",
                    "unece:cefactBieDomainClass": "cefact:AgriculturalProcess_CropInput.Details",
                    "rdfs:comment": "The textual description of this agricultural process crop input."
                },
                {
                    "@id": "cefact:SoilOccupation_Contract.Description.Text",
                    "@type": "unece:BasicBIE",
                    "unece:cefactUNId": "UN01002823",
                    "unece:cefactBieDomainClass": "cefact:SoilOccupation_Contract.Details",
                    "rdfs:comment": "The textual description of this soil occupation contract."
                },
                {
                    "@id": "cefact:AgronomicalObservation_Plot.Description.Text",
                    "@type": "unece:BasicBIE",
                    "unece:cefactUNId": "UN01009368",
                    "unece:cefactBieDomainClass": "cefact:AgronomicalObservation_Plot.Details",
                    "rdfs:comment": "The textual description of this agronomical observation plot."
                },
                {
                    "@id": "cefact:Agricultural_Plot.Description.Text",
                    "@type": "unece:BasicBIE",
                    "unece:cefactUNId": "UN01002654",
                    "unece:cefactBieDomainClass": "cefact:Agricultural_Plot.Details",
                    "rdfs:comment": "The textual description of this agricultural plot."
                },
                {
                    "@id": "cefact:Disease_ProtectionMeans.Description.Text",
                    "@type": "unece:BasicBIE",
                    "unece:cefactUNId": "UN01015114",
                    "unece:cefactBieDomainClass": "cefact:Disease_ProtectionMeans.Details",
                    "rdfs:comment": "A textual description of this disease protection means."
                },
                {
                    "@id": "cefact:Agricultural_Characteristic.Description.Text",
                    "@type": "unece:BasicBIE",
                    "unece:TDED": "7036",
                    "unece:cefactUNId": "UN01012362",
                    "unece:cefactBieDomainClass": "cefact:Agricultural_Characteristic.Details",
                    "rdfs:comment": "The textual description of this agricultural characteristic."
                },
                {
                    "@id": "cefact:Specified_GeographicalFeature.Description.Text",
                    "@type": "unece:BasicBIE",
                    "unece:cefactUNId": "UN01012169",
                    "unece:cefactBieDomainClass": "cefact:Specified_GeographicalFeature.Details",
                    "rdfs:comment": "The textual description of this specified geographical feature."
                },
                {
                    "@id": "cefact:Crop_SpeciesVariety.Description.Text",
                    "@type": "unece:BasicBIE",
                    "unece:cefactUNId": "UN01009347",
                    "unece:cefactBieDomainClass": "cefact:Crop_SpeciesVariety.Details",
                    "rdfs:comment": "The textual description for this crop species variety."
                },
                {
                    "@id": "cefact:AgronomicalObservation_Party.Description.Text",
                    "@type": "unece:BasicBIE",
                    "unece:cefactUNId": "UN01009304",
                    "unece:cefactBieDomainClass": "cefact:AgronomicalObservation_Party.Details",
                    "rdfs:comment": "The textual description for this agronomical observation party."
                },
                {
                    "@id": "cefact:CropDataSheet_Party.Description.Text",
                    "@type": "unece:BasicBIE",
                    "unece:cefactUNId": "UN01002810",
                    "unece:cefactBieDomainClass": "cefact:CropDataSheet_Party.Details",
                    "rdfs:comment": "The textual description for this crop data sheet party."
                },
                {
                    "@id": "cefact:Agricultural_Certificate.Description.Text",
                    "@type": "unece:BasicBIE",
                    "unece:cefactUNId": "UN01012285",
                    "unece:cefactBieDomainClass": "cefact:Agricultural_Certificate.Details",
                    "rdfs:comment": "The textual description of this agricultural certificate."
                },
                {
                    "@id": "cefact:Specified_GeographicalObjectCharacteristic.Description.Text",
                    "@type": "unece:BasicBIE",
                    "unece:cefactUNId": "UN01012370",
                    "unece:cefactBieDomainClass": "cefact:Specified_GeographicalObjectCharacteristic.Details",
                    "rdfs:comment": "The textual description for this geographical object characteristic."
                },
                {
                    "@id": "cefact:Agricultural_Crop.Description.Text",
                    "@type": "unece:BasicBIE",
                    "unece:cefactUNId": "UN01009345",
                    "unece:cefactBieDomainClass": "cefact:Agricultural_Crop.Details",
                    "rdfs:comment": "The textual description for this agricultural crop."
                },
                {
                    "@id": "cefact:AgriculturalInput_Product.Description.Text",
                    "@type": "unece:BasicBIE",
                    "unece:cefactUNId": "UN01012376",
                    "unece:cefactBieDomainClass": "cefact:AgriculturalInput_Product.Details",
                    "rdfs:comment": "The textual description of this agricultural input product."
                },
                {
                    "@id": "cefact:CropProduction_AgriculturalProcess.Description.Text",
                    "@type": "unece:BasicBIE",
                    "unece:cefactUNId": "UN01012416",
                    "unece:cefactBieDomainClass": "cefact:CropProduction_AgriculturalProcess.Details",
                    "rdfs:comment": "The textual description of the agricultural process for this crop production."
                },
                {
                    "@id": "cefact:SPS_TradeLineItem.Description.Text",
                    "@type": "unece:BasicBIE",
                    "unece:TDED": "7008",
                    "unece:cefactUNId": "UN03000148",
                    "unece:cefactBieDomainClass": "cefact:SPS_TradeLineItem.Details",
                    "rdfs:comment": "A textual description of this SPS trade line item."
                },
                {
                    "@id": "cefact:Specified_CropProtectionTreatment.Description.Text",
                    "@type": "unece:BasicBIE",
                    "unece:cefactUNId": "UN01014288",
                    "unece:cefactBieDomainClass": "cefact:Specified_CropProtectionTreatment.Details",
                    "rdfs:comment": "A textual description of this specified crop protection treatment."
                }
            ]
        },
        {
            "@id": "agriculture:descriptionCode",
            "@type": "rdf:Property",
            "schema:rangeIncludes": {
                "@id": "xsd:token"
            },
            "schema:domainIncludes": [
                {
                    "@id": "agriculture:Construction"
                },
                {
                    "@id": "agriculture:Product"
                }
            ],
            "rdfs:comment": [
                "A code specifying the description for this agricultural construction.",
                "The code specifying the description of this agricultural input product."
            ],
            "rdfs:label": "descriptionCode",
            "unece:cefactElementMetadata": [
                {
                    "@id": "cefact:AgriculturalInput_Product.Description.Code",
                    "@type": "unece:BasicBIE",
                    "unece:cefactUNId": "UN01012380",
                    "unece:cefactBieDomainClass": "cefact:AgriculturalInput_Product.Details",
                    "rdfs:comment": "The code specifying the description of this agricultural input product."
                },
                {
                    "@id": "cefact:Agricultural_Construction.Description.Code",
                    "@type": "unece:BasicBIE",
                    "unece:cefactUNId": "UN01012228",
                    "unece:cefactBieDomainClass": "cefact:Agricultural_Construction.Details",
                    "rdfs:comment": "A code specifying the description for this agricultural construction."
                }
            ]
        },
        {
            "@id": "agriculture:descriptionReference",
            "@type": "rdf:Property",
            "schema:rangeIncludes": {
                "@id": "xsd:string"
            },
            "schema:domainIncludes": {
                "@id": "agriculture:GeographicalObjectCharacteristic"
            },
            "rdfs:comment": "The description reference, expressed as text, for this geographical object characteristic.",
            "rdfs:label": "descriptionReference",
            "unece:cefactElementMetadata": [
                {
                    "@id": "cefact:Specified_GeographicalObjectCharacteristic.DescriptionReference.Text",
                    "@type": "unece:BasicBIE",
                    "unece:cefactUNId": "UN01012371",
                    "unece:cefactBieDomainClass": "cefact:Specified_GeographicalObjectCharacteristic.Details",
                    "rdfs:comment": "The description reference, expressed as text, for this geographical object characteristic."
                }
            ]
        },
        {
            "@id": "agriculture:designatedParty",
            "@type": "rdf:Property",
            "schema:rangeIncludes": {
                "@id": "agriculture:Party"
            },
            "schema:domainIncludes": {
                "@id": "agriculture:Party"
            },
            "rdfs:comment": "A specified party designated for this agricultural producer party.",
            "rdfs:label": "designatedParty",
            "unece:cefactElementMetadata": [
                {
                    "@id": "cefact:AgriculturalProducer_Party.Designated.Specified_Party",
                    "@type": "unece:AssociationBIE",
                    "unece:cefactUNId": "UN01012265",
                    "unece:cefactBieDomainClass": "cefact:AgriculturalProducer_Party.Details",
                    "rdfs:comment": "A specified party designated for this agricultural producer party."
                }
            ]
        },
        {
            "@id": "agriculture:designatedSection",
            "@type": "rdf:Property",
            "schema:rangeIncludes": {
                "@id": "xsd:string"
            },
            "schema:domainIncludes": {
                "@id": "agriculture:Area"
            },
            "rdfs:comment": "The designated section, expressed as text, of this agricultural zone area.",
            "rdfs:label": "designatedSection",
            "unece:cefactElementMetadata": [
                {
                    "@id": "cefact:AgriculturalZone_Area.DesignatedSection.Text",
                    "@type": "unece:BasicBIE",
                    "unece:cefactUNId": "UN01012217",
                    "unece:cefactBieDomainClass": "cefact:AgriculturalZone_Area.Details",
                    "rdfs:comment": "The designated section, expressed as text, of this agricultural zone area."
                }
            ]
        },
        {
            "@id": "agriculture:despatchEvent",
            "@type": "rdf:Property",
            "schema:rangeIncludes": {
                "@id": "agriculture:Event"
            },
            "schema:domainIncludes": {
                "@id": "agriculture:TradeDelivery"
            },
            "rdfs:comment": "A Track and Trace (TT) despatch event for this animal trade delivery.",
            "rdfs:label": "despatchEvent",
            "unece:cefactElementMetadata": [
                {
                    "@id": "cefact:Animal_TradeDelivery.Despatch.TT_Event",
                    "@type": "unece:AssociationBIE",
                    "unece:cefactUNId": "UN01011267",
                    "unece:cefactBieDomainClass": "cefact:Animal_TradeDelivery.Details",
                    "rdfs:comment": "A Track and Trace (TT) despatch event for this animal trade delivery."
                }
            ]
        },
        {
            "@id": "agriculture:despatchParty",
            "@type": "rdf:Property",
            "schema:rangeIncludes": {
                "@id": "agriculture:Party"
            },
            "schema:domainIncludes": {
                "@id": "agriculture:Consignment"
            },
            "rdfs:comment": "The party from whom this SPS consignment will be or has been despatched.",
            "rdfs:label": "despatchParty",
            "unece:cefactElementMetadata": [
                {
                    "@id": "cefact:SPS_Consignment.Despatch.SPS_Party",
                    "@type": "unece:AssociationBIE",
                    "unece:cefactUNId": "UN03000071",
                    "unece:cefactBieDomainClass": "cefact:SPS_Consignment.Details",
                    "rdfs:comment": "The party from whom this SPS consignment will be or has been despatched."
                }
            ]
        },
        {
            "@id": "agriculture:destinationRelatedCountry",
            "@type": "rdf:Property",
            "schema:rangeIncludes": {
                "@id": "agriculture:Country"
            },
            "schema:domainIncludes": {
                "@id": "agriculture:Event"
            },
            "rdfs:comment": "The referenced country of destination related to this cross border animal movement event.",
            "rdfs:label": "destinationRelatedCountry",
            "unece:cefactElementMetadata": [
                {
                    "@id": "cefact:CrossBorderAnimalMovement_Event.Destination_Related.Referenced_Country",
                    "@type": "unece:AssociationBIE",
                    "unece:cefactUNId": "UN01007666",
                    "unece:cefactBieDomainClass": "cefact:CrossBorderAnimalMovement_Event.Details",
                    "rdfs:comment": "The referenced country of destination related to this cross border animal movement event."
                }
            ]
        },
        {
            "@id": "agriculture:detailTypeCode",
            "@type": "rdf:Property",
            "schema:rangeIncludes": {
                "@id": "xsd:token"
            },
            "schema:domainIncludes": {
                "@id": "agriculture:Reason"
            },
            "rdfs:comment": "The code specifying the detail type for this agricultural process reason.",
            "rdfs:label": "detailTypeCode",
            "unece:cefactElementMetadata": [
                {
                    "@id": "cefact:AgriculturalProcess_Reason.Detail_Type.Code",
                    "@type": "unece:BasicBIE",
                    "unece:cefactUNId": "UN01002744",
                    "unece:cefactBieDomainClass": "cefact:AgriculturalProcess_Reason.Details",
                    "rdfs:comment": "The code specifying the detail type for this agricultural process reason."
                }
            ]
        },
        {
            "@id": "agriculture:developmentStageCode",
            "@type": "rdf:Property",
            "schema:rangeIncludes": {
                "@id": "xsd:token"
            },
            "schema:domainIncludes": [
                {
                    "@id": "agriculture:Crop"
                },
                {
                    "@id": "agriculture:TargetObject"
                }
            ],
            "rdfs:comment": [
                "The code specifying the development stage for this agricultural crop.",
                "The code specifying the development stage for this agronomical observation target object."
            ],
            "rdfs:label": "developmentStageCode",
            "unece:cefactElementMetadata": [
                {
                    "@id": "cefact:Agricultural_Crop.DevelopmentStage.Code",
                    "@type": "unece:BasicBIE",
                    "unece:cefactUNId": "UN01009346",
                    "unece:cefactBieDomainClass": "cefact:Agricultural_Crop.Details",
                    "rdfs:comment": "The code specifying the development stage for this agricultural crop."
                },
                {
                    "@id": "cefact:AgronomicalObservation_TargetObject.DevelopmentStage.Code",
                    "@type": "unece:BasicBIE",
                    "unece:cefactUNId": "UN01009321",
                    "unece:cefactBieDomainClass": "cefact:AgronomicalObservation_TargetObject.Details",
                    "rdfs:comment": "The code specifying the development stage for this agronomical observation target object."
                }
            ]
        },
        {
            "@id": "agriculture:dimensionNumeric",
            "@type": "rdf:Property",
            "schema:rangeIncludes": {
                "@id": "xsd:decimal"
            },
            "schema:domainIncludes": {
                "@id": "agriculture:GeographicalGrid"
            },
            "rdfs:comment": "The dimension, expressed as a number, of this geographical grid.",
            "rdfs:label": "dimensionNumeric",
            "unece:cefactElementMetadata": [
                {
                    "@id": "cefact:Specified_GeographicalGrid.Dimension.Numeric",
                    "@type": "unece:BasicBIE",
                    "unece:cefactUNId": "UN01012208",
                    "unece:cefactBieDomainClass": "cefact:Specified_GeographicalGrid.Details",
                    "rdfs:comment": "The dimension, expressed as a number, of this geographical grid."
                }
            ]
        },
        {
            "@id": "agriculture:dividedIndicator",
            "@type": "rdf:Property",
            "schema:rangeIncludes": {
                "@id": "xsd:boolean"
            },
            "schema:domainIncludes": {
                "@id": "agriculture:Plot"
            },
            "rdfs:comment": "The indication of whether or not this agricultural plot has been divided.",
            "rdfs:label": "dividedIndicator",
            "unece:cefactElementMetadata": [
                {
                    "@id": "cefact:Agricultural_Plot.Divided.Indicator",
                    "@type": "unece:BasicBIE",
                    "unece:cefactUNId": "UN01002658",
                    "unece:cefactBieDomainClass": "cefact:Agricultural_Plot.Details",
                    "rdfs:comment": "The indication of whether or not this agricultural plot has been divided."
                }
            ]
        },
        {
            "@id": "agriculture:documentTypeCode",
            "@type": "rdf:Property",
            "schema:rangeIncludes": {
                "@id": "unece:UNECECL1001Code"
            },
            "schema:domainIncludes": {
                "@id": "agriculture:Document"
            },
            "rdfs:comment": [
                "The code specifying the type of exchanged SPS document.",
                "The code specifying the type of referenced SPS document."
            ],
            "rdfs:label": "documentTypeCode",
            "unece:cefactElementMetadata": [
                {
                    "@id": "cefact:SPSExchanged_Document.Type.Code",
                    "@type": "unece:BasicBIE",
                    "unece:TDED": "1001",
                    "unece:cefactUNId": "UN03000005",
                    "unece:cefactBieDomainClass": "cefact:SPSExchanged_Document.Details",
                    "rdfs:comment": "The code specifying the type of exchanged SPS document."
                },
                {
                    "@id": "cefact:SPSReferenced_Document.Type.Code",
                    "@type": "unece:BasicBIE",
                    "unece:TDED": "1001",
                    "unece:cefactUNId": "UN03000016",
                    "unece:cefactBieDomainClass": "cefact:SPSReferenced_Document.Details",
                    "rdfs:comment": "The code specifying the type of referenced SPS document."
                }
            ]
        },
        {
            "@id": "agriculture:durationMeasure",
            "@type": "rdf:Property",
            "schema:rangeIncludes": {
                "@id": "xsd:decimal"
            },
            "schema:domainIncludes": {
                "@id": "agriculture:Period"
            },
            "rdfs:comment": "The measure of the length of time for this SPS period such as hours, days, weeks, months or years.",
            "rdfs:label": "durationMeasure",
            "unece:cefactElementMetadata": [
                {
                    "@id": "cefact:SPS_Period.Duration.Measure",
                    "@type": "unece:BasicBIE",
                    "unece:cefactUNId": "UN03000122",
                    "unece:cefactBieDomainClass": "cefact:SPS_Period.Details",
                    "rdfs:comment": "The measure of the length of time for this SPS period such as hours, days, weeks, months or years."
                }
            ]
        },
        {
            "@id": "agriculture:earliestStartDateTime",
            "@type": "rdf:Property",
            "schema:rangeIncludes": {
                "@id": "xsd:dateTime"
            },
            "schema:domainIncludes": {
                "@id": "agriculture:AgriculturalProcess"
            },
            "rdfs:comment": "The date, time, date time or other date time value for the earliest start of the crop production in this agricultural process.",
            "rdfs:label": "earliestStartDateTime",
            "unece:cefactElementMetadata": [
                {
                    "@id": "cefact:CropProduction_AgriculturalProcess.Earliest_Start.DateTime",
                    "@type": "unece:BasicBIE",
                    "unece:cefactUNId": "UN01012411",
                    "unece:cefactBieDomainClass": "cefact:CropProduction_AgriculturalProcess.Details",
                    "rdfs:comment": "The date, time, date time or other date time value for the earliest start of the crop production in this agricultural process."
                }
            ]
        },
        {
            "@id": "agriculture:endDateTime",
            "@type": "rdf:Property",
            "schema:rangeIncludes": {
                "@id": "xsd:dateTime"
            },
            "schema:domainIncludes": [
                {
                    "@id": "agriculture:CropProductionCycle"
                },
                {
                    "@id": "agriculture:Period"
                },
                {
                    "@id": "agriculture:Plot"
                },
                {
                    "@id": "agriculture:SoilOccupation"
                }
            ],
            "rdfs:comment": [
                "The date or date time value for the end of this plot soil occupation.",
                "The date or date time value of the end of this agricultural crop production cycle.",
                "The date, time, date time or other date time value for the end of this SPS period.",
                "The date, time, date time, or other date time value for the end of this crop plot."
            ],
            "rdfs:label": "endDateTime",
            "unece:cefactElementMetadata": [
                {
                    "@id": "cefact:SPS_Period.End.DateTime",
                    "@type": "unece:BasicBIE",
                    "unece:cefactUNId": "UN03000121",
                    "unece:cefactBieDomainClass": "cefact:SPS_Period.Details",
                    "rdfs:comment": "The date, time, date time or other date time value for the end of this SPS period."
                },
                {
                    "@id": "cefact:Agricultural_CropProductionCycle.End.DateTime",
                    "@type": "unece:BasicBIE",
                    "unece:cefactUNId": "UN01002765",
                    "unece:cefactBieDomainClass": "cefact:Agricultural_CropProductionCycle.Details",
                    "rdfs:comment": "The date or date time value of the end of this agricultural crop production cycle."
                },
                {
                    "@id": "cefact:Crop_Plot.End.DateTime",
                    "@type": "unece:BasicBIE",
                    "unece:cefactUNId": "UN01012141",
                    "unece:cefactBieDomainClass": "cefact:Crop_Plot.Details",
                    "rdfs:comment": "The date, time, date time, or other date time value for the end of this crop plot."
                },
                {
                    "@id": "cefact:Plot_SoilOccupation.End.DateTime",
                    "@type": "unece:BasicBIE",
                    "unece:cefactUNId": "UN01002753",
                    "unece:cefactBieDomainClass": "cefact:Plot_SoilOccupation.Details",
                    "rdfs:comment": "The date or date time value for the end of this plot soil occupation."
                }
            ]
        },
        {
            "@id": "agriculture:estimatedYieldMeasure",
            "@type": "rdf:Property",
            "schema:rangeIncludes": {
                "@id": "xsd:decimal"
            },
            "schema:domainIncludes": {
                "@id": "agriculture:Produce"
            },
            "rdfs:comment": [
                "A measure of the estimated yield, such as weight per surface area unit, of this crop produce.",
                "The measure of the estimated yield of this agricultural produce, such as weight per surface area unit."
            ],
            "rdfs:label": "estimatedYieldMeasure",
            "unece:cefactElementMetadata": [
                {
                    "@id": "cefact:Crop_Produce.Estimated_Yield.Measure",
                    "@type": "unece:BasicBIE",
                    "unece:cefactUNId": "UN01013744",
                    "unece:cefactBieDomainClass": "cefact:Crop_Produce.Details",
                    "rdfs:comment": "A measure of the estimated yield, such as weight per surface area unit, of this crop produce."
                },
                {
                    "@id": "cefact:Agricultural_Produce.Estimated_Yield.Measure",
                    "@type": "unece:BasicBIE",
                    "unece:cefactUNId": "UN01002706",
                    "unece:cefactBieDomainClass": "cefact:Agricultural_Produce.Details",
                    "rdfs:comment": "The measure of the estimated yield of this agricultural produce, such as weight per surface area unit."
                }
            ]
        },
        {
            "@id": "agriculture:europeanCAPId",
            "@type": "rdf:Property",
            "schema:rangeIncludes": {
                "@id": "xsd:token"
            },
            "schema:domainIncludes": {
                "@id": "agriculture:Plot"
            },
            "rdfs:comment": "The European Common Agricultural Policy (CAP) identifier for this agronomical observation plot.",
            "rdfs:label": "europeanCAPId",
            "unece:cefactElementMetadata": [
                {
                    "@id": "cefact:AgronomicalObservation_Plot.EuropeanCAP_Identification.Identifier",
                    "@type": "unece:BasicBIE",
                    "unece:cefactUNId": "UN01009374",
                    "unece:cefactBieDomainClass": "cefact:AgronomicalObservation_Plot.Details",
                    "rdfs:comment": "The European Common Agricultural Policy (CAP) identifier for this agronomical observation plot."
                }
            ]
        },
        {
            "@id": "agriculture:examinationEvent",
            "@type": "rdf:Property",
            "schema:rangeIncludes": {
                "@id": "agriculture:Event"
            },
            "schema:domainIncludes": {
                "@id": "agriculture:Consignment"
            },
            "rdfs:comment": "The examination event for this SPS consignment.",
            "rdfs:label": "examinationEvent",
            "unece:cefactElementMetadata": [
                {
                    "@id": "cefact:SPS_Consignment.Examination.SPS_Event",
                    "@type": "unece:AssociationBIE",
                    "unece:cefactUNId": "UN03000069",
                    "unece:cefactBieDomainClass": "cefact:SPS_Consignment.Details",
                    "rdfs:comment": "The examination event for this SPS consignment."
                }
            ]
        },
        {
            "@id": "agriculture:executionParty",
            "@type": "rdf:Property",
            "schema:rangeIncludes": {
                "@id": "agriculture:Party"
            },
            "schema:domainIncludes": [
                {
                    "@id": "agriculture:Analysis"
                },
                {
                    "@id": "agriculture:Inspection"
                }
            ],
            "rdfs:comment": [
                "The crop data sheet party executing this agricultural analysis.",
                "The specified party executing this animal inspection."
            ],
            "rdfs:label": "executionParty",
            "unece:cefactElementMetadata": [
                {
                    "@id": "cefact:Animal_Inspection.Execution.Specified_Party",
                    "@type": "unece:AssociationBIE",
                    "unece:cefactUNId": "UN01007693",
                    "unece:cefactBieDomainClass": "cefact:Animal_Inspection.Details",
                    "rdfs:comment": "The specified party executing this animal inspection."
                },
                {
                    "@id": "cefact:Agricultural_Analysis.Execution.CropDataSheet_Party",
                    "@type": "unece:AssociationBIE",
                    "unece:cefactUNId": "UN01002667",
                    "unece:cefactBieDomainClass": "cefact:Agricultural_Analysis.Details",
                    "rdfs:comment": "The crop data sheet party executing this agricultural analysis."
                }
            ]
        },
        {
            "@id": "agriculture:executionPerson",
            "@type": "rdf:Property",
            "schema:rangeIncludes": {
                "@id": "agriculture:Person"
            },
            "schema:domainIncludes": {
                "@id": "agriculture:Inspection"
            },
            "rdfs:comment": "The inspection person executing this animal inspection.",
            "rdfs:label": "executionPerson",
            "unece:cefactElementMetadata": [
                {
                    "@id": "cefact:Animal_Inspection.Execution.Inspection_Person",
                    "@type": "unece:AssociationBIE",
                    "unece:cefactUNId": "UN01007694",
                    "unece:cefactBieDomainClass": "cefact:Animal_Inspection.Details",
                    "rdfs:comment": "The inspection person executing this animal inspection."
                }
            ]
        },
        {
            "@id": "agriculture:expectedVolumeMeasure",
            "@type": "rdf:Property",
            "schema:rangeIncludes": {
                "@id": "xsd:decimal"
            },
            "schema:domainIncludes": {
                "@id": "agriculture:CropInput"
            },
            "rdfs:comment": "The measure of the expected volume of this agricultural process crop input.",
            "rdfs:label": "expectedVolumeMeasure",
            "unece:cefactElementMetadata": [
                {
                    "@id": "cefact:AgriculturalProcess_CropInput.Expected_Volume.Measure",
                    "@type": "unece:BasicBIE",
                    "unece:cefactUNId": "UN01002730",
                    "unece:cefactBieDomainClass": "cefact:AgriculturalProcess_CropInput.Details",
                    "rdfs:comment": "The measure of the expected volume of this agricultural process crop input."
                }
            ]
        },
        {
            "@id": "agriculture:expiryDateTime",
            "@type": "rdf:Property",
            "schema:rangeIncludes": {
                "@id": "xsd:dateTime"
            },
            "schema:domainIncludes": [
                {
                    "@id": "agriculture:Certificate"
                },
                {
                    "@id": "agriculture:TradeLineItem"
                }
            ],
            "rdfs:comment": [
                "A date, time, date time or other date time value of expiry up to which this SPS trade line item is fit for purpose.",
                "The date, time, date time, or other date time value when this agricultural certificate expires."
            ],
            "rdfs:label": "expiryDateTime",
            "unece:cefactElementMetadata": [
                {
                    "@id": "cefact:Agricultural_Certificate.Expiry.DateTime",
                    "@type": "unece:BasicBIE",
                    "unece:cefactUNId": "UN01012280",
                    "unece:cefactBieDomainClass": "cefact:Agricultural_Certificate.Details",
                    "rdfs:comment": "The date, time, date time, or other date time value when this agricultural certificate expires."
                },
                {
                    "@id": "cefact:SPS_TradeLineItem.Expiry.DateTime",
                    "@type": "unece:BasicBIE",
                    "unece:cefactUNId": "UN03000153",
                    "unece:cefactBieDomainClass": "cefact:SPS_TradeLineItem.Details",
                    "rdfs:comment": "A date, time, date time or other date time value of expiry up to which this SPS trade line item is fit for purpose."
                }
            ]
        },
        {
            "@id": "agriculture:exportCountry",
            "@type": "rdf:Property",
            "schema:rangeIncludes": {
                "@id": "agriculture:Country"
            },
            "schema:domainIncludes": {
                "@id": "agriculture:Consignment"
            },
            "rdfs:comment": "The export country for this SPS consignment.",
            "rdfs:label": "exportCountry",
            "unece:cefactElementMetadata": [
                {
                    "@id": "cefact:SPS_Consignment.Export.SPS_Country",
                    "@type": "unece:AssociationBIE",
                    "unece:cefactUNId": "UN03000060",
                    "unece:cefactBieDomainClass": "cefact:SPS_Consignment.Details",
                    "rdfs:comment": "The export country for this SPS consignment."
                }
            ]
        },
        {
            "@id": "agriculture:exportExitDateTime",
            "@type": "rdf:Property",
            "schema:rangeIncludes": {
                "@id": "xsd:dateTime"
            },
            "schema:domainIncludes": {
                "@id": "agriculture:Consignment"
            },
            "rdfs:comment": "The date, time, date time, or other date time value when this SPS consignment will exit, or has exited from the last port, airport, or border post of the country of export.",
            "rdfs:label": "exportExitDateTime",
            "unece:cefactElementMetadata": [
                {
                    "@id": "cefact:SPS_Consignment.ExportExit.DateTime",
                    "@type": "unece:BasicBIE",
                    "unece:TDED": "2043",
                    "unece:cefactUNId": "UN03000056",
                    "unece:cefactBieDomainClass": "cefact:SPS_Consignment.Details",
                    "rdfs:comment": "The date, time, date time, or other date time value when this SPS consignment will exit, or has exited from the last port, airport, or border post of the country of export."
                }
            ]
        },
        {
            "@id": "agriculture:exportOccurrenceDateTime",
            "@type": "rdf:Property",
            "schema:rangeIncludes": {
                "@id": "xsd:dateTime"
            },
            "schema:domainIncludes": {
                "@id": "agriculture:Event"
            },
            "rdfs:comment": "The date of the occurrence of the export for this cross border animal movement event.",
            "rdfs:label": "exportOccurrenceDateTime",
            "unece:cefactElementMetadata": [
                {
                    "@id": "cefact:CrossBorderAnimalMovement_Event.Export_Occurrence.DateTime",
                    "@type": "unece:BasicBIE",
                    "unece:TDED": "2193",
                    "unece:cefactUNId": "UN01007662",
                    "unece:cefactBieDomainClass": "cefact:CrossBorderAnimalMovement_Event.Details",
                    "rdfs:comment": "The date of the occurrence of the export for this cross border animal movement event."
                }
            ]
        },
        {
            "@id": "agriculture:externalOperatorParty",
            "@type": "rdf:Property",
            "schema:rangeIncludes": {
                "@id": "agriculture:Party"
            },
            "schema:domainIncludes": {
                "@id": "agriculture:AgriculturalProcess"
            },
            "rdfs:comment": "The crop data sheet party that is the external operator for this plot agricultural process.",
            "rdfs:label": "externalOperatorParty",
            "unece:cefactElementMetadata": [
                {
                    "@id": "cefact:Plot_AgriculturalProcess.External_Operator.CropDataSheet_Party",
                    "@type": "unece:AssociationBIE",
                    "unece:cefactUNId": "UN01002791",
                    "unece:cefactBieDomainClass": "cefact:Plot_AgriculturalProcess.Details",
                    "rdfs:comment": "The crop data sheet party that is the external operator for this plot agricultural process."
                }
            ]
        },
        {
            "@id": "agriculture:fLUXId",
            "@type": "rdf:Property",
            "schema:rangeIncludes": {
                "@id": "xsd:token"
            },
            "schema:domainIncludes": {
                "@id": "agriculture:Batch"
            },
            "rdfs:comment": "A Fisheries Language for Universal eXchange (FLUX) identifier for this animal batch.",
            "rdfs:label": "fLUXId",
            "unece:cefactElementMetadata": [
                {
                    "@id": "cefact:Animal_Batch.FLUX_Identification.Identifier",
                    "@type": "unece:BasicBIE",
                    "unece:cefactUNId": "UN01011250",
                    "unece:cefactBieDomainClass": "cefact:Animal_Batch.Details",
                    "rdfs:comment": "A Fisheries Language for Universal eXchange (FLUX) identifier for this animal batch."
                }
            ]
        },
        {
            "@id": "agriculture:functionCode",
            "@type": "rdf:Property",
            "schema:rangeIncludes": {
                "@id": "xsd:token"
            },
            "schema:domainIncludes": {
                "@id": "agriculture:Construction"
            },
            "rdfs:comment": "A code specifying a function of this agricultural construction.",
            "rdfs:label": "functionCode",
            "unece:cefactElementMetadata": [
                {
                    "@id": "cefact:Agricultural_Construction.Function.Code",
                    "@type": "unece:BasicBIE",
                    "unece:cefactUNId": "UN01012233",
                    "unece:cefactBieDomainClass": "cefact:Agricultural_Construction.Details",
                    "rdfs:comment": "A code specifying a function of this agricultural construction."
                }
            ]
        },
        {
            "@id": "agriculture:genderCode",
            "@type": "rdf:Property",
            "schema:rangeIncludes": {
                "@id": "xsd:token"
            },
            "schema:domainIncludes": {
                "@id": "agriculture:Animal"
            },
            "rdfs:comment": "The code specifying the gender of this livestock animal, such as male, female or castrated.",
            "rdfs:label": "genderCode",
            "unece:cefactElementMetadata": [
                {
                    "@id": "cefact:Livestock_Animal.Gender.Code",
                    "@type": "unece:BasicBIE",
                    "unece:TDED": "3499",
                    "unece:cefactUNId": "UN01007646",
                    "unece:cefactBieDomainClass": "cefact:Livestock_Animal.Details",
                    "rdfs:comment": "The code specifying the gender of this livestock animal, such as male, female or castrated."
                }
            ]
        },
        {
            "@id": "agriculture:governmentActionTypeCode",
            "@type": "rdf:Property",
            "schema:rangeIncludes": {
                "@id": "unece:UNECECL9417Code"
            },
            "schema:domainIncludes": {
                "@id": "agriculture:Authentication"
            },
            "rdfs:comment": "The code specifying the type of SPS authentication.",
            "rdfs:label": "governmentActionTypeCode",
            "unece:cefactElementMetadata": [
                {
                    "@id": "cefact:SPS_Authentication.Type.Code",
                    "@type": "unece:BasicBIE",
                    "unece:TDED": "9417",
                    "unece:cefactUNId": "UN03000034",
                    "unece:cefactBieDomainClass": "cefact:SPS_Authentication.Details",
                    "rdfs:comment": "The code specifying the type of SPS authentication."
                }
            ]
        },
        {
            "@id": "agriculture:grossVolumeMeasure",
            "@type": "rdf:Property",
            "schema:rangeIncludes": {
                "@id": "xsd:decimal"
            },
            "schema:domainIncludes": {
                "@id": "agriculture:TradeLineItem"
            },
            "rdfs:comment": "The measure of the gross volume of this SPS trade line item, including all unoccupied volume of the packaging.",
            "rdfs:label": "grossVolumeMeasure",
            "unece:cefactElementMetadata": [
                {
                    "@id": "cefact:SPS_TradeLineItem.GrossVolume.Measure",
                    "@type": "unece:BasicBIE",
                    "unece:TDED": "6316",
                    "unece:cefactUNId": "UN03000157",
                    "unece:cefactBieDomainClass": "cefact:SPS_TradeLineItem.Details",
                    "rdfs:comment": "The measure of the gross volume of this SPS trade line item, including all unoccupied volume of the packaging."
                }
            ]
        },
        {
            "@id": "agriculture:grossWeightMeasure",
            "@type": "rdf:Property",
            "schema:rangeIncludes": {
                "@id": "xsd:decimal"
            },
            "schema:domainIncludes": {
                "@id": "agriculture:TradeLineItem"
            },
            "rdfs:comment": "The measure of the gross weight (mass) of this SPS trade line item, including packaging but excluding any associated transport equipment.",
            "rdfs:label": "grossWeightMeasure",
            "unece:cefactElementMetadata": [
                {
                    "@id": "cefact:SPS_TradeLineItem.GrossWeight.Measure",
                    "@type": "unece:BasicBIE",
                    "unece:TDED": "6018",
                    "unece:cefactUNId": "UN03000155",
                    "unece:cefactBieDomainClass": "cefact:SPS_TradeLineItem.Details",
                    "rdfs:comment": "The measure of the gross weight (mass) of this SPS trade line item, including packaging but excluding any associated transport equipment."
                }
            ]
        },
        {
            "@id": "agriculture:grownCrop",
            "@type": "rdf:Property",
            "schema:rangeIncludes": {
                "@id": "agriculture:Crop"
            },
            "schema:domainIncludes": [
                {
                    "@id": "agriculture:Plot"
                },
                {
                    "@id": "agriculture:ProductionUnit"
                }
            ],
            "rdfs:comment": [
                "A field crop grown on this agricultural production unit.",
                "A field crop grown on this crop plot."
            ],
            "rdfs:label": "grownCrop",
            "unece:cefactElementMetadata": [
                {
                    "@id": "cefact:Agricultural_ProductionUnit.Grown.Field_Crop",
                    "@type": "unece:AssociationBIE",
                    "unece:cefactUNId": "UN01012252",
                    "unece:cefactBieDomainClass": "cefact:Agricultural_ProductionUnit.Details",
                    "rdfs:comment": "A field crop grown on this agricultural production unit."
                },
                {
                    "@id": "cefact:Crop_Plot.Grown.Field_Crop",
                    "@type": "unece:AssociationBIE",
                    "unece:cefactUNId": "UN01012151",
                    "unece:cefactBieDomainClass": "cefact:Crop_Plot.Details",
                    "rdfs:comment": "A field crop grown on this crop plot."
                }
            ]
        },
        {
            "@id": "agriculture:grownPlot",
            "@type": "rdf:Property",
            "schema:rangeIncludes": {
                "@id": "agriculture:Plot"
            },
            "schema:domainIncludes": {
                "@id": "agriculture:Crop"
            },
            "rdfs:comment": "The plot where this field crop is grown.",
            "rdfs:label": "grownPlot",
            "unece:cefactElementMetadata": [
                {
                    "@id": "cefact:Field_Crop.Grown.Crop_Plot",
                    "@type": "unece:AssociationBIE",
                    "unece:cefactUNId": "UN01012312",
                    "unece:cefactBieDomainClass": "cefact:Field_Crop.Details",
                    "rdfs:comment": "The plot where this field crop is grown."
                }
            ]
        },
        {
            "@id": "agriculture:grownPreviousCrop",
            "@type": "rdf:Property",
            "schema:rangeIncludes": {
                "@id": "agriculture:Crop"
            },
            "schema:domainIncludes": {
                "@id": "agriculture:Crop"
            },
            "rdfs:comment": "A field crop grown previous to this field crop.",
            "rdfs:label": "grownPreviousCrop",
            "unece:cefactElementMetadata": [
                {
                    "@id": "cefact:Field_Crop.Grown_Previous.Field_Crop",
                    "@type": "unece:AssociationBIE",
                    "unece:cefactUNId": "UN01012311",
                    "unece:cefactBieDomainClass": "cefact:Field_Crop.Details",
                    "rdfs:comment": "A field crop grown previous to this field crop."
                }
            ]
        },
        {
            "@id": "agriculture:harvestDateTime",
            "@type": "rdf:Property",
            "schema:rangeIncludes": {
                "@id": "xsd:dateTime"
            },
            "schema:domainIncludes": {
                "@id": "agriculture:Crop"
            },
            "rdfs:comment": "The date, time, date time, or other date time value for the harvest of this field crop.",
            "rdfs:label": "harvestDateTime",
            "unece:cefactElementMetadata": [
                {
                    "@id": "cefact:Field_Crop.Harvest.DateTime",
                    "@type": "unece:BasicBIE",
                    "unece:cefactUNId": "UN01012307",
                    "unece:cefactBieDomainClass": "cefact:Field_Crop.Details",
                    "rdfs:comment": "The date, time, date time, or other date time value for the harvest of this field crop."
                }
            ]
        },
        {
            "@id": "agriculture:harvestYearDateTime",
            "@type": "rdf:Property",
            "schema:rangeIncludes": {
                "@id": "xsd:dateTime"
            },
            "schema:domainIncludes": {
                "@id": "agriculture:Plot"
            },
            "rdfs:comment": [
                "The date value specified as the harvest year for this agricultural plot.",
                "The date value specified as the harvest year for this agronomical observation plot."
            ],
            "rdfs:label": "harvestYearDateTime",
            "unece:cefactElementMetadata": [
                {
                    "@id": "cefact:AgronomicalObservation_Plot.HarvestYear.DateTime",
                    "@type": "unece:BasicBIE",
                    "unece:cefactUNId": "UN01009373",
                    "unece:cefactBieDomainClass": "cefact:AgronomicalObservation_Plot.Details",
                    "rdfs:comment": "The date value specified as the harvest year for this agronomical observation plot."
                },
                {
                    "@id": "cefact:Agricultural_Plot.HarvestYear.DateTime",
                    "@type": "unece:BasicBIE",
                    "unece:cefactUNId": "UN01009351",
                    "unece:cefactBieDomainClass": "cefact:Agricultural_Plot.Details",
                    "rdfs:comment": "The date value specified as the harvest year for this agricultural plot."
                }
            ]
        },
        {
            "@id": "agriculture:harvestedBatch",
            "@type": "rdf:Property",
            "schema:rangeIncludes": {
                "@id": "agriculture:Batch"
            },
            "schema:domainIncludes": {
                "@id": "agriculture:AgriculturalProcess"
            },
            "rdfs:comment": "A crop produce batch harvested in the crop production for this agricultural process.",
            "rdfs:label": "harvestedBatch",
            "unece:cefactElementMetadata": [
                {
                    "@id": "cefact:CropProduction_AgriculturalProcess.Harvested.CropProduce_Batch",
                    "@type": "unece:AssociationBIE",
                    "unece:cefactUNId": "UN01012417",
                    "unece:cefactBieDomainClass": "cefact:CropProduction_AgriculturalProcess.Details",
                    "rdfs:comment": "A crop produce batch harvested in the crop production for this agricultural process."
                }
            ]
        },
        {
            "@id": "agriculture:harvestedProduce",
            "@type": "rdf:Property",
            "schema:rangeIncludes": {
                "@id": "agriculture:Produce"
            },
            "schema:domainIncludes": [
                {
                    "@id": "agriculture:AgriculturalProcess"
                },
                {
                    "@id": "agriculture:Area"
                },
                {
                    "@id": "agriculture:Crop"
                }
            ],
            "rdfs:comment": [
                "Agricultural produce harvested in this plot agricultural process.",
                "Crop produce harvested from this agricultural zone area.",
                "Produce harvested from this field crop."
            ],
            "rdfs:label": "harvestedProduce",
            "unece:cefactElementMetadata": [
                {
                    "@id": "cefact:AgriculturalZone_Area.Harvested.Crop_Produce",
                    "@type": "unece:AssociationBIE",
                    "unece:cefactUNId": "UN01012222",
                    "unece:cefactBieDomainClass": "cefact:AgriculturalZone_Area.Details",
                    "rdfs:comment": "Crop produce harvested from this agricultural zone area."
                },
                {
                    "@id": "cefact:Plot_AgriculturalProcess.Harvested.Agricultural_Produce",
                    "@type": "unece:AssociationBIE",
                    "unece:cefactUNId": "UN01002795",
                    "unece:cefactBieDomainClass": "cefact:Plot_AgriculturalProcess.Details",
                    "rdfs:comment": "Agricultural produce harvested in this plot agricultural process."
                },
                {
                    "@id": "cefact:Field_Crop.Harvested.Crop_Produce",
                    "@type": "unece:AssociationBIE",
                    "unece:cefactUNId": "UN01012314",
                    "unece:cefactBieDomainClass": "cefact:Field_Crop.Details",
                    "rdfs:comment": "Produce harvested from this field crop."
                }
            ]
        },
        {
            "@id": "agriculture:hierarchicalLevelCode",
            "@type": "rdf:Property",
            "schema:rangeIncludes": {
                "@id": "xsd:token"
            },
            "schema:domainIncludes": {
                "@id": "agriculture:CountrySubDivision"
            },
            "rdfs:comment": "The code specifying the hierarchical level of this SPS country sub-division.",
            "rdfs:label": "hierarchicalLevelCode",
            "unece:cefactElementMetadata": [
                {
                    "@id": "cefact:SPS_CountrySub-Division.HierarchicalLevel.Code",
                    "@type": "unece:BasicBIE",
                    "unece:TDED": "7168",
                    "unece:cefactUNId": "UN03000082",
                    "unece:cefactBieDomainClass": "cefact:SPS_CountrySubDivision.Details",
                    "rdfs:comment": "The code specifying the hierarchical level of this SPS country sub-division."
                }
            ]
        },
        {
            "@id": "agriculture:highLimit",
            "@type": "rdf:Property",
            "schema:rangeIncludes": {
                "@id": "xsd:string"
            },
            "schema:domainIncludes": {
                "@id": "agriculture:GeographicalGrid"
            },
            "rdfs:comment": "The tuple of elements, expressed as text, indicating the high limit of this geographical grid specifying the diagonally opposing corner of each axis.",
            "rdfs:label": "highLimit",
            "unece:cefactElementMetadata": [
                {
                    "@id": "cefact:Specified_GeographicalGrid.High_Limit.Text",
                    "@type": "unece:BasicBIE",
                    "unece:cefactUNId": "UN01012207",
                    "unece:cefactBieDomainClass": "cefact:Specified_GeographicalGrid.Details",
                    "rdfs:comment": "The tuple of elements, expressed as text, indicating the high limit of this geographical grid specifying the diagonally opposing corner of each axis."
                }
            ]
        },
        {
            "@id": "agriculture:id",
            "@type": "rdf:Property",
            "schema:rangeIncludes": {
                "@id": "xsd:token"
            },
            "schema:domainIncludes": [
                {
                    "@id": "agriculture:AgriculturalApplication"
                },
                {
                    "@id": "agriculture:AgriculturalDevice"
                },
                {
                    "@id": "agriculture:AgronomicalObservation"
                },
                {
                    "@id": "agriculture:Animal"
                },
                {
                    "@id": "agriculture:Area"
                },
                {
                    "@id": "agriculture:Batch"
                },
                {
                    "@id": "agriculture:Certificate"
                },
                {
                    "@id": "agriculture:Characteristic"
                },
                {
                    "@id": "agriculture:Chemical"
                },
                {
                    "@id": "agriculture:Clause"
                },
                {
                    "@id": "agriculture:Consignment"
                },
                {
                    "@id": "agriculture:Construction"
                },
                {
                    "@id": "agriculture:Contract"
                },
                {
                    "@id": "agriculture:CoordinateReferenceSystem"
                },
                {
                    "@id": "agriculture:Country"
                },
                {
                    "@id": "agriculture:CountrySubDivision"
                },
                {
                    "@id": "agriculture:CropInput"
                },
                {
                    "@id": "agriculture:CropProtectionTreatment"
                },
                {
                    "@id": "agriculture:Document"
                },
                {
                    "@id": "agriculture:GeographicalGrid"
                },
                {
                    "@id": "agriculture:GeographicalObjectCharacteristic"
                },
                {
                    "@id": "agriculture:Identity"
                },
                {
                    "@id": "agriculture:Issue"
                },
                {
                    "@id": "agriculture:Location"
                },
                {
                    "@id": "agriculture:Material"
                },
                {
                    "@id": "agriculture:Party"
                },
                {
                    "@id": "agriculture:Person"
                },
                {
                    "@id": "agriculture:Plot"
                },
                {
                    "@id": "agriculture:Produce"
                },
                {
                    "@id": "agriculture:Product"
                },
                {
                    "@id": "agriculture:ProductInstance"
                },
                {
                    "@id": "agriculture:ProductionUnit"
                },
                {
                    "@id": "agriculture:SampledObject"
                },
                {
                    "@id": "agriculture:Seal"
                },
                {
                    "@id": "agriculture:Tank"
                },
                {
                    "@id": "agriculture:TradeDelivery"
                },
                {
                    "@id": "agriculture:TransportEquipment"
                },
                {
                    "@id": "agriculture:TransportMovement"
                }
            ],
            "rdfs:comment": [
                "An identifier for this agricultural input material.",
                "An identifier for this crop produce.",
                "An identifier for this geographical grid.",
                "An identifier for this referenced country.",
                "An identifier of this specified crop protection treatment.",
                "The identifier for this CS engineering coordinate reference system.",
                "The identifier for this LA exchanged document.",
                "The identifier for this agricultural certificate.",
                "The identifier for this agricultural characteristic.",
                "The identifier for this agricultural construction.",
                "The identifier for this agricultural contract.",
                "The identifier for this agricultural input product.",
                "The identifier for this agricultural production unit.",
                "The identifier for this agricultural zone area.",
                "The identifier for this agronomical observation document.",
                "The identifier for this agronomical observation party.",
                "The identifier for this animal batch.",
                "The identifier for this animal certificate.",
                "The identifier for this animal identity.",
                "The identifier for this animal passport document.",
                "The identifier for this animal trade delivery.",
                "The identifier for this crop plot.",
                "The identifier for this crop produce batch.",
                "The identifier for this geographical object characteristic.",
                "The identifier for this livestock animal product instance, such as the number appearing on its ear tag.",
                "The identifier for this livestock animal, such as the number appearing on its ear tag.",
                "The identifier for this milk tank.",
                "The identifier for this mobile plot.",
                "The identifier for this operator person.",
                "The identifier for this product batch.",
                "The identifier for this sampled agricultural object.",
                "The identifier for this single agronomical observation.",
                "The identifier for this specified agricultural application.",
                "The identifier of the agricultural producer party.",
                "The identifier of the specified party.",
                "The identifier of this agricultural input chemical.",
                "The identifier of this complaint issue.",
                "The identifier of this crop report document.",
                "The unique identifier for this SPS country sub-division.",
                "The unique identifier for this SPS country.",
                "The unique identifier for this SPS location.",
                "The unique identifier for this agricultural country sub-division.",
                "The unique identifier for this agricultural plot.",
                "The unique identifier for this agricultural process crop input.",
                "The unique identifier for this agronomical observation plot.",
                "The unique identifier for this crop data sheet document.",
                "The unique identifier for this crop input batch.",
                "The unique identifier for this referenced SPS document.",
                "The unique identifier for this soil occupation contract.",
                "The unique identifier for this specified agricultural device.",
                "The unique identifier of this SPS clause.",
                "The unique identifier of this SPS consignment.",
                "The unique identifier of this SPS party.",
                "The unique identifier of this SPS seal.",
                "The unique identifier of this SPS transport movement, such as a voyage number, flight number, or trip number.",
                "The unique identifier of this crop data sheet party.",
                "The unique identifier of this exchanged SPS document.",
                "The unique identifier of this piece of SPS transport equipment."
            ],
            "rdfs:label": "id",
            "unece:cefactElementMetadata": [
                {
                    "@id": "cefact:Single_AgronomicalObservation.Identification.Identifier",
                    "@type": "unece:BasicBIE",
                    "unece:cefactUNId": "UN01009310",
                    "unece:cefactBieDomainClass": "cefact:Single_AgronomicalObservation.Details",
                    "rdfs:comment": "The identifier for this single agronomical observation."
                },
                {
                    "@id": "cefact:AgriculturalInput_Material.Identification.Identifier",
                    "@type": "unece:BasicBIE",
                    "unece:cefactUNId": "UN01012395",
                    "unece:cefactBieDomainClass": "cefact:AgriculturalInput_Material.Details",
                    "rdfs:comment": "An identifier for this agricultural input material."
                },
                {
                    "@id": "cefact:SPS_Seal.Identification.Identifier",
                    "@type": "unece:BasicBIE",
                    "unece:TDED": "9308",
                    "unece:cefactUNId": "UN03000136",
                    "unece:cefactBieDomainClass": "cefact:SPS_Seal.Details",
                    "rdfs:comment": "The unique identifier of this SPS seal."
                },
                {
                    "@id": "cefact:SPS_TransportMovement.Identification.Identifier",
                    "@type": "unece:BasicBIE",
                    "unece:TDED": "8028",
                    "unece:cefactUNId": "UN03000173",
                    "unece:cefactBieDomainClass": "cefact:SPS_TransportMovement.Details",
                    "rdfs:comment": "The unique identifier of this SPS transport movement, such as a voyage number, flight number, or trip number."
                },
                {
                    "@id": "cefact:SPS_TransportEquipment.Identification.Identifier",
                    "@type": "unece:BasicBIE",
                    "unece:TDED": "8260",
                    "unece:cefactUNId": "UN03000167",
                    "unece:cefactBieDomainClass": "cefact:SPS_TransportEquipment.Details",
                    "rdfs:comment": "The unique identifier of this piece of SPS transport equipment."
                },
                {
                    "@id": "cefact:Animal_Batch.Identification.Identifier",
                    "@type": "unece:BasicBIE",
                    "unece:cefactUNId": "UN01011245",
                    "unece:cefactBieDomainClass": "cefact:Animal_Batch.Details",
                    "rdfs:comment": "The identifier for this animal batch."
                },
                {
                    "@id": "cefact:CropDataSheet_Document.Identification.Identifier",
                    "@type": "unece:BasicBIE",
                    "unece:TDED": "1004",
                    "unece:cefactUNId": "UN01002814",
                    "unece:cefactBieDomainClass": "cefact:CropDataSheet_Document.Details",
                    "rdfs:comment": "The unique identifier for this crop data sheet document."
                },
                {
                    "@id": "cefact:Agricultural_Characteristic.Identification.Identifier",
                    "@type": "unece:BasicBIE",
                    "unece:cefactUNId": "UN01012360",
                    "unece:cefactBieDomainClass": "cefact:Agricultural_Characteristic.Details",
                    "rdfs:comment": "The identifier for this agricultural characteristic."
                },
                {
                    "@id": "cefact:AgriculturalInput_Chemical.Identification.Identifier",
                    "@type": "unece:BasicBIE",
                    "unece:cefactUNId": "UN01012402",
                    "unece:cefactBieDomainClass": "cefact:AgriculturalInput_Chemical.Details",
                    "rdfs:comment": "The identifier of this agricultural input chemical."
                },
                {
                    "@id": "cefact:Operator_Person.Identification.Identifier",
                    "@type": "unece:BasicBIE",
                    "unece:cefactUNId": "UN01012273",
                    "unece:cefactBieDomainClass": "cefact:Operator_Person.Details",
                    "rdfs:comment": "The identifier for this operator person."
                },
                {
                    "@id": "cefact:Agricultural_Contract.Identification.Identifier",
                    "@type": "unece:BasicBIE",
                    "unece:TDED": "1296",
                    "unece:cefactUNId": "UN01012445",
                    "unece:cefactBieDomainClass": "cefact:Agricultural_Contract.Details",
                    "rdfs:comment": "The identifier for this agricultural contract."
                },
                {
                    "@id": "cefact:CropProduce_Batch.Identification.Identifier",
                    "@type": "unece:BasicBIE",
                    "unece:cefactUNId": "UN01012332",
                    "unece:cefactBieDomainClass": "cefact:CropProduce_Batch.Details",
                    "rdfs:comment": "The identifier for this crop produce batch."
                },
                {
                    "@id": "cefact:Agricultural_Plot.Identification.Identifier",
                    "@type": "unece:BasicBIE",
                    "unece:cefactUNId": "UN01002652",
                    "unece:cefactBieDomainClass": "cefact:Agricultural_Plot.Details",
                    "rdfs:comment": "The unique identifier for this agricultural plot."
                },
                {
                    "@id": "cefact:Agricultural_Certificate.Identification.Identifier",
                    "@type": "unece:BasicBIE",
                    "unece:cefactUNId": "UN01012278",
                    "unece:cefactBieDomainClass": "cefact:Agricultural_Certificate.Details",
                    "rdfs:comment": "The identifier for this agricultural certificate."
                },
                {
                    "@id": "cefact:LAExchanged_Document.Identification.Identifier",
                    "@type": "unece:BasicBIE",
                    "unece:TDED": "1004",
                    "unece:cefactUNId": "UN01007698",
                    "unece:cefactBieDomainClass": "cefact:LAExchanged_Document.Details",
                    "rdfs:comment": "The identifier for this LA exchanged document."
                },
                {
                    "@id": "cefact:SPS_Location.Identification.Identifier",
                    "@type": "unece:BasicBIE",
                    "unece:TDED": "3225",
                    "unece:cefactUNId": "UN03000094",
                    "unece:cefactBieDomainClass": "cefact:SPS_Location.Details",
                    "rdfs:comment": "The unique identifier for this SPS location."
                },
                {
                    "@id": "cefact:SPS_Country.Identification.Identifier",
                    "@type": "unece:BasicBIE",
                    "unece:TDED": "3207",
                    "unece:cefactUNId": "UN03000088",
                    "unece:cefactBieDomainClass": "cefact:SPS_Country.Details",
                    "rdfs:comment": "The unique identifier for this SPS country."
                },
                {
                    "@id": "cefact:Specified_GeographicalGrid.Identification.Identifier",
                    "@type": "unece:BasicBIE",
                    "unece:cefactUNId": "UN01012204",
                    "unece:cefactBieDomainClass": "cefact:Specified_GeographicalGrid.Details",
                    "rdfs:comment": "An identifier for this geographical grid."
                },
                {
                    "@id": "cefact:SPS_CountrySub-Division.Identification.Identifier",
                    "@type": "unece:BasicBIE",
                    "unece:TDED": "3229",
                    "unece:cefactUNId": "UN03000080",
                    "unece:cefactBieDomainClass": "cefact:SPS_CountrySubDivision.Details",
                    "rdfs:comment": "The unique identifier for this SPS country sub-division."
                },
                {
                    "@id": "cefact:AgronomicalObservation_Document.Identification.Identifier",
                    "@type": "unece:BasicBIE",
                    "unece:TDED": "1004",
                    "unece:cefactUNId": "UN01009295",
                    "unece:cefactBieDomainClass": "cefact:AgronomicalObservation_Document.Details",
                    "rdfs:comment": "The identifier for this agronomical observation document."
                },
                {
                    "@id": "cefact:Livestock_Animal.Identification.Identifier",
                    "@type": "unece:BasicBIE",
                    "unece:cefactUNId": "UN01007643",
                    "unece:cefactBieDomainClass": "cefact:Livestock_Animal.Details",
                    "rdfs:comment": "The identifier for this livestock animal, such as the number appearing on its ear tag."
                },
                {
                    "@id": "cefact:Specified_AgriculturalDevice.Identification.Identifier",
                    "@type": "unece:BasicBIE",
                    "unece:cefactUNId": "UN01002737",
                    "unece:cefactBieDomainClass": "cefact:Specified_AgriculturalDevice.Details",
                    "rdfs:comment": "The unique identifier for this specified agricultural device."
                },
                {
                    "@id": "cefact:SPSExchanged_Document.Identification.Identifier",
                    "@type": "unece:BasicBIE",
                    "unece:TDED": "1004",
                    "unece:cefactUNId": "UN03000003",
                    "unece:cefactBieDomainClass": "cefact:SPSExchanged_Document.Details",
                    "rdfs:comment": "The unique identifier of this exchanged SPS document."
                },
                {
                    "@id": "cefact:AgriculturalInput_Product.Identification.Identifier",
                    "@type": "unece:BasicBIE",
                    "unece:TDED": "7135",
                    "unece:cefactUNId": "UN01012374",
                    "unece:cefactBieDomainClass": "cefact:AgriculturalInput_Product.Details",
                    "rdfs:comment": "The identifier for this agricultural input product."
                },
                {
                    "@id": "cefact:Milk_Tank.Identification.Identifier",
                    "@type": "unece:BasicBIE",
                    "unece:cefactUNId": "UN01009835",
                    "unece:cefactBieDomainClass": "cefact:Milk_Tank.Details",
                    "rdfs:comment": "The identifier for this milk tank."
                },
                {
                    "@id": "cefact:Crop_Produce.Identification.Identifier",
                    "@type": "unece:BasicBIE",
                    "unece:cefactUNId": "UN01012325",
                    "unece:cefactBieDomainClass": "cefact:Crop_Produce.Details",
                    "rdfs:comment": "An identifier for this crop produce."
                },
                {
                    "@id": "cefact:Animal_TradeDelivery.Identification.Identifier",
                    "@type": "unece:BasicBIE",
                    "unece:TDED": "1065",
                    "unece:cefactUNId": "UN01011262",
                    "unece:cefactBieDomainClass": "cefact:Animal_TradeDelivery.Details",
                    "rdfs:comment": "The identifier for this animal trade delivery."
                },
                {
                    "@id": "cefact:AgronomicalObservation_Party.Identification.Identifier",
                    "@type": "unece:BasicBIE",
                    "unece:TDED": "3039",
                    "unece:cefactUNId": "UN01009302",
                    "unece:cefactBieDomainClass": "cefact:AgronomicalObservation_Party.Details",
                    "rdfs:comment": "The identifier for this agronomical observation party."
                },
                {
                    "@id": "cefact:AgronomicalObservation_Plot.Identification.Identifier",
                    "@type": "unece:BasicBIE",
                    "unece:cefactUNId": "UN01009366",
                    "unece:cefactBieDomainClass": "cefact:AgronomicalObservation_Plot.Details",
                    "rdfs:comment": "The unique identifier for this agronomical observation plot."
                },
                {
                    "@id": "cefact:SPS_Party.Identification.Identifier",
                    "@type": "unece:BasicBIE",
                    "unece:TDED": "3039",
                    "unece:cefactUNId": "UN03000112",
                    "unece:cefactBieDomainClass": "cefact:SPS_Party.Details",
                    "rdfs:comment": "The unique identifier of this SPS party."
                },
                {
                    "@id": "cefact:Mobile_Plot.Identification.Identifier",
                    "@type": "unece:BasicBIE",
                    "unece:cefactUNId": "UN01012155",
                    "unece:cefactBieDomainClass": "cefact:Mobile_Plot.Details",
                    "rdfs:comment": "The identifier for this mobile plot."
                },
                {
                    "@id": "cefact:CropInput_Batch.Identification.Identifier",
                    "@type": "unece:BasicBIE",
                    "unece:cefactUNId": "UN01002710",
                    "unece:cefactBieDomainClass": "cefact:CropInput_Batch.Details",
                    "rdfs:comment": "The unique identifier for this crop input batch."
                },
                {
                    "@id": "cefact:LivestockAnimal_ProductInstance.Identification.Identifier",
                    "@type": "unece:BasicBIE",
                    "unece:cefactUNId": "UN01007711",
                    "unece:cefactBieDomainClass": "cefact:LivestockAnimal_ProductInstance.Details",
                    "rdfs:comment": "The identifier for this livestock animal product instance, such as the number appearing on its ear tag."
                },
                {
                    "@id": "cefact:AgriculturalProducer_Party.Identification.Identifier",
                    "@type": "unece:BasicBIE",
                    "unece:TDED": "3039",
                    "unece:cefactUNId": "UN01012259",
                    "unece:cefactBieDomainClass": "cefact:AgriculturalProducer_Party.Details",
                    "rdfs:comment": "The identifier of the agricultural producer party."
                },
                {
                    "@id": "cefact:AnimalPassport_Document.Identification.Identifier",
                    "@type": "unece:BasicBIE",
                    "unece:TDED": "1004",
                    "unece:cefactUNId": "UN01007672",
                    "unece:cefactBieDomainClass": "cefact:AnimalPassport_Document.Details",
                    "rdfs:comment": "The identifier for this animal passport document."
                },
                {
                    "@id": "cefact:Specified_GeographicalObjectCharacteristic.Identification.Identifier",
                    "@type": "unece:BasicBIE",
                    "unece:cefactUNId": "UN01012369",
                    "unece:cefactBieDomainClass": "cefact:Specified_GeographicalObjectCharacteristic.Details",
                    "rdfs:comment": "The identifier for this geographical object characteristic."
                },
                {
                    "@id": "cefact:Agricultural_SampledObject.Identification.Identifier",
                    "@type": "unece:BasicBIE",
                    "unece:cefactUNId": "UN01009610",
                    "unece:cefactBieDomainClass": "cefact:Agricultural_SampledObject.Details",
                    "rdfs:comment": "The identifier for this sampled agricultural object."
                },
                {
                    "@id": "cefact:Product_Batch.Identification.Identifier",
                    "@type": "unece:BasicBIE",
                    "unece:cefactUNId": "UN01012347",
                    "unece:cefactBieDomainClass": "cefact:Product_Batch.Details",
                    "rdfs:comment": "The identifier for this product batch."
                },
                {
                    "@id": "cefact:SPS_Consignment.Identification.Identifier",
                    "@type": "unece:BasicBIE",
                    "unece:TDED": "1202",
                    "unece:cefactUNId": "UN03000054",
                    "unece:cefactBieDomainClass": "cefact:SPS_Consignment.Details",
                    "rdfs:comment": "The unique identifier of this SPS consignment."
                },
                {
                    "@id": "cefact:Specified_AgriculturalApplication.Identification.Identifier",
                    "@type": "unece:BasicBIE",
                    "unece:cefactUNId": "UN01012423",
                    "unece:cefactBieDomainClass": "cefact:Specified_AgriculturalApplication.Details",
                    "rdfs:comment": "The identifier for this specified agricultural application."
                },
                {
                    "@id": "cefact:Specified_Party.Identification.Identifier",
                    "@type": "unece:BasicBIE",
                    "unece:TDED": "3039",
                    "unece:cefactUNId": "UN01007609",
                    "unece:cefactBieDomainClass": "cefact:Specified_Party.Details",
                    "rdfs:comment": "The identifier of the specified party."
                },
                {
                    "@id": "cefact:Crop_Plot.Identification.Identifier",
                    "@type": "unece:BasicBIE",
                    "unece:cefactUNId": "UN01012139",
                    "unece:cefactBieDomainClass": "cefact:Crop_Plot.Details",
                    "rdfs:comment": "The identifier for this crop plot."
                },
                {
                    "@id": "cefact:Agricultural_CountrySub-Division.Identification.Identifier",
                    "@type": "unece:BasicBIE",
                    "unece:TDED": "3229",
                    "unece:cefactUNId": "UN01002777",
                    "unece:cefactBieDomainClass": "cefact:Agricultural_CountrySubDivision.Details",
                    "rdfs:comment": "The unique identifier for this agricultural country sub-division."
                },
                {
                    "@id": "cefact:AgriculturalProcess_CropInput.Identification.Identifier",
                    "@type": "unece:BasicBIE",
                    "unece:cefactUNId": "UN01002724",
                    "unece:cefactBieDomainClass": "cefact:AgriculturalProcess_CropInput.Details",
                    "rdfs:comment": "The unique identifier for this agricultural process crop input."
                },
                {
                    "@id": "cefact:Animal_Identity.Identification.Identifier",
                    "@type": "unece:BasicBIE",
                    "unece:cefactUNId": "UN01007625",
                    "unece:cefactBieDomainClass": "cefact:Animal_Identity.Details",
                    "rdfs:comment": "The identifier for this animal identity."
                },
                {
                    "@id": "cefact:Referenced_Country.Identification.Identifier",
                    "@type": "unece:BasicBIE",
                    "unece:TDED": "3207",
                    "unece:cefactUNId": "UN01007616",
                    "unece:cefactBieDomainClass": "cefact:Referenced_Country.Details",
                    "rdfs:comment": "An identifier for this referenced country."
                },
                {
                    "@id": "cefact:Agricultural_ProductionUnit.Identification.Identifier",
                    "@type": "unece:BasicBIE",
                    "unece:cefactUNId": "UN01012245",
                    "unece:cefactBieDomainClass": "cefact:Agricultural_ProductionUnit.Details",
                    "rdfs:comment": "The identifier for this agricultural production unit."
                },
                {
                    "@id": "cefact:Agricultural_Construction.Identification.Identifier",
                    "@type": "unece:BasicBIE",
                    "unece:cefactUNId": "UN01012226",
                    "unece:cefactBieDomainClass": "cefact:Agricultural_Construction.Details",
                    "rdfs:comment": "The identifier for this agricultural construction."
                },
                {
                    "@id": "cefact:CropDataSheet_Party.Identification.Identifier",
                    "@type": "unece:BasicBIE",
                    "unece:TDED": "3039",
                    "unece:cefactUNId": "UN01002808",
                    "unece:cefactBieDomainClass": "cefact:CropDataSheet_Party.Details",
                    "rdfs:comment": "The unique identifier of this crop data sheet party."
                },
                {
                    "@id": "cefact:AgriculturalZone_Area.Identification.Identifier",
                    "@type": "unece:BasicBIE",
                    "unece:cefactUNId": "UN01012214",
                    "unece:cefactBieDomainClass": "cefact:AgriculturalZone_Area.Details",
                    "rdfs:comment": "The identifier for this agricultural zone area."
                },
                {
                    "@id": "cefact:CSEngineering_CoordinateReferenceSystem.Identification.Identifier",
                    "@type": "unece:BasicBIE",
                    "unece:cefactUNId": "UN01012163",
                    "unece:cefactBieDomainClass": "cefact:CSEngineering_CoordinateReferenceSystem.Details",
                    "rdfs:comment": "The identifier for this CS engineering coordinate reference system."
                },
                {
                    "@id": "cefact:CropReport_Document.Identification.Identifier",
                    "@type": "unece:BasicBIE",
                    "unece:TDED": "1004",
                    "unece:cefactUNId": "UN01012430",
                    "unece:cefactBieDomainClass": "cefact:CropReport_Document.Details",
                    "rdfs:comment": "The identifier of this crop report document."
                },
                {
                    "@id": "cefact:Specified_CropProtectionTreatment.Identification.Identifier",
                    "@type": "unece:BasicBIE",
                    "unece:cefactUNId": "UN01014286",
                    "unece:cefactBieDomainClass": "cefact:Specified_CropProtectionTreatment.Details",
                    "rdfs:comment": "An identifier of this specified crop protection treatment."
                },
                {
                    "@id": "cefact:Complaint_Issue.Identification.Identifier",
                    "@type": "unece:BasicBIE",
                    "unece:cefactUNId": "UN01012267",
                    "unece:cefactBieDomainClass": "cefact:Complaint_Issue.Details",
                    "rdfs:comment": "The identifier of this complaint issue."
                },
                {
                    "@id": "cefact:Animal_Certificate.Identification.Identifier",
                    "@type": "unece:BasicBIE",
                    "unece:cefactUNId": "UN01011238",
                    "unece:cefactBieDomainClass": "cefact:Animal_Certificate.Details",
                    "rdfs:comment": "The identifier for this animal certificate."
                },
                {
                    "@id": "cefact:SPSReferenced_Document.Identification.Identifier",
                    "@type": "unece:BasicBIE",
                    "unece:TDED": "1154",
                    "unece:cefactUNId": "UN03000018",
                    "unece:cefactBieDomainClass": "cefact:SPSReferenced_Document.Details",
                    "rdfs:comment": "The unique identifier for this referenced SPS document."
                },
                {
                    "@id": "cefact:SPS_Clause.Identification.Identifier",
                    "@type": "unece:BasicBIE",
                    "unece:TDED": "4181",
                    "unece:cefactUNId": "UN03000048",
                    "unece:cefactBieDomainClass": "cefact:SPS_Clause.Details",
                    "rdfs:comment": "The unique identifier of this SPS clause."
                },
                {
                    "@id": "cefact:SoilOccupation_Contract.Identification.Identifier",
                    "@type": "unece:BasicBIE",
                    "unece:TDED": "1296",
                    "unece:cefactUNId": "UN01002822",
                    "unece:cefactBieDomainClass": "cefact:SoilOccupation_Contract.Details",
                    "rdfs:comment": "The unique identifier for this soil occupation contract."
                }
            ]
        },
        {
            "@id": "agriculture:identification",
            "@type": "rdf:Property",
            "schema:rangeIncludes": {
                "@id": "xsd:string"
            },
            "schema:domainIncludes": [
                {
                    "@id": "agriculture:Reason"
                },
                {
                    "@id": "agriculture:TargetObject"
                }
            ],
            "rdfs:comment": [
                "The identification of this reason, expressed as text.",
                "The identification, expressed as text, for this agricultural process target object."
            ],
            "rdfs:label": "identification",
            "unece:cefactElementMetadata": [
                {
                    "@id": "cefact:AgriculturalProcess_TargetObject.Identification.Text",
                    "@type": "unece:BasicBIE",
                    "unece:cefactUNId": "UN01002773",
                    "unece:cefactBieDomainClass": "cefact:AgriculturalProcess_TargetObject.Details",
                    "rdfs:comment": "The identification, expressed as text, for this agricultural process target object."
                },
                {
                    "@id": "cefact:AgriculturalProcess_Reason.Identification.Text",
                    "@type": "unece:BasicBIE",
                    "unece:cefactUNId": "UN01002745",
                    "unece:cefactBieDomainClass": "cefact:AgriculturalProcess_Reason.Details",
                    "rdfs:comment": "The identification of this reason, expressed as text."
                }
            ]
        },
        {
            "@id": "agriculture:identifiedParty",
            "@type": "rdf:Property",
            "schema:rangeIncludes": {
                "@id": "agriculture:Party"
            },
            "schema:domainIncludes": {
                "@id": "agriculture:Contract"
            },
            "rdfs:comment": "The crop data sheet party that is identified in this soil occupation contract.",
            "rdfs:label": "identifiedParty",
            "unece:cefactElementMetadata": [
                {
                    "@id": "cefact:SoilOccupation_Contract.Identified.CropDataSheet_Party",
                    "@type": "unece:AssociationBIE",
                    "unece:cefactUNId": "UN01002825",
                    "unece:cefactBieDomainClass": "cefact:SoilOccupation_Contract.Details",
                    "rdfs:comment": "The crop data sheet party that is identified in this soil occupation contract."
                }
            ]
        },
        {
            "@id": "agriculture:identifierLengthNumeric",
            "@type": "rdf:Property",
            "schema:rangeIncludes": {
                "@id": "xsd:decimal"
            },
            "schema:domainIncludes": {
                "@id": "agriculture:Identity"
            },
            "rdfs:comment": "The length, expressed as the number of characters, of the identifier in this animal identity.",
            "rdfs:label": "identifierLengthNumeric",
            "unece:cefactElementMetadata": [
                {
                    "@id": "cefact:Animal_Identity.IdentifierLength.Numeric",
                    "@type": "unece:BasicBIE",
                    "unece:cefactUNId": "UN01007629",
                    "unece:cefactBieDomainClass": "cefact:Animal_Identity.Details",
                    "rdfs:comment": "The length, expressed as the number of characters, of the identifier in this animal identity."
                }
            ]
        },
        {
            "@id": "agriculture:importCountry",
            "@type": "rdf:Property",
            "schema:rangeIncludes": {
                "@id": "agriculture:Country"
            },
            "schema:domainIncludes": {
                "@id": "agriculture:Consignment"
            },
            "rdfs:comment": "The import country for this SPS consignment.",
            "rdfs:label": "importCountry",
            "unece:cefactElementMetadata": [
                {
                    "@id": "cefact:SPS_Consignment.Import.SPS_Country",
                    "@type": "unece:AssociationBIE",
                    "unece:cefactUNId": "UN03000064",
                    "unece:cefactBieDomainClass": "cefact:SPS_Consignment.Details",
                    "rdfs:comment": "The import country for this SPS consignment."
                }
            ]
        },
        {
            "@id": "agriculture:importOccurrenceDateTime",
            "@type": "rdf:Property",
            "schema:rangeIncludes": {
                "@id": "xsd:dateTime"
            },
            "schema:domainIncludes": {
                "@id": "agriculture:Event"
            },
            "rdfs:comment": "The date of the occurrence of the import for this cross border animal movement event.",
            "rdfs:label": "importOccurrenceDateTime",
            "unece:cefactElementMetadata": [
                {
                    "@id": "cefact:CrossBorderAnimalMovement_Event.Import_Occurrence.DateTime",
                    "@type": "unece:BasicBIE",
                    "unece:TDED": "2193",
                    "unece:cefactUNId": "UN01007661",
                    "unece:cefactBieDomainClass": "cefact:CrossBorderAnimalMovement_Event.Details",
                    "rdfs:comment": "The date of the occurrence of the import for this cross border animal movement event."
                }
            ]
        },
        {
            "@id": "agriculture:includedAnimal",
            "@type": "rdf:Property",
            "schema:rangeIncludes": {
                "@id": "agriculture:Animal"
            },
            "schema:domainIncludes": {
                "@id": "agriculture:TradeDelivery"
            },
            "rdfs:comment": "A Track and Trace (TT) animal included in this animal trade delivery.",
            "rdfs:label": "includedAnimal",
            "unece:cefactElementMetadata": [
                {
                    "@id": "cefact:Animal_TradeDelivery.Included.TT_Animal",
                    "@type": "unece:AssociationBIE",
                    "unece:cefactUNId": "UN01011264",
                    "unece:cefactBieDomainClass": "cefact:Animal_TradeDelivery.Details",
                    "rdfs:comment": "A Track and Trace (TT) animal included in this animal trade delivery."
                }
            ]
        },
        {
            "@id": "agriculture:includedArea",
            "@type": "rdf:Property",
            "schema:rangeIncludes": {
                "@id": "agriculture:Area"
            },
            "schema:domainIncludes": [
                {
                    "@id": "agriculture:CountrySubDivision"
                },
                {
                    "@id": "agriculture:Plot"
                }
            ],
            "rdfs:comment": [
                "An agricultural area included in this agricultural country sub-division.",
                "An agricultural area included in this agricultural plot."
            ],
            "rdfs:label": "includedArea",
            "unece:cefactElementMetadata": [
                {
                    "@id": "cefact:Agricultural_Plot.Included.Agricultural_Area",
                    "@type": "unece:AssociationBIE",
                    "unece:cefactUNId": "UN01002662",
                    "unece:cefactBieDomainClass": "cefact:Agricultural_Plot.Details",
                    "rdfs:comment": "An agricultural area included in this agricultural plot."
                },
                {
                    "@id": "cefact:Agricultural_CountrySub-Division.Included.Agricultural_Area",
                    "@type": "unece:AssociationBIE",
                    "unece:cefactUNId": "UN01002781",
                    "unece:cefactBieDomainClass": "cefact:Agricultural_CountrySubDivision.Details",
                    "rdfs:comment": "An agricultural area included in this agricultural country sub-division."
                }
            ]
        },
        {
            "@id": "agriculture:includedClause",
            "@type": "rdf:Property",
            "schema:rangeIncludes": {
                "@id": "agriculture:Clause"
            },
            "schema:domainIncludes": {
                "@id": "agriculture:Authentication"
            },
            "rdfs:comment": "A document clause included in this SPS authentication.",
            "rdfs:label": "includedClause",
            "unece:cefactElementMetadata": [
                {
                    "@id": "cefact:SPS_Authentication.Included.SPS_Clause",
                    "@type": "unece:AssociationBIE",
                    "unece:cefactUNId": "UN03000039",
                    "unece:cefactBieDomainClass": "cefact:SPS_Authentication.Details",
                    "rdfs:comment": "A document clause included in this SPS authentication."
                }
            ]
        },
        {
            "@id": "agriculture:includedConsignmentItem",
            "@type": "rdf:Property",
            "schema:rangeIncludes": {
                "@id": "agriculture:ConsignmentItem"
            },
            "schema:domainIncludes": {
                "@id": "agriculture:Consignment"
            },
            "rdfs:comment": "A separately defined consignment item included within this SPS consignment.",
            "rdfs:label": "includedConsignmentItem",
            "unece:cefactElementMetadata": [
                {
                    "@id": "cefact:SPS_Consignment.Included.SPS_ConsignmentItem",
                    "@type": "unece:AssociationBIE",
                    "unece:cefactUNId": "UN03000076",
                    "unece:cefactBieDomainClass": "cefact:SPS_Consignment.Details",
                    "rdfs:comment": "A separately defined consignment item included within this SPS consignment."
                }
            ]
        },
        {
            "@id": "agriculture:includedGeographicalGrid",
            "@type": "rdf:Property",
            "schema:rangeIncludes": {
                "@id": "agriculture:GeographicalGrid"
            },
            "schema:domainIncludes": {
                "@id": "agriculture:GeographicalFeature"
            },
            "rdfs:comment": "The geographical grid included in this geographical feature.",
            "rdfs:label": "includedGeographicalGrid",
            "unece:cefactElementMetadata": [
                {
                    "@id": "cefact:Specified_GeographicalFeature.Included.Specified_GeographicalGrid",
                    "@type": "unece:AssociationBIE",
                    "unece:cefactUNId": "UN01012179",
                    "unece:cefactBieDomainClass": "cefact:Specified_GeographicalFeature.Details",
                    "rdfs:comment": "The geographical grid included in this geographical feature."
                }
            ]
        },
        {
            "@id": "agriculture:includedGeographicalLine",
            "@type": "rdf:Property",
            "schema:rangeIncludes": {
                "@id": "agriculture:GeographicalLine"
            },
            "schema:domainIncludes": {
                "@id": "agriculture:GeographicalFeature"
            },
            "rdfs:comment": "The geographical line included in this geographical feature.",
            "rdfs:label": "includedGeographicalLine",
            "unece:cefactElementMetadata": [
                {
                    "@id": "cefact:Specified_GeographicalFeature.Included.Specified_GeographicalLine",
                    "@type": "unece:AssociationBIE",
                    "unece:cefactUNId": "UN01012173",
                    "unece:cefactBieDomainClass": "cefact:Specified_GeographicalFeature.Details",
                    "rdfs:comment": "The geographical line included in this geographical feature."
                }
            ]
        },
        {
            "@id": "agriculture:includedGeographicalMulti-Curve",
            "@type": "rdf:Property",
            "schema:rangeIncludes": {
                "@id": "agriculture:GeographicalMulti-Curve"
            },
            "schema:domainIncludes": {
                "@id": "agriculture:GeographicalFeature"
            },
            "rdfs:comment": "The geographical multi-curve included in this geographical feature.",
            "rdfs:label": "includedGeographicalMulti-Curve",
            "unece:cefactElementMetadata": [
                {
                    "@id": "cefact:Specified_GeographicalFeature.Included.Specified_GeographicalMulti-Curve",
                    "@type": "unece:AssociationBIE",
                    "unece:cefactUNId": "UN01012176",
                    "unece:cefactBieDomainClass": "cefact:Specified_GeographicalFeature.Details",
                    "rdfs:comment": "The geographical multi-curve included in this geographical feature."
                }
            ]
        },
        {
            "@id": "agriculture:includedGeographicalMulti-Point",
            "@type": "rdf:Property",
            "schema:rangeIncludes": {
                "@id": "agriculture:GeographicalMulti-Point"
            },
            "schema:domainIncludes": {
                "@id": "agriculture:GeographicalFeature"
            },
            "rdfs:comment": "The geographical multi-point included in this geographical feature.",
            "rdfs:label": "includedGeographicalMulti-Point",
            "unece:cefactElementMetadata": [
                {
                    "@id": "cefact:Specified_GeographicalFeature.Included.Specified_GeographicalMulti-Point",
                    "@type": "unece:AssociationBIE",
                    "unece:cefactUNId": "UN01012175",
                    "unece:cefactBieDomainClass": "cefact:Specified_GeographicalFeature.Details",
                    "rdfs:comment": "The geographical multi-point included in this geographical feature."
                }
            ]
        },
        {
            "@id": "agriculture:includedGeographicalMulti-Surface",
            "@type": "rdf:Property",
            "schema:rangeIncludes": {
                "@id": "agriculture:GeographicalMulti-Surface"
            },
            "schema:domainIncludes": {
                "@id": "agriculture:GeographicalFeature"
            },
            "rdfs:comment": "The geographical multi-surface included in this geographical feature.",
            "rdfs:label": "includedGeographicalMulti-Surface",
            "unece:cefactElementMetadata": [
                {
                    "@id": "cefact:Specified_GeographicalFeature.Included.Specified_GeographicalMulti-Surface",
                    "@type": "unece:AssociationBIE",
                    "unece:cefactUNId": "UN01012177",
                    "unece:cefactBieDomainClass": "cefact:Specified_GeographicalFeature.Details",
                    "rdfs:comment": "The geographical multi-surface included in this geographical feature."
                }
            ]
        },
        {
            "@id": "agriculture:includedGeographicalPoint",
            "@type": "rdf:Property",
            "schema:rangeIncludes": {
                "@id": "agriculture:GeographicalPoint"
            },
            "schema:domainIncludes": {
                "@id": "agriculture:GeographicalFeature"
            },
            "rdfs:comment": "The geographical point included in this geographical feature.",
            "rdfs:label": "includedGeographicalPoint",
            "unece:cefactElementMetadata": [
                {
                    "@id": "cefact:Specified_GeographicalFeature.Included.Specified_GeographicalPoint",
                    "@type": "unece:AssociationBIE",
                    "unece:cefactUNId": "UN01012172",
                    "unece:cefactBieDomainClass": "cefact:Specified_GeographicalFeature.Details",
                    "rdfs:comment": "The geographical point included in this geographical feature."
                }
            ]
        },
        {
            "@id": "agriculture:includedGeographicalSurface",
            "@type": "rdf:Property",
            "schema:rangeIncludes": {
                "@id": "agriculture:GeographicalSurface"
            },
            "schema:domainIncludes": {
                "@id": "agriculture:GeographicalFeature"
            },
            "rdfs:comment": "The geographical surface included in this geographical feature.",
            "rdfs:label": "includedGeographicalSurface",
            "unece:cefactElementMetadata": [
                {
                    "@id": "cefact:Specified_GeographicalFeature.Included.Specified_GeographicalSurface",
                    "@type": "unece:AssociationBIE",
                    "unece:cefactUNId": "UN01012174",
                    "unece:cefactBieDomainClass": "cefact:Specified_GeographicalFeature.Details",
                    "rdfs:comment": "The geographical surface included in this geographical feature."
                }
            ]
        },
        {
            "@id": "agriculture:includedInCountrySub-Division",
            "@type": "rdf:Property",
            "schema:rangeIncludes": {
                "@id": "agriculture:CountrySub-Division"
            },
            "schema:domainIncludes": {
                "@id": "agriculture:Plot"
            },
            "rdfs:comment": "An agricultural country sub-division in which this agricultural plot is included.",
            "rdfs:label": "includedInCountrySub-Division",
            "unece:cefactElementMetadata": [
                {
                    "@id": "cefact:Agricultural_Plot.IncludedIn.Agricultural_CountrySub-Division",
                    "@type": "unece:AssociationBIE",
                    "unece:cefactUNId": "UN01002659",
                    "unece:cefactBieDomainClass": "cefact:Agricultural_Plot.Details",
                    "rdfs:comment": "An agricultural country sub-division in which this agricultural plot is included."
                }
            ]
        },
        {
            "@id": "agriculture:includedNote",
            "@type": "rdf:Property",
            "schema:rangeIncludes": {
                "@id": "agriculture:Note"
            },
            "schema:domainIncludes": {
                "@id": "agriculture:Document"
            },
            "rdfs:comment": "An SPS note included in this exchanged SPS document.",
            "rdfs:label": "includedNote",
            "unece:cefactElementMetadata": [
                {
                    "@id": "cefact:SPSExchanged_Document.Included.SPS_Note",
                    "@type": "unece:AssociationBIE",
                    "unece:cefactUNId": "UN03000011",
                    "unece:cefactBieDomainClass": "cefact:SPSExchanged_Document.Details",
                    "rdfs:comment": "An SPS note included in this exchanged SPS document."
                }
            ]
        },
        {
            "@id": "agriculture:includedPlot",
            "@type": "rdf:Property",
            "schema:rangeIncludes": {
                "@id": "agriculture:Plot"
            },
            "schema:domainIncludes": {
                "@id": "agriculture:Plot"
            },
            "rdfs:comment": [
                "A crop plot included in this crop plot.",
                "The mobile plot included for this crop plot."
            ],
            "rdfs:label": "includedPlot",
            "unece:cefactElementMetadata": [
                {
                    "@id": "cefact:Crop_Plot.Included.Crop_Plot",
                    "@type": "unece:AssociationBIE",
                    "unece:cefactUNId": "UN01012147",
                    "unece:cefactBieDomainClass": "cefact:Crop_Plot.Details",
                    "rdfs:comment": "A crop plot included in this crop plot."
                },
                {
                    "@id": "cefact:Crop_Plot.Included.Mobile_Plot",
                    "@type": "unece:AssociationBIE",
                    "unece:cefactUNId": "UN01012149",
                    "unece:cefactBieDomainClass": "cefact:Crop_Plot.Details",
                    "rdfs:comment": "The mobile plot included for this crop plot."
                }
            ]
        },
        {
            "@id": "agriculture:includedPolygon",
            "@type": "rdf:Property",
            "schema:rangeIncludes": {
                "@id": "agriculture:Polygon"
            },
            "schema:domainIncludes": [
                {
                    "@id": "agriculture:GeographicalFeature"
                },
                {
                    "@id": "agriculture:GeographicalMultiSurface"
                },
                {
                    "@id": "agriculture:GeographicalSurface"
                }
            ],
            "rdfs:comment": [
                "A polygon included in this geographical multi-surface.",
                "The polygon included in this geographical feature.",
                "The polygon included in this geographical surface."
            ],
            "rdfs:label": "includedPolygon",
            "unece:cefactElementMetadata": [
                {
                    "@id": "cefact:Specified_GeographicalFeature.Included.Specified_Polygon",
                    "@type": "unece:AssociationBIE",
                    "unece:cefactUNId": "UN01012178",
                    "unece:cefactBieDomainClass": "cefact:Specified_GeographicalFeature.Details",
                    "rdfs:comment": "The polygon included in this geographical feature."
                },
                {
                    "@id": "cefact:Specified_GeographicalMulti-Surface.Included.Specified_Polygon",
                    "@type": "unece:AssociationBIE",
                    "unece:cefactUNId": "UN01012198",
                    "unece:cefactBieDomainClass": "cefact:Specified_GeographicalMultiSurface.Details",
                    "rdfs:comment": "A polygon included in this geographical multi-surface."
                },
                {
                    "@id": "cefact:Specified_GeographicalSurface.Included.Specified_Polygon",
                    "@type": "unece:AssociationBIE",
                    "unece:cefactUNId": "UN01012201",
                    "unece:cefactBieDomainClass": "cefact:Specified_GeographicalSurface.Details",
                    "rdfs:comment": "The polygon included in this geographical surface."
                }
            ]
        },
        {
            "@id": "agriculture:includedTradeLineItem",
            "@type": "rdf:Property",
            "schema:rangeIncludes": {
                "@id": "agriculture:TradeLineItem"
            },
            "schema:domainIncludes": {
                "@id": "agriculture:ConsignmentItem"
            },
            "rdfs:comment": "An SPS trade line item included in this SPS consignment item.",
            "rdfs:label": "includedTradeLineItem",
            "unece:cefactElementMetadata": [
                {
                    "@id": "cefact:SPS_ConsignmentItem.Included.SPS_TradeLineItem",
                    "@type": "unece:AssociationBIE",
                    "unece:cefactUNId": "UN03000052",
                    "unece:cefactBieDomainClass": "cefact:SPS_ConsignmentItem.Details",
                    "rdfs:comment": "An SPS trade line item included in this SPS consignment item."
                }
            ]
        },
        {
            "@id": "agriculture:indexNumeric",
            "@type": "rdf:Property",
            "schema:rangeIncludes": {
                "@id": "xsd:decimal"
            },
            "schema:domainIncludes": {
                "@id": "agriculture:Material"
            },
            "rdfs:comment": "The index number of this agricultural input material.",
            "rdfs:label": "indexNumeric",
            "unece:cefactElementMetadata": [
                {
                    "@id": "cefact:AgriculturalInput_Material.Index.Numeric",
                    "@type": "unece:BasicBIE",
                    "unece:cefactUNId": "UN01012397",
                    "unece:cefactBieDomainClass": "cefact:AgriculturalInput_Material.Details",
                    "rdfs:comment": "The index number of this agricultural input material."
                }
            ]
        },
        {
            "@id": "agriculture:individualProductInstance",
            "@type": "rdf:Property",
            "schema:rangeIncludes": {
                "@id": "agriculture:ProductInstance"
            },
            "schema:domainIncludes": {
                "@id": "agriculture:Product"
            },
            "rdfs:comment": "The product instance of an individual in this livestock animal product.",
            "rdfs:label": "individualProductInstance",
            "unece:cefactElementMetadata": [
                {
                    "@id": "cefact:LivestockAnimal_Product.Individual.LivestockAnimal_ProductInstance",
                    "@type": "unece:AssociationBIE",
                    "unece:cefactUNId": "UN01007709",
                    "unece:cefactBieDomainClass": "cefact:LivestockAnimal_Product.Details",
                    "rdfs:comment": "The product instance of an individual in this livestock animal product."
                }
            ]
        },
        {
            "@id": "agriculture:information",
            "@type": "rdf:Property",
            "schema:rangeIncludes": {
                "@id": "xsd:string"
            },
            "schema:domainIncludes": [
                {
                    "@id": "agriculture:Document"
                },
                {
                    "@id": "agriculture:Material"
                },
                {
                    "@id": "agriculture:Sample"
                }
            ],
            "rdfs:comment": [
                "Information, expressed as text, about this agricultural sample.",
                "Information, expressed as text, for this agricultural input material.",
                "Information, expressed as text, for this crop report document.",
                "Information, expressed as text, for this referenced SPS document."
            ],
            "rdfs:label": "information",
            "unece:cefactElementMetadata": [
                {
                    "@id": "cefact:Agricultural_Sample.Information.Text",
                    "@type": "unece:BasicBIE",
                    "unece:cefactUNId": "UN01009595",
                    "unece:cefactBieDomainClass": "cefact:Agricultural_Sample.Details",
                    "rdfs:comment": "Information, expressed as text, about this agricultural sample."
                },
                {
                    "@id": "cefact:AgriculturalInput_Material.Information.Text",
                    "@type": "unece:BasicBIE",
                    "unece:cefactUNId": "UN01012396",
                    "unece:cefactBieDomainClass": "cefact:AgriculturalInput_Material.Details",
                    "rdfs:comment": "Information, expressed as text, for this agricultural input material."
                },
                {
                    "@id": "cefact:CropReport_Document.Information.Text",
                    "@type": "unece:BasicBIE",
                    "unece:TDED": "4142",
                    "unece:cefactUNId": "UN01012439",
                    "unece:cefactBieDomainClass": "cefact:CropReport_Document.Details",
                    "rdfs:comment": "Information, expressed as text, for this crop report document."
                },
                {
                    "@id": "cefact:SPSReferenced_Document.Information.Text",
                    "@type": "unece:BasicBIE",
                    "unece:TDED": "4142",
                    "unece:cefactUNId": "UN01007575",
                    "unece:cefactBieDomainClass": "cefact:SPSReferenced_Document.Details",
                    "rdfs:comment": "Information, expressed as text, for this referenced SPS document."
                }
            ]
        },
        {
            "@id": "agriculture:informationRelatedBinaryFile",
            "@type": "rdf:Property",
            "schema:rangeIncludes": {
                "@id": "agriculture:BinaryFile"
            },
            "schema:domainIncludes": {
                "@id": "agriculture:SampledObject"
            },
            "rdfs:comment": "A binary file containing information related to this sampled agricultural object.",
            "rdfs:label": "informationRelatedBinaryFile",
            "unece:cefactElementMetadata": [
                {
                    "@id": "cefact:Agricultural_SampledObject.Information_Related.Specified_BinaryFile",
                    "@type": "unece:AssociationBIE",
                    "unece:cefactUNId": "UN01011949",
                    "unece:cefactBieDomainClass": "cefact:Agricultural_SampledObject.Details",
                    "rdfs:comment": "A binary file containing information related to this sampled agricultural object."
                }
            ]
        },
        {
            "@id": "agriculture:informationRelatedPicture",
            "@type": "rdf:Property",
            "schema:rangeIncludes": {
                "@id": "agriculture:Picture"
            },
            "schema:domainIncludes": {
                "@id": "agriculture:SampledObject"
            },
            "rdfs:comment": "A photographic picture showing information related to this sampled agricultural object.",
            "rdfs:label": "informationRelatedPicture",
            "unece:cefactElementMetadata": [
                {
                    "@id": "cefact:Agricultural_SampledObject.Information_Related.Photographic_Picture",
                    "@type": "unece:AssociationBIE",
                    "unece:cefactUNId": "UN01011948",
                    "unece:cefactBieDomainClass": "cefact:Agricultural_SampledObject.Details",
                    "rdfs:comment": "A photographic picture showing information related to this sampled agricultural object."
                }
            ]
        },
        {
            "@id": "agriculture:inputCapacityMeasure",
            "@type": "rdf:Property",
            "schema:rangeIncludes": {
                "@id": "xsd:decimal"
            },
            "schema:domainIncludes": {
                "@id": "agriculture:Construction"
            },
            "rdfs:comment": "The measure of the input capacity for this agricultural construction, such as maximum reach or average per month.",
            "rdfs:label": "inputCapacityMeasure",
            "unece:cefactElementMetadata": [
                {
                    "@id": "cefact:Agricultural_Construction.Input_Capacity.Measure",
                    "@type": "unece:BasicBIE",
                    "unece:cefactUNId": "UN01012238",
                    "unece:cefactBieDomainClass": "cefact:Agricultural_Construction.Details",
                    "rdfs:comment": "The measure of the input capacity for this agricultural construction, such as maximum reach or average per month."
                }
            ]
        },
        {
            "@id": "agriculture:inputSpecifiedBatch",
            "@type": "rdf:Property",
            "schema:rangeIncludes": {
                "@id": "agriculture:Batch"
            },
            "schema:domainIncludes": {
                "@id": "agriculture:Produce"
            },
            "rdfs:comment": "An input batch crop produce, such as seed or fertilizer, specified for this crop produce.",
            "rdfs:label": "inputSpecifiedBatch",
            "unece:cefactElementMetadata": [
                {
                    "@id": "cefact:Crop_Produce.Input_Specified.CropProduce_Batch",
                    "@type": "unece:AssociationBIE",
                    "unece:cefactUNId": "UN01012329",
                    "unece:cefactBieDomainClass": "cefact:Crop_Produce.Details",
                    "rdfs:comment": "An input batch crop produce, such as seed or fertilizer, specified for this crop produce."
                }
            ]
        },
        {
            "@id": "agriculture:inspectionPersonName",
            "@type": "rdf:Property",
            "schema:rangeIncludes": {
                "@id": "unece:UNECECL3403Code"
            },
            "schema:domainIncludes": {
                "@id": "agriculture:Person"
            },
            "rdfs:comment": "The name or set of names, expressed as text, by which this inspection person is known.",
            "rdfs:label": "inspectionPersonName",
            "unece:cefactElementMetadata": [
                {
                    "@id": "cefact:Inspection_Person.Name.Text",
                    "@type": "unece:BasicBIE",
                    "unece:TDED": "3403",
                    "unece:cefactUNId": "UN01007690",
                    "unece:cefactBieDomainClass": "cefact:Inspection_Person.Details",
                    "rdfs:comment": "The name or set of names, expressed as text, by which this inspection person is known."
                }
            ]
        },
        {
            "@id": "agriculture:intakeId",
            "@type": "rdf:Property",
            "schema:rangeIncludes": {
                "@id": "xsd:token"
            },
            "schema:domainIncludes": {
                "@id": "agriculture:Sample"
            },
            "rdfs:comment": "The identifier of the sample, assigned by the observer party during the intake of this agricultural sample.",
            "rdfs:label": "intakeId",
            "unece:cefactElementMetadata": [
                {
                    "@id": "cefact:Agricultural_Sample.Intake_Identification.Identifier",
                    "@type": "unece:BasicBIE",
                    "unece:cefactUNId": "UN01009585",
                    "unece:cefactBieDomainClass": "cefact:Agricultural_Sample.Details",
                    "rdfs:comment": "The identifier of the sample, assigned by the observer party during the intake of this agricultural sample."
                }
            ]
        },
        {
            "@id": "agriculture:intendedUse",
            "@type": "rdf:Property",
            "schema:rangeIncludes": {
                "@id": "xsd:string"
            },
            "schema:domainIncludes": [
                {
                    "@id": "agriculture:ProductInstance"
                },
                {
                    "@id": "agriculture:TradeLineItem"
                }
            ],
            "rdfs:comment": [
                "An intended use, expressed as text, of this SPS trade line item.",
                "The intended use, expressed as text, for this livestock animal product instance."
            ],
            "rdfs:label": "intendedUse",
            "unece:cefactElementMetadata": [
                {
                    "@id": "cefact:LivestockAnimal_ProductInstance.Intended_Use.Text",
                    "@type": "unece:BasicBIE",
                    "unece:cefactUNId": "UN01007712",
                    "unece:cefactBieDomainClass": "cefact:LivestockAnimal_ProductInstance.Details",
                    "rdfs:comment": "The intended use, expressed as text, for this livestock animal product instance."
                },
                {
                    "@id": "cefact:SPS_TradeLineItem.Intended_Use.Text",
                    "@type": "unece:BasicBIE",
                    "unece:TDED": "7110",
                    "unece:cefactUNId": "UN03000152",
                    "unece:cefactBieDomainClass": "cefact:SPS_TradeLineItem.Details",
                    "rdfs:comment": "An intended use, expressed as text, of this SPS trade line item."
                }
            ]
        },
        {
            "@id": "agriculture:internalOperatorParty",
            "@type": "rdf:Property",
            "schema:rangeIncludes": {
                "@id": "agriculture:Party"
            },
            "schema:domainIncludes": {
                "@id": "agriculture:AgriculturalProcess"
            },
            "rdfs:comment": "The crop data sheet party that is the internal operator for this plot agricultural process.",
            "rdfs:label": "internalOperatorParty",
            "unece:cefactElementMetadata": [
                {
                    "@id": "cefact:Plot_AgriculturalProcess.Internal_Operator.CropDataSheet_Party",
                    "@type": "unece:AssociationBIE",
                    "unece:cefactUNId": "UN01002790",
                    "unece:cefactBieDomainClass": "cefact:Plot_AgriculturalProcess.Details",
                    "rdfs:comment": "The crop data sheet party that is the internal operator for this plot agricultural process."
                }
            ]
        },
        {
            "@id": "agriculture:interpretationResult",
            "@type": "rdf:Property",
            "schema:rangeIncludes": {
                "@id": "xsd:string"
            },
            "schema:domainIncludes": {
                "@id": "agriculture:Sample"
            },
            "rdfs:comment": "The interpretation result, expressed as text, for this agricultural sample, indicating whether it complies with the normative values.",
            "rdfs:label": "interpretationResult",
            "unece:cefactElementMetadata": [
                {
                    "@id": "cefact:Agricultural_Sample.InterpretationResult.Text",
                    "@type": "unece:BasicBIE",
                    "unece:cefactUNId": "UN01009600",
                    "unece:cefactBieDomainClass": "cefact:Agricultural_Sample.Details",
                    "rdfs:comment": "The interpretation result, expressed as text, for this agricultural sample, indicating whether it complies with the normative values."
                }
            ]
        },
        {
            "@id": "agriculture:interpretationResultParameter",
            "@type": "rdf:Property",
            "schema:rangeIncludes": {
                "@id": "agriculture:Parameter"
            },
            "schema:domainIncludes": {
                "@id": "agriculture:Sample"
            },
            "rdfs:comment": "An observation objective parameter of the interpretation result for this agricultural sample.",
            "rdfs:label": "interpretationResultParameter",
            "unece:cefactElementMetadata": [
                {
                    "@id": "cefact:Agricultural_Sample.InterpretationResult.ObservationObjective_Parameter",
                    "@type": "unece:AssociationBIE",
                    "unece:cefactUNId": "UN01010480",
                    "unece:cefactBieDomainClass": "cefact:Agricultural_Sample.Details",
                    "rdfs:comment": "An observation objective parameter of the interpretation result for this agricultural sample."
                }
            ]
        },
        {
            "@id": "agriculture:issueDateTime",
            "@type": "rdf:Property",
            "schema:rangeIncludes": {
                "@id": "xsd:dateTime"
            },
            "schema:domainIncludes": [
                {
                    "@id": "agriculture:Certificate"
                },
                {
                    "@id": "agriculture:Document"
                }
            ],
            "rdfs:comment": [
                "The date for the issuance of this animal passport document.",
                "The date or date time for the issuance of this referenced SPS document.",
                "The date, time, date time or other date time value for the issuance of this LA exchanged document.",
                "The date, time, date time or other date time value for the issuance of this SPS acknowledgement document.",
                "The date, time, date time or other date time value for the issuance of this crop report document.",
                "The date, time, date time or other date time value for the issuance of this exchanged SPS document.",
                "The date, time, date time, or other date time value when this agricultural certificate was issued."
            ],
            "rdfs:label": "issueDateTime",
            "unece:cefactElementMetadata": [
                {
                    "@id": "cefact:CropReport_Document.Issue.DateTime",
                    "@type": "unece:BasicBIE",
                    "unece:TDED": "2007",
                    "unece:cefactUNId": "UN01012433",
                    "unece:cefactBieDomainClass": "cefact:CropReport_Document.Details",
                    "rdfs:comment": "The date, time, date time or other date time value for the issuance of this crop report document."
                },
                {
                    "@id": "cefact:SPSExchanged_Document.Issue.DateTime",
                    "@type": "unece:BasicBIE",
                    "unece:TDED": "2007",
                    "unece:cefactUNId": "UN03000007",
                    "unece:cefactBieDomainClass": "cefact:SPSExchanged_Document.Details",
                    "rdfs:comment": "The date, time, date time or other date time value for the issuance of this exchanged SPS document."
                },
                {
                    "@id": "cefact:Agricultural_Certificate.Issue.DateTime",
                    "@type": "unece:BasicBIE",
                    "unece:cefactUNId": "UN01012279",
                    "unece:cefactBieDomainClass": "cefact:Agricultural_Certificate.Details",
                    "rdfs:comment": "The date, time, date time, or other date time value when this agricultural certificate was issued."
                },
                {
                    "@id": "cefact:AnimalPassport_Document.Issue.DateTime",
                    "@type": "unece:BasicBIE",
                    "unece:TDED": "2007",
                    "unece:cefactUNId": "UN01007671",
                    "unece:cefactBieDomainClass": "cefact:AnimalPassport_Document.Details",
                    "rdfs:comment": "The date for the issuance of this animal passport document."
                },
                {
                    "@id": "cefact:LAExchanged_Document.Issue.DateTime",
                    "@type": "unece:BasicBIE",
                    "unece:TDED": "2007",
                    "unece:cefactUNId": "UN01007699",
                    "unece:cefactBieDomainClass": "cefact:LAExchanged_Document.Details",
                    "rdfs:comment": "The date, time, date time or other date time value for the issuance of this LA exchanged document."
                },
                {
                    "@id": "cefact:SPSAcknowledgement_Document.Issue.DateTime",
                    "@type": "unece:BasicBIE",
                    "unece:TDED": "2007",
                    "unece:cefactUNId": "UN03000184",
                    "unece:cefactBieDomainClass": "cefact:SPSAcknowledgement_Document.Details",
                    "rdfs:comment": "The date, time, date time or other date time value for the issuance of this SPS acknowledgement document."
                },
                {
                    "@id": "cefact:SPSReferenced_Document.Issue.DateTime",
                    "@type": "unece:BasicBIE",
                    "unece:TDED": "2007",
                    "unece:cefactUNId": "UN03000015",
                    "unece:cefactBieDomainClass": "cefact:SPSReferenced_Document.Details",
                    "rdfs:comment": "The date or date time for the issuance of this referenced SPS document."
                }
            ]
        },
        {
            "@id": "agriculture:issueLocation",
            "@type": "rdf:Property",
            "schema:rangeIncludes": {
                "@id": "agriculture:Location"
            },
            "schema:domainIncludes": {
                "@id": "agriculture:Authentication"
            },
            "rdfs:comment": "The SPS location of issue of this SPS authentication.",
            "rdfs:label": "issueLocation",
            "unece:cefactElementMetadata": [
                {
                    "@id": "cefact:SPS_Authentication.Issue.SPS_Location",
                    "@type": "unece:AssociationBIE",
                    "unece:cefactUNId": "UN03000036",
                    "unece:cefactBieDomainClass": "cefact:SPS_Authentication.Details",
                    "rdfs:comment": "The SPS location of issue of this SPS authentication."
                }
            ]
        },
        {
            "@id": "agriculture:issueReasonCode",
            "@type": "rdf:Property",
            "schema:rangeIncludes": {
                "@id": "xsd:token"
            },
            "schema:domainIncludes": {
                "@id": "agriculture:Certificate"
            },
            "rdfs:comment": "The code specifying the reason why the agricultural certificate was issued.",
            "rdfs:label": "issueReasonCode",
            "unece:cefactElementMetadata": [
                {
                    "@id": "cefact:Agricultural_Certificate.IssueReason.Code",
                    "@type": "unece:BasicBIE",
                    "unece:cefactUNId": "UN01012281",
                    "unece:cefactBieDomainClass": "cefact:Agricultural_Certificate.Details",
                    "rdfs:comment": "The code specifying the reason why the agricultural certificate was issued."
                }
            ]
        },
        {
            "@id": "agriculture:issuerAssignedId",
            "@type": "rdf:Property",
            "schema:rangeIncludes": {
                "@id": "xsd:token"
            },
            "schema:domainIncludes": {
                "@id": "agriculture:Plot"
            },
            "rdfs:comment": "The issuer assigned internal identifier for this agronomical observation plot.",
            "rdfs:label": "issuerAssignedId",
            "unece:cefactElementMetadata": [
                {
                    "@id": "cefact:AgronomicalObservation_Plot.IssuerAssigned_Identification.Identifier",
                    "@type": "unece:BasicBIE",
                    "unece:cefactUNId": "UN01009371",
                    "unece:cefactBieDomainClass": "cefact:AgronomicalObservation_Plot.Details",
                    "rdfs:comment": "The issuer assigned internal identifier for this agronomical observation plot."
                }
            ]
        },
        {
            "@id": "agriculture:issuerInternalId",
            "@type": "rdf:Property",
            "schema:rangeIncludes": {
                "@id": "xsd:token"
            },
            "schema:domainIncludes": {
                "@id": "agriculture:Plot"
            },
            "rdfs:comment": "The issuer internal identifier for this agricultural plot.",
            "rdfs:label": "issuerInternalId",
            "unece:cefactElementMetadata": [
                {
                    "@id": "cefact:Agricultural_Plot.IssuerInternal_Identification.Identifier",
                    "@type": "unece:BasicBIE",
                    "unece:cefactUNId": "UN01009349",
                    "unece:cefactBieDomainClass": "cefact:Agricultural_Plot.Details",
                    "rdfs:comment": "The issuer internal identifier for this agricultural plot."
                }
            ]
        },
        {
            "@id": "agriculture:issuerParty",
            "@type": "rdf:Property",
            "schema:rangeIncludes": {
                "@id": "agriculture:Party"
            },
            "schema:domainIncludes": {
                "@id": "agriculture:Document"
            },
            "rdfs:comment": [
                "The SPS party that issues this exchanged SPS document.",
                "The crop data sheet party that issues this crop data sheet document.",
                "The party that issues this agronomical observation document."
            ],
            "rdfs:label": "issuerParty",
            "unece:cefactElementMetadata": [
                {
                    "@id": "cefact:AgronomicalObservation_Document.Issuer.AgronomicalObservation_Party",
                    "@type": "unece:AssociationBIE",
                    "unece:cefactUNId": "UN01009298",
                    "unece:cefactBieDomainClass": "cefact:AgronomicalObservation_Document.Details",
                    "rdfs:comment": "The party that issues this agronomical observation document."
                },
                {
                    "@id": "cefact:CropDataSheet_Document.Issuer.CropDataSheet_Party",
                    "@type": "unece:AssociationBIE",
                    "unece:cefactUNId": "UN01002819",
                    "unece:cefactBieDomainClass": "cefact:CropDataSheet_Document.Details",
                    "rdfs:comment": "The crop data sheet party that issues this crop data sheet document."
                },
                {
                    "@id": "cefact:SPSExchanged_Document.Issuer.SPS_Party",
                    "@type": "unece:AssociationBIE",
                    "unece:cefactUNId": "UN03000009",
                    "unece:cefactBieDomainClass": "cefact:SPSExchanged_Document.Details",
                    "rdfs:comment": "The SPS party that issues this exchanged SPS document."
                }
            ]
        },
        {
            "@id": "agriculture:issuerPartyName",
            "@type": "rdf:Property",
            "schema:rangeIncludes": {
                "@id": "xsd:string"
            },
            "schema:domainIncludes": {
                "@id": "agriculture:Identity"
            },
            "rdfs:comment": "The name, expressed as text, of the party issuing this animal identity.",
            "rdfs:label": "issuerPartyName",
            "unece:cefactElementMetadata": [
                {
                    "@id": "cefact:Animal_Identity.IssuerPartyName.Text",
                    "@type": "unece:BasicBIE",
                    "unece:cefactUNId": "UN01007627",
                    "unece:cefactBieDomainClass": "cefact:Animal_Identity.Details",
                    "rdfs:comment": "The name, expressed as text, of the party issuing this animal identity."
                }
            ]
        },
        {
            "@id": "agriculture:issuingParty",
            "@type": "rdf:Property",
            "schema:rangeIncludes": {
                "@id": "agriculture:Party"
            },
            "schema:domainIncludes": {
                "@id": "agriculture:Seal"
            },
            "rdfs:comment": "The party issuing the SPS seal.",
            "rdfs:label": "issuingParty",
            "unece:cefactElementMetadata": [
                {
                    "@id": "cefact:SPS_Seal.Issuing.SPS_Party",
                    "@type": "unece:AssociationBIE",
                    "unece:cefactUNId": "UN03000138",
                    "unece:cefactBieDomainClass": "cefact:SPS_Seal.Details",
                    "rdfs:comment": "The party issuing the SPS seal."
                }
            ]
        },
        {
            "@id": "agriculture:issuingPartyId",
            "@type": "rdf:Property",
            "schema:rangeIncludes": {
                "@id": "xsd:token"
            },
            "schema:domainIncludes": {
                "@id": "agriculture:Certificate"
            },
            "rdfs:comment": "The identifier for the issuing party of this agricultural certificate.",
            "rdfs:label": "issuingPartyId",
            "unece:cefactElementMetadata": [
                {
                    "@id": "cefact:Agricultural_Certificate.Issuing_Party.Identifier",
                    "@type": "unece:BasicBIE",
                    "unece:cefactUNId": "UN01012287",
                    "unece:cefactBieDomainClass": "cefact:Agricultural_Certificate.Details",
                    "rdfs:comment": "The identifier for the issuing party of this agricultural certificate."
                }
            ]
        },
        {
            "@id": "agriculture:item",
            "@type": "rdf:Property",
            "schema:rangeIncludes": {
                "@id": "xsd:string"
            },
            "schema:domainIncludes": {
                "@id": "agriculture:ProtectionMeans"
            },
            "rdfs:comment": "An item, expressed as text, for this disease protection means.",
            "rdfs:label": "item",
            "unece:cefactElementMetadata": [
                {
                    "@id": "cefact:Disease_ProtectionMeans.Item.Text",
                    "@type": "unece:BasicBIE",
                    "unece:cefactUNId": "UN01015111",
                    "unece:cefactBieDomainClass": "cefact:Disease_ProtectionMeans.Details",
                    "rdfs:comment": "An item, expressed as text, for this disease protection means."
                }
            ]
        },
        {
            "@id": "agriculture:itemQuantity",
            "@type": "rdf:Property",
            "schema:rangeIncludes": {
                "@id": "xsd:decimal"
            },
            "schema:domainIncludes": [
                {
                    "@id": "agriculture:Document"
                },
                {
                    "@id": "agriculture:Package"
                }
            ],
            "rdfs:comment": [
                "The quantity of items in this LA exchanged document.",
                "The quantity of items within this SPS package."
            ],
            "rdfs:label": "itemQuantity",
            "unece:cefactElementMetadata": [
                {
                    "@id": "cefact:SPS_Package.Item.Quantity",
                    "@type": "unece:BasicBIE",
                    "unece:TDED": "7224",
                    "unece:cefactUNId": "UN03000107",
                    "unece:cefactBieDomainClass": "cefact:SPS_Package.Details",
                    "rdfs:comment": "The quantity of items within this SPS package."
                },
                {
                    "@id": "cefact:LAExchanged_Document.Item.Quantity",
                    "@type": "unece:BasicBIE",
                    "unece:cefactUNId": "UN01007702",
                    "unece:cefactBieDomainClass": "cefact:LAExchanged_Document.Details",
                    "rdfs:comment": "The quantity of items in this LA exchanged document."
                }
            ]
        },
        {
            "@id": "agriculture:lAExchangedDocumentStatusCode",
            "@type": "rdf:Property",
            "schema:rangeIncludes": {
                "@id": "unece:UNECECL1373Code"
            },
            "schema:domainIncludes": {
                "@id": "agriculture:Document"
            },
            "rdfs:comment": "The code specifying the status of this LA exchanged document.",
            "rdfs:label": "lAExchangedDocumentStatusCode",
            "unece:cefactElementMetadata": [
                {
                    "@id": "cefact:LAExchanged_Document.Status.Code",
                    "@type": "unece:BasicBIE",
                    "unece:TDED": "1373",
                    "unece:cefactUNId": "UN01007701",
                    "unece:cefactBieDomainClass": "cefact:LAExchanged_Document.Details",
                    "rdfs:comment": "The code specifying the status of this LA exchanged document."
                }
            ]
        },
        {
            "@id": "agriculture:lAExchangedDocumentTypeCode",
            "@type": "rdf:Property",
            "schema:rangeIncludes": {
                "@id": "unece:UNECECL1001Code"
            },
            "schema:domainIncludes": {
                "@id": "agriculture:Document"
            },
            "rdfs:comment": "The code specifying the type of LA exchanged document.",
            "rdfs:label": "lAExchangedDocumentTypeCode",
            "unece:cefactElementMetadata": [
                {
                    "@id": "cefact:LAExchanged_Document.Type.Code",
                    "@type": "unece:BasicBIE",
                    "unece:TDED": "1001",
                    "unece:cefactUNId": "UN01007700",
                    "unece:cefactBieDomainClass": "cefact:LAExchanged_Document.Details",
                    "rdfs:comment": "The code specifying the type of LA exchanged document."
                }
            ]
        },
        {
            "@id": "agriculture:lIMSRegistrationDateTime",
            "@type": "rdf:Property",
            "schema:rangeIncludes": {
                "@id": "xsd:dateTime"
            },
            "schema:domainIncludes": {
                "@id": "agriculture:Sample"
            },
            "rdfs:comment": "The date, time, date time, or other date time value for the Laboratory Information Management System (LIMS) registration of this agricultural sample.",
            "rdfs:label": "lIMSRegistrationDateTime",
            "unece:cefactElementMetadata": [
                {
                    "@id": "cefact:Agricultural_Sample.LIMS_Registration.DateTime",
                    "@type": "unece:BasicBIE",
                    "unece:cefactUNId": "UN01009587",
                    "unece:cefactBieDomainClass": "cefact:Agricultural_Sample.Details",
                    "rdfs:comment": "The date, time, date time, or other date time value for the Laboratory Information Management System (LIMS) registration of this agricultural sample."
                }
            ]
        },
        {
            "@id": "agriculture:lORExchangedDocumentId",
            "@type": "rdf:Property",
            "schema:rangeIncludes": {
                "@id": "xsd:token"
            },
            "schema:domainIncludes": {
                "@id": "agriculture:ObservationResult"
            },
            "rdfs:comment": "An identifier of the Laboratory Observation Report (LOR) exchanged document for this referenced observation result.",
            "rdfs:label": "lORExchangedDocumentId",
            "unece:cefactElementMetadata": [
                {
                    "@id": "cefact:Referenced_ObservationResult.LORExchangedDocument_Identification.Identifier",
                    "@type": "unece:BasicBIE",
                    "unece:cefactUNId": "UN01012455",
                    "unece:cefactBieDomainClass": "cefact:Referenced_ObservationResult.Details",
                    "rdfs:comment": "An identifier of the Laboratory Observation Report (LOR) exchanged document for this referenced observation result."
                }
            ]
        },
        {
            "@id": "agriculture:latestEndDateTime",
            "@type": "rdf:Property",
            "schema:rangeIncludes": {
                "@id": "xsd:dateTime"
            },
            "schema:domainIncludes": {
                "@id": "agriculture:AgriculturalProcess"
            },
            "rdfs:comment": "The date, time, date time or other date time value of the latest end for the crop production in this agricultural process.",
            "rdfs:label": "latestEndDateTime",
            "unece:cefactElementMetadata": [
                {
                    "@id": "cefact:CropProduction_AgriculturalProcess.Latest_End.DateTime",
                    "@type": "unece:BasicBIE",
                    "unece:cefactUNId": "UN01012413",
                    "unece:cefactBieDomainClass": "cefact:CropProduction_AgriculturalProcess.Details",
                    "rdfs:comment": "The date, time, date time or other date time value of the latest end for the crop production in this agricultural process."
                }
            ]
        },
        {
            "@id": "agriculture:legalBasis",
            "@type": "rdf:Property",
            "schema:rangeIncludes": {
                "@id": "xsd:string"
            },
            "schema:domainIncludes": {
                "@id": "agriculture:Identity"
            },
            "rdfs:comment": "The legal basis, expressed as text, for this animal identity.",
            "rdfs:label": "legalBasis",
            "unece:cefactElementMetadata": [
                {
                    "@id": "cefact:Animal_Identity.LegalBasis.Text",
                    "@type": "unece:BasicBIE",
                    "unece:cefactUNId": "UN01007626",
                    "unece:cefactBieDomainClass": "cefact:Animal_Identity.Details",
                    "rdfs:comment": "The legal basis, expressed as text, for this animal identity."
                }
            ]
        },
        {
            "@id": "agriculture:level",
            "@type": "rdf:Property",
            "schema:rangeIncludes": {
                "@id": "xsd:string"
            },
            "schema:domainIncludes": {
                "@id": "agriculture:CoordinateReferenceSystem"
            },
            "rdfs:comment": "The level, expressed as text, of this CS engineering coordinate reference system.",
            "rdfs:label": "level",
            "unece:cefactElementMetadata": [
                {
                    "@id": "cefact:CSEngineering_CoordinateReferenceSystem.Level.Text",
                    "@type": "unece:BasicBIE",
                    "unece:cefactUNId": "UN01012165",
                    "unece:cefactBieDomainClass": "cefact:CSEngineering_CoordinateReferenceSystem.Details",
                    "rdfs:comment": "The level, expressed as text, of this CS engineering coordinate reference system."
                }
            ]
        },
        {
            "@id": "agriculture:licence",
            "@type": "rdf:Property",
            "schema:rangeIncludes": {
                "@id": "xsd:string"
            },
            "schema:domainIncludes": {
                "@id": "agriculture:Construction"
            },
            "rdfs:comment": "The licence, expressed as text, for this agricultural construction.",
            "rdfs:label": "licence",
            "unece:cefactElementMetadata": [
                {
                    "@id": "cefact:Agricultural_Construction.Licence.Text",
                    "@type": "unece:BasicBIE",
                    "unece:cefactUNId": "UN01012234",
                    "unece:cefactBieDomainClass": "cefact:Agricultural_Construction.Details",
                    "rdfs:comment": "The licence, expressed as text, for this agricultural construction."
                }
            ]
        },
        {
            "@id": "agriculture:lineCountNumeric",
            "@type": "rdf:Property",
            "schema:rangeIncludes": {
                "@id": "xsd:decimal"
            },
            "schema:domainIncludes": {
                "@id": "agriculture:Document"
            },
            "rdfs:comment": [
                "The count of the number of lines in this crop data sheet document.",
                "The number of lines in this crop report document."
            ],
            "rdfs:label": "lineCountNumeric",
            "unece:cefactElementMetadata": [
                {
                    "@id": "cefact:CropReport_Document.LineCount.Numeric",
                    "@type": "unece:BasicBIE",
                    "unece:cefactUNId": "UN01012438",
                    "unece:cefactBieDomainClass": "cefact:CropReport_Document.Details",
                    "rdfs:comment": "The number of lines in this crop report document."
                },
                {
                    "@id": "cefact:CropDataSheet_Document.LineCount.Numeric",
                    "@type": "unece:BasicBIE",
                    "unece:cefactUNId": "UN01002818",
                    "unece:cefactBieDomainClass": "cefact:CropDataSheet_Document.Details",
                    "rdfs:comment": "The count of the number of lines in this crop data sheet document."
                }
            ]
        },
        {
            "@id": "agriculture:lineFive",
            "@type": "rdf:Property",
            "schema:rangeIncludes": {
                "@id": "xsd:string"
            },
            "schema:domainIncludes": {
                "@id": "agriculture:Address"
            },
            "rdfs:comment": "The fifth free form line, expressed as text, of the SPS address.",
            "rdfs:label": "lineFive",
            "unece:cefactElementMetadata": [
                {
                    "@id": "cefact:SPS_Address.LineFive.Text",
                    "@type": "unece:BasicBIE",
                    "unece:TDED": "3286",
                    "unece:cefactUNId": "UN03000025",
                    "unece:cefactBieDomainClass": "cefact:SPS_Address.Details",
                    "rdfs:comment": "The fifth free form line, expressed as text, of the SPS address."
                }
            ]
        },
        {
            "@id": "agriculture:lineFour",
            "@type": "rdf:Property",
            "schema:rangeIncludes": {
                "@id": "xsd:string"
            },
            "schema:domainIncludes": {
                "@id": "agriculture:Address"
            },
            "rdfs:comment": "The fourth free form line, expressed as text, of the SPS address.",
            "rdfs:label": "lineFour",
            "unece:cefactElementMetadata": [
                {
                    "@id": "cefact:SPS_Address.LineFour.Text",
                    "@type": "unece:BasicBIE",
                    "unece:TDED": "3286",
                    "unece:cefactUNId": "UN03000024",
                    "unece:cefactBieDomainClass": "cefact:SPS_Address.Details",
                    "rdfs:comment": "The fourth free form line, expressed as text, of the SPS address."
                }
            ]
        },
        {
            "@id": "agriculture:lineOne",
            "@type": "rdf:Property",
            "schema:rangeIncludes": {
                "@id": "xsd:string"
            },
            "schema:domainIncludes": {
                "@id": "agriculture:Address"
            },
            "rdfs:comment": "The first free form line, expressed as text, of the SPS address.",
            "rdfs:label": "lineOne",
            "unece:cefactElementMetadata": [
                {
                    "@id": "cefact:SPS_Address.LineOne.Text",
                    "@type": "unece:BasicBIE",
                    "unece:TDED": "3286",
                    "unece:cefactUNId": "UN03000021",
                    "unece:cefactBieDomainClass": "cefact:SPS_Address.Details",
                    "rdfs:comment": "The first free form line, expressed as text, of the SPS address."
                }
            ]
        },
        {
            "@id": "agriculture:lineThree",
            "@type": "rdf:Property",
            "schema:rangeIncludes": {
                "@id": "xsd:string"
            },
            "schema:domainIncludes": {
                "@id": "agriculture:Address"
            },
            "rdfs:comment": "The third free form line, expressed as text, of the SPS address.",
            "rdfs:label": "lineThree",
            "unece:cefactElementMetadata": [
                {
                    "@id": "cefact:SPS_Address.LineThree.Text",
                    "@type": "unece:BasicBIE",
                    "unece:TDED": "3286",
                    "unece:cefactUNId": "UN03000023",
                    "unece:cefactBieDomainClass": "cefact:SPS_Address.Details",
                    "rdfs:comment": "The third free form line, expressed as text, of the SPS address."
                }
            ]
        },
        {
            "@id": "agriculture:lineTwo",
            "@type": "rdf:Property",
            "schema:rangeIncludes": {
                "@id": "xsd:string"
            },
            "schema:domainIncludes": {
                "@id": "agriculture:Address"
            },
            "rdfs:comment": "The second free form line, expressed as text, of the SPS address.",
            "rdfs:label": "lineTwo",
            "unece:cefactElementMetadata": [
                {
                    "@id": "cefact:SPS_Address.LineTwo.Text",
                    "@type": "unece:BasicBIE",
                    "unece:TDED": "3286",
                    "unece:cefactUNId": "UN03000022",
                    "unece:cefactBieDomainClass": "cefact:SPS_Address.Details",
                    "rdfs:comment": "The second free form line, expressed as text, of the SPS address."
                }
            ]
        },
        {
            "@id": "agriculture:loadingBaseportLocation",
            "@type": "rdf:Property",
            "schema:rangeIncludes": {
                "@id": "agriculture:Location"
            },
            "schema:domainIncludes": {
                "@id": "agriculture:Consignment"
            },
            "rdfs:comment": "The baseport location at which this SPS consignment is to be loaded on a means of transport according to the transport contract.",
            "rdfs:label": "loadingBaseportLocation",
            "unece:cefactElementMetadata": [
                {
                    "@id": "cefact:SPS_Consignment.LoadingBaseport.SPS_Location",
                    "@type": "unece:AssociationBIE",
                    "unece:cefactUNId": "UN03000063",
                    "unece:cefactBieDomainClass": "cefact:SPS_Consignment.Details",
                    "rdfs:comment": "The baseport location at which this SPS consignment is to be loaded on a means of transport according to the transport contract."
                }
            ]
        },
        {
            "@id": "agriculture:localTypeCode",
            "@type": "rdf:Property",
            "schema:rangeIncludes": {
                "@id": "xsd:token"
            },
            "schema:domainIncludes": [
                {
                    "@id": "agriculture:SampleType"
                },
                {
                    "@id": "agriculture:SampledObject"
                }
            ],
            "rdfs:comment": [
                "The code specifying the local type of this agricultural sample type.",
                "The local code specifying the type of sampled agricultural object, used by the observer party or the customer."
            ],
            "rdfs:label": "localTypeCode",
            "unece:cefactElementMetadata": [
                {
                    "@id": "cefact:Agricultural_SampledObject.Local_Type.Code",
                    "@type": "unece:BasicBIE",
                    "unece:cefactUNId": "UN01009613",
                    "unece:cefactBieDomainClass": "cefact:Agricultural_SampledObject.Details",
                    "rdfs:comment": "The local code specifying the type of sampled agricultural object, used by the observer party or the customer."
                },
                {
                    "@id": "cefact:Agricultural_SampleType.Local_Type.Code",
                    "@type": "unece:BasicBIE",
                    "unece:cefactUNId": "UN01009580",
                    "unece:cefactBieDomainClass": "cefact:Agricultural_SampleType.Details",
                    "rdfs:comment": "The code specifying the local type of this agricultural sample type."
                }
            ]
        },
        {
            "@id": "agriculture:locationFunctionTypeCode",
            "@type": "rdf:Property",
            "schema:rangeIncludes": {
                "@id": "unece:UNECECL3227Code"
            },
            "schema:domainIncludes": {
                "@id": "agriculture:CountrySubDivision"
            },
            "rdfs:comment": "The code specifying the function type of this SPS country sub-division.",
            "rdfs:label": "locationFunctionTypeCode",
            "unece:cefactElementMetadata": [
                {
                    "@id": "cefact:SPS_CountrySub-Division.Function_Type.Code",
                    "@type": "unece:BasicBIE",
                    "unece:TDED": "3227",
                    "unece:cefactUNId": "UN03000083",
                    "unece:cefactBieDomainClass": "cefact:SPS_CountrySubDivision.Details",
                    "rdfs:comment": "The code specifying the function type of this SPS country sub-division."
                }
            ]
        },
        {
            "@id": "agriculture:locationId",
            "@type": "rdf:Property",
            "schema:rangeIncludes": {
                "@id": "xsd:token"
            },
            "schema:domainIncludes": {
                "@id": "agriculture:Event"
            },
            "rdfs:comment": "The identifier of the location for this animal holding event.",
            "rdfs:label": "locationId",
            "unece:cefactElementMetadata": [
                {
                    "@id": "cefact:AnimalHolding_Event.Location.Identifier",
                    "@type": "unece:BasicBIE",
                    "unece:cefactUNId": "UN01007635",
                    "unece:cefactBieDomainClass": "cefact:AnimalHolding_Event.Details",
                    "rdfs:comment": "The identifier of the location for this animal holding event."
                }
            ]
        },
        {
            "@id": "agriculture:locationProviderParty",
            "@type": "rdf:Property",
            "schema:rangeIncludes": {
                "@id": "agriculture:Party"
            },
            "schema:domainIncludes": {
                "@id": "agriculture:Authentication"
            },
            "rdfs:comment": "The SPS party providing the location for this SPS authentication.",
            "rdfs:label": "locationProviderParty",
            "unece:cefactElementMetadata": [
                {
                    "@id": "cefact:SPS_Authentication.LocationProvider.SPS_Party",
                    "@type": "unece:AssociationBIE",
                    "unece:cefactUNId": "UN03000038",
                    "unece:cefactBieDomainClass": "cefact:SPS_Authentication.Details",
                    "rdfs:comment": "The SPS party providing the location for this SPS authentication."
                }
            ]
        },
        {
            "@id": "agriculture:lowLimit",
            "@type": "rdf:Property",
            "schema:rangeIncludes": {
                "@id": "xsd:string"
            },
            "schema:domainIncludes": {
                "@id": "agriculture:GeographicalGrid"
            },
            "rdfs:comment": "The tuple of elements, expressed as text, indicating the low limit of this geographical grid specifying the offset of each axis.",
            "rdfs:label": "lowLimit",
            "unece:cefactElementMetadata": [
                {
                    "@id": "cefact:Specified_GeographicalGrid.Low_Limit.Text",
                    "@type": "unece:BasicBIE",
                    "unece:cefactUNId": "UN01012206",
                    "unece:cefactBieDomainClass": "cefact:Specified_GeographicalGrid.Details",
                    "rdfs:comment": "The tuple of elements, expressed as text, indicating the low limit of this geographical grid specifying the offset of each axis."
                }
            ]
        },
        {
            "@id": "agriculture:mainCarriageTransportMovement",
            "@type": "rdf:Property",
            "schema:rangeIncludes": {
                "@id": "agriculture:TransportMovement"
            },
            "schema:domainIncludes": {
                "@id": "agriculture:Consignment"
            },
            "rdfs:comment": "A transport movement of the main carriage of this SPS consignment.",
            "rdfs:label": "mainCarriageTransportMovement",
            "unece:cefactElementMetadata": [
                {
                    "@id": "cefact:SPS_Consignment.MainCarriage.SPS_TransportMovement",
                    "@type": "unece:AssociationBIE",
                    "unece:cefactUNId": "UN03000074",
                    "unece:cefactBieDomainClass": "cefact:SPS_Consignment.Details",
                    "rdfs:comment": "A transport movement of the main carriage of this SPS consignment."
                }
            ]
        },
        {
            "@id": "agriculture:managedProductionUnit",
            "@type": "rdf:Property",
            "schema:rangeIncludes": {
                "@id": "agriculture:ProductionUnit"
            },
            "schema:domainIncludes": {
                "@id": "agriculture:Party"
            },
            "rdfs:comment": "An agricultural production unit managed by this agricultural producer party.",
            "rdfs:label": "managedProductionUnit",
            "unece:cefactElementMetadata": [
                {
                    "@id": "cefact:AgriculturalProducer_Party.Managed.Agricultural_ProductionUnit",
                    "@type": "unece:AssociationBIE",
                    "unece:cefactUNId": "UN01012263",
                    "unece:cefactBieDomainClass": "cefact:AgriculturalProducer_Party.Details",
                    "rdfs:comment": "An agricultural production unit managed by this agricultural producer party."
                }
            ]
        },
        {
            "@id": "agriculture:marking",
            "@type": "rdf:Property",
            "schema:rangeIncludes": {
                "@id": "xsd:string"
            },
            "schema:domainIncludes": {
                "@id": "agriculture:ShippingMarks"
            },
            "rdfs:comment": "Marking, expressed as text, for these SPS shipping marks.",
            "rdfs:label": "marking",
            "unece:cefactElementMetadata": [
                {
                    "@id": "cefact:SPS_ShippingMarks.Marking.Text",
                    "@type": "unece:BasicBIE",
                    "unece:TDED": "7102",
                    "unece:cefactUNId": "UN03000140",
                    "unece:cefactBieDomainClass": "cefact:SPS_ShippingMarks.Details",
                    "rdfs:comment": "Marking, expressed as text, for these SPS shipping marks."
                }
            ]
        },
        {
            "@id": "agriculture:massMeasure",
            "@type": "rdf:Property",
            "schema:rangeIncludes": {
                "@id": "xsd:decimal"
            },
            "schema:domainIncludes": {
                "@id": "agriculture:Material"
            },
            "rdfs:comment": "The measure of the mass of this agricultural input material.",
            "rdfs:label": "massMeasure",
            "unece:cefactElementMetadata": [
                {
                    "@id": "cefact:AgriculturalInput_Material.Mass.Measure",
                    "@type": "unece:BasicBIE",
                    "unece:cefactUNId": "UN01012390",
                    "unece:cefactBieDomainClass": "cefact:AgriculturalInput_Material.Details",
                    "rdfs:comment": "The measure of the mass of this agricultural input material."
                }
            ]
        },
        {
            "@id": "agriculture:massRatioMeasure",
            "@type": "rdf:Property",
            "schema:rangeIncludes": {
                "@id": "xsd:decimal"
            },
            "schema:domainIncludes": {
                "@id": "agriculture:Material"
            },
            "rdfs:comment": "The mass measure of the this agricultural input material expressed as a ratio to another mass, such as the total mass.",
            "rdfs:label": "massRatioMeasure",
            "unece:cefactElementMetadata": [
                {
                    "@id": "cefact:AgriculturalInput_Material.MassRatio.Measure",
                    "@type": "unece:BasicBIE",
                    "unece:cefactUNId": "UN01012391",
                    "unece:cefactBieDomainClass": "cefact:AgriculturalInput_Material.Details",
                    "rdfs:comment": "The mass measure of the this agricultural input material expressed as a ratio to another mass, such as the total mass."
                }
            ]
        },
        {
            "@id": "agriculture:materialType",
            "@type": "rdf:Property",
            "schema:rangeIncludes": {
                "@id": "xsd:string"
            },
            "schema:domainIncludes": {
                "@id": "agriculture:SampleType"
            },
            "rdfs:comment": "The material type, expressed as text, of this agricultural sample type.",
            "rdfs:label": "materialType",
            "unece:cefactElementMetadata": [
                {
                    "@id": "cefact:Agricultural_SampleType.Material_Type.Text",
                    "@type": "unece:BasicBIE",
                    "unece:cefactUNId": "UN01009581",
                    "unece:cefactBieDomainClass": "cefact:Agricultural_SampleType.Details",
                    "rdfs:comment": "The material type, expressed as text, of this agricultural sample type."
                }
            ]
        },
        {
            "@id": "agriculture:materialTypeCode",
            "@type": "rdf:Property",
            "schema:rangeIncludes": {
                "@id": "xsd:token"
            },
            "schema:domainIncludes": {
                "@id": "agriculture:SampleType"
            },
            "rdfs:comment": "The code specifying a material type for this agricultural sample type.",
            "rdfs:label": "materialTypeCode",
            "unece:cefactElementMetadata": [
                {
                    "@id": "cefact:Agricultural_SampleType.Material_Type.Code",
                    "@type": "unece:BasicBIE",
                    "unece:cefactUNId": "UN01010478",
                    "unece:cefactBieDomainClass": "cefact:Agricultural_SampleType.Details",
                    "rdfs:comment": "The code specifying a material type for this agricultural sample type."
                }
            ]
        },
        {
            "@id": "agriculture:maximumId",
            "@type": "rdf:Property",
            "schema:rangeIncludes": {
                "@id": "xsd:token"
            },
            "schema:domainIncludes": {
                "@id": "agriculture:Seal"
            },
            "rdfs:comment": "The maximum unique identifier used for these SPS seals.",
            "rdfs:label": "maximumId",
            "unece:cefactElementMetadata": [
                {
                    "@id": "cefact:SPS_Seal.Maximum_Identification.Identifier",
                    "@type": "unece:BasicBIE",
                    "unece:TDED": "9308",
                    "unece:cefactUNId": "UN03000137",
                    "unece:cefactBieDomainClass": "cefact:SPS_Seal.Details",
                    "rdfs:comment": "The maximum unique identifier used for these SPS seals."
                }
            ]
        },
        {
            "@id": "agriculture:maximumSizeMeasure",
            "@type": "rdf:Property",
            "schema:rangeIncludes": {
                "@id": "xsd:decimal"
            },
            "schema:domainIncludes": {
                "@id": "agriculture:Batch"
            },
            "rdfs:comment": "The maximum size, expressed as a measure, of the animals for this animal batch.",
            "rdfs:label": "maximumSizeMeasure",
            "unece:cefactElementMetadata": [
                {
                    "@id": "cefact:Animal_Batch.Maximum_Size.Measure",
                    "@type": "unece:BasicBIE",
                    "unece:cefactUNId": "UN01011252",
                    "unece:cefactBieDomainClass": "cefact:Animal_Batch.Details",
                    "rdfs:comment": "The maximum size, expressed as a measure, of the animals for this animal batch."
                }
            ]
        },
        {
            "@id": "agriculture:maximumValueMeasure",
            "@type": "rdf:Property",
            "schema:rangeIncludes": {
                "@id": "xsd:decimal"
            },
            "schema:domainIncludes": [
                {
                    "@id": "agriculture:Characteristic"
                },
                {
                    "@id": "agriculture:Temperature"
                }
            ],
            "rdfs:comment": [
                "The measure of a maximum value for this SPS process characteristic.",
                "The measure of the highest value of this SPS temperature, such as a maximum temperature value of fourteen degrees Celsius."
            ],
            "rdfs:label": "maximumValueMeasure",
            "unece:cefactElementMetadata": [
                {
                    "@id": "cefact:SPSProcess_Characteristic.Maximum_Value.Measure",
                    "@type": "unece:BasicBIE",
                    "unece:TDED": "6314",
                    "unece:cefactUNId": "UN03000189",
                    "unece:cefactBieDomainClass": "cefact:SPSProcess_Characteristic.Details",
                    "rdfs:comment": "The measure of a maximum value for this SPS process characteristic."
                },
                {
                    "@id": "cefact:SPS_Temperature.Maximum_Value.Measure",
                    "@type": "unece:BasicBIE",
                    "unece:TDED": "6246",
                    "unece:cefactUNId": "UN03000144",
                    "unece:cefactBieDomainClass": "cefact:SPS_Temperature.Details",
                    "rdfs:comment": "The measure of the highest value of this SPS temperature, such as a maximum temperature value of fourteen degrees Celsius."
                }
            ]
        },
        {
            "@id": "agriculture:measuredAttributeTypeCode",
            "@type": "rdf:Property",
            "schema:rangeIncludes": {
                "@id": "unece:UNECECL6313Code"
            },
            "schema:domainIncludes": {
                "@id": "agriculture:Characteristic"
            },
            "rdfs:comment": "The code specifying a type of SPS process characteristic.",
            "rdfs:label": "measuredAttributeTypeCode",
            "unece:cefactElementMetadata": [
                {
                    "@id": "cefact:SPSProcess_Characteristic.Type.Code",
                    "@type": "unece:BasicBIE",
                    "unece:TDED": "6313",
                    "unece:cefactUNId": "UN03000178",
                    "unece:cefactBieDomainClass": "cefact:SPSProcess_Characteristic.Details",
                    "rdfs:comment": "The code specifying a type of SPS process characteristic."
                }
            ]
        },
        {
            "@id": "agriculture:memberGeographicalLine",
            "@type": "rdf:Property",
            "schema:rangeIncludes": {
                "@id": "agriculture:GeographicalLine"
            },
            "schema:domainIncludes": {
                "@id": "agriculture:GeographicalMultiCurve"
            },
            "rdfs:comment": "A geographical line member of this geographical multi-curve.",
            "rdfs:label": "memberGeographicalLine",
            "unece:cefactElementMetadata": [
                {
                    "@id": "cefact:Specified_GeographicalMulti-Curve.Member.Specified_GeographicalLine",
                    "@type": "unece:AssociationBIE",
                    "unece:cefactUNId": "UN01012193",
                    "unece:cefactBieDomainClass": "cefact:Specified_GeographicalMultiCurve.Details",
                    "rdfs:comment": "A geographical line member of this geographical multi-curve."
                }
            ]
        },
        {
            "@id": "agriculture:memberGeographicalPoint",
            "@type": "rdf:Property",
            "schema:rangeIncludes": {
                "@id": "agriculture:GeographicalPoint"
            },
            "schema:domainIncludes": {
                "@id": "agriculture:GeographicalMultiPoint"
            },
            "rdfs:comment": "A geographical point member of this geographical multi-point feature.",
            "rdfs:label": "memberGeographicalPoint",
            "unece:cefactElementMetadata": [
                {
                    "@id": "cefact:Specified_GeographicalMulti-Point.Member.Specified_GeographicalPoint",
                    "@type": "unece:AssociationBIE",
                    "unece:cefactUNId": "UN01012186",
                    "unece:cefactBieDomainClass": "cefact:Specified_GeographicalMultiPoint.Details",
                    "rdfs:comment": "A geographical point member of this geographical multi-point feature."
                }
            ]
        },
        {
            "@id": "agriculture:microbiologyStartDateTime",
            "@type": "rdf:Property",
            "schema:rangeIncludes": {
                "@id": "xsd:dateTime"
            },
            "schema:domainIncludes": {
                "@id": "agriculture:Sample"
            },
            "rdfs:comment": "The date, time, date time, or other date time value for the start of microbiology for this agricultural sample, such as when the sample is infected by a laboratory.",
            "rdfs:label": "microbiologyStartDateTime",
            "unece:cefactElementMetadata": [
                {
                    "@id": "cefact:Agricultural_Sample.Microbiology_Start.DateTime",
                    "@type": "unece:BasicBIE",
                    "unece:cefactUNId": "UN01009598",
                    "unece:cefactBieDomainClass": "cefact:Agricultural_Sample.Details",
                    "rdfs:comment": "The date, time, date time, or other date time value for the start of microbiology for this agricultural sample, such as when the sample is infected by a laboratory."
                }
            ]
        },
        {
            "@id": "agriculture:minimumSizeMeasure",
            "@type": "rdf:Property",
            "schema:rangeIncludes": {
                "@id": "xsd:decimal"
            },
            "schema:domainIncludes": {
                "@id": "agriculture:Batch"
            },
            "rdfs:comment": "The minimum size, expressed as a measure, of the animals for this animal batch.",
            "rdfs:label": "minimumSizeMeasure",
            "unece:cefactElementMetadata": [
                {
                    "@id": "cefact:Animal_Batch.Minimum_Size.Measure",
                    "@type": "unece:BasicBIE",
                    "unece:cefactUNId": "UN01011251",
                    "unece:cefactBieDomainClass": "cefact:Animal_Batch.Details",
                    "rdfs:comment": "The minimum size, expressed as a measure, of the animals for this animal batch."
                }
            ]
        },
        {
            "@id": "agriculture:minimumValueMeasure",
            "@type": "rdf:Property",
            "schema:rangeIncludes": {
                "@id": "xsd:decimal"
            },
            "schema:domainIncludes": [
                {
                    "@id": "agriculture:Characteristic"
                },
                {
                    "@id": "agriculture:Temperature"
                }
            ],
            "rdfs:comment": [
                "The measure of a minimum value for this SPS process characteristic.",
                "The measure of the lowest value of this SPS temperature, such as a minimum temperature value of four degrees Celsius."
            ],
            "rdfs:label": "minimumValueMeasure",
            "unece:cefactElementMetadata": [
                {
                    "@id": "cefact:SPS_Temperature.Minimum_Value.Measure",
                    "@type": "unece:BasicBIE",
                    "unece:TDED": "6246",
                    "unece:cefactUNId": "UN03000143",
                    "unece:cefactBieDomainClass": "cefact:SPS_Temperature.Details",
                    "rdfs:comment": "The measure of the lowest value of this SPS temperature, such as a minimum temperature value of four degrees Celsius."
                },
                {
                    "@id": "cefact:SPSProcess_Characteristic.Minimum_Value.Measure",
                    "@type": "unece:BasicBIE",
                    "unece:TDED": "6314",
                    "unece:cefactUNId": "UN03000188",
                    "unece:cefactBieDomainClass": "cefact:SPSProcess_Characteristic.Details",
                    "rdfs:comment": "The measure of a minimum value for this SPS process characteristic."
                }
            ]
        },
        {
            "@id": "agriculture:modeCode",
            "@type": "rdf:Property",
            "schema:rangeIncludes": {
                "@id": "xsd:token"
            },
            "schema:domainIncludes": {
                "@id": "agriculture:TransportMovement"
            },
            "rdfs:comment": "The code specifying a mode, such as by air, sea, rail, road or inland waterway, for this SPS transport movement.",
            "rdfs:label": "modeCode",
            "unece:cefactElementMetadata": [
                {
                    "@id": "cefact:SPS_TransportMovement.Mode.Code",
                    "@type": "unece:BasicBIE",
                    "unece:TDED": "8067",
                    "unece:cefactUNId": "UN03000174",
                    "unece:cefactBieDomainClass": "cefact:SPS_TransportMovement.Details",
                    "rdfs:comment": "The code specifying a mode, such as by air, sea, rail, road or inland waterway, for this SPS transport movement."
                }
            ]
        },
        {
            "@id": "agriculture:motherId",
            "@type": "rdf:Property",
            "schema:rangeIncludes": {
                "@id": "xsd:token"
            },
            "schema:domainIncludes": {
                "@id": "agriculture:Animal"
            },
            "rdfs:comment": "The identifier of the mother of this livestock animal.",
            "rdfs:label": "motherId",
            "unece:cefactElementMetadata": [
                {
                    "@id": "cefact:Livestock_Animal.Mother.Identifier",
                    "@type": "unece:BasicBIE",
                    "unece:cefactUNId": "UN01007647",
                    "unece:cefactBieDomainClass": "cefact:Livestock_Animal.Details",
                    "rdfs:comment": "The identifier of the mother of this livestock animal."
                }
            ]
        },
        {
            "@id": "agriculture:multiSurfaceTypeCode",
            "@type": "rdf:Property",
            "schema:rangeIncludes": {
                "@id": "xsd:token"
            },
            "schema:domainIncludes": {
                "@id": "agriculture:Area"
            },
            "rdfs:comment": "The code specifying the multi-surface type for this agricultural zone area.",
            "rdfs:label": "multiSurfaceTypeCode",
            "unece:cefactElementMetadata": [
                {
                    "@id": "cefact:AgriculturalZone_Area.Multi-Surface_Type.Code",
                    "@type": "unece:BasicBIE",
                    "unece:cefactUNId": "UN01012218",
                    "unece:cefactBieDomainClass": "cefact:AgriculturalZone_Area.Details",
                    "rdfs:comment": "The code specifying the multi-surface type for this agricultural zone area."
                }
            ]
        },
        {
            "@id": "agriculture:name",
            "@type": "rdf:Property",
            "schema:rangeIncludes": {
                "@id": "xsd:string"
            },
            "schema:domainIncludes": [
                {
                    "@id": "agriculture:Area"
                },
                {
                    "@id": "agriculture:Chemical"
                },
                {
                    "@id": "agriculture:Construction"
                },
                {
                    "@id": "agriculture:CoordinateReferenceSystem"
                },
                {
                    "@id": "agriculture:Country"
                },
                {
                    "@id": "agriculture:CountrySubDivision"
                },
                {
                    "@id": "agriculture:DirectPositionList"
                },
                {
                    "@id": "agriculture:Document"
                },
                {
                    "@id": "agriculture:GeographicalFeature"
                },
                {
                    "@id": "agriculture:GeographicalObjectCharacteristic"
                },
                {
                    "@id": "agriculture:Location"
                },
                {
                    "@id": "agriculture:Material"
                },
                {
                    "@id": "agriculture:Party"
                },
                {
                    "@id": "agriculture:Person"
                },
                {
                    "@id": "agriculture:Produce"
                },
                {
                    "@id": "agriculture:Product"
                },
                {
                    "@id": "agriculture:ProductionUnit"
                },
                {
                    "@id": "agriculture:Qualification"
                },
                {
                    "@id": "agriculture:SampledObject"
                },
                {
                    "@id": "agriculture:TransportMeans"
                }
            ],
            "rdfs:comment": [
                "A name, expressed as text, of this SPS country sub-division.",
                "A name, expressed as text, of this SPS country.",
                "A name, expressed as text, of this SPS location.",
                "A name, expressed as text, of this SPS qualification.",
                "A name, expressed as text, of this exchanged SPS document.",
                "A name, expressed as text, of this referenced country.",
                "The name, expressed as text, for this CS engineering coordinate reference system.",
                "The name, expressed as text, for this agricultural input chemical.",
                "The name, expressed as text, for this agricultural input product.",
                "The name, expressed as text, for this agricultural produce.",
                "The name, expressed as text, for this agricultural producer party.",
                "The name, expressed as text, for this agricultural production unit.",
                "The name, expressed as text, for this agricultural zone area.",
                "The name, expressed as text, for this agronomical observation party.",
                "The name, expressed as text, for this crop data sheet party.",
                "The name, expressed as text, for this crop produce.",
                "The name, expressed as text, for this geographical object characteristic.",
                "The name, expressed as text, for this sampled agricultural object.",
                "The name, expressed as text, for this specified party.",
                "The name, expressed as text, of this SPS means of transport.",
                "The name, expressed as text, of this SPS party.",
                "The name, expressed as text, of this SPS person.",
                "The name, expressed as text, of this agricultural construction.",
                "The name, expressed as text, of this agricultural input material.",
                "The name, expressed as text, of this operator person.",
                "The name, expressed as text, of this specified direct position list.",
                "The name, expressed as text, of this specified geographical feature.",
                "The name, expressed as text, of this specified qualification."
            ],
            "rdfs:label": "name",
            "unece:cefactElementMetadata": [
                {
                    "@id": "cefact:AgriculturalProducer_Party.Name.Text",
                    "@type": "unece:BasicBIE",
                    "unece:TDED": "3036",
                    "unece:cefactUNId": "UN01012260",
                    "unece:cefactBieDomainClass": "cefact:AgriculturalProducer_Party.Details",
                    "rdfs:comment": "The name, expressed as text, for this agricultural producer party."
                },
                {
                    "@id": "cefact:Agricultural_ProductionUnit.Name.Text",
                    "@type": "unece:BasicBIE",
                    "unece:cefactUNId": "UN01012247",
                    "unece:cefactBieDomainClass": "cefact:Agricultural_ProductionUnit.Details",
                    "rdfs:comment": "The name, expressed as text, for this agricultural production unit."
                },
                {
                    "@id": "cefact:Crop_Produce.Name.Text",
                    "@type": "unece:BasicBIE",
                    "unece:cefactUNId": "UN01012328",
                    "unece:cefactBieDomainClass": "cefact:Crop_Produce.Details",
                    "rdfs:comment": "The name, expressed as text, for this crop produce."
                },
                {
                    "@id": "cefact:SPS_Party.Name.Text",
                    "@type": "unece:BasicBIE",
                    "unece:TDED": "3036",
                    "unece:cefactUNId": "UN03000113",
                    "unece:cefactBieDomainClass": "cefact:SPS_Party.Details",
                    "rdfs:comment": "The name, expressed as text, of this SPS party."
                },
                {
                    "@id": "cefact:AgronomicalObservation_Party.Name.Text",
                    "@type": "unece:BasicBIE",
                    "unece:TDED": "3036",
                    "unece:cefactUNId": "UN01009303",
                    "unece:cefactBieDomainClass": "cefact:AgronomicalObservation_Party.Details",
                    "rdfs:comment": "The name, expressed as text, for this agronomical observation party."
                },
                {
                    "@id": "cefact:Agricultural_Construction.Name.Text",
                    "@type": "unece:BasicBIE",
                    "unece:cefactUNId": "UN01012227",
                    "unece:cefactBieDomainClass": "cefact:Agricultural_Construction.Details",
                    "rdfs:comment": "The name, expressed as text, of this agricultural construction."
                },
                {
                    "@id": "cefact:AgriculturalZone_Area.Name.Text",
                    "@type": "unece:BasicBIE",
                    "unece:cefactUNId": "UN01012215",
                    "unece:cefactBieDomainClass": "cefact:AgriculturalZone_Area.Details",
                    "rdfs:comment": "The name, expressed as text, for this agricultural zone area."
                },
                {
                    "@id": "cefact:AgriculturalInput_Chemical.Name.Text",
                    "@type": "unece:BasicBIE",
                    "unece:cefactUNId": "UN01012403",
                    "unece:cefactBieDomainClass": "cefact:AgriculturalInput_Chemical.Details",
                    "rdfs:comment": "The name, expressed as text, for this agricultural input chemical."
                },
                {
                    "@id": "cefact:CSEngineering_CoordinateReferenceSystem.Name.Text",
                    "@type": "unece:BasicBIE",
                    "unece:cefactUNId": "UN01012164",
                    "unece:cefactBieDomainClass": "cefact:CSEngineering_CoordinateReferenceSystem.Details",
                    "rdfs:comment": "The name, expressed as text, for this CS engineering coordinate reference system."
                },
                {
                    "@id": "cefact:AgriculturalInput_Product.Name.Text",
                    "@type": "unece:BasicBIE",
                    "unece:TDED": "7134",
                    "unece:cefactUNId": "UN01012375",
                    "unece:cefactBieDomainClass": "cefact:AgriculturalInput_Product.Details",
                    "rdfs:comment": "The name, expressed as text, for this agricultural input product."
                },
                {
                    "@id": "cefact:CropDataSheet_Party.Name.Text",
                    "@type": "unece:BasicBIE",
                    "unece:TDED": "3036",
                    "unece:cefactUNId": "UN01002809",
                    "unece:cefactBieDomainClass": "cefact:CropDataSheet_Party.Details",
                    "rdfs:comment": "The name, expressed as text, for this crop data sheet party."
                },
                {
                    "@id": "cefact:Specified_Party.Name.Text",
                    "@type": "unece:BasicBIE",
                    "unece:TDED": "3036",
                    "unece:cefactUNId": "UN01007610",
                    "unece:cefactBieDomainClass": "cefact:Specified_Party.Details",
                    "rdfs:comment": "The name, expressed as text, for this specified party."
                },
                {
                    "@id": "cefact:Operator_Person.Name.Text",
                    "@type": "unece:BasicBIE",
                    "unece:TDED": "3404",
                    "unece:cefactUNId": "UN01012274",
                    "unece:cefactBieDomainClass": "cefact:Operator_Person.Details",
                    "rdfs:comment": "The name, expressed as text, of this operator person."
                },
                {
                    "@id": "cefact:Agricultural_SampledObject.Name.Text",
                    "@type": "unece:BasicBIE",
                    "unece:cefactUNId": "UN01009611",
                    "unece:cefactBieDomainClass": "cefact:Agricultural_SampledObject.Details",
                    "rdfs:comment": "The name, expressed as text, for this sampled agricultural object."
                },
                {
                    "@id": "cefact:AgriculturalInput_Material.Name.Text",
                    "@type": "unece:BasicBIE",
                    "unece:cefactUNId": "UN01012387",
                    "unece:cefactBieDomainClass": "cefact:AgriculturalInput_Material.Details",
                    "rdfs:comment": "The name, expressed as text, of this agricultural input material."
                },
                {
                    "@id": "cefact:SPS_Location.Name.Text",
                    "@type": "unece:BasicBIE",
                    "unece:TDED": "3224",
                    "unece:cefactUNId": "UN03000095",
                    "unece:cefactBieDomainClass": "cefact:SPS_Location.Details",
                    "rdfs:comment": "A name, expressed as text, of this SPS location."
                },
                {
                    "@id": "cefact:SPS_CountrySub-Division.Name.Text",
                    "@type": "unece:BasicBIE",
                    "unece:TDED": "3228",
                    "unece:cefactUNId": "UN03000081",
                    "unece:cefactBieDomainClass": "cefact:SPS_CountrySubDivision.Details",
                    "rdfs:comment": "A name, expressed as text, of this SPS country sub-division."
                },
                {
                    "@id": "cefact:Specified_Qualification.Name.Text",
                    "@type": "unece:BasicBIE",
                    "unece:cefactUNId": "UN01007688",
                    "unece:cefactBieDomainClass": "cefact:Specified_Qualification.Details",
                    "rdfs:comment": "The name, expressed as text, of this specified qualification."
                },
                {
                    "@id": "cefact:Specified_GeographicalObjectCharacteristic.Name.Text",
                    "@type": "unece:BasicBIE",
                    "unece:cefactUNId": "UN01012372",
                    "unece:cefactBieDomainClass": "cefact:Specified_GeographicalObjectCharacteristic.Details",
                    "rdfs:comment": "The name, expressed as text, for this geographical object characteristic."
                },
                {
                    "@id": "cefact:SPS_Qualification.Name.Text",
                    "@type": "unece:BasicBIE",
                    "unece:TDED": "9006",
                    "unece:cefactUNId": "UN03000133",
                    "unece:cefactBieDomainClass": "cefact:SPS_Qualification.Details",
                    "rdfs:comment": "A name, expressed as text, of this SPS qualification."
                },
                {
                    "@id": "cefact:SPS_TransportMeans.Name.Text",
                    "@type": "unece:BasicBIE",
                    "unece:TDED": "8212",
                    "unece:cefactUNId": "UN03000171",
                    "unece:cefactBieDomainClass": "cefact:SPS_TransportMeans.Details",
                    "rdfs:comment": "The name, expressed as text, of this SPS means of transport."
                },
                {
                    "@id": "cefact:Agricultural_Produce.Name.Text",
                    "@type": "unece:BasicBIE",
                    "unece:cefactUNId": "UN01002702",
                    "unece:cefactBieDomainClass": "cefact:Agricultural_Produce.Details",
                    "rdfs:comment": "The name, expressed as text, for this agricultural produce."
                },
                {
                    "@id": "cefact:SPSExchanged_Document.Name.Text",
                    "@type": "unece:BasicBIE",
                    "unece:TDED": "1000",
                    "unece:cefactUNId": "UN03000002",
                    "unece:cefactBieDomainClass": "cefact:SPSExchanged_Document.Details",
                    "rdfs:comment": "A name, expressed as text, of this exchanged SPS document."
                },
                {
                    "@id": "cefact:Specified_GeographicalFeature.Name.Text",
                    "@type": "unece:BasicBIE",
                    "unece:cefactUNId": "UN01012170",
                    "unece:cefactBieDomainClass": "cefact:Specified_GeographicalFeature.Details",
                    "rdfs:comment": "The name, expressed as text, of this specified geographical feature."
                },
                {
                    "@id": "cefact:SPS_Country.Name.Text",
                    "@type": "unece:BasicBIE",
                    "unece:TDED": "3206",
                    "unece:cefactUNId": "UN03000089",
                    "unece:cefactBieDomainClass": "cefact:SPS_Country.Details",
                    "rdfs:comment": "A name, expressed as text, of this SPS country."
                },
                {
                    "@id": "cefact:Specified_DirectPositionList.Name.Text",
                    "@type": "unece:BasicBIE",
                    "unece:cefactUNId": "UN01012473",
                    "unece:cefactBieDomainClass": "cefact:Specified_DirectPositionList.Details",
                    "rdfs:comment": "The name, expressed as text, of this specified direct position list."
                },
                {
                    "@id": "cefact:Referenced_Country.Name.Text",
                    "@type": "unece:BasicBIE",
                    "unece:TDED": "3206",
                    "unece:cefactUNId": "UN01007615",
                    "unece:cefactBieDomainClass": "cefact:Referenced_Country.Details",
                    "rdfs:comment": "A name, expressed as text, of this referenced country."
                },
                {
                    "@id": "cefact:SPS_Person.Name.Text",
                    "@type": "unece:BasicBIE",
                    "unece:TDED": "3412",
                    "unece:cefactUNId": "UN03000124",
                    "unece:cefactBieDomainClass": "cefact:SPS_Person.Details",
                    "rdfs:comment": "The name, expressed as text, of this SPS person."
                }
            ]
        },
        {
            "@id": "agriculture:nationalAppearanceApplicableClassification",
            "@type": "rdf:Property",
            "schema:rangeIncludes": {
                "@id": "agriculture:Classification"
            },
            "schema:domainIncludes": {
                "@id": "agriculture:Animal"
            },
            "rdfs:comment": "A national appearance classification applicable to this livestock animal.",
            "rdfs:label": "nationalAppearanceApplicableClassification",
            "unece:cefactElementMetadata": [
                {
                    "@id": "cefact:Livestock_Animal.NationalAppearance_Applicable.Specified_Classification",
                    "@type": "unece:AssociationBIE",
                    "unece:cefactUNId": "UN01007650",
                    "unece:cefactBieDomainClass": "cefact:Livestock_Animal.Details",
                    "rdfs:comment": "A national appearance classification applicable to this livestock animal."
                }
            ]
        },
        {
            "@id": "agriculture:nationalApplicableClassification",
            "@type": "rdf:Property",
            "schema:rangeIncludes": {
                "@id": "agriculture:Classification"
            },
            "schema:domainIncludes": {
                "@id": "agriculture:Event"
            },
            "rdfs:comment": "The national classification applicable to this animal movement event.",
            "rdfs:label": "nationalApplicableClassification",
            "unece:cefactElementMetadata": [
                {
                    "@id": "cefact:AnimalMovement_Event.National_Applicable.Specified_Classification",
                    "@type": "unece:AssociationBIE",
                    "unece:cefactUNId": "UN01007640",
                    "unece:cefactBieDomainClass": "cefact:AnimalMovement_Event.Details",
                    "rdfs:comment": "The national classification applicable to this animal movement event."
                }
            ]
        },
        {
            "@id": "agriculture:nationalAuthorityIssuerParty",
            "@type": "rdf:Property",
            "schema:rangeIncludes": {
                "@id": "agriculture:Party"
            },
            "schema:domainIncludes": {
                "@id": "agriculture:Document"
            },
            "rdfs:comment": "The national authority party that issues this animal passport document.",
            "rdfs:label": "nationalAuthorityIssuerParty",
            "unece:cefactElementMetadata": [
                {
                    "@id": "cefact:AnimalPassport_Document.NationalAuthority_Issuer.Specified_Party",
                    "@type": "unece:AssociationBIE",
                    "unece:cefactUNId": "UN01007674",
                    "unece:cefactBieDomainClass": "cefact:AnimalPassport_Document.Details",
                    "rdfs:comment": "The national authority party that issues this animal passport document."
                }
            ]
        },
        {
            "@id": "agriculture:nationalColourApplicableClassification",
            "@type": "rdf:Property",
            "schema:rangeIncludes": {
                "@id": "agriculture:Classification"
            },
            "schema:domainIncludes": {
                "@id": "agriculture:Animal"
            },
            "rdfs:comment": "A national colour or pattern classification applicable to this livestock animal.",
            "rdfs:label": "nationalColourApplicableClassification",
            "unece:cefactElementMetadata": [
                {
                    "@id": "cefact:Livestock_Animal.NationalColour_Applicable.Specified_Classification",
                    "@type": "unece:AssociationBIE",
                    "unece:cefactUNId": "UN01007652",
                    "unece:cefactBieDomainClass": "cefact:Livestock_Animal.Details",
                    "rdfs:comment": "A national colour or pattern classification applicable to this livestock animal."
                }
            ]
        },
        {
            "@id": "agriculture:natureIdentificationCargo",
            "@type": "rdf:Property",
            "schema:rangeIncludes": {
                "@id": "agriculture:Cargo"
            },
            "schema:domainIncludes": {
                "@id": "agriculture:ConsignmentItem"
            },
            "rdfs:comment": "Cargo details of this SPS consignment item sufficient to identify its nature for customs, statistical or transport purposes.",
            "rdfs:label": "natureIdentificationCargo",
            "unece:cefactElementMetadata": [
                {
                    "@id": "cefact:SPS_ConsignmentItem.NatureIdentification.SPS_Cargo",
                    "@type": "unece:AssociationBIE",
                    "unece:cefactUNId": "UN03000051",
                    "unece:cefactBieDomainClass": "cefact:SPS_ConsignmentItem.Details",
                    "rdfs:comment": "Cargo details of this SPS consignment item sufficient to identify its nature for customs, statistical or transport purposes."
                }
            ]
        },
        {
            "@id": "agriculture:netVolumeMeasure",
            "@type": "rdf:Property",
            "schema:rangeIncludes": {
                "@id": "xsd:decimal"
            },
            "schema:domainIncludes": {
                "@id": "agriculture:TradeLineItem"
            },
            "rdfs:comment": "The measure of the net volume of this SPS trade line item, excluding unoccupied volume of the packaging.",
            "rdfs:label": "netVolumeMeasure",
            "unece:cefactElementMetadata": [
                {
                    "@id": "cefact:SPS_TradeLineItem.NetVolume.Measure",
                    "@type": "unece:BasicBIE",
                    "unece:TDED": "6316",
                    "unece:cefactUNId": "UN03000156",
                    "unece:cefactBieDomainClass": "cefact:SPS_TradeLineItem.Details",
                    "rdfs:comment": "The measure of the net volume of this SPS trade line item, excluding unoccupied volume of the packaging."
                }
            ]
        },
        {
            "@id": "agriculture:netWeightMeasure",
            "@type": "rdf:Property",
            "schema:rangeIncludes": {
                "@id": "xsd:decimal"
            },
            "schema:domainIncludes": {
                "@id": "agriculture:TradeLineItem"
            },
            "rdfs:comment": "The measure of the net weight (mass) of this SPS trade line item, excluding all packaging.",
            "rdfs:label": "netWeightMeasure",
            "unece:cefactElementMetadata": [
                {
                    "@id": "cefact:SPS_TradeLineItem.NetWeight.Measure",
                    "@type": "unece:BasicBIE",
                    "unece:TDED": "6020",
                    "unece:cefactUNId": "UN03000154",
                    "unece:cefactBieDomainClass": "cefact:SPS_TradeLineItem.Details",
                    "rdfs:comment": "The measure of the net weight (mass) of this SPS trade line item, excluding all packaging."
                }
            ]
        },
        {
            "@id": "agriculture:nominalGrossVolumeMeasure",
            "@type": "rdf:Property",
            "schema:rangeIncludes": {
                "@id": "xsd:decimal"
            },
            "schema:domainIncludes": {
                "@id": "agriculture:Package"
            },
            "rdfs:comment": "The measure of the nominal gross volume of this SPS package.",
            "rdfs:label": "nominalGrossVolumeMeasure",
            "unece:cefactElementMetadata": [
                {
                    "@id": "cefact:SPS_Package.Nominal_GrossVolume.Measure",
                    "@type": "unece:BasicBIE",
                    "unece:TDED": "6028",
                    "unece:cefactUNId": "UN03000109",
                    "unece:cefactBieDomainClass": "cefact:SPS_Package.Details",
                    "rdfs:comment": "The measure of the nominal gross volume of this SPS package."
                }
            ]
        },
        {
            "@id": "agriculture:nominalGrossWeightMeasure",
            "@type": "rdf:Property",
            "schema:rangeIncludes": {
                "@id": "xsd:decimal"
            },
            "schema:domainIncludes": {
                "@id": "agriculture:Package"
            },
            "rdfs:comment": "The measure of the nominal gross weight (mass) of this SPS package and its contents.",
            "rdfs:label": "nominalGrossWeightMeasure",
            "unece:cefactElementMetadata": [
                {
                    "@id": "cefact:SPS_Package.Nominal_GrossWeight.Measure",
                    "@type": "unece:BasicBIE",
                    "unece:TDED": "6022",
                    "unece:cefactUNId": "UN03000108",
                    "unece:cefactBieDomainClass": "cefact:SPS_Package.Details",
                    "rdfs:comment": "The measure of the nominal gross weight (mass) of this SPS package and its contents."
                }
            ]
        },
        {
            "@id": "agriculture:nominalSizeNumeric",
            "@type": "rdf:Property",
            "schema:rangeIncludes": {
                "@id": "xsd:decimal"
            },
            "schema:domainIncludes": {
                "@id": "agriculture:Batch"
            },
            "rdfs:comment": "The value of the nominal size for this crop produce batch.",
            "rdfs:label": "nominalSizeNumeric",
            "unece:cefactElementMetadata": [
                {
                    "@id": "cefact:CropProduce_Batch.NominalSize.Numeric",
                    "@type": "unece:BasicBIE",
                    "unece:cefactUNId": "UN01012340",
                    "unece:cefactBieDomainClass": "cefact:CropProduce_Batch.Details",
                    "rdfs:comment": "The value of the nominal size for this crop produce batch."
                }
            ]
        },
        {
            "@id": "agriculture:observationBasisScope",
            "@type": "rdf:Property",
            "schema:rangeIncludes": {
                "@id": "agriculture:Scope"
            },
            "schema:domainIncludes": {
                "@id": "agriculture:TargetObject"
            },
            "rdfs:comment": "A scope for an observation basis related to this agronomical observation target object.",
            "rdfs:label": "observationBasisScope",
            "unece:cefactElementMetadata": [
                {
                    "@id": "cefact:AgronomicalObservation_TargetObject.ObservationBasis.AgronomicalObservation_Scope",
                    "@type": "unece:AssociationBIE",
                    "unece:cefactUNId": "UN01009323",
                    "unece:cefactBieDomainClass": "cefact:AgronomicalObservation_TargetObject.Details",
                    "rdfs:comment": "A scope for an observation basis related to this agronomical observation target object."
                }
            ]
        },
        {
            "@id": "agriculture:observationProcessTrapTypeCode",
            "@type": "rdf:Property",
            "schema:rangeIncludes": {
                "@id": "unece:UNECECL7187Code"
            },
            "schema:domainIncludes": {
                "@id": "agriculture:Process"
            },
            "rdfs:comment": "The code specifying the type of trap used for this observation process.",
            "rdfs:label": "observationProcessTrapTypeCode",
            "unece:cefactElementMetadata": [
                {
                    "@id": "cefact:Observation_Process.Trap_Type.Code",
                    "@type": "unece:BasicBIE",
                    "unece:TDED": "7187",
                    "unece:cefactUNId": "UN01009335",
                    "unece:cefactBieDomainClass": "cefact:Observation_Process.Details",
                    "rdfs:comment": "The code specifying the type of trap used for this observation process."
                }
            ]
        },
        {
            "@id": "agriculture:occurrenceArea",
            "@type": "rdf:Property",
            "schema:rangeIncludes": {
                "@id": "agriculture:Area"
            },
            "schema:domainIncludes": {
                "@id": "agriculture:AgriculturalProcess"
            },
            "rdfs:comment": "An agricultural area within which this plot agricultural process occurs.",
            "rdfs:label": "occurrenceArea",
            "unece:cefactElementMetadata": [
                {
                    "@id": "cefact:Plot_AgriculturalProcess.Occurrence.Agricultural_Area",
                    "@type": "unece:AssociationBIE",
                    "unece:cefactUNId": "UN01002793",
                    "unece:cefactBieDomainClass": "cefact:Plot_AgriculturalProcess.Details",
                    "rdfs:comment": "An agricultural area within which this plot agricultural process occurs."
                }
            ]
        },
        {
            "@id": "agriculture:occurrenceCountrySub-Division",
            "@type": "rdf:Property",
            "schema:rangeIncludes": {
                "@id": "agriculture:CountrySub-Division"
            },
            "schema:domainIncludes": {
                "@id": "agriculture:SoilOccupation"
            },
            "rdfs:comment": "An agricultural country sub-division in which this plot soil occupation occurs.",
            "rdfs:label": "occurrenceCountrySub-Division",
            "unece:cefactElementMetadata": [
                {
                    "@id": "cefact:Plot_SoilOccupation.Occurrence.Agricultural_CountrySub-Division",
                    "@type": "unece:AssociationBIE",
                    "unece:cefactUNId": "UN01002756",
                    "unece:cefactBieDomainClass": "cefact:Plot_SoilOccupation.Details",
                    "rdfs:comment": "An agricultural country sub-division in which this plot soil occupation occurs."
                }
            ]
        },
        {
            "@id": "agriculture:occurrenceDateTime",
            "@type": "rdf:Property",
            "schema:rangeIncludes": {
                "@id": "xsd:dateTime"
            },
            "schema:domainIncludes": {
                "@id": "agriculture:Event"
            },
            "rdfs:comment": [
                "The date of the occurrence of this animal movement event.",
                "The date of the occurrence of this veterinarian event, such as the date of vaccination.",
                "The date, time, date time, or other date time value of the occurrence of this animal holding event."
            ],
            "rdfs:label": "occurrenceDateTime",
            "unece:cefactElementMetadata": [
                {
                    "@id": "cefact:AnimalHolding_Event.Occurrence.DateTime",
                    "@type": "unece:BasicBIE",
                    "unece:TDED": "2193",
                    "unece:cefactUNId": "UN01011241",
                    "unece:cefactBieDomainClass": "cefact:AnimalHolding_Event.Details",
                    "rdfs:comment": "The date, time, date time, or other date time value of the occurrence of this animal holding event."
                },
                {
                    "@id": "cefact:Veterinarian_Event.Occurrence.DateTime",
                    "@type": "unece:BasicBIE",
                    "unece:TDED": "2193",
                    "unece:cefactUNId": "UN01007633",
                    "unece:cefactBieDomainClass": "cefact:Veterinarian_Event.Details",
                    "rdfs:comment": "The date of the occurrence of this veterinarian event, such as the date of vaccination."
                },
                {
                    "@id": "cefact:AnimalMovement_Event.Occurrence.DateTime",
                    "@type": "unece:BasicBIE",
                    "unece:TDED": "2193",
                    "unece:cefactUNId": "UN01007639",
                    "unece:cefactBieDomainClass": "cefact:AnimalMovement_Event.Details",
                    "rdfs:comment": "The date of the occurrence of this animal movement event."
                }
            ]
        },
        {
            "@id": "agriculture:occurrenceLocation",
            "@type": "rdf:Property",
            "schema:rangeIncludes": {
                "@id": "agriculture:Location"
            },
            "schema:domainIncludes": [
                {
                    "@id": "agriculture:AgronomicalObservation"
                },
                {
                    "@id": "agriculture:Event"
                }
            ],
            "rdfs:comment": [
                "The location where this SPS event will occur or has occurred.",
                "The specified location where this single agronomical observation occurs."
            ],
            "rdfs:label": "occurrenceLocation",
            "unece:cefactElementMetadata": [
                {
                    "@id": "cefact:Single_AgronomicalObservation.Occurrence.Specified_Location",
                    "@type": "unece:AssociationBIE",
                    "unece:cefactUNId": "UN01009314",
                    "unece:cefactBieDomainClass": "cefact:Single_AgronomicalObservation.Details",
                    "rdfs:comment": "The specified location where this single agronomical observation occurs."
                },
                {
                    "@id": "cefact:SPS_Event.Occurrence.SPS_Location",
                    "@type": "unece:AssociationBIE",
                    "unece:cefactUNId": "UN03000092",
                    "unece:cefactBieDomainClass": "cefact:SPS_Event.Details",
                    "rdfs:comment": "The location where this SPS event will occur or has occurred."
                }
            ]
        },
        {
            "@id": "agriculture:occurrencePeriod",
            "@type": "rdf:Property",
            "schema:rangeIncludes": {
                "@id": "agriculture:Period"
            },
            "schema:domainIncludes": {
                "@id": "agriculture:AgriculturalProcess"
            },
            "rdfs:comment": "A delimited period within which this plot agricultural process occurs.",
            "rdfs:label": "occurrencePeriod",
            "unece:cefactElementMetadata": [
                {
                    "@id": "cefact:Plot_AgriculturalProcess.Occurrence.Delimited_Period",
                    "@type": "unece:AssociationBIE",
                    "unece:cefactUNId": "UN01002787",
                    "unece:cefactBieDomainClass": "cefact:Plot_AgriculturalProcess.Details",
                    "rdfs:comment": "A delimited period within which this plot agricultural process occurs."
                }
            ]
        },
        {
            "@id": "agriculture:officeAddress",
            "@type": "rdf:Property",
            "schema:rangeIncludes": {
                "@id": "agriculture:Address"
            },
            "schema:domainIncludes": {
                "@id": "agriculture:Party"
            },
            "rdfs:comment": "The unstructured office address for this specified party.",
            "rdfs:label": "officeAddress",
            "unece:cefactElementMetadata": [
                {
                    "@id": "cefact:Specified_Party.Office.Unstructured_Address",
                    "@type": "unece:AssociationBIE",
                    "unece:cefactUNId": "UN01007613",
                    "unece:cefactBieDomainClass": "cefact:Specified_Party.Details",
                    "rdfs:comment": "The unstructured office address for this specified party."
                }
            ]
        },
        {
            "@id": "agriculture:officeIssuerParty",
            "@type": "rdf:Property",
            "schema:rangeIncludes": {
                "@id": "agriculture:Party"
            },
            "schema:domainIncludes": {
                "@id": "agriculture:Document"
            },
            "rdfs:comment": "The issuing office party for this animal passport document.",
            "rdfs:label": "officeIssuerParty",
            "unece:cefactElementMetadata": [
                {
                    "@id": "cefact:AnimalPassport_Document.Office_Issuer.Specified_Party",
                    "@type": "unece:AssociationBIE",
                    "unece:cefactUNId": "UN01007675",
                    "unece:cefactBieDomainClass": "cefact:AnimalPassport_Document.Details",
                    "rdfs:comment": "The issuing office party for this animal passport document."
                }
            ]
        },
        {
            "@id": "agriculture:offsetVectorNumeric",
            "@type": "rdf:Property",
            "schema:rangeIncludes": {
                "@id": "xsd:decimal"
            },
            "schema:domainIncludes": {
                "@id": "agriculture:GeographicalGrid"
            },
            "rdfs:comment": "The offset vector, expressed as a number, which indicates the offset of cells along each axis for this geographical grid.",
            "rdfs:label": "offsetVectorNumeric",
            "unece:cefactElementMetadata": [
                {
                    "@id": "cefact:Specified_GeographicalGrid.OffsetVector.Numeric",
                    "@type": "unece:BasicBIE",
                    "unece:cefactUNId": "UN01012205",
                    "unece:cefactBieDomainClass": "cefact:Specified_GeographicalGrid.Details",
                    "rdfs:comment": "The offset vector, expressed as a number, which indicates the offset of cells along each axis for this geographical grid."
                }
            ]
        },
        {
            "@id": "agriculture:operationCountry",
            "@type": "rdf:Property",
            "schema:rangeIncludes": {
                "@id": "agriculture:Country"
            },
            "schema:domainIncludes": {
                "@id": "agriculture:Process"
            },
            "rdfs:comment": "The country where the operation of this SPS process occurs.",
            "rdfs:label": "operationCountry",
            "unece:cefactElementMetadata": [
                {
                    "@id": "cefact:SPS_Process.Operation.SPS_Country",
                    "@type": "unece:AssociationBIE",
                    "unece:cefactUNId": "UN03000130",
                    "unece:cefactBieDomainClass": "cefact:SPS_Process.Details",
                    "rdfs:comment": "The country where the operation of this SPS process occurs."
                }
            ]
        },
        {
            "@id": "agriculture:operatorParty",
            "@type": "rdf:Property",
            "schema:rangeIncludes": {
                "@id": "agriculture:Party"
            },
            "schema:domainIncludes": {
                "@id": "agriculture:Process"
            },
            "rdfs:comment": "The party who is the operator of this SPS process.",
            "rdfs:label": "operatorParty",
            "unece:cefactElementMetadata": [
                {
                    "@id": "cefact:SPS_Process.Operator.SPS_Party",
                    "@type": "unece:AssociationBIE",
                    "unece:cefactUNId": "UN03000131",
                    "unece:cefactBieDomainClass": "cefact:SPS_Process.Details",
                    "rdfs:comment": "The party who is the operator of this SPS process."
                }
            ]
        },
        {
            "@id": "agriculture:originAssociatedDirectPositionList",
            "@type": "rdf:Property",
            "schema:rangeIncludes": {
                "@id": "agriculture:DirectPositionList"
            },
            "schema:domainIncludes": {
                "@id": "agriculture:GeographicalGrid"
            },
            "rdfs:comment": "The direct position list associated with the origin of this geographical grid.",
            "rdfs:label": "originAssociatedDirectPositionList",
            "unece:cefactElementMetadata": [
                {
                    "@id": "cefact:Specified_GeographicalGrid.Origin_Associated.Specified_DirectPositionList",
                    "@type": "unece:AssociationBIE",
                    "unece:cefactUNId": "UN01012210",
                    "unece:cefactBieDomainClass": "cefact:Specified_GeographicalGrid.Details",
                    "rdfs:comment": "The direct position list associated with the origin of this geographical grid."
                }
            ]
        },
        {
            "@id": "agriculture:originCountry",
            "@type": "rdf:Property",
            "schema:rangeIncludes": {
                "@id": "agriculture:Country"
            },
            "schema:domainIncludes": {
                "@id": "agriculture:TradeLineItem"
            },
            "rdfs:comment": "A country of origin for this SPS trade line item.",
            "rdfs:label": "originCountry",
            "unece:cefactElementMetadata": [
                {
                    "@id": "cefact:SPS_TradeLineItem.Origin.SPS_Country",
                    "@type": "unece:AssociationBIE",
                    "unece:cefactUNId": "UN03000162",
                    "unece:cefactBieDomainClass": "cefact:SPS_TradeLineItem.Details",
                    "rdfs:comment": "A country of origin for this SPS trade line item."
                }
            ]
        },
        {
            "@id": "agriculture:originLocation",
            "@type": "rdf:Property",
            "schema:rangeIncludes": {
                "@id": "agriculture:Location"
            },
            "schema:domainIncludes": {
                "@id": "agriculture:TradeLineItem"
            },
            "rdfs:comment": "A location of origin for this SPS trade line item.",
            "rdfs:label": "originLocation",
            "unece:cefactElementMetadata": [
                {
                    "@id": "cefact:SPS_TradeLineItem.Origin.SPS_Location",
                    "@type": "unece:AssociationBIE",
                    "unece:cefactUNId": "UN03000163",
                    "unece:cefactBieDomainClass": "cefact:SPS_TradeLineItem.Details",
                    "rdfs:comment": "A location of origin for this SPS trade line item."
                }
            ]
        },
        {
            "@id": "agriculture:originRelatedCountry",
            "@type": "rdf:Property",
            "schema:rangeIncludes": {
                "@id": "agriculture:Country"
            },
            "schema:domainIncludes": {
                "@id": "agriculture:Event"
            },
            "rdfs:comment": "The referenced country of origin related to this cross border animal movement event.",
            "rdfs:label": "originRelatedCountry",
            "unece:cefactElementMetadata": [
                {
                    "@id": "cefact:CrossBorderAnimalMovement_Event.Origin_Related.Referenced_Country",
                    "@type": "unece:AssociationBIE",
                    "unece:cefactUNId": "UN01007665",
                    "unece:cefactBieDomainClass": "cefact:CrossBorderAnimalMovement_Event.Details",
                    "rdfs:comment": "The referenced country of origin related to this cross border animal movement event."
                }
            ]
        },
        {
            "@id": "agriculture:outputCapacityMeasure",
            "@type": "rdf:Property",
            "schema:rangeIncludes": {
                "@id": "xsd:decimal"
            },
            "schema:domainIncludes": {
                "@id": "agriculture:Construction"
            },
            "rdfs:comment": "The measure of the output capacity for this agricultural construction.",
            "rdfs:label": "outputCapacityMeasure",
            "unece:cefactElementMetadata": [
                {
                    "@id": "cefact:Agricultural_Construction.Output_Capacity.Measure",
                    "@type": "unece:BasicBIE",
                    "unece:cefactUNId": "UN01012239",
                    "unece:cefactBieDomainClass": "cefact:Agricultural_Construction.Details",
                    "rdfs:comment": "The measure of the output capacity for this agricultural construction."
                }
            ]
        },
        {
            "@id": "agriculture:outputSpecifiedBatch",
            "@type": "rdf:Property",
            "schema:rangeIncludes": {
                "@id": "agriculture:Batch"
            },
            "schema:domainIncludes": {
                "@id": "agriculture:Produce"
            },
            "rdfs:comment": "An output batch crop produce, such as potatoes, grain, straw, specified for this crop produce.",
            "rdfs:label": "outputSpecifiedBatch",
            "unece:cefactElementMetadata": [
                {
                    "@id": "cefact:Crop_Produce.Output_Specified.CropProduce_Batch",
                    "@type": "unece:AssociationBIE",
                    "unece:cefactUNId": "UN01012330",
                    "unece:cefactBieDomainClass": "cefact:Crop_Produce.Details",
                    "rdfs:comment": "An output batch crop produce, such as potatoes, grain, straw, specified for this crop produce."
                }
            ]
        },
        {
            "@id": "agriculture:ownerParty",
            "@type": "rdf:Property",
            "schema:rangeIncludes": {
                "@id": "agriculture:Party"
            },
            "schema:domainIncludes": [
                {
                    "@id": "agriculture:AgriculturalDevice"
                },
                {
                    "@id": "agriculture:CountrySubDivision"
                },
                {
                    "@id": "agriculture:Plot"
                },
                {
                    "@id": "agriculture:SampledObject"
                }
            ],
            "rdfs:comment": [
                "A party that owns this agronomical observation plot.",
                "An agronomical observation party that owns this agricultural plot.",
                "The crop data sheet party that owns this agricultural country sub-division.",
                "The crop data sheet party that owns this specified agricultural device.",
                "The owner party for this sampled agricultural object."
            ],
            "rdfs:label": "ownerParty",
            "unece:cefactElementMetadata": [
                {
                    "@id": "cefact:Specified_AgriculturalDevice.Owner.CropDataSheet_Party",
                    "@type": "unece:AssociationBIE",
                    "unece:cefactUNId": "UN01002740",
                    "unece:cefactBieDomainClass": "cefact:Specified_AgriculturalDevice.Details",
                    "rdfs:comment": "The crop data sheet party that owns this specified agricultural device."
                },
                {
                    "@id": "cefact:Agricultural_SampledObject.Owner.LaboratoryObservation_Party",
                    "@type": "unece:AssociationBIE",
                    "unece:cefactUNId": "UN01009633",
                    "unece:cefactBieDomainClass": "cefact:Agricultural_SampledObject.Details",
                    "rdfs:comment": "The owner party for this sampled agricultural object."
                },
                {
                    "@id": "cefact:AgronomicalObservation_Plot.Owner.AgronomicalObservation_Party",
                    "@type": "unece:AssociationBIE",
                    "unece:cefactUNId": "UN01009376",
                    "unece:cefactBieDomainClass": "cefact:AgronomicalObservation_Plot.Details",
                    "rdfs:comment": "A party that owns this agronomical observation plot."
                },
                {
                    "@id": "cefact:Agricultural_Plot.Owner.AgronomicalObservation_Party",
                    "@type": "unece:AssociationBIE",
                    "unece:cefactUNId": "UN01009353",
                    "unece:cefactBieDomainClass": "cefact:Agricultural_Plot.Details",
                    "rdfs:comment": "An agronomical observation party that owns this agricultural plot."
                },
                {
                    "@id": "cefact:Agricultural_CountrySub-Division.Owner.CropDataSheet_Party",
                    "@type": "unece:AssociationBIE",
                    "unece:cefactUNId": "UN01002782",
                    "unece:cefactBieDomainClass": "cefact:Agricultural_CountrySubDivision.Details",
                    "rdfs:comment": "The crop data sheet party that owns this agricultural country sub-division."
                }
            ]
        },
        {
            "@id": "agriculture:packagingType",
            "@type": "rdf:Property",
            "schema:rangeIncludes": {
                "@id": "xsd:string"
            },
            "schema:domainIncludes": {
                "@id": "agriculture:Sample"
            },
            "rdfs:comment": "The packaging type, expressed as text, for this agricultural sample.",
            "rdfs:label": "packagingType",
            "unece:cefactElementMetadata": [
                {
                    "@id": "cefact:Agricultural_Sample.PackagingType.Text",
                    "@type": "unece:BasicBIE",
                    "unece:cefactUNId": "UN01009591",
                    "unece:cefactBieDomainClass": "cefact:Agricultural_Sample.Details",
                    "rdfs:comment": "The packaging type, expressed as text, for this agricultural sample."
                }
            ]
        },
        {
            "@id": "agriculture:packerParty",
            "@type": "rdf:Property",
            "schema:rangeIncludes": {
                "@id": "agriculture:Party"
            },
            "schema:domainIncludes": {
                "@id": "agriculture:SampledObject"
            },
            "rdfs:comment": "The party who packed this sampled agricultural object.",
            "rdfs:label": "packerParty",
            "unece:cefactElementMetadata": [
                {
                    "@id": "cefact:Agricultural_SampledObject.Packer.LaboratoryObservation_Party",
                    "@type": "unece:AssociationBIE",
                    "unece:cefactUNId": "UN01009631",
                    "unece:cefactBieDomainClass": "cefact:Agricultural_SampledObject.Details",
                    "rdfs:comment": "The party who packed this sampled agricultural object."
                }
            ]
        },
        {
            "@id": "agriculture:parentParty",
            "@type": "rdf:Property",
            "schema:rangeIncludes": {
                "@id": "agriculture:Party"
            },
            "schema:domainIncludes": {
                "@id": "agriculture:Party"
            },
            "rdfs:comment": "A party that is a parent of this agricultural producer party.",
            "rdfs:label": "parentParty",
            "unece:cefactElementMetadata": [
                {
                    "@id": "cefact:AgriculturalProducer_Party.Parent.AgriculturalProducer_Party",
                    "@type": "unece:AssociationBIE",
                    "unece:cefactUNId": "UN01012264",
                    "unece:cefactBieDomainClass": "cefact:AgriculturalProducer_Party.Details",
                    "rdfs:comment": "A party that is a parent of this agricultural producer party."
                }
            ]
        },
        {
            "@id": "agriculture:partyRoleCode",
            "@type": "rdf:Property",
            "schema:rangeIncludes": {
                "@id": "unece:UNECECL3035Code"
            },
            "schema:domainIncludes": {
                "@id": "agriculture:Party"
            },
            "rdfs:comment": "The code specifying the role of this SPS party.",
            "rdfs:label": "partyRoleCode",
            "unece:cefactElementMetadata": [
                {
                    "@id": "cefact:SPS_Party.Role.Code",
                    "@type": "unece:BasicBIE",
                    "unece:TDED": "3035",
                    "unece:cefactUNId": "UN03000114",
                    "unece:cefactBieDomainClass": "cefact:SPS_Party.Details",
                    "rdfs:comment": "The code specifying the role of this SPS party."
                }
            ]
        },
        {
            "@id": "agriculture:performedWorkItem",
            "@type": "rdf:Property",
            "schema:rangeIncludes": {
                "@id": "agriculture:WorkItem"
            },
            "schema:domainIncludes": {
                "@id": "agriculture:AgriculturalProcess"
            },
            "rdfs:comment": "An agricultural process work item performed within this plot agricultural process.",
            "rdfs:label": "performedWorkItem",
            "unece:cefactElementMetadata": [
                {
                    "@id": "cefact:Plot_AgriculturalProcess.Performed.AgriculturalProcess_WorkItem",
                    "@type": "unece:AssociationBIE",
                    "unece:cefactUNId": "UN01002788",
                    "unece:cefactBieDomainClass": "cefact:Plot_AgriculturalProcess.Details",
                    "rdfs:comment": "An agricultural process work item performed within this plot agricultural process."
                }
            ]
        },
        {
            "@id": "agriculture:personName",
            "@type": "rdf:Property",
            "schema:rangeIncludes": {
                "@id": "xsd:string"
            },
            "schema:domainIncludes": {
                "@id": "agriculture:Contact"
            },
            "rdfs:comment": "The person name, expressed as text, of this SPS contact.",
            "rdfs:label": "personName",
            "unece:cefactElementMetadata": [
                {
                    "@id": "cefact:SPS_Contact.PersonName.Text",
                    "@type": "unece:BasicBIE",
                    "unece:TDED": "3412",
                    "unece:cefactUNId": "UN03000078",
                    "unece:cefactBieDomainClass": "cefact:SPS_Contact.Details",
                    "rdfs:comment": "The person name, expressed as text, of this SPS contact."
                }
            ]
        },
        {
            "@id": "agriculture:physicalGeographicalFeature",
            "@type": "rdf:Property",
            "schema:rangeIncludes": {
                "@id": "agriculture:GeographicalFeature"
            },
            "schema:domainIncludes": {
                "@id": "agriculture:Location"
            },
            "rdfs:comment": "The physical geographical feature specified for this referenced location.",
            "rdfs:label": "physicalGeographicalFeature",
            "unece:cefactElementMetadata": [
                {
                    "@id": "cefact:Referenced_Location.Physical.Specified_GeographicalFeature",
                    "@type": "unece:AssociationBIE",
                    "unece:cefactUNId": "UN01012160",
                    "unece:cefactBieDomainClass": "cefact:Referenced_Location.Details",
                    "rdfs:comment": "The physical geographical feature specified for this referenced location."
                }
            ]
        },
        {
            "@id": "agriculture:physicalPackage",
            "@type": "rdf:Property",
            "schema:rangeIncludes": {
                "@id": "agriculture:Package"
            },
            "schema:domainIncludes": {
                "@id": "agriculture:TradeLineItem"
            },
            "rdfs:comment": "A physical package for this SPS trade line item.",
            "rdfs:label": "physicalPackage",
            "unece:cefactElementMetadata": [
                {
                    "@id": "cefact:SPS_TradeLineItem.Physical.SPS_Package",
                    "@type": "unece:AssociationBIE",
                    "unece:cefactUNId": "UN03000160",
                    "unece:cefactBieDomainClass": "cefact:SPS_TradeLineItem.Details",
                    "rdfs:comment": "A physical package for this SPS trade line item."
                }
            ]
        },
        {
            "@id": "agriculture:physicalShippingMarks",
            "@type": "rdf:Property",
            "schema:rangeIncludes": {
                "@id": "agriculture:ShippingMarks"
            },
            "schema:domainIncludes": {
                "@id": "agriculture:Package"
            },
            "rdfs:comment": "Physical shipping marks for this SPS package.",
            "rdfs:label": "physicalShippingMarks",
            "unece:cefactElementMetadata": [
                {
                    "@id": "cefact:SPS_Package.Physical.SPS_ShippingMarks",
                    "@type": "unece:AssociationBIE",
                    "unece:cefactUNId": "UN03000110",
                    "unece:cefactBieDomainClass": "cefact:SPS_Package.Details",
                    "rdfs:comment": "Physical shipping marks for this SPS package."
                }
            ]
        },
        {
            "@id": "agriculture:plantingReasonCode",
            "@type": "rdf:Property",
            "schema:rangeIncludes": {
                "@id": "xsd:token"
            },
            "schema:domainIncludes": {
                "@id": "agriculture:Crop"
            },
            "rdfs:comment": [
                "A code specifying a reason for planting this field crop.",
                "The code specifying the planting reason for this agricultural crop."
            ],
            "rdfs:label": "plantingReasonCode",
            "unece:cefactElementMetadata": [
                {
                    "@id": "cefact:Agricultural_Crop.PlantingReason.Code",
                    "@type": "unece:BasicBIE",
                    "unece:cefactUNId": "UN01002690",
                    "unece:cefactBieDomainClass": "cefact:Agricultural_Crop.Details",
                    "rdfs:comment": "The code specifying the planting reason for this agricultural crop."
                },
                {
                    "@id": "cefact:Field_Crop.PlantingReason.Code",
                    "@type": "unece:BasicBIE",
                    "unece:cefactUNId": "UN01012299",
                    "unece:cefactBieDomainClass": "cefact:Field_Crop.Details",
                    "rdfs:comment": "A code specifying a reason for planting this field crop."
                }
            ]
        },
        {
            "@id": "agriculture:postalAddress",
            "@type": "rdf:Property",
            "schema:rangeIncludes": {
                "@id": "agriculture:Address"
            },
            "schema:domainIncludes": {
                "@id": "agriculture:Party"
            },
            "rdfs:comment": "The unstructured postal address of this agronomical observation party.",
            "rdfs:label": "postalAddress",
            "unece:cefactElementMetadata": [
                {
                    "@id": "cefact:AgronomicalObservation_Party.Postal.Unstructured_Address",
                    "@type": "unece:AssociationBIE",
                    "unece:cefactUNId": "UN01009306",
                    "unece:cefactBieDomainClass": "cefact:AgronomicalObservation_Party.Details",
                    "rdfs:comment": "The unstructured postal address of this agronomical observation party."
                }
            ]
        },
        {
            "@id": "agriculture:postcodeCode",
            "@type": "rdf:Property",
            "schema:rangeIncludes": {
                "@id": "xsd:token"
            },
            "schema:domainIncludes": {
                "@id": "agriculture:Address"
            },
            "rdfs:comment": "The code specifying the postcode in the SPS address.",
            "rdfs:label": "postcodeCode",
            "unece:cefactElementMetadata": [
                {
                    "@id": "cefact:SPS_Address.Postcode.Code",
                    "@type": "unece:BasicBIE",
                    "unece:TDED": "3251",
                    "unece:cefactUNId": "UN03000020",
                    "unece:cefactBieDomainClass": "cefact:SPS_Address.Details",
                    "rdfs:comment": "The code specifying the postcode in the SPS address."
                }
            ]
        },
        {
            "@id": "agriculture:presencePercent",
            "@type": "rdf:Property",
            "schema:rangeIncludes": {
                "@id": "xsd:decimal"
            },
            "schema:domainIncludes": {
                "@id": "agriculture:Chemical"
            },
            "rdfs:comment": [
                "The percent of the presence of this crop input chemical.",
                "The percentage of the presence of the chemical in this agricultural input."
            ],
            "rdfs:label": "presencePercent",
            "unece:cefactElementMetadata": [
                {
                    "@id": "cefact:CropInput_Chemical.Presence.Percent",
                    "@type": "unece:BasicBIE",
                    "unece:cefactUNId": "UN01002748",
                    "unece:cefactBieDomainClass": "cefact:CropInput_Chemical.Details",
                    "rdfs:comment": "The percent of the presence of this crop input chemical."
                },
                {
                    "@id": "cefact:AgriculturalInput_Chemical.Presence.Percent",
                    "@type": "unece:BasicBIE",
                    "unece:cefactUNId": "UN01012407",
                    "unece:cefactBieDomainClass": "cefact:AgriculturalInput_Chemical.Details",
                    "rdfs:comment": "The percentage of the presence of the chemical in this agricultural input."
                }
            ]
        },
        {
            "@id": "agriculture:preservationEndDateTime",
            "@type": "rdf:Property",
            "schema:rangeIncludes": {
                "@id": "xsd:dateTime"
            },
            "schema:domainIncludes": {
                "@id": "agriculture:Sample"
            },
            "rdfs:comment": "The date, time, date time, or other date time value for the end of preservation for this agricultural sample.",
            "rdfs:label": "preservationEndDateTime",
            "unece:cefactElementMetadata": [
                {
                    "@id": "cefact:Agricultural_Sample.Preservation_End.DateTime",
                    "@type": "unece:BasicBIE",
                    "unece:cefactUNId": "UN01009599",
                    "unece:cefactBieDomainClass": "cefact:Agricultural_Sample.Details",
                    "rdfs:comment": "The date, time, date time, or other date time value for the end of preservation for this agricultural sample."
                }
            ]
        },
        {
            "@id": "agriculture:previousCropResidue",
            "@type": "rdf:Property",
            "schema:rangeIncludes": {
                "@id": "agriculture:CropResidue"
            },
            "schema:domainIncludes": {
                "@id": "agriculture:SoilOccupation"
            },
            "rdfs:comment": "A soil occupation crop residue from the previous plot soil occupation.",
            "rdfs:label": "previousCropResidue",
            "unece:cefactElementMetadata": [
                {
                    "@id": "cefact:Plot_SoilOccupation.Previous.SoilOccupation_CropResidue",
                    "@type": "unece:AssociationBIE",
                    "unece:cefactUNId": "UN01002755",
                    "unece:cefactBieDomainClass": "cefact:Plot_SoilOccupation.Details",
                    "rdfs:comment": "A soil occupation crop residue from the previous plot soil occupation."
                }
            ]
        },
        {
            "@id": "agriculture:previousId",
            "@type": "rdf:Property",
            "schema:rangeIncludes": {
                "@id": "xsd:token"
            },
            "schema:domainIncludes": {
                "@id": "agriculture:Plot"
            },
            "rdfs:comment": [
                "An identifier that previously (last) identified this agronomical observation plot.",
                "The unique identifier that previously identified (last) this agricultural plot, such as in a plot division."
            ],
            "rdfs:label": "previousId",
            "unece:cefactElementMetadata": [
                {
                    "@id": "cefact:Agricultural_Plot.Previous_Identification.Identifier",
                    "@type": "unece:BasicBIE",
                    "unece:cefactUNId": "UN01002653",
                    "unece:cefactBieDomainClass": "cefact:Agricultural_Plot.Details",
                    "rdfs:comment": "The unique identifier that previously identified (last) this agricultural plot, such as in a plot division."
                },
                {
                    "@id": "cefact:AgronomicalObservation_Plot.Previous_Identification.Identifier",
                    "@type": "unece:BasicBIE",
                    "unece:cefactUNId": "UN01009367",
                    "unece:cefactBieDomainClass": "cefact:AgronomicalObservation_Plot.Details",
                    "rdfs:comment": "An identifier that previously (last) identified this agronomical observation plot."
                }
            ]
        },
        {
            "@id": "agriculture:procedure",
            "@type": "rdf:Property",
            "schema:rangeIncludes": {
                "@id": "xsd:string"
            },
            "schema:domainIncludes": {
                "@id": "agriculture:Autopsy"
            },
            "rdfs:comment": "The procedure, expressed as text, for this agricultural sample autopsy.",
            "rdfs:label": "procedure",
            "unece:cefactElementMetadata": [
                {
                    "@id": "cefact:AgriculturalSample_Autopsy.Procedure.Text",
                    "@type": "unece:BasicBIE",
                    "unece:cefactUNId": "UN01009574",
                    "unece:cefactBieDomainClass": "cefact:AgriculturalSample_Autopsy.Details",
                    "rdfs:comment": "The procedure, expressed as text, for this agricultural sample autopsy."
                }
            ]
        },
        {
            "@id": "agriculture:processTypeCode",
            "@type": "rdf:Property",
            "schema:rangeIncludes": {
                "@id": "unece:UNECECL7187Code"
            },
            "schema:domainIncludes": {
                "@id": "agriculture:Process"
            },
            "rdfs:comment": "The code specifying the type of SPS process.",
            "rdfs:label": "processTypeCode",
            "unece:cefactElementMetadata": [
                {
                    "@id": "cefact:SPS_Process.Type.Code",
                    "@type": "unece:BasicBIE",
                    "unece:TDED": "7187",
                    "unece:cefactUNId": "UN03000127",
                    "unece:cefactBieDomainClass": "cefact:SPS_Process.Details",
                    "rdfs:comment": "The code specifying the type of SPS process."
                }
            ]
        },
        {
            "@id": "agriculture:producerParty",
            "@type": "rdf:Property",
            "schema:rangeIncludes": {
                "@id": "agriculture:Party"
            },
            "schema:domainIncludes": {
                "@id": "agriculture:SampledObject"
            },
            "rdfs:comment": "The party that produced this sampled agricultural object.",
            "rdfs:label": "producerParty",
            "unece:cefactElementMetadata": [
                {
                    "@id": "cefact:Agricultural_SampledObject.Producer.LaboratoryObservation_Party",
                    "@type": "unece:AssociationBIE",
                    "unece:cefactUNId": "UN01009628",
                    "unece:cefactBieDomainClass": "cefact:Agricultural_SampledObject.Details",
                    "rdfs:comment": "The party that produced this sampled agricultural object."
                }
            ]
        },
        {
            "@id": "agriculture:productName",
            "@type": "rdf:Property",
            "schema:rangeIncludes": {
                "@id": "xsd:string"
            },
            "schema:domainIncludes": {
                "@id": "agriculture:Batch"
            },
            "rdfs:comment": [
                "The product name, expressed as text, for this crop produce batch.",
                "The product name, expressed as text, for this product batch."
            ],
            "rdfs:label": "productName",
            "unece:cefactElementMetadata": [
                {
                    "@id": "cefact:Product_Batch.ProductName.Text",
                    "@type": "unece:BasicBIE",
                    "unece:cefactUNId": "UN01012349",
                    "unece:cefactBieDomainClass": "cefact:Product_Batch.Details",
                    "rdfs:comment": "The product name, expressed as text, for this product batch."
                },
                {
                    "@id": "cefact:CropProduce_Batch.ProductName.Text",
                    "@type": "unece:BasicBIE",
                    "unece:cefactUNId": "UN01012335",
                    "unece:cefactBieDomainClass": "cefact:CropProduce_Batch.Details",
                    "rdfs:comment": "The product name, expressed as text, for this crop produce batch."
                }
            ]
        },
        {
            "@id": "agriculture:productionBatchId",
            "@type": "rdf:Property",
            "schema:rangeIncludes": {
                "@id": "xsd:token"
            },
            "schema:domainIncludes": {
                "@id": "agriculture:TradeLineItem"
            },
            "rdfs:comment": "A unique identifier of the production batch of this SPS trade line item.",
            "rdfs:label": "productionBatchId",
            "unece:cefactElementMetadata": [
                {
                    "@id": "cefact:SPS_TradeLineItem.ProductionBatch.Identifier",
                    "@type": "unece:BasicBIE",
                    "unece:TDED": "7338",
                    "unece:cefactUNId": "UN03000151",
                    "unece:cefactBieDomainClass": "cefact:SPS_TradeLineItem.Details",
                    "rdfs:comment": "A unique identifier of the production batch of this SPS trade line item."
                }
            ]
        },
        {
            "@id": "agriculture:productionDateTime",
            "@type": "rdf:Property",
            "schema:rangeIncludes": {
                "@id": "xsd:dateTime"
            },
            "schema:domainIncludes": {
                "@id": "agriculture:SampledObject"
            },
            "rdfs:comment": "The date, time, date time, or other date time value when this sampled agricultural object was produced.",
            "rdfs:label": "productionDateTime",
            "unece:cefactElementMetadata": [
                {
                    "@id": "cefact:Agricultural_SampledObject.Production.DateTime",
                    "@type": "unece:BasicBIE",
                    "unece:cefactUNId": "UN01009615",
                    "unece:cefactBieDomainClass": "cefact:Agricultural_SampledObject.Details",
                    "rdfs:comment": "The date, time, date time, or other date time value when this sampled agricultural object was produced."
                }
            ]
        },
        {
            "@id": "agriculture:productionEnvironmentCode",
            "@type": "rdf:Property",
            "schema:rangeIncludes": {
                "@id": "xsd:token"
            },
            "schema:domainIncludes": {
                "@id": "agriculture:Crop"
            },
            "rdfs:comment": "The code specifying the production environment for this field crop.",
            "rdfs:label": "productionEnvironmentCode",
            "unece:cefactElementMetadata": [
                {
                    "@id": "cefact:Field_Crop.Production_Environment.Code",
                    "@type": "unece:BasicBIE",
                    "unece:cefactUNId": "UN01012310",
                    "unece:cefactBieDomainClass": "cefact:Field_Crop.Details",
                    "rdfs:comment": "The code specifying the production environment for this field crop."
                }
            ]
        },
        {
            "@id": "agriculture:productionModeCode",
            "@type": "rdf:Property",
            "schema:rangeIncludes": {
                "@id": "xsd:token"
            },
            "schema:domainIncludes": {
                "@id": "agriculture:Product"
            },
            "rdfs:comment": "The code specifying the production mode for this agricultural input product.",
            "rdfs:label": "productionModeCode",
            "unece:cefactElementMetadata": [
                {
                    "@id": "cefact:AgriculturalInput_Product.ProductionMode.Code",
                    "@type": "unece:BasicBIE",
                    "unece:cefactUNId": "UN01012381",
                    "unece:cefactBieDomainClass": "cefact:AgriculturalInput_Product.Details",
                    "rdfs:comment": "The code specifying the production mode for this agricultural input product."
                }
            ]
        },
        {
            "@id": "agriculture:productionPeriodCode",
            "@type": "rdf:Property",
            "schema:rangeIncludes": {
                "@id": "xsd:token"
            },
            "schema:domainIncludes": {
                "@id": "agriculture:Crop"
            },
            "rdfs:comment": "The code specifying the production period for this field crop.",
            "rdfs:label": "productionPeriodCode",
            "unece:cefactElementMetadata": [
                {
                    "@id": "cefact:Field_Crop.Production_Period.Code",
                    "@type": "unece:BasicBIE",
                    "unece:cefactUNId": "UN01012309",
                    "unece:cefactBieDomainClass": "cefact:Field_Crop.Details",
                    "rdfs:comment": "The code specifying the production period for this field crop."
                }
            ]
        },
        {
            "@id": "agriculture:productionWasteInstructions",
            "@type": "rdf:Property",
            "schema:rangeIncludes": {
                "@id": "agriculture:Instructions"
            },
            "schema:domainIncludes": {
                "@id": "agriculture:AgriculturalProcess"
            },
            "rdfs:comment": "Disposal instructions related to production waste for this agricultural crop production process.",
            "rdfs:label": "productionWasteInstructions",
            "unece:cefactElementMetadata": [
                {
                    "@id": "cefact:CropProduction_AgriculturalProcess.ProductionWaste.Disposal_Instructions",
                    "@type": "unece:AssociationBIE",
                    "unece:cefactUNId": "UN01013741",
                    "unece:cefactBieDomainClass": "cefact:CropProduction_AgriculturalProcess.Details",
                    "rdfs:comment": "Disposal instructions related to production waste for this agricultural crop production process."
                }
            ]
        },
        {
            "@id": "agriculture:productionYearDateTime",
            "@type": "rdf:Property",
            "schema:rangeIncludes": {
                "@id": "xsd:dateTime"
            },
            "schema:domainIncludes": {
                "@id": "agriculture:CropProductionCycle"
            },
            "rdfs:comment": "The date, specified as a year, of the crop production in this agricultural crop production cycle.",
            "rdfs:label": "productionYearDateTime",
            "unece:cefactElementMetadata": [
                {
                    "@id": "cefact:Agricultural_CropProductionCycle.Production_Year.DateTime",
                    "@type": "unece:BasicBIE",
                    "unece:cefactUNId": "UN01002766",
                    "unece:cefactBieDomainClass": "cefact:Agricultural_CropProductionCycle.Details",
                    "rdfs:comment": "The date, specified as a year, of the crop production in this agricultural crop production cycle."
                }
            ]
        },
        {
            "@id": "agriculture:propagationMaterialIndicator",
            "@type": "rdf:Property",
            "schema:rangeIncludes": {
                "@id": "xsd:boolean"
            },
            "schema:domainIncludes": {
                "@id": "agriculture:Crop"
            },
            "rdfs:comment": "The indication of whether or not a field crop is to be used as propagation material.",
            "rdfs:label": "propagationMaterialIndicator",
            "unece:cefactElementMetadata": [
                {
                    "@id": "cefact:Field_Crop.PropagationMaterial.Indicator",
                    "@type": "unece:BasicBIE",
                    "unece:cefactUNId": "UN01012303",
                    "unece:cefactBieDomainClass": "cefact:Field_Crop.Details",
                    "rdfs:comment": "The indication of whether or not a field crop is to be used as propagation material."
                }
            ]
        },
        {
            "@id": "agriculture:providerParty",
            "@type": "rdf:Property",
            "schema:rangeIncludes": {
                "@id": "agriculture:Party"
            },
            "schema:domainIncludes": {
                "@id": "agriculture:Authentication"
            },
            "rdfs:comment": "The SPS party providing this SPS authentication.",
            "rdfs:label": "providerParty",
            "unece:cefactElementMetadata": [
                {
                    "@id": "cefact:SPS_Authentication.Provider.SPS_Party",
                    "@type": "unece:AssociationBIE",
                    "unece:cefactUNId": "UN03000037",
                    "unece:cefactBieDomainClass": "cefact:SPS_Authentication.Details",
                    "rdfs:comment": "The SPS party providing this SPS authentication."
                }
            ]
        },
        {
            "@id": "agriculture:purposeCode",
            "@type": "rdf:Property",
            "schema:rangeIncludes": {
                "@id": "xsd:token"
            },
            "schema:domainIncludes": [
                {
                    "@id": "agriculture:Certificate"
                },
                {
                    "@id": "agriculture:Crop"
                }
            ],
            "rdfs:comment": [
                "A code specifying a purpose for this field crop.",
                "A code specifying the purpose of this agricultural certificate.",
                "The code specifying the purpose for this agricultural crop.",
                "The code specifying the purpose for this botanical crop."
            ],
            "rdfs:label": "purposeCode",
            "unece:cefactElementMetadata": [
                {
                    "@id": "cefact:Botanical_Crop.Purpose.Code",
                    "@type": "unece:BasicBIE",
                    "unece:cefactUNId": "UN01012292",
                    "unece:cefactBieDomainClass": "cefact:Botanical_Crop.Details",
                    "rdfs:comment": "The code specifying the purpose for this botanical crop."
                },
                {
                    "@id": "cefact:Field_Crop.Purpose.Code",
                    "@type": "unece:BasicBIE",
                    "unece:cefactUNId": "UN01012298",
                    "unece:cefactBieDomainClass": "cefact:Field_Crop.Details",
                    "rdfs:comment": "A code specifying a purpose for this field crop."
                },
                {
                    "@id": "cefact:Agricultural_Crop.Purpose.Code",
                    "@type": "unece:BasicBIE",
                    "unece:cefactUNId": "UN01002689",
                    "unece:cefactBieDomainClass": "cefact:Agricultural_Crop.Details",
                    "rdfs:comment": "The code specifying the purpose for this agricultural crop."
                },
                {
                    "@id": "cefact:Agricultural_Certificate.Purpose.Code",
                    "@type": "unece:BasicBIE",
                    "unece:cefactUNId": "UN01012288",
                    "unece:cefactBieDomainClass": "cefact:Agricultural_Certificate.Details",
                    "rdfs:comment": "A code specifying the purpose of this agricultural certificate."
                }
            ]
        },
        {
            "@id": "agriculture:reExportCountry",
            "@type": "rdf:Property",
            "schema:rangeIncludes": {
                "@id": "agriculture:Country"
            },
            "schema:domainIncludes": {
                "@id": "agriculture:Consignment"
            },
            "rdfs:comment": "A re-export country for this SPS consignment.",
            "rdfs:label": "reExportCountry",
            "unece:cefactElementMetadata": [
                {
                    "@id": "cefact:SPS_Consignment.Re-Export.SPS_Country",
                    "@type": "unece:AssociationBIE",
                    "unece:cefactUNId": "UN03000061",
                    "unece:cefactBieDomainClass": "cefact:SPS_Consignment.Details",
                    "rdfs:comment": "A re-export country for this SPS consignment."
                }
            ]
        },
        {
            "@id": "agriculture:receiptDateTime",
            "@type": "rdf:Property",
            "schema:rangeIncludes": {
                "@id": "xsd:dateTime"
            },
            "schema:domainIncludes": {
                "@id": "agriculture:Sample"
            },
            "rdfs:comment": "The date, time, date time, or other date time value for the receipt of this agricultural sample.",
            "rdfs:label": "receiptDateTime",
            "unece:cefactElementMetadata": [
                {
                    "@id": "cefact:Agricultural_Sample.Receipt.DateTime",
                    "@type": "unece:BasicBIE",
                    "unece:cefactUNId": "UN01009593",
                    "unece:cefactBieDomainClass": "cefact:Agricultural_Sample.Details",
                    "rdfs:comment": "The date, time, date time, or other date time value for the receipt of this agricultural sample."
                }
            ]
        },
        {
            "@id": "agriculture:receiverParty",
            "@type": "rdf:Property",
            "schema:rangeIncludes": {
                "@id": "agriculture:Party"
            },
            "schema:domainIncludes": {
                "@id": "agriculture:Grant"
            },
            "rdfs:comment": "The party that receives this animal grant.",
            "rdfs:label": "receiverParty",
            "unece:cefactElementMetadata": [
                {
                    "@id": "cefact:Animal_Grant.Receiver.Specified_Party",
                    "@type": "unece:AssociationBIE",
                    "unece:cefactUNId": "UN01007680",
                    "unece:cefactBieDomainClass": "cefact:Animal_Grant.Details",
                    "rdfs:comment": "The party that receives this animal grant."
                }
            ]
        },
        {
            "@id": "agriculture:recipientAssignedId",
            "@type": "rdf:Property",
            "schema:rangeIncludes": {
                "@id": "xsd:token"
            },
            "schema:domainIncludes": {
                "@id": "agriculture:Plot"
            },
            "rdfs:comment": "A recipient assigned identifier for this agronomical observation plot.",
            "rdfs:label": "recipientAssignedId",
            "unece:cefactElementMetadata": [
                {
                    "@id": "cefact:AgronomicalObservation_Plot.RecipientAssigned_Identification.Identifier",
                    "@type": "unece:BasicBIE",
                    "unece:cefactUNId": "UN01009372",
                    "unece:cefactBieDomainClass": "cefact:AgronomicalObservation_Plot.Details",
                    "rdfs:comment": "A recipient assigned identifier for this agronomical observation plot."
                }
            ]
        },
        {
            "@id": "agriculture:recipientInternalId",
            "@type": "rdf:Property",
            "schema:rangeIncludes": {
                "@id": "xsd:token"
            },
            "schema:domainIncludes": {
                "@id": "agriculture:Plot"
            },
            "rdfs:comment": "A recipient internal identifier for this agricultural plot.",
            "rdfs:label": "recipientInternalId",
            "unece:cefactElementMetadata": [
                {
                    "@id": "cefact:Agricultural_Plot.RecipientInternal_Identification.Identifier",
                    "@type": "unece:BasicBIE",
                    "unece:cefactUNId": "UN01009350",
                    "unece:cefactBieDomainClass": "cefact:Agricultural_Plot.Details",
                    "rdfs:comment": "A recipient internal identifier for this agricultural plot."
                }
            ]
        },
        {
            "@id": "agriculture:recipientParty",
            "@type": "rdf:Property",
            "schema:rangeIncludes": {
                "@id": "agriculture:Party"
            },
            "schema:domainIncludes": {
                "@id": "agriculture:Document"
            },
            "rdfs:comment": [
                "A party that receives this agronomical observation document.",
                "An SPS party that receives this exchanged SPS document.",
                "The crop data sheet party that receives this crop data sheet document.",
                "The party that receives this crop report document.",
                "The specified party that receives this LA exchanged document."
            ],
            "rdfs:label": "recipientParty",
            "unece:cefactElementMetadata": [
                {
                    "@id": "cefact:AgronomicalObservation_Document.Recipient.AgronomicalObservation_Party",
                    "@type": "unece:AssociationBIE",
                    "unece:cefactUNId": "UN01009299",
                    "unece:cefactBieDomainClass": "cefact:AgronomicalObservation_Document.Details",
                    "rdfs:comment": "A party that receives this agronomical observation document."
                },
                {
                    "@id": "cefact:CropDataSheet_Document.Recipient.CropDataSheet_Party",
                    "@type": "unece:AssociationBIE",
                    "unece:cefactUNId": "UN01002820",
                    "unece:cefactBieDomainClass": "cefact:CropDataSheet_Document.Details",
                    "rdfs:comment": "The crop data sheet party that receives this crop data sheet document."
                },
                {
                    "@id": "cefact:LAExchanged_Document.Recipient.Specified_Party",
                    "@type": "unece:AssociationBIE",
                    "unece:cefactUNId": "UN01007704",
                    "unece:cefactBieDomainClass": "cefact:LAExchanged_Document.Details",
                    "rdfs:comment": "The specified party that receives this LA exchanged document."
                },
                {
                    "@id": "cefact:CropReport_Document.Recipient.Specified_Party",
                    "@type": "unece:AssociationBIE",
                    "unece:cefactUNId": "UN01012443",
                    "unece:cefactBieDomainClass": "cefact:CropReport_Document.Details",
                    "rdfs:comment": "The party that receives this crop report document."
                },
                {
                    "@id": "cefact:SPSExchanged_Document.Recipient.SPS_Party",
                    "@type": "unece:AssociationBIE",
                    "unece:cefactUNId": "UN03000010",
                    "unece:cefactBieDomainClass": "cefact:SPSExchanged_Document.Details",
                    "rdfs:comment": "An SPS party that receives this exchanged SPS document."
                }
            ]
        },
        {
            "@id": "agriculture:referenceDocument",
            "@type": "rdf:Property",
            "schema:rangeIncludes": {
                "@id": "agriculture:Document"
            },
            "schema:domainIncludes": [
                {
                    "@id": "agriculture:Document"
                },
                {
                    "@id": "agriculture:TradeLineItem"
                }
            ],
            "rdfs:comment": [
                "An SPS document referenced by this SPS acknowledgement document.",
                "An SPS document referenced by this SPS trade line item.",
                "An SPS document referenced by this exchanged SPS document."
            ],
            "rdfs:label": "referenceDocument",
            "unece:cefactElementMetadata": [
                {
                    "@id": "cefact:SPSAcknowledgement_Document.Reference.SPSReferenced_Document",
                    "@type": "unece:AssociationBIE",
                    "unece:cefactUNId": "UN03000186",
                    "unece:cefactBieDomainClass": "cefact:SPSAcknowledgement_Document.Details",
                    "rdfs:comment": "An SPS document referenced by this SPS acknowledgement document."
                },
                {
                    "@id": "cefact:SPSExchanged_Document.Reference.SPSReferenced_Document",
                    "@type": "unece:AssociationBIE",
                    "unece:cefactUNId": "UN03000012",
                    "unece:cefactBieDomainClass": "cefact:SPSExchanged_Document.Details",
                    "rdfs:comment": "An SPS document referenced by this exchanged SPS document."
                },
                {
                    "@id": "cefact:SPS_TradeLineItem.Reference.SPSReferenced_Document",
                    "@type": "unece:AssociationBIE",
                    "unece:cefactUNId": "UN03000187",
                    "unece:cefactBieDomainClass": "cefact:SPS_TradeLineItem.Details",
                    "rdfs:comment": "An SPS document referenced by this SPS trade line item."
                }
            ]
        },
        {
            "@id": "agriculture:referenceRelationshipTypeCode",
            "@type": "rdf:Property",
            "schema:rangeIncludes": {
                "@id": "unece:UNECECL1153Code"
            },
            "schema:domainIncludes": {
                "@id": "agriculture:Document"
            },
            "rdfs:comment": "The code specifying the type of relationship between this referenced SPS document and another artefact, such as a replacement of an original document.",
            "rdfs:label": "referenceRelationshipTypeCode",
            "unece:cefactElementMetadata": [
                {
                    "@id": "cefact:SPSReferenced_Document.RelationshipType.Code",
                    "@type": "unece:BasicBIE",
                    "unece:TDED": "1153",
                    "unece:cefactUNId": "UN03000017",
                    "unece:cefactBieDomainClass": "cefact:SPSReferenced_Document.Details",
                    "rdfs:comment": "The code specifying the type of relationship between this referenced SPS document and another artefact, such as a replacement of an original document."
                }
            ]
        },
        {
            "@id": "agriculture:referencedLocationReferenceTypeCode",
            "@type": "rdf:Property",
            "schema:rangeIncludes": {
                "@id": "unece:UNECECL3227Code"
            },
            "schema:domainIncludes": {
                "@id": "agriculture:Location"
            },
            "rdfs:comment": "The code specifying the reference type of this referenced location.",
            "rdfs:label": "referencedLocationReferenceTypeCode",
            "unece:cefactElementMetadata": [
                {
                    "@id": "cefact:Referenced_Location.Reference_Type.Code",
                    "@type": "unece:BasicBIE",
                    "unece:TDED": "3227",
                    "unece:cefactUNId": "UN01012158",
                    "unece:cefactBieDomainClass": "cefact:Referenced_Location.Details",
                    "rdfs:comment": "The code specifying the reference type of this referenced location."
                }
            ]
        },
        {
            "@id": "agriculture:registeredBirthLocationId",
            "@type": "rdf:Property",
            "schema:rangeIncludes": {
                "@id": "xsd:token"
            },
            "schema:domainIncludes": {
                "@id": "agriculture:Animal"
            },
            "rdfs:comment": "The identifier of the registered location of the birth of this livestock animal.",
            "rdfs:label": "registeredBirthLocationId",
            "unece:cefactElementMetadata": [
                {
                    "@id": "cefact:Livestock_Animal.RegisteredBirth_Location.Identifier",
                    "@type": "unece:BasicBIE",
                    "unece:cefactUNId": "UN01007648",
                    "unece:cefactBieDomainClass": "cefact:Livestock_Animal.Details",
                    "rdfs:comment": "The identifier of the registered location of the birth of this livestock animal."
                }
            ]
        },
        {
            "@id": "agriculture:regulatoryOrganicIndicator",
            "@type": "rdf:Property",
            "schema:rangeIncludes": {
                "@id": "xsd:boolean"
            },
            "schema:domainIncludes": {
                "@id": "agriculture:Plot"
            },
            "rdfs:comment": "The indication of whether or not this crop plot is certified as regulatory organic.",
            "rdfs:label": "regulatoryOrganicIndicator",
            "unece:cefactElementMetadata": [
                {
                    "@id": "cefact:Crop_Plot.Regulatory_Organic.Indicator",
                    "@type": "unece:BasicBIE",
                    "unece:cefactUNId": "UN01012144",
                    "unece:cefactBieDomainClass": "cefact:Crop_Plot.Details",
                    "rdfs:comment": "The indication of whether or not this crop plot is certified as regulatory organic."
                }
            ]
        },
        {
            "@id": "agriculture:regulatorySoilTypeCode",
            "@type": "rdf:Property",
            "schema:rangeIncludes": {
                "@id": "xsd:token"
            },
            "schema:domainIncludes": {
                "@id": "agriculture:Plot"
            },
            "rdfs:comment": "The code specifying the type of regulatory soil for this crop plot.",
            "rdfs:label": "regulatorySoilTypeCode",
            "unece:cefactElementMetadata": [
                {
                    "@id": "cefact:Crop_Plot.Regulatory_SoilType.Code",
                    "@type": "unece:BasicBIE",
                    "unece:cefactUNId": "UN01012143",
                    "unece:cefactBieDomainClass": "cefact:Crop_Plot.Details",
                    "rdfs:comment": "The code specifying the type of regulatory soil for this crop plot."
                }
            ]
        },
        {
            "@id": "agriculture:relatedCharacteristic",
            "@type": "rdf:Property",
            "schema:rangeIncludes": {
                "@id": "agriculture:Characteristic"
            },
            "schema:domainIncludes": {
                "@id": "agriculture:Event"
            },
            "rdfs:comment": "A technical characteristic related to this animal holding event.",
            "rdfs:label": "relatedCharacteristic",
            "unece:cefactElementMetadata": [
                {
                    "@id": "cefact:AnimalHolding_Event.Related.Technical_Characteristic",
                    "@type": "unece:AssociationBIE",
                    "unece:cefactUNId": "UN01011243",
                    "unece:cefactBieDomainClass": "cefact:AnimalHolding_Event.Details",
                    "rdfs:comment": "A technical characteristic related to this animal holding event."
                }
            ]
        },
        {
            "@id": "agriculture:relatedConsignment",
            "@type": "rdf:Property",
            "schema:rangeIncludes": {
                "@id": "agriculture:Consignment"
            },
            "schema:domainIncludes": {
                "@id": "agriculture:TradeDelivery"
            },
            "rdfs:comment": "A Track and Trace (TT) consignment related to this animal trade delivery.",
            "rdfs:label": "relatedConsignment",
            "unece:cefactElementMetadata": [
                {
                    "@id": "cefact:Animal_TradeDelivery.Related.TT_Consignment",
                    "@type": "unece:AssociationBIE",
                    "unece:cefactUNId": "UN01011265",
                    "unece:cefactBieDomainClass": "cefact:Animal_TradeDelivery.Details",
                    "rdfs:comment": "A Track and Trace (TT) consignment related to this animal trade delivery."
                }
            ]
        },
        {
            "@id": "agriculture:relatedLocation",
            "@type": "rdf:Property",
            "schema:rangeIncludes": {
                "@id": "agriculture:Location"
            },
            "schema:domainIncludes": [
                {
                    "@id": "agriculture:Certification"
                },
                {
                    "@id": "agriculture:Event"
                }
            ],
            "rdfs:comment": [
                "A Track and Trace (TT) location related to this animal holding event.",
                "A referenced location related to this animal certification."
            ],
            "rdfs:label": "relatedLocation",
            "unece:cefactElementMetadata": [
                {
                    "@id": "cefact:AnimalHolding_Event.Related.TT_Location",
                    "@type": "unece:AssociationBIE",
                    "unece:cefactUNId": "UN01011242",
                    "unece:cefactBieDomainClass": "cefact:AnimalHolding_Event.Details",
                    "rdfs:comment": "A Track and Trace (TT) location related to this animal holding event."
                },
                {
                    "@id": "cefact:Animal_Certification.Related.Referenced_Location",
                    "@type": "unece:AssociationBIE",
                    "unece:cefactUNId": "UN01013726",
                    "unece:cefactBieDomainClass": "cefact:Animal_Certification.Details",
                    "rdfs:comment": "A referenced location related to this animal certification."
                }
            ]
        },
        {
            "@id": "agriculture:relatedParty",
            "@type": "rdf:Property",
            "schema:rangeIncludes": {
                "@id": "agriculture:Party"
            },
            "schema:domainIncludes": {
                "@id": "agriculture:ProductionUnit"
            },
            "rdfs:comment": [
                "A party related to this agricultural production unit.",
                "An agricultural producer party related to this agricultural production unit."
            ],
            "rdfs:label": "relatedParty",
            "unece:cefactElementMetadata": [
                {
                    "@id": "cefact:Agricultural_ProductionUnit.Related.Specified_Party",
                    "@type": "unece:AssociationBIE",
                    "unece:cefactUNId": "UN01012256",
                    "unece:cefactBieDomainClass": "cefact:Agricultural_ProductionUnit.Details",
                    "rdfs:comment": "A party related to this agricultural production unit."
                },
                {
                    "@id": "cefact:Agricultural_ProductionUnit.Related.AgriculturalProducer_Party",
                    "@type": "unece:AssociationBIE",
                    "unece:cefactUNId": "UN01012257",
                    "unece:cefactBieDomainClass": "cefact:Agricultural_ProductionUnit.Details",
                    "rdfs:comment": "An agricultural producer party related to this agricultural production unit."
                }
            ]
        },
        {
            "@id": "agriculture:renovationDateTime",
            "@type": "rdf:Property",
            "schema:rangeIncludes": {
                "@id": "xsd:dateTime"
            },
            "schema:domainIncludes": {
                "@id": "agriculture:Construction"
            },
            "rdfs:comment": "A date of a renovation of this agricultural construction.",
            "rdfs:label": "renovationDateTime",
            "unece:cefactElementMetadata": [
                {
                    "@id": "cefact:Agricultural_Construction.Renovation.DateTime",
                    "@type": "unece:BasicBIE",
                    "unece:cefactUNId": "UN01012236",
                    "unece:cefactBieDomainClass": "cefact:Agricultural_Construction.Details",
                    "rdfs:comment": "A date of a renovation of this agricultural construction."
                }
            ]
        },
        {
            "@id": "agriculture:reportCountNumeric",
            "@type": "rdf:Property",
            "schema:rangeIncludes": {
                "@id": "xsd:decimal"
            },
            "schema:domainIncludes": {
                "@id": "agriculture:Document"
            },
            "rdfs:comment": "The number of reports in this crop report document.",
            "rdfs:label": "reportCountNumeric",
            "unece:cefactElementMetadata": [
                {
                    "@id": "cefact:CropReport_Document.ReportCount.Numeric",
                    "@type": "unece:BasicBIE",
                    "unece:cefactUNId": "UN01012431",
                    "unece:cefactBieDomainClass": "cefact:CropReport_Document.Details",
                    "rdfs:comment": "The number of reports in this crop report document."
                }
            ]
        },
        {
            "@id": "agriculture:reportedMaterial",
            "@type": "rdf:Property",
            "schema:rangeIncludes": {
                "@id": "agriculture:Material"
            },
            "schema:domainIncludes": {
                "@id": "agriculture:AgriculturalProcess"
            },
            "rdfs:comment": "Production waste material reported for this agricultural crop production process.",
            "rdfs:label": "reportedMaterial",
            "unece:cefactElementMetadata": [
                {
                    "@id": "cefact:CropProduction_AgriculturalProcess.Reported.ProductionWaste_Material",
                    "@type": "unece:AssociationBIE",
                    "unece:cefactUNId": "UN01013742",
                    "unece:cefactBieDomainClass": "cefact:CropProduction_AgriculturalProcess.Details",
                    "rdfs:comment": "Production waste material reported for this agricultural crop production process."
                }
            ]
        },
        {
            "@id": "agriculture:requestedEffectiveDateTime",
            "@type": "rdf:Property",
            "schema:rangeIncludes": {
                "@id": "xsd:dateTime"
            },
            "schema:domainIncludes": {
                "@id": "agriculture:Certificate"
            },
            "rdfs:comment": "The requested effective date, time, date time or other date time value for this agricultural certificate.",
            "rdfs:label": "requestedEffectiveDateTime",
            "unece:cefactElementMetadata": [
                {
                    "@id": "cefact:Agricultural_Certificate.RequestedEffective.DateTime",
                    "@type": "unece:BasicBIE",
                    "unece:cefactUNId": "UN01012283",
                    "unece:cefactBieDomainClass": "cefact:Agricultural_Certificate.Details",
                    "rdfs:comment": "The requested effective date, time, date time or other date time value for this agricultural certificate."
                }
            ]
        },
        {
            "@id": "agriculture:responsibleAgency",
            "@type": "rdf:Property",
            "schema:rangeIncludes": {
                "@id": "xsd:string"
            },
            "schema:domainIncludes": {
                "@id": "agriculture:Certification"
            },
            "rdfs:comment": "An agency, expressed as text, responsible for this animal certification.",
            "rdfs:label": "responsibleAgency",
            "unece:cefactElementMetadata": [
                {
                    "@id": "cefact:Animal_Certification.ResponsibleAgency.Text",
                    "@type": "unece:BasicBIE",
                    "unece:cefactUNId": "UN01013724",
                    "unece:cefactBieDomainClass": "cefact:Animal_Certification.Details",
                    "rdfs:comment": "An agency, expressed as text, responsible for this animal certification."
                }
            ]
        },
        {
            "@id": "agriculture:responsibleParty",
            "@type": "rdf:Property",
            "schema:rangeIncludes": {
                "@id": "agriculture:Party"
            },
            "schema:domainIncludes": {
                "@id": "agriculture:TradeDelivery"
            },
            "rdfs:comment": "The Track and Trace (TT) party responsible for this animal trade delivery.",
            "rdfs:label": "responsibleParty",
            "unece:cefactElementMetadata": [
                {
                    "@id": "cefact:Animal_TradeDelivery.Responsible.TT_Party",
                    "@type": "unece:AssociationBIE",
                    "unece:cefactUNId": "UN01011263",
                    "unece:cefactBieDomainClass": "cefact:Animal_TradeDelivery.Details",
                    "rdfs:comment": "The Track and Trace (TT) party responsible for this animal trade delivery."
                }
            ]
        },
        {
            "@id": "agriculture:restriction",
            "@type": "rdf:Property",
            "schema:rangeIncludes": {
                "@id": "xsd:string"
            },
            "schema:domainIncludes": {
                "@id": "agriculture:ProtectionMeans"
            },
            "rdfs:comment": "A restriction, expressed as text, for this disease protection means.",
            "rdfs:label": "restriction",
            "unece:cefactElementMetadata": [
                {
                    "@id": "cefact:Disease_ProtectionMeans.Restriction.Text",
                    "@type": "unece:BasicBIE",
                    "unece:cefactUNId": "UN01015112",
                    "unece:cefactBieDomainClass": "cefact:Disease_ProtectionMeans.Details",
                    "rdfs:comment": "A restriction, expressed as text, for this disease protection means."
                }
            ]
        },
        {
            "@id": "agriculture:resultDocument",
            "@type": "rdf:Property",
            "schema:rangeIncludes": {
                "@id": "agriculture:Document"
            },
            "schema:domainIncludes": {
                "@id": "agriculture:Analysis"
            },
            "rdfs:comment": "The referenced analysis result document for this agricultural analysis.",
            "rdfs:label": "resultDocument",
            "unece:cefactElementMetadata": [
                {
                    "@id": "cefact:Agricultural_Analysis.Result.Analysis_Referenced_Document",
                    "@type": "unece:AssociationBIE",
                    "unece:cefactUNId": "UN01002666",
                    "unece:cefactBieDomainClass": "cefact:Agricultural_Analysis.Details",
                    "rdfs:comment": "The referenced analysis result document for this agricultural analysis."
                }
            ]
        },
        {
            "@id": "agriculture:sPSAcknowledgementDocumentReasonInformation",
            "@type": "rdf:Property",
            "schema:rangeIncludes": {
                "@id": "unece:UNECECL9013Code"
            },
            "schema:domainIncludes": {
                "@id": "agriculture:Document"
            },
            "rdfs:comment": "Reason information, expressed as text, for this SPS acknowledgement document.",
            "rdfs:label": "sPSAcknowledgementDocumentReasonInformation",
            "unece:cefactElementMetadata": [
                {
                    "@id": "cefact:SPSAcknowledgement_Document.Reason_Information.Text",
                    "@type": "unece:BasicBIE",
                    "unece:TDED": "9013",
                    "unece:cefactUNId": "UN03000183",
                    "unece:cefactBieDomainClass": "cefact:SPSAcknowledgement_Document.Details",
                    "rdfs:comment": "Reason information, expressed as text, for this SPS acknowledgement document."
                }
            ]
        },
        {
            "@id": "agriculture:sPSAcknowledgementDocumentStatusCode",
            "@type": "rdf:Property",
            "schema:rangeIncludes": {
                "@id": "unece:UNECECL4405Code"
            },
            "schema:domainIncludes": {
                "@id": "agriculture:Document"
            },
            "rdfs:comment": "The code specifying the status of this SPS acknowledgement document.",
            "rdfs:label": "sPSAcknowledgementDocumentStatusCode",
            "unece:cefactElementMetadata": [
                {
                    "@id": "cefact:SPSAcknowledgement_Document.Status.Code",
                    "@type": "unece:BasicBIE",
                    "unece:TDED": "4405",
                    "unece:cefactUNId": "UN03000185",
                    "unece:cefactBieDomainClass": "cefact:SPSAcknowledgement_Document.Details",
                    "rdfs:comment": "The code specifying the status of this SPS acknowledgement document."
                }
            ]
        },
        {
            "@id": "agriculture:sPSConsignmentShipStoresIndicator",
            "@type": "rdf:Property",
            "schema:rangeIncludes": {
                "@id": "unece:UNECECL7365Code"
            },
            "schema:domainIncludes": {
                "@id": "agriculture:Consignment"
            },
            "rdfs:comment": "The indication of whether or not this SPS consignment is for ship stores, such as for consumption on the means of transport.",
            "rdfs:label": "sPSConsignmentShipStoresIndicator",
            "unece:cefactElementMetadata": [
                {
                    "@id": "cefact:SPS_Consignment.ShipStores.Indicator",
                    "@type": "unece:BasicBIE",
                    "unece:TDED": "7365",
                    "unece:cefactUNId": "UN03000057",
                    "unece:cefactBieDomainClass": "cefact:SPS_Consignment.Details",
                    "rdfs:comment": "The indication of whether or not this SPS consignment is for ship stores, such as for consumption on the means of transport."
                }
            ]
        },
        {
            "@id": "agriculture:sPSExchangedDocumentStatusCode",
            "@type": "rdf:Property",
            "schema:rangeIncludes": {
                "@id": "unece:UNECECL4405Code"
            },
            "schema:domainIncludes": {
                "@id": "agriculture:Document"
            },
            "rdfs:comment": "The code specifying the status of this exchanged SPS document.",
            "rdfs:label": "sPSExchangedDocumentStatusCode",
            "unece:cefactElementMetadata": [
                {
                    "@id": "cefact:SPSExchanged_Document.Status.Code",
                    "@type": "unece:BasicBIE",
                    "unece:TDED": "4405",
                    "unece:cefactUNId": "UN03000006",
                    "unece:cefactBieDomainClass": "cefact:SPSExchanged_Document.Details",
                    "rdfs:comment": "The code specifying the status of this exchanged SPS document."
                }
            ]
        },
        {
            "@id": "agriculture:sPSPackageLevelCode",
            "@type": "rdf:Property",
            "schema:rangeIncludes": {
                "@id": "unece:UNECECL7075Code"
            },
            "schema:domainIncludes": {
                "@id": "agriculture:Package"
            },
            "rdfs:comment": "The code specifying the level of this SPS package.",
            "rdfs:label": "sPSPackageLevelCode",
            "unece:cefactElementMetadata": [
                {
                    "@id": "cefact:SPS_Package.Level.Code",
                    "@type": "unece:BasicBIE",
                    "unece:TDED": "7075",
                    "unece:cefactUNId": "UN03000105",
                    "unece:cefactBieDomainClass": "cefact:SPS_Package.Details",
                    "rdfs:comment": "The code specifying the level of this SPS package."
                }
            ]
        },
        {
            "@id": "agriculture:saleDateTime",
            "@type": "rdf:Property",
            "schema:rangeIncludes": {
                "@id": "xsd:dateTime"
            },
            "schema:domainIncludes": {
                "@id": "agriculture:Batch"
            },
            "rdfs:comment": "The date, time, date time, or other date time value of the sale for this animal batch.",
            "rdfs:label": "saleDateTime",
            "unece:cefactElementMetadata": [
                {
                    "@id": "cefact:Animal_Batch.Sale.DateTime",
                    "@type": "unece:BasicBIE",
                    "unece:cefactUNId": "UN01011248",
                    "unece:cefactBieDomainClass": "cefact:Animal_Batch.Details",
                    "rdfs:comment": "The date, time, date time, or other date time value of the sale for this animal batch."
                }
            ]
        },
        {
            "@id": "agriculture:salesNoteId",
            "@type": "rdf:Property",
            "schema:rangeIncludes": {
                "@id": "xsd:token"
            },
            "schema:domainIncludes": {
                "@id": "agriculture:Batch"
            },
            "rdfs:comment": "The identifier for the sales note for this animal batch.",
            "rdfs:label": "salesNoteId",
            "unece:cefactElementMetadata": [
                {
                    "@id": "cefact:Animal_Batch.SalesNote.Identifier",
                    "@type": "unece:BasicBIE",
                    "unece:cefactUNId": "UN01011249",
                    "unece:cefactBieDomainClass": "cefact:Animal_Batch.Details",
                    "rdfs:comment": "The identifier for the sales note for this animal batch."
                }
            ]
        },
        {
            "@id": "agriculture:sampleId",
            "@type": "rdf:Property",
            "schema:rangeIncludes": {
                "@id": "xsd:token"
            },
            "schema:domainIncludes": {
                "@id": "agriculture:ObservationResult"
            },
            "rdfs:comment": "An identifier of the sample observation result for this referenced observation result.",
            "rdfs:label": "sampleId",
            "unece:cefactElementMetadata": [
                {
                    "@id": "cefact:Referenced_ObservationResult.Sample_Identification.Identifier",
                    "@type": "unece:BasicBIE",
                    "unece:cefactUNId": "UN01012456",
                    "unece:cefactBieDomainClass": "cefact:Referenced_ObservationResult.Details",
                    "rdfs:comment": "An identifier of the sample observation result for this referenced observation result."
                }
            ]
        },
        {
            "@id": "agriculture:samplerAssignedId",
            "@type": "rdf:Property",
            "schema:rangeIncludes": {
                "@id": "xsd:token"
            },
            "schema:domainIncludes": {
                "@id": "agriculture:Sample"
            },
            "rdfs:comment": "The identifier of this agricultural sample as assigned by the sampler.",
            "rdfs:label": "samplerAssignedId",
            "unece:cefactElementMetadata": [
                {
                    "@id": "cefact:Agricultural_Sample.SamplerAssigned_Identification.Identifier",
                    "@type": "unece:BasicBIE",
                    "unece:cefactUNId": "UN01012465",
                    "unece:cefactBieDomainClass": "cefact:Agricultural_Sample.Details",
                    "rdfs:comment": "The identifier of this agricultural sample as assigned by the sampler."
                }
            ]
        },
        {
            "@id": "agriculture:samplingDateTime",
            "@type": "rdf:Property",
            "schema:rangeIncludes": {
                "@id": "xsd:dateTime"
            },
            "schema:domainIncludes": [
                {
                    "@id": "agriculture:Analysis"
                },
                {
                    "@id": "agriculture:Sample"
                }
            ],
            "rdfs:comment": [
                "The date or date time value of a sampling for this agricultural analysis.",
                "The date, time, date time, or other date time value for the sampling of this agricultural sample."
            ],
            "rdfs:label": "samplingDateTime",
            "unece:cefactElementMetadata": [
                {
                    "@id": "cefact:Agricultural_Sample.Sampling.DateTime",
                    "@type": "unece:BasicBIE",
                    "unece:cefactUNId": "UN01009588",
                    "unece:cefactBieDomainClass": "cefact:Agricultural_Sample.Details",
                    "rdfs:comment": "The date, time, date time, or other date time value for the sampling of this agricultural sample."
                },
                {
                    "@id": "cefact:Agricultural_Analysis.Sampling.DateTime",
                    "@type": "unece:BasicBIE",
                    "unece:cefactUNId": "UN01002665",
                    "unece:cefactBieDomainClass": "cefact:Agricultural_Analysis.Details",
                    "rdfs:comment": "The date or date time value of a sampling for this agricultural analysis."
                }
            ]
        },
        {
            "@id": "agriculture:samplingLocation",
            "@type": "rdf:Property",
            "schema:rangeIncludes": {
                "@id": "agriculture:Location"
            },
            "schema:domainIncludes": {
                "@id": "agriculture:Sample"
            },
            "rdfs:comment": "A referenced location for the sampling of this agricultural sample.",
            "rdfs:label": "samplingLocation",
            "unece:cefactElementMetadata": [
                {
                    "@id": "cefact:Agricultural_Sample.Sampling.Referenced_Location",
                    "@type": "unece:AssociationBIE",
                    "unece:cefactUNId": "UN01009601",
                    "unece:cefactBieDomainClass": "cefact:Agricultural_Sample.Details",
                    "rdfs:comment": "A referenced location for the sampling of this agricultural sample."
                }
            ]
        },
        {
            "@id": "agriculture:samplingParty",
            "@type": "rdf:Property",
            "schema:rangeIncludes": {
                "@id": "agriculture:Party"
            },
            "schema:domainIncludes": {
                "@id": "agriculture:Sample"
            },
            "rdfs:comment": "The laboratory observation party sampling this agricultural sample.",
            "rdfs:label": "samplingParty",
            "unece:cefactElementMetadata": [
                {
                    "@id": "cefact:Agricultural_Sample.Sampling.LaboratoryObservation_Party",
                    "@type": "unece:AssociationBIE",
                    "unece:cefactUNId": "UN01009602",
                    "unece:cefactBieDomainClass": "cefact:Agricultural_Sample.Details",
                    "rdfs:comment": "The laboratory observation party sampling this agricultural sample."
                }
            ]
        },
        {
            "@id": "agriculture:samplingProcedureId",
            "@type": "rdf:Property",
            "schema:rangeIncludes": {
                "@id": "xsd:token"
            },
            "schema:domainIncludes": {
                "@id": "agriculture:SampledObject"
            },
            "rdfs:comment": "The identifier of the sampling procedure used for this sampled agricultural object.",
            "rdfs:label": "samplingProcedureId",
            "unece:cefactElementMetadata": [
                {
                    "@id": "cefact:Agricultural_SampledObject.SamplingProcedure.Identifier",
                    "@type": "unece:BasicBIE",
                    "unece:cefactUNId": "UN01009617",
                    "unece:cefactBieDomainClass": "cefact:Agricultural_SampledObject.Details",
                    "rdfs:comment": "The identifier of the sampling procedure used for this sampled agricultural object."
                }
            ]
        },
        {
            "@id": "agriculture:samplingProcedureTypeCode",
            "@type": "rdf:Property",
            "schema:rangeIncludes": {
                "@id": "xsd:token"
            },
            "schema:domainIncludes": {
                "@id": "agriculture:SampledObject"
            },
            "rdfs:comment": "The code specifying the type of sampling procedure used for this sampled agricultural object.",
            "rdfs:label": "samplingProcedureTypeCode",
            "unece:cefactElementMetadata": [
                {
                    "@id": "cefact:Agricultural_SampledObject.SamplingProcedureType.Code",
                    "@type": "unece:BasicBIE",
                    "unece:cefactUNId": "UN01009616",
                    "unece:cefactBieDomainClass": "cefact:Agricultural_SampledObject.Details",
                    "rdfs:comment": "The code specifying the type of sampling procedure used for this sampled agricultural object."
                }
            ]
        },
        {
            "@id": "agriculture:scientificName",
            "@type": "rdf:Property",
            "schema:rangeIncludes": {
                "@id": "xsd:string"
            },
            "schema:domainIncludes": {
                "@id": "agriculture:TradeLineItem"
            },
            "rdfs:comment": "A scientific name, expressed as text, of this SPS trade line item.",
            "rdfs:label": "scientificName",
            "unece:cefactElementMetadata": [
                {
                    "@id": "cefact:SPS_TradeLineItem.Scientific_Name.Text",
                    "@type": "unece:BasicBIE",
                    "unece:TDED": "7036",
                    "unece:cefactUNId": "UN03000150",
                    "unece:cefactBieDomainClass": "cefact:SPS_TradeLineItem.Details",
                    "rdfs:comment": "A scientific name, expressed as text, of this SPS trade line item."
                }
            ]
        },
        {
            "@id": "agriculture:scientificSpeciesName",
            "@type": "rdf:Property",
            "schema:rangeIncludes": {
                "@id": "xsd:string"
            },
            "schema:domainIncludes": {
                "@id": "agriculture:Product"
            },
            "rdfs:comment": "The scientific species name, expressed as text, for this livestock animal product.",
            "rdfs:label": "scientificSpeciesName",
            "unece:cefactElementMetadata": [
                {
                    "@id": "cefact:LivestockAnimal_Product.ScientificSpecies_Name.Text",
                    "@type": "unece:BasicBIE",
                    "unece:TDED": "7134",
                    "unece:cefactUNId": "UN01007707",
                    "unece:cefactBieDomainClass": "cefact:LivestockAnimal_Product.Details",
                    "rdfs:comment": "The scientific species name, expressed as text, for this livestock animal product."
                }
            ]
        },
        {
            "@id": "agriculture:sealedDateTime",
            "@type": "rdf:Property",
            "schema:rangeIncludes": {
                "@id": "xsd:dateTime"
            },
            "schema:domainIncludes": {
                "@id": "agriculture:Sample"
            },
            "rdfs:comment": "The date, time, date time, or other date time value for the sealing of this agricultural sample.",
            "rdfs:label": "sealedDateTime",
            "unece:cefactElementMetadata": [
                {
                    "@id": "cefact:Agricultural_Sample.Sealed.DateTime",
                    "@type": "unece:BasicBIE",
                    "unece:cefactUNId": "UN01009590",
                    "unece:cefactBieDomainClass": "cefact:Agricultural_Sample.Details",
                    "rdfs:comment": "The date, time, date time, or other date time value for the sealing of this agricultural sample."
                }
            ]
        },
        {
            "@id": "agriculture:sealedIndicator",
            "@type": "rdf:Property",
            "schema:rangeIncludes": {
                "@id": "xsd:boolean"
            },
            "schema:domainIncludes": {
                "@id": "agriculture:Sample"
            },
            "rdfs:comment": "The indication of whether or not this agricultural sampled is sealed.",
            "rdfs:label": "sealedIndicator",
            "unece:cefactElementMetadata": [
                {
                    "@id": "cefact:Agricultural_Sample.Sealed.Indicator",
                    "@type": "unece:BasicBIE",
                    "unece:cefactUNId": "UN01009589",
                    "unece:cefactBieDomainClass": "cefact:Agricultural_Sample.Details",
                    "rdfs:comment": "The indication of whether or not this agricultural sampled is sealed."
                }
            ]
        },
        {
            "@id": "agriculture:sellerParty",
            "@type": "rdf:Property",
            "schema:rangeIncludes": {
                "@id": "agriculture:Party"
            },
            "schema:domainIncludes": {
                "@id": "agriculture:Contract"
            },
            "rdfs:comment": "The seller party for this agricultural contract.",
            "rdfs:label": "sellerParty",
            "unece:cefactElementMetadata": [
                {
                    "@id": "cefact:Agricultural_Contract.Seller.Specified_Party",
                    "@type": "unece:AssociationBIE",
                    "unece:cefactUNId": "UN01012449",
                    "unece:cefactBieDomainClass": "cefact:Agricultural_Contract.Details",
                    "rdfs:comment": "The seller party for this agricultural contract."
                }
            ]
        },
        {
            "@id": "agriculture:senderAssignedId",
            "@type": "rdf:Property",
            "schema:rangeIncludes": {
                "@id": "xsd:token"
            },
            "schema:domainIncludes": {
                "@id": "agriculture:Sample"
            },
            "rdfs:comment": "The identifier of this agricultural sample, assigned by the sender of the sample.",
            "rdfs:label": "senderAssignedId",
            "unece:cefactElementMetadata": [
                {
                    "@id": "cefact:Agricultural_Sample.SenderAssigned_Identification.Identifier",
                    "@type": "unece:BasicBIE",
                    "unece:cefactUNId": "UN01009592",
                    "unece:cefactBieDomainClass": "cefact:Agricultural_Sample.Details",
                    "rdfs:comment": "The identifier of this agricultural sample, assigned by the sender of the sample."
                }
            ]
        },
        {
            "@id": "agriculture:senderParty",
            "@type": "rdf:Property",
            "schema:rangeIncludes": {
                "@id": "agriculture:Party"
            },
            "schema:domainIncludes": [
                {
                    "@id": "agriculture:Document"
                },
                {
                    "@id": "agriculture:Sample"
                }
            ],
            "rdfs:comment": [
                "The laboratory observation party that sends this agricultural sample.",
                "The party that sends this crop report document.",
                "The specified party that sends this LA exchanged document."
            ],
            "rdfs:label": "senderParty",
            "unece:cefactElementMetadata": [
                {
                    "@id": "cefact:Agricultural_Sample.Sender.LaboratoryObservation_Party",
                    "@type": "unece:AssociationBIE",
                    "unece:cefactUNId": "UN01012468",
                    "unece:cefactBieDomainClass": "cefact:Agricultural_Sample.Details",
                    "rdfs:comment": "The laboratory observation party that sends this agricultural sample."
                },
                {
                    "@id": "cefact:LAExchanged_Document.Sender.Specified_Party",
                    "@type": "unece:AssociationBIE",
                    "unece:cefactUNId": "UN01007703",
                    "unece:cefactBieDomainClass": "cefact:LAExchanged_Document.Details",
                    "rdfs:comment": "The specified party that sends this LA exchanged document."
                },
                {
                    "@id": "cefact:CropReport_Document.Sender.Specified_Party",
                    "@type": "unece:AssociationBIE",
                    "unece:cefactUNId": "UN01012442",
                    "unece:cefactBieDomainClass": "cefact:CropReport_Document.Details",
                    "rdfs:comment": "The party that sends this crop report document."
                }
            ]
        },
        {
            "@id": "agriculture:sequenceId",
            "@type": "rdf:Property",
            "schema:rangeIncludes": {
                "@id": "xsd:token"
            },
            "schema:domainIncludes": {
                "@id": "agriculture:Document"
            },
            "rdfs:comment": "The identifier for the sequence of this crop report document.",
            "rdfs:label": "sequenceId",
            "unece:cefactElementMetadata": [
                {
                    "@id": "cefact:CropReport_Document.Sequence.Identifier",
                    "@type": "unece:BasicBIE",
                    "unece:cefactUNId": "UN01012441",
                    "unece:cefactBieDomainClass": "cefact:CropReport_Document.Details",
                    "rdfs:comment": "The identifier for the sequence of this crop report document."
                }
            ]
        },
        {
            "@id": "agriculture:sequenceNumeric",
            "@type": "rdf:Property",
            "schema:rangeIncludes": {
                "@id": "xsd:decimal"
            },
            "schema:domainIncludes": [
                {
                    "@id": "agriculture:CropProductionCycle"
                },
                {
                    "@id": "agriculture:Plot"
                },
                {
                    "@id": "agriculture:SoilOccupation"
                },
                {
                    "@id": "agriculture:TradeLineItem"
                }
            ],
            "rdfs:comment": [
                "The sequence number for this SPS trade line item.",
                "The sequence number for this agricultural crop production cycle.",
                "The sequence number for this agricultural plot.",
                "The sequence number for this plot soil occupation."
            ],
            "rdfs:label": "sequenceNumeric",
            "unece:cefactElementMetadata": [
                {
                    "@id": "cefact:SPS_TradeLineItem.Sequence.Numeric",
                    "@type": "unece:BasicBIE",
                    "unece:TDED": "1082",
                    "unece:cefactUNId": "UN03000147",
                    "unece:cefactBieDomainClass": "cefact:SPS_TradeLineItem.Details",
                    "rdfs:comment": "The sequence number for this SPS trade line item."
                },
                {
                    "@id": "cefact:Plot_SoilOccupation.Sequence.Numeric",
                    "@type": "unece:BasicBIE",
                    "unece:cefactUNId": "UN01002751",
                    "unece:cefactBieDomainClass": "cefact:Plot_SoilOccupation.Details",
                    "rdfs:comment": "The sequence number for this plot soil occupation."
                },
                {
                    "@id": "cefact:Agricultural_CropProductionCycle.Sequence.Numeric",
                    "@type": "unece:BasicBIE",
                    "unece:cefactUNId": "UN01002763",
                    "unece:cefactBieDomainClass": "cefact:Agricultural_CropProductionCycle.Details",
                    "rdfs:comment": "The sequence number for this agricultural crop production cycle."
                },
                {
                    "@id": "cefact:Agricultural_Plot.Sequence.Numeric",
                    "@type": "unece:BasicBIE",
                    "unece:cefactUNId": "UN01002657",
                    "unece:cefactBieDomainClass": "cefact:Agricultural_Plot.Details",
                    "rdfs:comment": "The sequence number for this agricultural plot."
                }
            ]
        },
        {
            "@id": "agriculture:serialId",
            "@type": "rdf:Property",
            "schema:rangeIncludes": {
                "@id": "xsd:token"
            },
            "schema:domainIncludes": [
                {
                    "@id": "agriculture:Sample"
                },
                {
                    "@id": "agriculture:Tank"
                }
            ],
            "rdfs:comment": [
                "The serial identifier for this agricultural sample.",
                "The serial number assigned to this milk tank."
            ],
            "rdfs:label": "serialId",
            "unece:cefactElementMetadata": [
                {
                    "@id": "cefact:Milk_Tank.Serial_Identification.Identifier",
                    "@type": "unece:BasicBIE",
                    "unece:cefactUNId": "UN01009836",
                    "unece:cefactBieDomainClass": "cefact:Milk_Tank.Details",
                    "rdfs:comment": "The serial number assigned to this milk tank."
                },
                {
                    "@id": "cefact:Agricultural_Sample.Serial_Identification.Identifier",
                    "@type": "unece:BasicBIE",
                    "unece:cefactUNId": "UN01009586",
                    "unece:cefactBieDomainClass": "cefact:Agricultural_Sample.Details",
                    "rdfs:comment": "The serial identifier for this agricultural sample."
                }
            ]
        },
        {
            "@id": "agriculture:settingTemperature",
            "@type": "rdf:Property",
            "schema:rangeIncludes": {
                "@id": "agriculture:Temperature"
            },
            "schema:domainIncludes": {
                "@id": "agriculture:TransportEquipment"
            },
            "rdfs:comment": "A temperature setting, such as the storage temperature or operational temperature, for this piece of SPS transport equipment.",
            "rdfs:label": "settingTemperature",
            "unece:cefactElementMetadata": [
                {
                    "@id": "cefact:SPS_TransportEquipment.Setting.SPS_Temperature",
                    "@type": "unece:AssociationBIE",
                    "unece:cefactUNId": "UN03000169",
                    "unece:cefactBieDomainClass": "cefact:SPS_TransportEquipment.Details",
                    "rdfs:comment": "A temperature setting, such as the storage temperature or operational temperature, for this piece of SPS transport equipment."
                }
            ]
        },
        {
            "@id": "agriculture:severityCode",
            "@type": "rdf:Property",
            "schema:rangeIncludes": {
                "@id": "xsd:token"
            },
            "schema:domainIncludes": {
                "@id": "agriculture:Issue"
            },
            "rdfs:comment": "A code specifying a severity of this complaint issue, such as alarming, severe.",
            "rdfs:label": "severityCode",
            "unece:cefactElementMetadata": [
                {
                    "@id": "cefact:Complaint_Issue.Severity.Code",
                    "@type": "unece:BasicBIE",
                    "unece:cefactUNId": "UN01012269",
                    "unece:cefactBieDomainClass": "cefact:Complaint_Issue.Details",
                    "rdfs:comment": "A code specifying a severity of this complaint issue, such as alarming, severe."
                }
            ]
        },
        {
            "@id": "agriculture:signatoryAuthentication",
            "@type": "rdf:Property",
            "schema:rangeIncludes": {
                "@id": "agriculture:Authentication"
            },
            "schema:domainIncludes": {
                "@id": "agriculture:Document"
            },
            "rdfs:comment": "An SPS signatory document authentication for this exchanged SPS document.",
            "rdfs:label": "signatoryAuthentication",
            "unece:cefactElementMetadata": [
                {
                    "@id": "cefact:SPSExchanged_Document.Signatory.SPS_Authentication",
                    "@type": "unece:AssociationBIE",
                    "unece:cefactUNId": "UN03000013",
                    "unece:cefactBieDomainClass": "cefact:SPSExchanged_Document.Details",
                    "rdfs:comment": "An SPS signatory document authentication for this exchanged SPS document."
                }
            ]
        },
        {
            "@id": "agriculture:signedDateTime",
            "@type": "rdf:Property",
            "schema:rangeIncludes": {
                "@id": "xsd:dateTime"
            },
            "schema:domainIncludes": {
                "@id": "agriculture:Contract"
            },
            "rdfs:comment": "A date, time, date time, or other date time value on which this agricultural contract was or will be signed.",
            "rdfs:label": "signedDateTime",
            "unece:cefactElementMetadata": [
                {
                    "@id": "cefact:Agricultural_Contract.Signed.DateTime",
                    "@type": "unece:BasicBIE",
                    "unece:cefactUNId": "UN01012447",
                    "unece:cefactBieDomainClass": "cefact:Agricultural_Contract.Details",
                    "rdfs:comment": "A date, time, date time, or other date time value on which this agricultural contract was or will be signed."
                }
            ]
        },
        {
            "@id": "agriculture:sizeMeasure",
            "@type": "rdf:Property",
            "schema:rangeIncludes": {
                "@id": "xsd:decimal"
            },
            "schema:domainIncludes": [
                {
                    "@id": "agriculture:Batch"
                },
                {
                    "@id": "agriculture:Sample"
                },
                {
                    "@id": "agriculture:SampledObject"
                }
            ],
            "rdfs:comment": [
                "A measure of the size of this agricultural sample, such as volume or weight.",
                "The measure of size of this sampled agricultural object.",
                "The size, expressed as a measure, for this crop produce batch.",
                "The size, expressed as a measure, for this product batch."
            ],
            "rdfs:label": "sizeMeasure",
            "unece:cefactElementMetadata": [
                {
                    "@id": "cefact:Agricultural_SampledObject.Size.Measure",
                    "@type": "unece:BasicBIE",
                    "unece:cefactUNId": "UN01009620",
                    "unece:cefactBieDomainClass": "cefact:Agricultural_SampledObject.Details",
                    "rdfs:comment": "The measure of size of this sampled agricultural object."
                },
                {
                    "@id": "cefact:Product_Batch.Size.Measure",
                    "@type": "unece:BasicBIE",
                    "unece:cefactUNId": "UN01012351",
                    "unece:cefactBieDomainClass": "cefact:Product_Batch.Details",
                    "rdfs:comment": "The size, expressed as a measure, for this product batch."
                },
                {
                    "@id": "cefact:Agricultural_Sample.Size.Measure",
                    "@type": "unece:BasicBIE",
                    "unece:cefactUNId": "UN01009596",
                    "unece:cefactBieDomainClass": "cefact:Agricultural_Sample.Details",
                    "rdfs:comment": "A measure of the size of this agricultural sample, such as volume or weight."
                },
                {
                    "@id": "cefact:CropProduce_Batch.Size.Measure",
                    "@type": "unece:BasicBIE",
                    "unece:cefactUNId": "UN01012337",
                    "unece:cefactBieDomainClass": "cefact:CropProduce_Batch.Details",
                    "rdfs:comment": "The size, expressed as a measure, for this crop produce batch."
                }
            ]
        },
        {
            "@id": "agriculture:soilAnalysis",
            "@type": "rdf:Property",
            "schema:rangeIncludes": {
                "@id": "agriculture:Analysis"
            },
            "schema:domainIncludes": {
                "@id": "agriculture:Plot"
            },
            "rdfs:comment": "An agricultural analysis of the soil for this agricultural plot.",
            "rdfs:label": "soilAnalysis",
            "unece:cefactElementMetadata": [
                {
                    "@id": "cefact:Agricultural_Plot.Soil.Agricultural_Analysis",
                    "@type": "unece:AssociationBIE",
                    "unece:cefactUNId": "UN01002663",
                    "unece:cefactBieDomainClass": "cefact:Agricultural_Plot.Details",
                    "rdfs:comment": "An agricultural analysis of the soil for this agricultural plot."
                }
            ]
        },
        {
            "@id": "agriculture:sowingPeriodCode",
            "@type": "rdf:Property",
            "schema:rangeIncludes": {
                "@id": "xsd:token"
            },
            "schema:domainIncludes": {
                "@id": "agriculture:Crop"
            },
            "rdfs:comment": [
                "The code specifying the sowing period for this field crop, such as spring or winter.",
                "The code specifying the sowing period of this agricultural crop, such as spring or winter."
            ],
            "rdfs:label": "sowingPeriodCode",
            "unece:cefactElementMetadata": [
                {
                    "@id": "cefact:Field_Crop.Sowing_Period.Code",
                    "@type": "unece:BasicBIE",
                    "unece:cefactUNId": "UN01012297",
                    "unece:cefactBieDomainClass": "cefact:Field_Crop.Details",
                    "rdfs:comment": "The code specifying the sowing period for this field crop, such as spring or winter."
                },
                {
                    "@id": "cefact:Agricultural_Crop.SowingPeriod.Code",
                    "@type": "unece:BasicBIE",
                    "unece:cefactUNId": "UN01002688",
                    "unece:cefactBieDomainClass": "cefact:Agricultural_Crop.Details",
                    "rdfs:comment": "The code specifying the sowing period of this agricultural crop, such as spring or winter."
                }
            ]
        },
        {
            "@id": "agriculture:sownCrop",
            "@type": "rdf:Property",
            "schema:rangeIncludes": {
                "@id": "agriculture:Crop"
            },
            "schema:domainIncludes": {
                "@id": "agriculture:SoilOccupation"
            },
            "rdfs:comment": "An agricultural crop sown in this plot soil occupation.",
            "rdfs:label": "sownCrop",
            "unece:cefactElementMetadata": [
                {
                    "@id": "cefact:Plot_SoilOccupation.Sown.Agricultural_Crop",
                    "@type": "unece:AssociationBIE",
                    "unece:cefactUNId": "UN01002754",
                    "unece:cefactBieDomainClass": "cefact:Plot_SoilOccupation.Details",
                    "rdfs:comment": "An agricultural crop sown in this plot soil occupation."
                }
            ]
        },
        {
            "@id": "agriculture:sownSpeciesVariety",
            "@type": "rdf:Property",
            "schema:rangeIncludes": {
                "@id": "agriculture:SpeciesVariety"
            },
            "schema:domainIncludes": {
                "@id": "agriculture:Crop"
            },
            "rdfs:comment": [
                "A crop species variety sown for this botanical crop.",
                "A sown crop species variety for this agricultural crop."
            ],
            "rdfs:label": "sownSpeciesVariety",
            "unece:cefactElementMetadata": [
                {
                    "@id": "cefact:Agricultural_Crop.Sown.Crop_SpeciesVariety",
                    "@type": "unece:AssociationBIE",
                    "unece:cefactUNId": "UN01002691",
                    "unece:cefactBieDomainClass": "cefact:Agricultural_Crop.Details",
                    "rdfs:comment": "A sown crop species variety for this agricultural crop."
                },
                {
                    "@id": "cefact:Botanical_Crop.Sown.Crop_SpeciesVariety",
                    "@type": "unece:AssociationBIE",
                    "unece:cefactUNId": "UN01012295",
                    "unece:cefactBieDomainClass": "cefact:Botanical_Crop.Details",
                    "rdfs:comment": "A crop species variety sown for this botanical crop."
                }
            ]
        },
        {
            "@id": "agriculture:speciesCode",
            "@type": "rdf:Property",
            "schema:rangeIncludes": {
                "@id": "xsd:token"
            },
            "schema:domainIncludes": {
                "@id": "agriculture:Product"
            },
            "rdfs:comment": "The code specifying the species for this agricultural input product.",
            "rdfs:label": "speciesCode",
            "unece:cefactElementMetadata": [
                {
                    "@id": "cefact:AgriculturalInput_Product.Species.Code",
                    "@type": "unece:BasicBIE",
                    "unece:cefactUNId": "UN01012379",
                    "unece:cefactBieDomainClass": "cefact:AgriculturalInput_Product.Details",
                    "rdfs:comment": "The code specifying the species for this agricultural input product."
                }
            ]
        },
        {
            "@id": "agriculture:speciesTypeCode",
            "@type": "rdf:Property",
            "schema:rangeIncludes": {
                "@id": "xsd:token"
            },
            "schema:domainIncludes": {
                "@id": "agriculture:Animal"
            },
            "rdfs:comment": "The code specifying the type of species for this livestock animal, such as bovine, sheep or goat.",
            "rdfs:label": "speciesTypeCode",
            "unece:cefactElementMetadata": [
                {
                    "@id": "cefact:Livestock_Animal.Species_Type.Code",
                    "@type": "unece:BasicBIE",
                    "unece:cefactUNId": "UN01007649",
                    "unece:cefactBieDomainClass": "cefact:Livestock_Animal.Details",
                    "rdfs:comment": "The code specifying the type of species for this livestock animal, such as bovine, sheep or goat."
                }
            ]
        },
        {
            "@id": "agriculture:specifiedAddress",
            "@type": "rdf:Property",
            "schema:rangeIncludes": {
                "@id": "agriculture:Address"
            },
            "schema:domainIncludes": [
                {
                    "@id": "agriculture:Party"
                },
                {
                    "@id": "agriculture:ProductionUnit"
                }
            ],
            "rdfs:comment": [
                "A structured address specified for this party.",
                "The specified address for this SPS party.",
                "The specified structured address for this crop data sheet party.",
                "The structured address specified for this agricultural production unit."
            ],
            "rdfs:label": "specifiedAddress",
            "unece:cefactElementMetadata": [
                {
                    "@id": "cefact:Agricultural_ProductionUnit.Specified.Structured_Address",
                    "@type": "unece:AssociationBIE",
                    "unece:cefactUNId": "UN01012255",
                    "unece:cefactBieDomainClass": "cefact:Agricultural_ProductionUnit.Details",
                    "rdfs:comment": "The structured address specified for this agricultural production unit."
                },
                {
                    "@id": "cefact:SPS_Party.Specified.SPS_Address",
                    "@type": "unece:AssociationBIE",
                    "unece:cefactUNId": "UN03000116",
                    "unece:cefactBieDomainClass": "cefact:SPS_Party.Details",
                    "rdfs:comment": "The specified address for this SPS party."
                },
                {
                    "@id": "cefact:Specified_Party.Specified.Structured_Address",
                    "@type": "unece:AssociationBIE",
                    "unece:cefactUNId": "UN01012459",
                    "unece:cefactBieDomainClass": "cefact:Specified_Party.Details",
                    "rdfs:comment": "A structured address specified for this party."
                },
                {
                    "@id": "cefact:CropDataSheet_Party.Specified.Structured_Address",
                    "@type": "unece:AssociationBIE",
                    "unece:cefactUNId": "UN01002812",
                    "unece:cefactBieDomainClass": "cefact:CropDataSheet_Party.Details",
                    "rdfs:comment": "The specified structured address for this crop data sheet party."
                }
            ]
        },
        {
            "@id": "agriculture:specifiedAgriculturalProcess",
            "@type": "rdf:Property",
            "schema:rangeIncludes": {
                "@id": "agriculture:AgriculturalProcess"
            },
            "schema:domainIncludes": {
                "@id": "agriculture:ManMachineSystem"
            },
            "rdfs:comment": "A crop production process specified for this agricultural man machine system.",
            "rdfs:label": "specifiedAgriculturalProcess",
            "unece:cefactElementMetadata": [
                {
                    "@id": "cefact:Agricultural_ManMachineSystem.Specified.CropProduction_AgriculturalProcess",
                    "@type": "unece:AssociationBIE",
                    "unece:cefactUNId": "UN01012458",
                    "unece:cefactBieDomainClass": "cefact:Agricultural_ManMachineSystem.Details",
                    "rdfs:comment": "A crop production process specified for this agricultural man machine system."
                }
            ]
        },
        {
            "@id": "agriculture:specifiedAgronomicalObservation",
            "@type": "rdf:Property",
            "schema:rangeIncludes": {
                "@id": "agriculture:AgronomicalObservation"
            },
            "schema:domainIncludes": {
                "@id": "agriculture:Crop"
            },
            "rdfs:comment": "A single agronomical observation specified for this field crop.",
            "rdfs:label": "specifiedAgronomicalObservation",
            "unece:cefactElementMetadata": [
                {
                    "@id": "cefact:Field_Crop.Specified.Single_AgronomicalObservation",
                    "@type": "unece:AssociationBIE",
                    "unece:cefactUNId": "UN01012317",
                    "unece:cefactBieDomainClass": "cefact:Field_Crop.Details",
                    "rdfs:comment": "A single agronomical observation specified for this field crop."
                }
            ]
        },
        {
            "@id": "agriculture:specifiedArea",
            "@type": "rdf:Property",
            "schema:rangeIncludes": {
                "@id": "agriculture:Area"
            },
            "schema:domainIncludes": {
                "@id": "agriculture:Plot"
            },
            "rdfs:comment": "An agricultural zone area specified for this crop plot.",
            "rdfs:label": "specifiedArea",
            "unece:cefactElementMetadata": [
                {
                    "@id": "cefact:Crop_Plot.Specified.AgriculturalZone_Area",
                    "@type": "unece:AssociationBIE",
                    "unece:cefactUNId": "UN01012146",
                    "unece:cefactBieDomainClass": "cefact:Crop_Plot.Details",
                    "rdfs:comment": "An agricultural zone area specified for this crop plot."
                }
            ]
        },
        {
            "@id": "agriculture:specifiedAsAnimal",
            "@type": "rdf:Property",
            "schema:rangeIncludes": {
                "@id": "agriculture:Animal"
            },
            "schema:domainIncludes": {
                "@id": "agriculture:SampledObject"
            },
            "rdfs:comment": "The animal specified as this sampled agricultural object.",
            "rdfs:label": "specifiedAsAnimal",
            "unece:cefactElementMetadata": [
                {
                    "@id": "cefact:Agricultural_SampledObject.SpecifiedAs.SampledObject_Animal",
                    "@type": "unece:AssociationBIE",
                    "unece:cefactUNId": "UN01009643",
                    "unece:cefactBieDomainClass": "cefact:Agricultural_SampledObject.Details",
                    "rdfs:comment": "The animal specified as this sampled agricultural object."
                }
            ]
        },
        {
            "@id": "agriculture:specifiedAsSilage",
            "@type": "rdf:Property",
            "schema:rangeIncludes": {
                "@id": "agriculture:Silage"
            },
            "schema:domainIncludes": {
                "@id": "agriculture:SampledObject"
            },
            "rdfs:comment": "Silage specified as this sampled agricultural object.",
            "rdfs:label": "specifiedAsSilage",
            "unece:cefactElementMetadata": [
                {
                    "@id": "cefact:Agricultural_SampledObject.SpecifiedAs.SampledObject_Silage",
                    "@type": "unece:AssociationBIE",
                    "unece:cefactUNId": "UN01009642",
                    "unece:cefactBieDomainClass": "cefact:Agricultural_SampledObject.Details",
                    "rdfs:comment": "Silage specified as this sampled agricultural object."
                }
            ]
        },
        {
            "@id": "agriculture:specifiedAsSoil",
            "@type": "rdf:Property",
            "schema:rangeIncludes": {
                "@id": "agriculture:Soil"
            },
            "schema:domainIncludes": {
                "@id": "agriculture:SampledObject"
            },
            "rdfs:comment": "Soil specified as this sampled agricultural object.",
            "rdfs:label": "specifiedAsSoil",
            "unece:cefactElementMetadata": [
                {
                    "@id": "cefact:Agricultural_SampledObject.SpecifiedAs.SampledObject_Soil",
                    "@type": "unece:AssociationBIE",
                    "unece:cefactUNId": "UN01009641",
                    "unece:cefactBieDomainClass": "cefact:Agricultural_SampledObject.Details",
                    "rdfs:comment": "Soil specified as this sampled agricultural object."
                }
            ]
        },
        {
            "@id": "agriculture:specifiedAssertion",
            "@type": "rdf:Property",
            "schema:rangeIncludes": {
                "@id": "agriculture:Assertion"
            },
            "schema:domainIncludes": {
                "@id": "agriculture:Certification"
            },
            "rdfs:comment": "A sustainability assertion specified for this animal certification.",
            "rdfs:label": "specifiedAssertion",
            "unece:cefactElementMetadata": [
                {
                    "@id": "cefact:Animal_Certification.Specified.Sustainability_Assertion",
                    "@type": "unece:AssociationBIE",
                    "unece:cefactUNId": "UN01013725",
                    "unece:cefactBieDomainClass": "cefact:Animal_Certification.Details",
                    "rdfs:comment": "A sustainability assertion specified for this animal certification."
                }
            ]
        },
        {
            "@id": "agriculture:specifiedAutopsy",
            "@type": "rdf:Property",
            "schema:rangeIncludes": {
                "@id": "agriculture:Autopsy"
            },
            "schema:domainIncludes": {
                "@id": "agriculture:SampleType"
            },
            "rdfs:comment": "The autopsy specified for this agricultural sample type.",
            "rdfs:label": "specifiedAutopsy",
            "unece:cefactElementMetadata": [
                {
                    "@id": "cefact:Agricultural_SampleType.Specified.AgriculturalSample_Autopsy",
                    "@type": "unece:AssociationBIE",
                    "unece:cefactUNId": "UN01009583",
                    "unece:cefactBieDomainClass": "cefact:Agricultural_SampleType.Details",
                    "rdfs:comment": "The autopsy specified for this agricultural sample type."
                }
            ]
        },
        {
            "@id": "agriculture:specifiedBatch",
            "@type": "rdf:Property",
            "schema:rangeIncludes": {
                "@id": "agriculture:Batch"
            },
            "schema:domainIncludes": [
                {
                    "@id": "agriculture:AgriculturalApplication"
                },
                {
                    "@id": "agriculture:CropInput"
                },
                {
                    "@id": "agriculture:Produce"
                },
                {
                    "@id": "agriculture:ProductionUnit"
                }
            ],
            "rdfs:comment": [
                "A batch of crop produce specified for this agricultural production unit.",
                "A crop input batch specified for this agricultural process crop input.",
                "A produce batch specified for this agricultural produce.",
                "A product batch specified for this specified agricultural application."
            ],
            "rdfs:label": "specifiedBatch",
            "unece:cefactElementMetadata": [
                {
                    "@id": "cefact:Agricultural_Produce.Specified.Produce_Batch",
                    "@type": "unece:AssociationBIE",
                    "unece:cefactUNId": "UN01002708",
                    "unece:cefactBieDomainClass": "cefact:Agricultural_Produce.Details",
                    "rdfs:comment": "A produce batch specified for this agricultural produce."
                },
                {
                    "@id": "cefact:Agricultural_ProductionUnit.Specified.CropProduce_Batch",
                    "@type": "unece:AssociationBIE",
                    "unece:cefactUNId": "UN01012251",
                    "unece:cefactBieDomainClass": "cefact:Agricultural_ProductionUnit.Details",
                    "rdfs:comment": "A batch of crop produce specified for this agricultural production unit."
                },
                {
                    "@id": "cefact:AgriculturalProcess_CropInput.Specified.CropInput_Batch",
                    "@type": "unece:AssociationBIE",
                    "unece:cefactUNId": "UN01002732",
                    "unece:cefactBieDomainClass": "cefact:AgriculturalProcess_CropInput.Details",
                    "rdfs:comment": "A crop input batch specified for this agricultural process crop input."
                },
                {
                    "@id": "cefact:Specified_AgriculturalApplication.Specified.Product_Batch",
                    "@type": "unece:AssociationBIE",
                    "unece:cefactUNId": "UN01012426",
                    "unece:cefactBieDomainClass": "cefact:Specified_AgriculturalApplication.Details",
                    "rdfs:comment": "A product batch specified for this specified agricultural application."
                }
            ]
        },
        {
            "@id": "agriculture:specifiedBatchHistoryRecord",
            "@type": "rdf:Property",
            "schema:rangeIncludes": {
                "@id": "agriculture:BatchHistoryRecord"
            },
            "schema:domainIncludes": {
                "@id": "agriculture:Batch"
            },
            "rdfs:comment": "A Track and Trace (TT) batch history record specified for this animal batch.",
            "rdfs:label": "specifiedBatchHistoryRecord",
            "unece:cefactElementMetadata": [
                {
                    "@id": "cefact:Animal_Batch.Specified.TT_BatchHistoryRecord",
                    "@type": "unece:AssociationBIE",
                    "unece:cefactUNId": "UN01011258",
                    "unece:cefactBieDomainClass": "cefact:Animal_Batch.Details",
                    "rdfs:comment": "A Track and Trace (TT) batch history record specified for this animal batch."
                }
            ]
        },
        {
            "@id": "agriculture:specifiedCargo",
            "@type": "rdf:Property",
            "schema:rangeIncludes": {
                "@id": "agriculture:Cargo"
            },
            "schema:domainIncludes": {
                "@id": "agriculture:SampledObject"
            },
            "rdfs:comment": "Cargo details specified for this sampled agricultural object.",
            "rdfs:label": "specifiedCargo",
            "unece:cefactElementMetadata": [
                {
                    "@id": "cefact:Agricultural_SampledObject.Specified.SampledObject_Cargo",
                    "@type": "unece:AssociationBIE",
                    "unece:cefactUNId": "UN01009640",
                    "unece:cefactBieDomainClass": "cefact:Agricultural_SampledObject.Details",
                    "rdfs:comment": "Cargo details specified for this sampled agricultural object."
                }
            ]
        },
        {
            "@id": "agriculture:specifiedCatch",
            "@type": "rdf:Property",
            "schema:rangeIncludes": {
                "@id": "agriculture:Catch"
            },
            "schema:domainIncludes": {
                "@id": "agriculture:Batch"
            },
            "rdfs:comment": "A batch catch specified for this animal batch.",
            "rdfs:label": "specifiedCatch",
            "unece:cefactElementMetadata": [
                {
                    "@id": "cefact:Animal_Batch.Specified.Batch_Catch",
                    "@type": "unece:AssociationBIE",
                    "unece:cefactUNId": "UN01011260",
                    "unece:cefactBieDomainClass": "cefact:Animal_Batch.Details",
                    "rdfs:comment": "A batch catch specified for this animal batch."
                }
            ]
        },
        {
            "@id": "agriculture:specifiedCertificate",
            "@type": "rdf:Property",
            "schema:rangeIncludes": {
                "@id": "agriculture:Certificate"
            },
            "schema:domainIncludes": [
                {
                    "@id": "agriculture:Batch"
                },
                {
                    "@id": "agriculture:Person"
                },
                {
                    "@id": "agriculture:Plot"
                },
                {
                    "@id": "agriculture:Product"
                },
                {
                    "@id": "agriculture:ProductionUnit"
                }
            ],
            "rdfs:comment": [
                "An agricultural certificate specified for this agricultural input product.",
                "An agricultural certificate specified for this agricultural production unit.",
                "An agricultural certificate specified for this crop plot.",
                "An agricultural certificate specified for this crop produce batch.",
                "An agricultural certificate specified for this operator person.",
                "An agricultural certificate specified for this product batch."
            ],
            "rdfs:label": "specifiedCertificate",
            "unece:cefactElementMetadata": [
                {
                    "@id": "cefact:Operator_Person.Specified.Agricultural_Certificate",
                    "@type": "unece:AssociationBIE",
                    "unece:cefactUNId": "UN01012275",
                    "unece:cefactBieDomainClass": "cefact:Operator_Person.Details",
                    "rdfs:comment": "An agricultural certificate specified for this operator person."
                },
                {
                    "@id": "cefact:Agricultural_ProductionUnit.Specified.Agricultural_Certificate",
                    "@type": "unece:AssociationBIE",
                    "unece:cefactUNId": "UN01012253",
                    "unece:cefactBieDomainClass": "cefact:Agricultural_ProductionUnit.Details",
                    "rdfs:comment": "An agricultural certificate specified for this agricultural production unit."
                },
                {
                    "@id": "cefact:Product_Batch.Specified.Agricultural_Certificate",
                    "@type": "unece:AssociationBIE",
                    "unece:cefactUNId": "UN01012356",
                    "unece:cefactBieDomainClass": "cefact:Product_Batch.Details",
                    "rdfs:comment": "An agricultural certificate specified for this product batch."
                },
                {
                    "@id": "cefact:Crop_Plot.Specified.Agricultural_Certificate",
                    "@type": "unece:AssociationBIE",
                    "unece:cefactUNId": "UN01012150",
                    "unece:cefactBieDomainClass": "cefact:Crop_Plot.Details",
                    "rdfs:comment": "An agricultural certificate specified for this crop plot."
                },
                {
                    "@id": "cefact:AgriculturalInput_Product.Specified.Agricultural_Certificate",
                    "@type": "unece:AssociationBIE",
                    "unece:cefactUNId": "UN01012384",
                    "unece:cefactBieDomainClass": "cefact:AgriculturalInput_Product.Details",
                    "rdfs:comment": "An agricultural certificate specified for this agricultural input product."
                },
                {
                    "@id": "cefact:CropProduce_Batch.Specified.Agricultural_Certificate",
                    "@type": "unece:AssociationBIE",
                    "unece:cefactUNId": "UN01012343",
                    "unece:cefactBieDomainClass": "cefact:CropProduce_Batch.Details",
                    "rdfs:comment": "An agricultural certificate specified for this crop produce batch."
                }
            ]
        },
        {
            "@id": "agriculture:specifiedCharacteristic",
            "@type": "rdf:Property",
            "schema:rangeIncludes": {
                "@id": "agriculture:Characteristic"
            },
            "schema:domainIncludes": [
                {
                    "@id": "agriculture:Batch"
                },
                {
                    "@id": "agriculture:Crop"
                },
                {
                    "@id": "agriculture:Plot"
                }
            ],
            "rdfs:comment": [
                "A fish catch characteristic specified for this animal batch.",
                "An agricultural characteristic specified for this crop plot.",
                "An agricultural characteristic specified for this crop produce batch.",
                "An agricultural characteristic specified for this field crop.",
                "An agricultural characteristic specified for this product batch."
            ],
            "rdfs:label": "specifiedCharacteristic",
            "unece:cefactElementMetadata": [
                {
                    "@id": "cefact:Field_Crop.Specified.Agricultural_Characteristic",
                    "@type": "unece:AssociationBIE",
                    "unece:cefactUNId": "UN01012318",
                    "unece:cefactBieDomainClass": "cefact:Field_Crop.Details",
                    "rdfs:comment": "An agricultural characteristic specified for this field crop."
                },
                {
                    "@id": "cefact:Product_Batch.Specified.Agricultural_Characteristic",
                    "@type": "unece:AssociationBIE",
                    "unece:cefactUNId": "UN01012355",
                    "unece:cefactBieDomainClass": "cefact:Product_Batch.Details",
                    "rdfs:comment": "An agricultural characteristic specified for this product batch."
                },
                {
                    "@id": "cefact:Animal_Batch.Specified.FishCatch_Characteristic",
                    "@type": "unece:AssociationBIE",
                    "unece:cefactUNId": "UN01011259",
                    "unece:cefactBieDomainClass": "cefact:Animal_Batch.Details",
                    "rdfs:comment": "A fish catch characteristic specified for this animal batch."
                },
                {
                    "@id": "cefact:Crop_Plot.Specified.Agricultural_Characteristic",
                    "@type": "unece:AssociationBIE",
                    "unece:cefactUNId": "UN01012145",
                    "unece:cefactBieDomainClass": "cefact:Crop_Plot.Details",
                    "rdfs:comment": "An agricultural characteristic specified for this crop plot."
                },
                {
                    "@id": "cefact:CropProduce_Batch.Specified.Agricultural_Characteristic",
                    "@type": "unece:AssociationBIE",
                    "unece:cefactUNId": "UN01012342",
                    "unece:cefactBieDomainClass": "cefact:CropProduce_Batch.Details",
                    "rdfs:comment": "An agricultural characteristic specified for this crop produce batch."
                }
            ]
        },
        {
            "@id": "agriculture:specifiedChemical",
            "@type": "rdf:Property",
            "schema:rangeIncludes": {
                "@id": "agriculture:Chemical"
            },
            "schema:domainIncludes": {
                "@id": "agriculture:Product"
            },
            "rdfs:comment": "An agricultural input chemical specified for this agricultural input product.",
            "rdfs:label": "specifiedChemical",
            "unece:cefactElementMetadata": [
                {
                    "@id": "cefact:AgriculturalInput_Product.Specified.AgriculturalInput_Chemical",
                    "@type": "unece:AssociationBIE",
                    "unece:cefactUNId": "UN01012385",
                    "unece:cefactBieDomainClass": "cefact:AgriculturalInput_Product.Details",
                    "rdfs:comment": "An agricultural input chemical specified for this agricultural input product."
                }
            ]
        },
        {
            "@id": "agriculture:specifiedCondition",
            "@type": "rdf:Property",
            "schema:rangeIncludes": {
                "@id": "agriculture:Condition"
            },
            "schema:domainIncludes": {
                "@id": "agriculture:AgriculturalProcess"
            },
            "rdfs:comment": "An agricultural process condition specified for this plot agricultural process.",
            "rdfs:label": "specifiedCondition",
            "unece:cefactElementMetadata": [
                {
                    "@id": "cefact:Plot_AgriculturalProcess.Specified.AgriculturalProcess_Condition",
                    "@type": "unece:AssociationBIE",
                    "unece:cefactUNId": "UN01002799",
                    "unece:cefactBieDomainClass": "cefact:Plot_AgriculturalProcess.Details",
                    "rdfs:comment": "An agricultural process condition specified for this plot agricultural process."
                }
            ]
        },
        {
            "@id": "agriculture:specifiedContact",
            "@type": "rdf:Property",
            "schema:rangeIncludes": {
                "@id": "agriculture:Contact"
            },
            "schema:domainIncludes": {
                "@id": "agriculture:AgronomicalObservation"
            },
            "rdfs:comment": "The party contact specified for this single agronomical observation.",
            "rdfs:label": "specifiedContact",
            "unece:cefactElementMetadata": [
                {
                    "@id": "cefact:Single_AgronomicalObservation.Specified.Party_Contact",
                    "@type": "unece:AssociationBIE",
                    "unece:cefactUNId": "UN01009317",
                    "unece:cefactBieDomainClass": "cefact:Single_AgronomicalObservation.Details",
                    "rdfs:comment": "The party contact specified for this single agronomical observation."
                }
            ]
        },
        {
            "@id": "agriculture:specifiedContract",
            "@type": "rdf:Property",
            "schema:rangeIncludes": {
                "@id": "agriculture:Contract"
            },
            "schema:domainIncludes": [
                {
                    "@id": "agriculture:ProductionUnit"
                },
                {
                    "@id": "agriculture:Sample"
                },
                {
                    "@id": "agriculture:SampledObject"
                }
            ],
            "rdfs:comment": [
                "A contract specified for this sampled agricultural object.",
                "The agricultural contract specified for this agricultural production unit.",
                "The laboratory observation contract specified for this agricultural sample."
            ],
            "rdfs:label": "specifiedContract",
            "unece:cefactElementMetadata": [
                {
                    "@id": "cefact:Agricultural_ProductionUnit.Specified.Agricultural_Contract",
                    "@type": "unece:AssociationBIE",
                    "unece:cefactUNId": "UN01012254",
                    "unece:cefactBieDomainClass": "cefact:Agricultural_ProductionUnit.Details",
                    "rdfs:comment": "The agricultural contract specified for this agricultural production unit."
                },
                {
                    "@id": "cefact:Agricultural_Sample.Specified.LaboratoryObservation_Contract",
                    "@type": "unece:AssociationBIE",
                    "unece:cefactUNId": "UN01009604",
                    "unece:cefactBieDomainClass": "cefact:Agricultural_Sample.Details",
                    "rdfs:comment": "The laboratory observation contract specified for this agricultural sample."
                },
                {
                    "@id": "cefact:Agricultural_SampledObject.Specified.SampledObject_Contract",
                    "@type": "unece:AssociationBIE",
                    "unece:cefactUNId": "UN01009637",
                    "unece:cefactBieDomainClass": "cefact:Agricultural_SampledObject.Details",
                    "rdfs:comment": "A contract specified for this sampled agricultural object."
                }
            ]
        },
        {
            "@id": "agriculture:specifiedCrop",
            "@type": "rdf:Property",
            "schema:rangeIncludes": {
                "@id": "agriculture:Crop"
            },
            "schema:domainIncludes": [
                {
                    "@id": "agriculture:AgriculturalProcess"
                },
                {
                    "@id": "agriculture:CropMixtureConstituent"
                },
                {
                    "@id": "agriculture:SampledObject"
                }
            ],
            "rdfs:comment": [
                "A field crop specified for this crop production agricultural process.",
                "The botanical crop specified for this field crop mixture constituent.",
                "The crop specified for this sampled agricultural object."
            ],
            "rdfs:label": "specifiedCrop",
            "unece:cefactElementMetadata": [
                {
                    "@id": "cefact:Field_CropMixtureConstituent.Specified.Botanical_Crop",
                    "@type": "unece:AssociationBIE",
                    "unece:cefactUNId": "UN01012323",
                    "unece:cefactBieDomainClass": "cefact:Field_CropMixtureConstituent.Details",
                    "rdfs:comment": "The botanical crop specified for this field crop mixture constituent."
                },
                {
                    "@id": "cefact:Agricultural_SampledObject.Specified.SampledObject_Crop",
                    "@type": "unece:AssociationBIE",
                    "unece:cefactUNId": "UN01009636",
                    "unece:cefactBieDomainClass": "cefact:Agricultural_SampledObject.Details",
                    "rdfs:comment": "The crop specified for this sampled agricultural object."
                },
                {
                    "@id": "cefact:CropProduction_AgriculturalProcess.Specified.Field_Crop",
                    "@type": "unece:AssociationBIE",
                    "unece:cefactUNId": "UN01012421",
                    "unece:cefactBieDomainClass": "cefact:CropProduction_AgriculturalProcess.Details",
                    "rdfs:comment": "A field crop specified for this crop production agricultural process."
                }
            ]
        },
        {
            "@id": "agriculture:specifiedCropMixtureConstituent",
            "@type": "rdf:Property",
            "schema:rangeIncludes": {
                "@id": "agriculture:CropMixtureConstituent"
            },
            "schema:domainIncludes": {
                "@id": "agriculture:Crop"
            },
            "rdfs:comment": "A field crop mixture constituent specified for this field crop.",
            "rdfs:label": "specifiedCropMixtureConstituent",
            "unece:cefactElementMetadata": [
                {
                    "@id": "cefact:Field_Crop.Specified.Field_CropMixtureConstituent",
                    "@type": "unece:AssociationBIE",
                    "unece:cefactUNId": "UN01012313",
                    "unece:cefactBieDomainClass": "cefact:Field_Crop.Details",
                    "rdfs:comment": "A field crop mixture constituent specified for this field crop."
                }
            ]
        },
        {
            "@id": "agriculture:specifiedCropProductionCycle",
            "@type": "rdf:Property",
            "schema:rangeIncludes": {
                "@id": "agriculture:CropProductionCycle"
            },
            "schema:domainIncludes": {
                "@id": "agriculture:SoilOccupation"
            },
            "rdfs:comment": "An agricultural crop production cycle specified for this plot soil occupation.",
            "rdfs:label": "specifiedCropProductionCycle",
            "unece:cefactElementMetadata": [
                {
                    "@id": "cefact:Plot_SoilOccupation.Specified.Agricultural_CropProductionCycle",
                    "@type": "unece:AssociationBIE",
                    "unece:cefactUNId": "UN01002757",
                    "unece:cefactBieDomainClass": "cefact:Plot_SoilOccupation.Details",
                    "rdfs:comment": "An agricultural crop production cycle specified for this plot soil occupation."
                }
            ]
        },
        {
            "@id": "agriculture:specifiedCropStage",
            "@type": "rdf:Property",
            "schema:rangeIncludes": {
                "@id": "agriculture:CropStage"
            },
            "schema:domainIncludes": {
                "@id": "agriculture:AgriculturalProcess"
            },
            "rdfs:comment": "An agricultural process crop stage specified for this plot agricultural process.",
            "rdfs:label": "specifiedCropStage",
            "unece:cefactElementMetadata": [
                {
                    "@id": "cefact:Plot_AgriculturalProcess.Specified.AgriculturalProcess_CropStage",
                    "@type": "unece:AssociationBIE",
                    "unece:cefactUNId": "UN01002798",
                    "unece:cefactBieDomainClass": "cefact:Plot_AgriculturalProcess.Details",
                    "rdfs:comment": "An agricultural process crop stage specified for this plot agricultural process."
                }
            ]
        },
        {
            "@id": "agriculture:specifiedEvent",
            "@type": "rdf:Property",
            "schema:rangeIncludes": {
                "@id": "agriculture:Event"
            },
            "schema:domainIncludes": [
                {
                    "@id": "agriculture:Animal"
                },
                {
                    "@id": "agriculture:Inspection"
                },
                {
                    "@id": "agriculture:Issue"
                }
            ],
            "rdfs:comment": [
                "A cross border movement event specified for this livestock animal.",
                "A veterinarian event specified for this livestock animal.",
                "An animal holding event specified for this livestock animal.",
                "The cross border animal movement event specified for this cross border animal movement issue.",
                "The inspection event specified for this animal inspection."
            ],
            "rdfs:label": "specifiedEvent",
            "unece:cefactElementMetadata": [
                {
                    "@id": "cefact:CrossBorderAnimalMovement_Issue.Specified.CrossBorderAnimalMovement_Event",
                    "@type": "unece:AssociationBIE",
                    "unece:cefactUNId": "UN01007669",
                    "unece:cefactBieDomainClass": "cefact:CrossBorderAnimalMovement_Issue.Details",
                    "rdfs:comment": "The cross border animal movement event specified for this cross border animal movement issue."
                },
                {
                    "@id": "cefact:Livestock_Animal.Specified.CrossBorderAnimalMovement_Event",
                    "@type": "unece:AssociationBIE",
                    "unece:cefactUNId": "UN01007657",
                    "unece:cefactBieDomainClass": "cefact:Livestock_Animal.Details",
                    "rdfs:comment": "A cross border movement event specified for this livestock animal."
                },
                {
                    "@id": "cefact:Animal_Inspection.Specified.Inspection_Event",
                    "@type": "unece:AssociationBIE",
                    "unece:cefactUNId": "UN01007695",
                    "unece:cefactBieDomainClass": "cefact:Animal_Inspection.Details",
                    "rdfs:comment": "The inspection event specified for this animal inspection."
                },
                {
                    "@id": "cefact:Livestock_Animal.Specified.AnimalHolding_Event",
                    "@type": "unece:AssociationBIE",
                    "unece:cefactUNId": "UN01007656",
                    "unece:cefactBieDomainClass": "cefact:Livestock_Animal.Details",
                    "rdfs:comment": "An animal holding event specified for this livestock animal."
                },
                {
                    "@id": "cefact:Livestock_Animal.Specified.Veterinarian_Event",
                    "@type": "unece:AssociationBIE",
                    "unece:cefactUNId": "UN01007655",
                    "unece:cefactBieDomainClass": "cefact:Livestock_Animal.Details",
                    "rdfs:comment": "A veterinarian event specified for this livestock animal."
                }
            ]
        },
        {
            "@id": "agriculture:specifiedExaminationResult",
            "@type": "rdf:Property",
            "schema:rangeIncludes": {
                "@id": "agriculture:ExaminationResult"
            },
            "schema:domainIncludes": {
                "@id": "agriculture:Inspection"
            },
            "rdfs:comment": "The examination result specified for this animal inspection.",
            "rdfs:label": "specifiedExaminationResult",
            "unece:cefactElementMetadata": [
                {
                    "@id": "cefact:Animal_Inspection.Specified.Animal_ExaminationResult",
                    "@type": "unece:AssociationBIE",
                    "unece:cefactUNId": "UN01007696",
                    "unece:cefactBieDomainClass": "cefact:Animal_Inspection.Details",
                    "rdfs:comment": "The examination result specified for this animal inspection."
                }
            ]
        },
        {
            "@id": "agriculture:specifiedIdentity",
            "@type": "rdf:Property",
            "schema:rangeIncludes": {
                "@id": "agriculture:Identity"
            },
            "schema:domainIncludes": {
                "@id": "agriculture:Animal"
            },
            "rdfs:comment": "Identifying information specified for this livestock animal.",
            "rdfs:label": "specifiedIdentity",
            "unece:cefactElementMetadata": [
                {
                    "@id": "cefact:Livestock_Animal.Specified.Animal_Identity",
                    "@type": "unece:AssociationBIE",
                    "unece:cefactUNId": "UN01007654",
                    "unece:cefactBieDomainClass": "cefact:Livestock_Animal.Details",
                    "rdfs:comment": "Identifying information specified for this livestock animal."
                }
            ]
        },
        {
            "@id": "agriculture:specifiedIllness",
            "@type": "rdf:Property",
            "schema:rangeIncludes": {
                "@id": "agriculture:Illness"
            },
            "schema:domainIncludes": {
                "@id": "agriculture:SampledObject"
            },
            "rdfs:comment": "The Illness or disease specified for this sampled agricultural object.",
            "rdfs:label": "specifiedIllness",
            "unece:cefactElementMetadata": [
                {
                    "@id": "cefact:Agricultural_SampledObject.Specified.SampledObject_Illness",
                    "@type": "unece:AssociationBIE",
                    "unece:cefactUNId": "UN01009638",
                    "unece:cefactBieDomainClass": "cefact:Agricultural_SampledObject.Details",
                    "rdfs:comment": "The Illness or disease specified for this sampled agricultural object."
                }
            ]
        },
        {
            "@id": "agriculture:specifiedInstructions",
            "@type": "rdf:Property",
            "schema:rangeIncludes": {
                "@id": "agriculture:Instructions"
            },
            "schema:domainIncludes": [
                {
                    "@id": "agriculture:Sample"
                },
                {
                    "@id": "agriculture:SampledObject"
                }
            ],
            "rdfs:comment": [
                "A set of laboratory observation instructions specified for this agricultural sample.",
                "A set of laboratory observation instructions specified for this agricultural sampled object."
            ],
            "rdfs:label": "specifiedInstructions",
            "unece:cefactElementMetadata": [
                {
                    "@id": "cefact:Agricultural_Sample.Specified.LaboratoryObservation_Instructions",
                    "@type": "unece:AssociationBIE",
                    "unece:cefactUNId": "UN01009608",
                    "unece:cefactBieDomainClass": "cefact:Agricultural_Sample.Details",
                    "rdfs:comment": "A set of laboratory observation instructions specified for this agricultural sample."
                },
                {
                    "@id": "cefact:Agricultural_SampledObject.Specified.LaboratoryObservation_Instructions",
                    "@type": "unece:AssociationBIE",
                    "unece:cefactUNId": "UN01009645",
                    "unece:cefactBieDomainClass": "cefact:Agricultural_SampledObject.Details",
                    "rdfs:comment": "A set of laboratory observation instructions specified for this agricultural sampled object."
                }
            ]
        },
        {
            "@id": "agriculture:specifiedLabel",
            "@type": "rdf:Property",
            "schema:rangeIncludes": {
                "@id": "agriculture:Label"
            },
            "schema:domainIncludes": {
                "@id": "agriculture:Identity"
            },
            "rdfs:comment": "A label specified for this animal identity, such as an identification tag, a transponder or a tattoo.",
            "rdfs:label": "specifiedLabel",
            "unece:cefactElementMetadata": [
                {
                    "@id": "cefact:Animal_Identity.Specified.Animal_Label",
                    "@type": "unece:AssociationBIE",
                    "unece:cefactUNId": "UN01007630",
                    "unece:cefactBieDomainClass": "cefact:Animal_Identity.Details",
                    "rdfs:comment": "A label specified for this animal identity, such as an identification tag, a transponder or a tattoo."
                }
            ]
        },
        {
            "@id": "agriculture:specifiedLocation",
            "@type": "rdf:Property",
            "schema:rangeIncludes": {
                "@id": "agriculture:Location"
            },
            "schema:domainIncludes": [
                {
                    "@id": "agriculture:AgriculturalApplication"
                },
                {
                    "@id": "agriculture:Area"
                },
                {
                    "@id": "agriculture:Construction"
                },
                {
                    "@id": "agriculture:Plot"
                }
            ],
            "rdfs:comment": [
                "A referenced location specified for this specified agricultural application.",
                "The referenced location specified for this agricultural construction.",
                "The referenced location specified for this agricultural zone area.",
                "The referenced location specified for this crop plot."
            ],
            "rdfs:label": "specifiedLocation",
            "unece:cefactElementMetadata": [
                {
                    "@id": "cefact:Crop_Plot.Specified.Referenced_Location",
                    "@type": "unece:AssociationBIE",
                    "unece:cefactUNId": "UN01012148",
                    "unece:cefactBieDomainClass": "cefact:Crop_Plot.Details",
                    "rdfs:comment": "The referenced location specified for this crop plot."
                },
                {
                    "@id": "cefact:AgriculturalZone_Area.Specified.Referenced_Location",
                    "@type": "unece:AssociationBIE",
                    "unece:cefactUNId": "UN01012220",
                    "unece:cefactBieDomainClass": "cefact:AgriculturalZone_Area.Details",
                    "rdfs:comment": "The referenced location specified for this agricultural zone area."
                },
                {
                    "@id": "cefact:Specified_AgriculturalApplication.Specified.Referenced_Location",
                    "@type": "unece:AssociationBIE",
                    "unece:cefactUNId": "UN01012424",
                    "unece:cefactBieDomainClass": "cefact:Specified_AgriculturalApplication.Details",
                    "rdfs:comment": "A referenced location specified for this specified agricultural application."
                },
                {
                    "@id": "cefact:Agricultural_Construction.Specified.Referenced_Location",
                    "@type": "unece:AssociationBIE",
                    "unece:cefactUNId": "UN01012241",
                    "unece:cefactBieDomainClass": "cefact:Agricultural_Construction.Details",
                    "rdfs:comment": "The referenced location specified for this agricultural construction."
                }
            ]
        },
        {
            "@id": "agriculture:specifiedManMachineSystem",
            "@type": "rdf:Property",
            "schema:rangeIncludes": {
                "@id": "agriculture:ManMachineSystem"
            },
            "schema:domainIncludes": [
                {
                    "@id": "agriculture:AgriculturalDevice"
                },
                {
                    "@id": "agriculture:Person"
                }
            ],
            "rdfs:comment": [
                "A man machine system specified for this agricultural device.",
                "An agricultural man machine system specified for this operator person."
            ],
            "rdfs:label": "specifiedManMachineSystem",
            "unece:cefactElementMetadata": [
                {
                    "@id": "cefact:Operator_Person.Specified.Agricultural_ManMachineSystem",
                    "@type": "unece:AssociationBIE",
                    "unece:cefactUNId": "UN01012276",
                    "unece:cefactBieDomainClass": "cefact:Operator_Person.Details",
                    "rdfs:comment": "An agricultural man machine system specified for this operator person."
                },
                {
                    "@id": "cefact:Specified_AgriculturalDevice.Specified.Agricultural_ManMachineSystem",
                    "@type": "unece:AssociationBIE",
                    "unece:cefactUNId": "UN01012464",
                    "unece:cefactBieDomainClass": "cefact:Specified_AgriculturalDevice.Details",
                    "rdfs:comment": "A man machine system specified for this agricultural device."
                }
            ]
        },
        {
            "@id": "agriculture:specifiedObservationRequest",
            "@type": "rdf:Property",
            "schema:rangeIncludes": {
                "@id": "agriculture:ObservationRequest"
            },
            "schema:domainIncludes": {
                "@id": "agriculture:Sample"
            },
            "rdfs:comment": "An observation request specified for this agricultural sample.",
            "rdfs:label": "specifiedObservationRequest",
            "unece:cefactElementMetadata": [
                {
                    "@id": "cefact:Agricultural_Sample.Specified.Sample_ObservationRequest",
                    "@type": "unece:AssociationBIE",
                    "unece:cefactUNId": "UN01010479",
                    "unece:cefactBieDomainClass": "cefact:Agricultural_Sample.Details",
                    "rdfs:comment": "An observation request specified for this agricultural sample."
                }
            ]
        },
        {
            "@id": "agriculture:specifiedObservationResult",
            "@type": "rdf:Property",
            "schema:rangeIncludes": {
                "@id": "agriculture:ObservationResult"
            },
            "schema:domainIncludes": [
                {
                    "@id": "agriculture:Batch"
                },
                {
                    "@id": "agriculture:Crop"
                },
                {
                    "@id": "agriculture:Sample"
                }
            ],
            "rdfs:comment": [
                "A referenced observation result specified for this crop produce batch.",
                "A referenced sample observation result specified for this field crop.",
                "An observation result specified for this agricultural sample."
            ],
            "rdfs:label": "specifiedObservationResult",
            "unece:cefactElementMetadata": [
                {
                    "@id": "cefact:Agricultural_Sample.Specified.Sample_ObservationResult",
                    "@type": "unece:AssociationBIE",
                    "unece:cefactUNId": "UN01009603",
                    "unece:cefactBieDomainClass": "cefact:Agricultural_Sample.Details",
                    "rdfs:comment": "An observation result specified for this agricultural sample."
                },
                {
                    "@id": "cefact:Field_Crop.Specified.Referenced_ObservationResult",
                    "@type": "unece:AssociationBIE",
                    "unece:cefactUNId": "UN01012315",
                    "unece:cefactBieDomainClass": "cefact:Field_Crop.Details",
                    "rdfs:comment": "A referenced sample observation result specified for this field crop."
                },
                {
                    "@id": "cefact:CropProduce_Batch.Specified.Referenced_ObservationResult",
                    "@type": "unece:AssociationBIE",
                    "unece:cefactUNId": "UN01012344",
                    "unece:cefactBieDomainClass": "cefact:CropProduce_Batch.Details",
                    "rdfs:comment": "A referenced observation result specified for this crop produce batch."
                }
            ]
        },
        {
            "@id": "agriculture:specifiedPackage",
            "@type": "rdf:Property",
            "schema:rangeIncludes": {
                "@id": "agriculture:Package"
            },
            "schema:domainIncludes": {
                "@id": "agriculture:Sample"
            },
            "rdfs:comment": "A referenced logistics package for this agricultural sample.",
            "rdfs:label": "specifiedPackage",
            "unece:cefactElementMetadata": [
                {
                    "@id": "cefact:Agricultural_Sample.Specified.Referenced_Logistics_Package",
                    "@type": "unece:AssociationBIE",
                    "unece:cefactUNId": "UN01012467",
                    "unece:cefactBieDomainClass": "cefact:Agricultural_Sample.Details",
                    "rdfs:comment": "A referenced logistics package for this agricultural sample."
                }
            ]
        },
        {
            "@id": "agriculture:specifiedPeriod",
            "@type": "rdf:Property",
            "schema:rangeIncludes": {
                "@id": "agriculture:Period"
            },
            "schema:domainIncludes": [
                {
                    "@id": "agriculture:Batch"
                },
                {
                    "@id": "agriculture:CoordinateReferenceSystem"
                },
                {
                    "@id": "agriculture:Plot"
                }
            ],
            "rdfs:comment": [
                "A delimited period specified for this CS engineering coordinate reference system.",
                "A delimited period specified for this mobile plot.",
                "The delimited period specified for this animal batch."
            ],
            "rdfs:label": "specifiedPeriod",
            "unece:cefactElementMetadata": [
                {
                    "@id": "cefact:Animal_Batch.Specified.Delimited_Period",
                    "@type": "unece:AssociationBIE",
                    "unece:cefactUNId": "UN01011255",
                    "unece:cefactBieDomainClass": "cefact:Animal_Batch.Details",
                    "rdfs:comment": "The delimited period specified for this animal batch."
                },
                {
                    "@id": "cefact:CSEngineering_CoordinateReferenceSystem.Specified.Delimited_Period",
                    "@type": "unece:AssociationBIE",
                    "unece:cefactUNId": "UN01012167",
                    "unece:cefactBieDomainClass": "cefact:CSEngineering_CoordinateReferenceSystem.Details",
                    "rdfs:comment": "A delimited period specified for this CS engineering coordinate reference system."
                },
                {
                    "@id": "cefact:Mobile_Plot.Specified.Delimited_Period",
                    "@type": "unece:AssociationBIE",
                    "unece:cefactUNId": "UN01012156",
                    "unece:cefactBieDomainClass": "cefact:Mobile_Plot.Details",
                    "rdfs:comment": "A delimited period specified for this mobile plot."
                }
            ]
        },
        {
            "@id": "agriculture:specifiedPerson",
            "@type": "rdf:Property",
            "schema:rangeIncludes": {
                "@id": "agriculture:Person"
            },
            "schema:domainIncludes": {
                "@id": "agriculture:Party"
            },
            "rdfs:comment": [
                "An operator person specified for this party.",
                "The specified person of this SPS party."
            ],
            "rdfs:label": "specifiedPerson",
            "unece:cefactElementMetadata": [
                {
                    "@id": "cefact:SPS_Party.Specified.SPS_Person",
                    "@type": "unece:AssociationBIE",
                    "unece:cefactUNId": "UN03000118",
                    "unece:cefactBieDomainClass": "cefact:SPS_Party.Details",
                    "rdfs:comment": "The specified person of this SPS party."
                },
                {
                    "@id": "cefact:Specified_Party.Specified.Operator_Person",
                    "@type": "unece:AssociationBIE",
                    "unece:cefactUNId": "UN01012462",
                    "unece:cefactBieDomainClass": "cefact:Specified_Party.Details",
                    "rdfs:comment": "An operator person specified for this party."
                }
            ]
        },
        {
            "@id": "agriculture:specifiedPlot",
            "@type": "rdf:Property",
            "schema:rangeIncludes": {
                "@id": "agriculture:Plot"
            },
            "schema:domainIncludes": [
                {
                    "@id": "agriculture:AgriculturalApplication"
                },
                {
                    "@id": "agriculture:Area"
                },
                {
                    "@id": "agriculture:Construction"
                },
                {
                    "@id": "agriculture:GeographicalGrid"
                },
                {
                    "@id": "agriculture:ProductionUnit"
                }
            ],
            "rdfs:comment": [
                "A crop plot specified for this agricultural application.",
                "A crop plot specified for this agricultural construction.",
                "A crop plot specified for this agricultural production unit.",
                "A crop plot specified for this agricultural zone area.",
                "A crop plot specified for this geographical grid."
            ],
            "rdfs:label": "specifiedPlot",
            "unece:cefactElementMetadata": [
                {
                    "@id": "cefact:Agricultural_Construction.Specified.Crop_Plot",
                    "@type": "unece:AssociationBIE",
                    "unece:cefactUNId": "UN01012242",
                    "unece:cefactBieDomainClass": "cefact:Agricultural_Construction.Details",
                    "rdfs:comment": "A crop plot specified for this agricultural construction."
                },
                {
                    "@id": "cefact:Specified_AgriculturalApplication.Specified.Crop_Plot",
                    "@type": "unece:AssociationBIE",
                    "unece:cefactUNId": "UN01012428",
                    "unece:cefactBieDomainClass": "cefact:Specified_AgriculturalApplication.Details",
                    "rdfs:comment": "A crop plot specified for this agricultural application."
                },
                {
                    "@id": "cefact:AgriculturalZone_Area.Specified.Crop_Plot",
                    "@type": "unece:AssociationBIE",
                    "unece:cefactUNId": "UN01012224",
                    "unece:cefactBieDomainClass": "cefact:AgriculturalZone_Area.Details",
                    "rdfs:comment": "A crop plot specified for this agricultural zone area."
                },
                {
                    "@id": "cefact:Agricultural_ProductionUnit.Specified.Crop_Plot",
                    "@type": "unece:AssociationBIE",
                    "unece:cefactUNId": "UN01012249",
                    "unece:cefactBieDomainClass": "cefact:Agricultural_ProductionUnit.Details",
                    "rdfs:comment": "A crop plot specified for this agricultural production unit."
                },
                {
                    "@id": "cefact:Specified_GeographicalGrid.Specified.Crop_Plot",
                    "@type": "unece:AssociationBIE",
                    "unece:cefactUNId": "UN01012212",
                    "unece:cefactBieDomainClass": "cefact:Specified_GeographicalGrid.Details",
                    "rdfs:comment": "A crop plot specified for this geographical grid."
                }
            ]
        },
        {
            "@id": "agriculture:specifiedProduce",
            "@type": "rdf:Property",
            "schema:rangeIncludes": {
                "@id": "agriculture:Produce"
            },
            "schema:domainIncludes": {
                "@id": "agriculture:Batch"
            },
            "rdfs:comment": "A crop produce specified for this crop produce batch.",
            "rdfs:label": "specifiedProduce",
            "unece:cefactElementMetadata": [
                {
                    "@id": "cefact:CropProduce_Batch.Specified.Crop_Produce",
                    "@type": "unece:AssociationBIE",
                    "unece:cefactUNId": "UN01012345",
                    "unece:cefactBieDomainClass": "cefact:CropProduce_Batch.Details",
                    "rdfs:comment": "A crop produce specified for this crop produce batch."
                }
            ]
        },
        {
            "@id": "agriculture:specifiedProduct",
            "@type": "rdf:Property",
            "schema:rangeIncludes": {
                "@id": "agriculture:Product"
            },
            "schema:domainIncludes": {
                "@id": "agriculture:Batch"
            },
            "rdfs:comment": [
                "An agricultural input product specified for this product batch.",
                "Track and Trace (TT) additional product information for the species in this animal batch."
            ],
            "rdfs:label": "specifiedProduct",
            "unece:cefactElementMetadata": [
                {
                    "@id": "cefact:Product_Batch.Specified.AgriculturalInput_Product",
                    "@type": "unece:AssociationBIE",
                    "unece:cefactUNId": "UN01012357",
                    "unece:cefactBieDomainClass": "cefact:Product_Batch.Details",
                    "rdfs:comment": "An agricultural input product specified for this product batch."
                },
                {
                    "@id": "cefact:Animal_Batch.Specified.SpeciesAdditional_TT_Product",
                    "@type": "unece:AssociationBIE",
                    "unece:cefactUNId": "UN01011256",
                    "unece:cefactBieDomainClass": "cefact:Animal_Batch.Details",
                    "rdfs:comment": "Track and Trace (TT) additional product information for the species in this animal batch."
                }
            ]
        },
        {
            "@id": "agriculture:specifiedProduction",
            "@type": "rdf:Property",
            "schema:rangeIncludes": {
                "@id": "agriculture:Production"
            },
            "schema:domainIncludes": {
                "@id": "agriculture:Batch"
            },
            "rdfs:comment": "Track and Trace (TT) additional production information for the species specified in this animal batch.",
            "rdfs:label": "specifiedProduction",
            "unece:cefactElementMetadata": [
                {
                    "@id": "cefact:Animal_Batch.Specified.SpeciesAdditional_TT_Production",
                    "@type": "unece:AssociationBIE",
                    "unece:cefactUNId": "UN01012663",
                    "unece:cefactBieDomainClass": "cefact:Animal_Batch.Details",
                    "rdfs:comment": "Track and Trace (TT) additional production information for the species specified in this animal batch."
                }
            ]
        },
        {
            "@id": "agriculture:specifiedQuantity",
            "@type": "rdf:Property",
            "schema:rangeIncludes": {
                "@id": "xsd:decimal"
            },
            "schema:domainIncludes": {
                "@id": "agriculture:Batch"
            },
            "rdfs:comment": "The quantity specified for this crop produce batch.",
            "rdfs:label": "specifiedQuantity",
            "unece:cefactElementMetadata": [
                {
                    "@id": "cefact:CropProduce_Batch.Specified.Quantity",
                    "@type": "unece:BasicBIE",
                    "unece:cefactUNId": "UN01012339",
                    "unece:cefactBieDomainClass": "cefact:CropProduce_Batch.Details",
                    "rdfs:comment": "The quantity specified for this crop produce batch."
                }
            ]
        },
        {
            "@id": "agriculture:specifiedReason",
            "@type": "rdf:Property",
            "schema:rangeIncludes": {
                "@id": "agriculture:Reason"
            },
            "schema:domainIncludes": {
                "@id": "agriculture:AgriculturalProcess"
            },
            "rdfs:comment": "An agricultural process reason specified for this plot agricultural process.",
            "rdfs:label": "specifiedReason",
            "unece:cefactElementMetadata": [
                {
                    "@id": "cefact:Plot_AgriculturalProcess.Specified.AgriculturalProcess_Reason",
                    "@type": "unece:AssociationBIE",
                    "unece:cefactUNId": "UN01002789",
                    "unece:cefactBieDomainClass": "cefact:Plot_AgriculturalProcess.Details",
                    "rdfs:comment": "An agricultural process reason specified for this plot agricultural process."
                }
            ]
        },
        {
            "@id": "agriculture:specifiedReference",
            "@type": "rdf:Property",
            "schema:rangeIncludes": {
                "@id": "agriculture:Reference"
            },
            "schema:domainIncludes": [
                {
                    "@id": "agriculture:Sample"
                },
                {
                    "@id": "agriculture:SampledObject"
                }
            ],
            "rdfs:comment": [
                "A laboratory observation reference specified for this agricultural sample.",
                "A laboratory observation reference specified for this agricultural sampled object."
            ],
            "rdfs:label": "specifiedReference",
            "unece:cefactElementMetadata": [
                {
                    "@id": "cefact:Agricultural_Sample.Specified.LaboratoryObservation_Reference",
                    "@type": "unece:AssociationBIE",
                    "unece:cefactUNId": "UN01009607",
                    "unece:cefactBieDomainClass": "cefact:Agricultural_Sample.Details",
                    "rdfs:comment": "A laboratory observation reference specified for this agricultural sample."
                },
                {
                    "@id": "cefact:Agricultural_SampledObject.Specified.LaboratoryObservation_Reference",
                    "@type": "unece:AssociationBIE",
                    "unece:cefactUNId": "UN01011090",
                    "unece:cefactBieDomainClass": "cefact:Agricultural_SampledObject.Details",
                    "rdfs:comment": "A laboratory observation reference specified for this agricultural sampled object."
                }
            ]
        },
        {
            "@id": "agriculture:specifiedSampleType",
            "@type": "rdf:Property",
            "schema:rangeIncludes": {
                "@id": "agriculture:SampleType"
            },
            "schema:domainIncludes": {
                "@id": "agriculture:Sample"
            },
            "rdfs:comment": "The sample type specified for this agricultural sample.",
            "rdfs:label": "specifiedSampleType",
            "unece:cefactElementMetadata": [
                {
                    "@id": "cefact:Agricultural_Sample.Specified.Agricultural_SampleType",
                    "@type": "unece:AssociationBIE",
                    "unece:cefactUNId": "UN01009606",
                    "unece:cefactBieDomainClass": "cefact:Agricultural_Sample.Details",
                    "rdfs:comment": "The sample type specified for this agricultural sample."
                }
            ]
        },
        {
            "@id": "agriculture:specifiedSampledObject",
            "@type": "rdf:Property",
            "schema:rangeIncludes": {
                "@id": "agriculture:SampledObject"
            },
            "schema:domainIncludes": {
                "@id": "agriculture:Sample"
            },
            "rdfs:comment": "The sampled object specified for this agricultural sample.",
            "rdfs:label": "specifiedSampledObject",
            "unece:cefactElementMetadata": [
                {
                    "@id": "cefact:Agricultural_Sample.Specified.Agricultural_SampledObject",
                    "@type": "unece:AssociationBIE",
                    "unece:cefactUNId": "UN01009605",
                    "unece:cefactBieDomainClass": "cefact:Agricultural_Sample.Details",
                    "rdfs:comment": "The sampled object specified for this agricultural sample."
                }
            ]
        },
        {
            "@id": "agriculture:specifiedTargetObject",
            "@type": "rdf:Property",
            "schema:rangeIncludes": {
                "@id": "agriculture:TargetObject"
            },
            "schema:domainIncludes": [
                {
                    "@id": "agriculture:AgriculturalProcess"
                },
                {
                    "@id": "agriculture:AgronomicalObservation"
                }
            ],
            "rdfs:comment": [
                "An agricultural process target object specified for this plot agricultural process.",
                "An agronomical observation target object specified for this single agronomical observation."
            ],
            "rdfs:label": "specifiedTargetObject",
            "unece:cefactElementMetadata": [
                {
                    "@id": "cefact:Plot_AgriculturalProcess.Specified.AgriculturalProcess_TargetObject",
                    "@type": "unece:AssociationBIE",
                    "unece:cefactUNId": "UN01002797",
                    "unece:cefactBieDomainClass": "cefact:Plot_AgriculturalProcess.Details",
                    "rdfs:comment": "An agricultural process target object specified for this plot agricultural process."
                },
                {
                    "@id": "cefact:Single_AgronomicalObservation.Specified.AgronomicalObservation_TargetObject",
                    "@type": "unece:AssociationBIE",
                    "unece:cefactUNId": "UN01009315",
                    "unece:cefactBieDomainClass": "cefact:Single_AgronomicalObservation.Details",
                    "rdfs:comment": "An agronomical observation target object specified for this single agronomical observation."
                }
            ]
        },
        {
            "@id": "agriculture:specifiedTissue",
            "@type": "rdf:Property",
            "schema:rangeIncludes": {
                "@id": "agriculture:Tissue"
            },
            "schema:domainIncludes": {
                "@id": "agriculture:SampleType"
            },
            "rdfs:comment": "The tissue specified for this agricultural sample type.",
            "rdfs:label": "specifiedTissue",
            "unece:cefactElementMetadata": [
                {
                    "@id": "cefact:Agricultural_SampleType.Specified.AgriculturalSample_Tissue",
                    "@type": "unece:AssociationBIE",
                    "unece:cefactUNId": "UN01009582",
                    "unece:cefactBieDomainClass": "cefact:Agricultural_SampleType.Details",
                    "rdfs:comment": "The tissue specified for this agricultural sample type."
                }
            ]
        },
        {
            "@id": "agriculture:specifiedWaterLocation",
            "@type": "rdf:Property",
            "schema:rangeIncludes": {
                "@id": "agriculture:WaterLocation"
            },
            "schema:domainIncludes": {
                "@id": "agriculture:SampledObject"
            },
            "rdfs:comment": "The water location specified for this sampled agricultural object.",
            "rdfs:label": "specifiedWaterLocation",
            "unece:cefactElementMetadata": [
                {
                    "@id": "cefact:Agricultural_SampledObject.Specified.SampledObject_WaterLocation",
                    "@type": "unece:AssociationBIE",
                    "unece:cefactUNId": "UN01009644",
                    "unece:cefactBieDomainClass": "cefact:Agricultural_SampledObject.Details",
                    "rdfs:comment": "The water location specified for this sampled agricultural object."
                }
            ]
        },
        {
            "@id": "agriculture:specifiedWeatherCondition",
            "@type": "rdf:Property",
            "schema:rangeIncludes": {
                "@id": "agriculture:WeatherCondition"
            },
            "schema:domainIncludes": {
                "@id": "agriculture:Crop"
            },
            "rdfs:comment": "An agricultural extreme weather condition specified for this field crop.",
            "rdfs:label": "specifiedWeatherCondition",
            "unece:cefactElementMetadata": [
                {
                    "@id": "cefact:Field_Crop.Specified.AgriculturalExtreme_WeatherCondition",
                    "@type": "unece:AssociationBIE",
                    "unece:cefactUNId": "UN01012320",
                    "unece:cefactBieDomainClass": "cefact:Field_Crop.Details",
                    "rdfs:comment": "An agricultural extreme weather condition specified for this field crop."
                }
            ]
        },
        {
            "@id": "agriculture:standard",
            "@type": "rdf:Property",
            "schema:rangeIncludes": {
                "@id": "xsd:string"
            },
            "schema:domainIncludes": {
                "@id": "agriculture:Certification"
            },
            "rdfs:comment": "A standard, expressed as text, used for this animal certification.",
            "rdfs:label": "standard",
            "unece:cefactElementMetadata": [
                {
                    "@id": "cefact:Animal_Certification.Standard.Text",
                    "@type": "unece:BasicBIE",
                    "unece:cefactUNId": "UN01013723",
                    "unece:cefactBieDomainClass": "cefact:Animal_Certification.Details",
                    "rdfs:comment": "A standard, expressed as text, used for this animal certification."
                }
            ]
        },
        {
            "@id": "agriculture:standardTypeCode",
            "@type": "rdf:Property",
            "schema:rangeIncludes": {
                "@id": "xsd:token"
            },
            "schema:domainIncludes": [
                {
                    "@id": "agriculture:SampleType"
                },
                {
                    "@id": "agriculture:SampledObject"
                }
            ],
            "rdfs:comment": [
                "The code specifying the standard type of this agricultural sample type.",
                "The standard code specifying the type of sampled agricultural object."
            ],
            "rdfs:label": "standardTypeCode",
            "unece:cefactElementMetadata": [
                {
                    "@id": "cefact:Agricultural_SampleType.Standard_Type.Code",
                    "@type": "unece:BasicBIE",
                    "unece:cefactUNId": "UN01009579",
                    "unece:cefactBieDomainClass": "cefact:Agricultural_SampleType.Details",
                    "rdfs:comment": "The code specifying the standard type of this agricultural sample type."
                },
                {
                    "@id": "cefact:Agricultural_SampledObject.Standard_Type.Code",
                    "@type": "unece:BasicBIE",
                    "unece:cefactUNId": "UN01009612",
                    "unece:cefactBieDomainClass": "cefact:Agricultural_SampledObject.Details",
                    "rdfs:comment": "The standard code specifying the type of sampled agricultural object."
                }
            ]
        },
        {
            "@id": "agriculture:startDate",
            "@type": "rdf:Property",
            "schema:rangeIncludes": {
                "@id": "xsd:base64Binary"
            },
            "schema:domainIncludes": {
                "@id": "agriculture:Contract"
            },
            "rdfs:comment": "The date on which this soil occupation contract starts.",
            "rdfs:label": "startDate",
            "unece:cefactElementMetadata": [
                {
                    "@id": "cefact:SoilOccupation_Contract.Start.Date",
                    "@type": "unece:BasicBIE",
                    "unece:cefactUNId": "UN01002824",
                    "unece:cefactBieDomainClass": "cefact:SoilOccupation_Contract.Details",
                    "rdfs:comment": "The date on which this soil occupation contract starts."
                }
            ]
        },
        {
            "@id": "agriculture:startDateTime",
            "@type": "rdf:Property",
            "schema:rangeIncludes": {
                "@id": "xsd:dateTime"
            },
            "schema:domainIncludes": [
                {
                    "@id": "agriculture:CropProductionCycle"
                },
                {
                    "@id": "agriculture:Period"
                },
                {
                    "@id": "agriculture:Plot"
                },
                {
                    "@id": "agriculture:SoilOccupation"
                }
            ],
            "rdfs:comment": [
                "The date or date time value for the start of this plot soil occupation.",
                "The date or date time value of the start of this agricultural crop production cycle.",
                "The date, time, date time or other date time value for the start of this SPS period.",
                "The date, time, date time, or other date time value for the start of this crop plot."
            ],
            "rdfs:label": "startDateTime",
            "unece:cefactElementMetadata": [
                {
                    "@id": "cefact:Agricultural_CropProductionCycle.Start.DateTime",
                    "@type": "unece:BasicBIE",
                    "unece:cefactUNId": "UN01002764",
                    "unece:cefactBieDomainClass": "cefact:Agricultural_CropProductionCycle.Details",
                    "rdfs:comment": "The date or date time value of the start of this agricultural crop production cycle."
                },
                {
                    "@id": "cefact:Crop_Plot.Start.DateTime",
                    "@type": "unece:BasicBIE",
                    "unece:cefactUNId": "UN01012140",
                    "unece:cefactBieDomainClass": "cefact:Crop_Plot.Details",
                    "rdfs:comment": "The date, time, date time, or other date time value for the start of this crop plot."
                },
                {
                    "@id": "cefact:Plot_SoilOccupation.Start.DateTime",
                    "@type": "unece:BasicBIE",
                    "unece:cefactUNId": "UN01002752",
                    "unece:cefactBieDomainClass": "cefact:Plot_SoilOccupation.Details",
                    "rdfs:comment": "The date or date time value for the start of this plot soil occupation."
                },
                {
                    "@id": "cefact:SPS_Period.Start.DateTime",
                    "@type": "unece:BasicBIE",
                    "unece:cefactUNId": "UN03000120",
                    "unece:cefactBieDomainClass": "cefact:SPS_Period.Details",
                    "rdfs:comment": "The date, time, date time or other date time value for the start of this SPS period."
                }
            ]
        },
        {
            "@id": "agriculture:statement",
            "@type": "rdf:Property",
            "schema:rangeIncludes": {
                "@id": "xsd:string"
            },
            "schema:domainIncludes": {
                "@id": "agriculture:ExaminationResult"
            },
            "rdfs:comment": "A statement, expressed as text, for this animal examination result.",
            "rdfs:label": "statement",
            "unece:cefactElementMetadata": [
                {
                    "@id": "cefact:Animal_ExaminationResult.Statement.Text",
                    "@type": "unece:BasicBIE",
                    "unece:cefactUNId": "UN01007683",
                    "unece:cefactBieDomainClass": "cefact:Animal_ExaminationResult.Details",
                    "rdfs:comment": "A statement, expressed as text, for this animal examination result."
                }
            ]
        },
        {
            "@id": "agriculture:statusCode",
            "@type": "rdf:Property",
            "schema:rangeIncludes": {
                "@id": "xsd:token"
            },
            "schema:domainIncludes": [
                {
                    "@id": "agriculture:AgriculturalProcess"
                },
                {
                    "@id": "agriculture:AgronomicalObservation"
                }
            ],
            "rdfs:comment": [
                "The code specifying the status for this single agronomical observation.",
                "The code specifying the status of the agricultural process for this crop production."
            ],
            "rdfs:label": "statusCode",
            "unece:cefactElementMetadata": [
                {
                    "@id": "cefact:CropProduction_AgriculturalProcess.Status.Code",
                    "@type": "unece:BasicBIE",
                    "unece:cefactUNId": "UN01012415",
                    "unece:cefactBieDomainClass": "cefact:CropProduction_AgriculturalProcess.Details",
                    "rdfs:comment": "The code specifying the status of the agricultural process for this crop production."
                },
                {
                    "@id": "cefact:Single_AgronomicalObservation.Status.Code",
                    "@type": "unece:BasicBIE",
                    "unece:cefactUNId": "UN01009313",
                    "unece:cefactBieDomainClass": "cefact:Single_AgronomicalObservation.Details",
                    "rdfs:comment": "The code specifying the status for this single agronomical observation."
                }
            ]
        },
        {
            "@id": "agriculture:storageEvent",
            "@type": "rdf:Property",
            "schema:rangeIncludes": {
                "@id": "agriculture:Event"
            },
            "schema:domainIncludes": {
                "@id": "agriculture:Consignment"
            },
            "rdfs:comment": "A storage event for this SPS consignment.",
            "rdfs:label": "storageEvent",
            "unece:cefactElementMetadata": [
                {
                    "@id": "cefact:SPS_Consignment.Storage.SPS_Event",
                    "@type": "unece:AssociationBIE",
                    "unece:cefactUNId": "UN03000062",
                    "unece:cefactBieDomainClass": "cefact:SPS_Consignment.Details",
                    "rdfs:comment": "A storage event for this SPS consignment."
                }
            ]
        },
        {
            "@id": "agriculture:storageTemperatureMeasure",
            "@type": "rdf:Property",
            "schema:rangeIncludes": {
                "@id": "xsd:decimal"
            },
            "schema:domainIncludes": {
                "@id": "agriculture:Sample"
            },
            "rdfs:comment": "The measure of the storage temperature for this agricultural sample.",
            "rdfs:label": "storageTemperatureMeasure",
            "unece:cefactElementMetadata": [
                {
                    "@id": "cefact:Agricultural_Sample.Storage_Temperature.Measure",
                    "@type": "unece:BasicBIE",
                    "unece:cefactUNId": "UN01009597",
                    "unece:cefactBieDomainClass": "cefact:Agricultural_Sample.Details",
                    "rdfs:comment": "The measure of the storage temperature for this agricultural sample."
                }
            ]
        },
        {
            "@id": "agriculture:subject",
            "@type": "rdf:Property",
            "schema:rangeIncludes": {
                "@id": "xsd:string"
            },
            "schema:domainIncludes": {
                "@id": "agriculture:Note"
            },
            "rdfs:comment": "The subject, expressed as text, of this SPS note.",
            "rdfs:label": "subject",
            "unece:cefactElementMetadata": [
                {
                    "@id": "cefact:SPS_Note.Subject.Text",
                    "@type": "unece:BasicBIE",
                    "unece:TDED": "4148",
                    "unece:cefactUNId": "UN03000097",
                    "unece:cefactBieDomainClass": "cefact:SPS_Note.Details",
                    "rdfs:comment": "The subject, expressed as text, of this SPS note."
                }
            ]
        },
        {
            "@id": "agriculture:subjectCode",
            "@type": "rdf:Property",
            "schema:rangeIncludes": {
                "@id": "xsd:token"
            },
            "schema:domainIncludes": {
                "@id": "agriculture:Note"
            },
            "rdfs:comment": "The code specifying the subject of this SPS note.",
            "rdfs:label": "subjectCode",
            "unece:cefactElementMetadata": [
                {
                    "@id": "cefact:SPS_Note.Subject.Code",
                    "@type": "unece:BasicBIE",
                    "unece:TDED": "4149",
                    "unece:cefactUNId": "UN03000100",
                    "unece:cefactBieDomainClass": "cefact:SPS_Note.Details",
                    "rdfs:comment": "The code specifying the subject of this SPS note."
                }
            ]
        },
        {
            "@id": "agriculture:subjectCrop",
            "@type": "rdf:Property",
            "schema:rangeIncludes": {
                "@id": "agriculture:Crop"
            },
            "schema:domainIncludes": {
                "@id": "agriculture:AgronomicalObservation"
            },
            "rdfs:comment": "The agricultural crop that is the subject of this single agronomical observation.",
            "rdfs:label": "subjectCrop",
            "unece:cefactElementMetadata": [
                {
                    "@id": "cefact:Single_AgronomicalObservation.Subject.Agricultural_Crop",
                    "@type": "unece:AssociationBIE",
                    "unece:cefactUNId": "UN01009316",
                    "unece:cefactBieDomainClass": "cefact:Single_AgronomicalObservation.Details",
                    "rdfs:comment": "The agricultural crop that is the subject of this single agronomical observation."
                }
            ]
        },
        {
            "@id": "agriculture:submitterParty",
            "@type": "rdf:Property",
            "schema:rangeIncludes": {
                "@id": "agriculture:Party"
            },
            "schema:domainIncludes": {
                "@id": "agriculture:Document"
            },
            "rdfs:comment": "The party submitting this agronomical observation document.",
            "rdfs:label": "submitterParty",
            "unece:cefactElementMetadata": [
                {
                    "@id": "cefact:AgronomicalObservation_Document.Submitter.AgronomicalObservation_Party",
                    "@type": "unece:AssociationBIE",
                    "unece:cefactUNId": "UN01009300",
                    "unece:cefactBieDomainClass": "cefact:AgronomicalObservation_Document.Details",
                    "rdfs:comment": "The party submitting this agronomical observation document."
                }
            ]
        },
        {
            "@id": "agriculture:subordinateArea",
            "@type": "rdf:Property",
            "schema:rangeIncludes": {
                "@id": "agriculture:Area"
            },
            "schema:domainIncludes": {
                "@id": "agriculture:Area"
            },
            "rdfs:comment": "An agricultural zone area subordinate to this agricultural zone area.",
            "rdfs:label": "subordinateArea",
            "unece:cefactElementMetadata": [
                {
                    "@id": "cefact:AgriculturalZone_Area.Subordinate.AgriculturalZone_Area",
                    "@type": "unece:AssociationBIE",
                    "unece:cefactUNId": "UN01012221",
                    "unece:cefactBieDomainClass": "cefact:AgriculturalZone_Area.Details",
                    "rdfs:comment": "An agricultural zone area subordinate to this agricultural zone area."
                }
            ]
        },
        {
            "@id": "agriculture:subordinateConstruction",
            "@type": "rdf:Property",
            "schema:rangeIncludes": {
                "@id": "agriculture:Construction"
            },
            "schema:domainIncludes": {
                "@id": "agriculture:Construction"
            },
            "rdfs:comment": "An agricultural construction subordinate to this agricultural construction.",
            "rdfs:label": "subordinateConstruction",
            "unece:cefactElementMetadata": [
                {
                    "@id": "cefact:Agricultural_Construction.Subordinate.Agricultural_Construction",
                    "@type": "unece:AssociationBIE",
                    "unece:cefactUNId": "UN01012243",
                    "unece:cefactBieDomainClass": "cefact:Agricultural_Construction.Details",
                    "rdfs:comment": "An agricultural construction subordinate to this agricultural construction."
                }
            ]
        },
        {
            "@id": "agriculture:subordinateCoordinateReferenceSystem",
            "@type": "rdf:Property",
            "schema:rangeIncludes": {
                "@id": "agriculture:CoordinateReferenceSystem"
            },
            "schema:domainIncludes": {
                "@id": "agriculture:CoordinateReferenceSystem"
            },
            "rdfs:comment": "A CS engineering coordinate reference system subordinate to this CS engineering coordinate reference system.",
            "rdfs:label": "subordinateCoordinateReferenceSystem",
            "unece:cefactElementMetadata": [
                {
                    "@id": "cefact:CSEngineering_CoordinateReferenceSystem.Subordinate.CSEngineering_CoordinateReferenceSystem",
                    "@type": "unece:AssociationBIE",
                    "unece:cefactUNId": "UN01012166",
                    "unece:cefactBieDomainClass": "cefact:CSEngineering_CoordinateReferenceSystem.Details",
                    "rdfs:comment": "A CS engineering coordinate reference system subordinate to this CS engineering coordinate reference system."
                }
            ]
        },
        {
            "@id": "agriculture:subordinateCountrySub-Division",
            "@type": "rdf:Property",
            "schema:rangeIncludes": {
                "@id": "agriculture:CountrySub-Division"
            },
            "schema:domainIncludes": [
                {
                    "@id": "agriculture:Country"
                },
                {
                    "@id": "agriculture:CountrySubDivision"
                }
            ],
            "rdfs:comment": [
                "A country sub-division that is subordinate to this SPS country, such as a state, a county, a canton, a province.",
                "A subordinate country sub-division within this SPS country sub-division."
            ],
            "rdfs:label": "subordinateCountrySub-Division",
            "unece:cefactElementMetadata": [
                {
                    "@id": "cefact:SPS_CountrySub-Division.Subordinate.SPS_CountrySub-Division",
                    "@type": "unece:AssociationBIE",
                    "unece:cefactUNId": "UN03000085",
                    "unece:cefactBieDomainClass": "cefact:SPS_CountrySubDivision.Details",
                    "rdfs:comment": "A subordinate country sub-division within this SPS country sub-division."
                },
                {
                    "@id": "cefact:SPS_Country.Subordinate.SPS_CountrySub-Division",
                    "@type": "unece:AssociationBIE",
                    "unece:cefactUNId": "UN03000090",
                    "unece:cefactBieDomainClass": "cefact:SPS_Country.Details",
                    "rdfs:comment": "A country sub-division that is subordinate to this SPS country, such as a state, a county, a canton, a province."
                }
            ]
        },
        {
            "@id": "agriculture:subordinateTypeCode",
            "@type": "rdf:Property",
            "schema:rangeIncludes": {
                "@id": "xsd:token"
            },
            "schema:domainIncludes": [
                {
                    "@id": "agriculture:AgriculturalDevice"
                },
                {
                    "@id": "agriculture:AgriculturalProcess"
                },
                {
                    "@id": "agriculture:Condition"
                },
                {
                    "@id": "agriculture:Construction"
                },
                {
                    "@id": "agriculture:CropInput"
                },
                {
                    "@id": "agriculture:CropStage"
                },
                {
                    "@id": "agriculture:Produce"
                },
                {
                    "@id": "agriculture:Reason"
                },
                {
                    "@id": "agriculture:TargetObject"
                }
            ],
            "rdfs:comment": [
                "A code specifying a subordinate type for this agricultural construction.",
                "The code specifying the subordinate type for this agricultural process condition, such as wind, rain or snow.",
                "The code specifying the subordinate type for this agricultural process crop input.",
                "The code specifying the subordinate type for this agricultural process crop stage, such as phenological growth stage.",
                "The code specifying the subordinate type for this agricultural process reason, such as technical advices, analysis results, plant diseases or pests.",
                "The code specifying the subordinate type for this agricultural process target object.",
                "The code specifying the subordinate type for this agricultural produce, such as product or by-product.",
                "The code specifying the subordinate type for this plot agricultural process.",
                "The code specifying the subordinate type for this specified agricultural device.",
                "The code specifying the subordinate type of crop produce, such as product or by-product.",
                "The code specifying the subordinate type of the agricultural process for this crop production."
            ],
            "rdfs:label": "subordinateTypeCode",
            "unece:cefactElementMetadata": [
                {
                    "@id": "cefact:AgriculturalProcess_CropStage.Subordinate_Type.Code",
                    "@type": "unece:BasicBIE",
                    "unece:cefactUNId": "UN01002697",
                    "unece:cefactBieDomainClass": "cefact:AgriculturalProcess_CropStage.Details",
                    "rdfs:comment": "The code specifying the subordinate type for this agricultural process crop stage, such as phenological growth stage."
                },
                {
                    "@id": "cefact:Agricultural_Construction.Subordinate_Type.Code",
                    "@type": "unece:BasicBIE",
                    "unece:cefactUNId": "UN01012230",
                    "unece:cefactBieDomainClass": "cefact:Agricultural_Construction.Details",
                    "rdfs:comment": "A code specifying a subordinate type for this agricultural construction."
                },
                {
                    "@id": "cefact:Plot_AgriculturalProcess.Subordinate_Type.Code",
                    "@type": "unece:BasicBIE",
                    "unece:cefactUNId": "UN01002785",
                    "unece:cefactBieDomainClass": "cefact:Plot_AgriculturalProcess.Details",
                    "rdfs:comment": "The code specifying the subordinate type for this plot agricultural process."
                },
                {
                    "@id": "cefact:Crop_Produce.Subordinate_Type.Code",
                    "@type": "unece:BasicBIE",
                    "unece:cefactUNId": "UN01012327",
                    "unece:cefactBieDomainClass": "cefact:Crop_Produce.Details",
                    "rdfs:comment": "The code specifying the subordinate type of crop produce, such as product or by-product."
                },
                {
                    "@id": "cefact:Agricultural_Produce.Subordinate_Type.Code",
                    "@type": "unece:BasicBIE",
                    "unece:cefactUNId": "UN01002701",
                    "unece:cefactBieDomainClass": "cefact:Agricultural_Produce.Details",
                    "rdfs:comment": "The code specifying the subordinate type for this agricultural produce, such as product or by-product."
                },
                {
                    "@id": "cefact:Specified_AgriculturalDevice.Subordinate_Type.Code",
                    "@type": "unece:BasicBIE",
                    "unece:cefactUNId": "UN01002739",
                    "unece:cefactBieDomainClass": "cefact:Specified_AgriculturalDevice.Details",
                    "rdfs:comment": "The code specifying the subordinate type for this specified agricultural device."
                },
                {
                    "@id": "cefact:AgriculturalProcess_Reason.Subordinate_Type.Code",
                    "@type": "unece:BasicBIE",
                    "unece:cefactUNId": "UN01002743",
                    "unece:cefactBieDomainClass": "cefact:AgriculturalProcess_Reason.Details",
                    "rdfs:comment": "The code specifying the subordinate type for this agricultural process reason, such as technical advices, analysis results, plant diseases or pests."
                },
                {
                    "@id": "cefact:CropProduction_AgriculturalProcess.Subordinate_Type.Code",
                    "@type": "unece:BasicBIE",
                    "unece:cefactUNId": "UN01012410",
                    "unece:cefactBieDomainClass": "cefact:CropProduction_AgriculturalProcess.Details",
                    "rdfs:comment": "The code specifying the subordinate type of the agricultural process for this crop production."
                },
                {
                    "@id": "cefact:AgriculturalProcess_Condition.Subordinate_Type.Code",
                    "@type": "unece:BasicBIE",
                    "unece:cefactUNId": "UN01002683",
                    "unece:cefactBieDomainClass": "cefact:AgriculturalProcess_Condition.Details",
                    "rdfs:comment": "The code specifying the subordinate type for this agricultural process condition, such as wind, rain or snow."
                },
                {
                    "@id": "cefact:AgriculturalProcess_TargetObject.Subordinate_Type.Code",
                    "@type": "unece:BasicBIE",
                    "unece:cefactUNId": "UN01002772",
                    "unece:cefactBieDomainClass": "cefact:AgriculturalProcess_TargetObject.Details",
                    "rdfs:comment": "The code specifying the subordinate type for this agricultural process target object."
                },
                {
                    "@id": "cefact:AgriculturalProcess_CropInput.Subordinate_Type.Code",
                    "@type": "unece:BasicBIE",
                    "unece:cefactUNId": "UN01002727",
                    "unece:cefactBieDomainClass": "cefact:AgriculturalProcess_CropInput.Details",
                    "rdfs:comment": "The code specifying the subordinate type for this agricultural process crop input."
                }
            ]
        },
        {
            "@id": "agriculture:subtypeCode",
            "@type": "rdf:Property",
            "schema:rangeIncludes": {
                "@id": "xsd:token"
            },
            "schema:domainIncludes": [
                {
                    "@id": "agriculture:Scope"
                },
                {
                    "@id": "agriculture:TargetObject"
                }
            ],
            "rdfs:comment": [
                "The code specifying the subtype of this agronomical observation scope.",
                "The code specifying the subtype of this agronomical observation target object."
            ],
            "rdfs:label": "subtypeCode",
            "unece:cefactElementMetadata": [
                {
                    "@id": "cefact:AgronomicalObservation_Scope.Subtype.Code",
                    "@type": "unece:BasicBIE",
                    "unece:cefactUNId": "UN01009327",
                    "unece:cefactBieDomainClass": "cefact:AgronomicalObservation_Scope.Details",
                    "rdfs:comment": "The code specifying the subtype of this agronomical observation scope."
                },
                {
                    "@id": "cefact:AgronomicalObservation_TargetObject.Subtype.Code",
                    "@type": "unece:BasicBIE",
                    "unece:cefactUNId": "UN01009320",
                    "unece:cefactBieDomainClass": "cefact:AgronomicalObservation_TargetObject.Details",
                    "rdfs:comment": "The code specifying the subtype of this agronomical observation target object."
                }
            ]
        },
        {
            "@id": "agriculture:superordinateCountrySub-Division",
            "@type": "rdf:Property",
            "schema:rangeIncludes": {
                "@id": "agriculture:CountrySub-Division"
            },
            "schema:domainIncludes": {
                "@id": "agriculture:CountrySubDivision"
            },
            "rdfs:comment": "A superordinate country sub-division for this SPS country sub-division.",
            "rdfs:label": "superordinateCountrySub-Division",
            "unece:cefactElementMetadata": [
                {
                    "@id": "cefact:SPS_CountrySub-Division.Superordinate.SPS_CountrySub-Division",
                    "@type": "unece:AssociationBIE",
                    "unece:cefactUNId": "UN03000084",
                    "unece:cefactBieDomainClass": "cefact:SPS_CountrySubDivision.Details",
                    "rdfs:comment": "A superordinate country sub-division for this SPS country sub-division."
                }
            ]
        },
        {
            "@id": "agriculture:supplementaryBotanicalSpeciesCode",
            "@type": "rdf:Property",
            "schema:rangeIncludes": {
                "@id": "xsd:token"
            },
            "schema:domainIncludes": {
                "@id": "agriculture:Crop"
            },
            "rdfs:comment": "The code specifying the supplementary botanical species for this agricultural crop.",
            "rdfs:label": "supplementaryBotanicalSpeciesCode",
            "unece:cefactElementMetadata": [
                {
                    "@id": "cefact:Agricultural_Crop.Supplementary_BotanicalSpecies.Code",
                    "@type": "unece:BasicBIE",
                    "unece:cefactUNId": "UN01002687",
                    "unece:cefactBieDomainClass": "cefact:Agricultural_Crop.Details",
                    "rdfs:comment": "The code specifying the supplementary botanical species for this agricultural crop."
                }
            ]
        },
        {
            "@id": "agriculture:supplierParty",
            "@type": "rdf:Property",
            "schema:rangeIncludes": {
                "@id": "agriculture:Party"
            },
            "schema:domainIncludes": [
                {
                    "@id": "agriculture:CropInput"
                },
                {
                    "@id": "agriculture:SampledObject"
                },
                {
                    "@id": "agriculture:SoilSupplement"
                }
            ],
            "rdfs:comment": [
                "The crop data sheet party that supplies this agricultural process crop input.",
                "The crop data sheet party that supplies this specified soil supplement.",
                "The supplier party for this sampled agricultural object."
            ],
            "rdfs:label": "supplierParty",
            "unece:cefactElementMetadata": [
                {
                    "@id": "cefact:AgriculturalProcess_CropInput.Supplier.CropDataSheet_Party",
                    "@type": "unece:AssociationBIE",
                    "unece:cefactUNId": "UN01002735",
                    "unece:cefactBieDomainClass": "cefact:AgriculturalProcess_CropInput.Details",
                    "rdfs:comment": "The crop data sheet party that supplies this agricultural process crop input."
                },
                {
                    "@id": "cefact:Agricultural_SampledObject.Supplier.LaboratoryObservation_Party",
                    "@type": "unece:AssociationBIE",
                    "unece:cefactUNId": "UN01009632",
                    "unece:cefactBieDomainClass": "cefact:Agricultural_SampledObject.Details",
                    "rdfs:comment": "The supplier party for this sampled agricultural object."
                },
                {
                    "@id": "cefact:Specified_SoilSupplement.Supplier.CropDataSheet_Party",
                    "@type": "unece:AssociationBIE",
                    "unece:cefactUNId": "UN01002722",
                    "unece:cefactBieDomainClass": "cefact:Specified_SoilSupplement.Details",
                    "rdfs:comment": "The crop data sheet party that supplies this specified soil supplement."
                }
            ]
        },
        {
            "@id": "agriculture:systemId",
            "@type": "rdf:Property",
            "schema:rangeIncludes": {
                "@id": "xsd:token"
            },
            "schema:domainIncludes": {
                "@id": "agriculture:Classification"
            },
            "rdfs:comment": "The unique identifier of the classification system for this SPS classification.",
            "rdfs:label": "systemId",
            "unece:cefactElementMetadata": [
                {
                    "@id": "cefact:SPS_Classification.System.Identifier",
                    "@type": "unece:BasicBIE",
                    "unece:TDED": "9019",
                    "unece:cefactUNId": "UN03000043",
                    "unece:cefactBieDomainClass": "cefact:SPS_Classification.Details",
                    "rdfs:comment": "The unique identifier of the classification system for this SPS classification."
                }
            ]
        },
        {
            "@id": "agriculture:systemName",
            "@type": "rdf:Property",
            "schema:rangeIncludes": {
                "@id": "xsd:string"
            },
            "schema:domainIncludes": {
                "@id": "agriculture:Classification"
            },
            "rdfs:comment": "A name, expressed as text, of the classification system for this SPS classification.",
            "rdfs:label": "systemName",
            "unece:cefactElementMetadata": [
                {
                    "@id": "cefact:SPS_Classification.SystemName.Text",
                    "@type": "unece:BasicBIE",
                    "unece:TDED": "9018",
                    "unece:cefactUNId": "UN03000044",
                    "unece:cefactBieDomainClass": "cefact:SPS_Classification.Details",
                    "rdfs:comment": "A name, expressed as text, of the classification system for this SPS classification."
                }
            ]
        },
        {
            "@id": "agriculture:telephoneCommunication",
            "@type": "rdf:Property",
            "schema:rangeIncludes": {
                "@id": "agriculture:Communication"
            },
            "schema:domainIncludes": {
                "@id": "agriculture:Party"
            },
            "rdfs:comment": "Telephone communication information specified for this party.",
            "rdfs:label": "telephoneCommunication",
            "unece:cefactElementMetadata": [
                {
                    "@id": "cefact:Specified_Party.Telephone.Specified_Communication",
                    "@type": "unece:AssociationBIE",
                    "unece:cefactUNId": "UN01012460",
                    "unece:cefactBieDomainClass": "cefact:Specified_Party.Details",
                    "rdfs:comment": "Telephone communication information specified for this party."
                }
            ]
        },
        {
            "@id": "agriculture:temperatureTypeCode",
            "@type": "rdf:Property",
            "schema:rangeIncludes": {
                "@id": "unece:UNECECL6245Code"
            },
            "schema:domainIncludes": {
                "@id": "agriculture:Temperature"
            },
            "rdfs:comment": "The code specifying the type of SPS temperature.",
            "rdfs:label": "temperatureTypeCode",
            "unece:cefactElementMetadata": [
                {
                    "@id": "cefact:SPS_Temperature.Type.Code",
                    "@type": "unece:BasicBIE",
                    "unece:TDED": "6245",
                    "unece:cefactUNId": "UN03000145",
                    "unece:cefactBieDomainClass": "cefact:SPS_Temperature.Details",
                    "rdfs:comment": "The code specifying the type of SPS temperature."
                }
            ]
        },
        {
            "@id": "agriculture:thirdPartyIssuedId",
            "@type": "rdf:Property",
            "schema:rangeIncludes": {
                "@id": "xsd:token"
            },
            "schema:domainIncludes": [
                {
                    "@id": "agriculture:Area"
                },
                {
                    "@id": "agriculture:Contract"
                }
            ],
            "rdfs:comment": [
                "An identifier issued by a third party for this agricultural contract.",
                "An identifier issued by a third party for this agricultural zone area."
            ],
            "rdfs:label": "thirdPartyIssuedId",
            "unece:cefactElementMetadata": [
                {
                    "@id": "cefact:Agricultural_Contract.ThirdPartyIssued_Identification.Identifier",
                    "@type": "unece:BasicBIE",
                    "unece:TDED": "1296",
                    "unece:cefactUNId": "UN01012446",
                    "unece:cefactBieDomainClass": "cefact:Agricultural_Contract.Details",
                    "rdfs:comment": "An identifier issued by a third party for this agricultural contract."
                },
                {
                    "@id": "cefact:AgriculturalZone_Area.ThirdPartyIssued_Identification.Identifier",
                    "@type": "unece:BasicBIE",
                    "unece:cefactUNId": "UN01012216",
                    "unece:cefactBieDomainClass": "cefact:AgriculturalZone_Area.Details",
                    "rdfs:comment": "An identifier issued by a third party for this agricultural zone area."
                }
            ]
        },
        {
            "@id": "agriculture:traderParty",
            "@type": "rdf:Property",
            "schema:rangeIncludes": {
                "@id": "agriculture:Party"
            },
            "schema:domainIncludes": {
                "@id": "agriculture:SampledObject"
            },
            "rdfs:comment": "A trader party for this sampled agricultural object.",
            "rdfs:label": "traderParty",
            "unece:cefactElementMetadata": [
                {
                    "@id": "cefact:Agricultural_SampledObject.Trader.LaboratoryObservation_Party",
                    "@type": "unece:AssociationBIE",
                    "unece:cefactUNId": "UN01009634",
                    "unece:cefactBieDomainClass": "cefact:Agricultural_SampledObject.Details",
                    "rdfs:comment": "A trader party for this sampled agricultural object."
                }
            ]
        },
        {
            "@id": "agriculture:transitCountry",
            "@type": "rdf:Property",
            "schema:rangeIncludes": {
                "@id": "agriculture:Country"
            },
            "schema:domainIncludes": {
                "@id": "agriculture:Consignment"
            },
            "rdfs:comment": "A transit country for this SPS consignment.",
            "rdfs:label": "transitCountry",
            "unece:cefactElementMetadata": [
                {
                    "@id": "cefact:SPS_Consignment.Transit.SPS_Country",
                    "@type": "unece:AssociationBIE",
                    "unece:cefactUNId": "UN03000066",
                    "unece:cefactBieDomainClass": "cefact:SPS_Consignment.Details",
                    "rdfs:comment": "A transit country for this SPS consignment."
                }
            ]
        },
        {
            "@id": "agriculture:transitLocation",
            "@type": "rdf:Property",
            "schema:rangeIncludes": {
                "@id": "agriculture:Location"
            },
            "schema:domainIncludes": {
                "@id": "agriculture:Consignment"
            },
            "rdfs:comment": "A transit location for this SPS consignment.",
            "rdfs:label": "transitLocation",
            "unece:cefactElementMetadata": [
                {
                    "@id": "cefact:SPS_Consignment.Transit.SPS_Location",
                    "@type": "unece:AssociationBIE",
                    "unece:cefactUNId": "UN03000067",
                    "unece:cefactBieDomainClass": "cefact:SPS_Consignment.Details",
                    "rdfs:comment": "A transit location for this SPS consignment."
                }
            ]
        },
        {
            "@id": "agriculture:treatment",
            "@type": "rdf:Property",
            "schema:rangeIncludes": {
                "@id": "xsd:string"
            },
            "schema:domainIncludes": {
                "@id": "agriculture:SampledObject"
            },
            "rdfs:comment": "The treatment, expressed as text, for this sampled agricultural object, such as disinfection.",
            "rdfs:label": "treatment",
            "unece:cefactElementMetadata": [
                {
                    "@id": "cefact:Agricultural_SampledObject.Treatment.Text",
                    "@type": "unece:BasicBIE",
                    "unece:cefactUNId": "UN01009623",
                    "unece:cefactBieDomainClass": "cefact:Agricultural_SampledObject.Details",
                    "rdfs:comment": "The treatment, expressed as text, for this sampled agricultural object, such as disinfection."
                }
            ]
        },
        {
            "@id": "agriculture:type",
            "@type": "rdf:Property",
            "schema:rangeIncludes": {
                "@id": "xsd:string"
            },
            "schema:domainIncludes": [
                {
                    "@id": "agriculture:Autopsy"
                },
                {
                    "@id": "agriculture:Label"
                }
            ],
            "rdfs:comment": [
                "The type of animal label, expressed as text.",
                "The type, expressed as text, of this agricultural sample autopsy."
            ],
            "rdfs:label": "type",
            "unece:cefactElementMetadata": [
                {
                    "@id": "cefact:AgriculturalSample_Autopsy.Type.Text",
                    "@type": "unece:BasicBIE",
                    "unece:cefactUNId": "UN01009573",
                    "unece:cefactBieDomainClass": "cefact:AgriculturalSample_Autopsy.Details",
                    "rdfs:comment": "The type, expressed as text, of this agricultural sample autopsy."
                },
                {
                    "@id": "cefact:Animal_Label.Type.Text",
                    "@type": "unece:BasicBIE",
                    "unece:cefactUNId": "UN01007623",
                    "unece:cefactBieDomainClass": "cefact:Animal_Label.Details",
                    "rdfs:comment": "The type of animal label, expressed as text."
                }
            ]
        },
        {
            "@id": "agriculture:typeCode",
            "@type": "rdf:Property",
            "schema:rangeIncludes": {
                "@id": "xsd:token"
            },
            "schema:domainIncludes": [
                {
                    "@id": "agriculture:AgriculturalDevice"
                },
                {
                    "@id": "agriculture:AgriculturalProcess"
                },
                {
                    "@id": "agriculture:Area"
                },
                {
                    "@id": "agriculture:Batch"
                },
                {
                    "@id": "agriculture:Certificate"
                },
                {
                    "@id": "agriculture:Characteristic"
                },
                {
                    "@id": "agriculture:Chemical"
                },
                {
                    "@id": "agriculture:Condition"
                },
                {
                    "@id": "agriculture:Construction"
                },
                {
                    "@id": "agriculture:CountrySubDivision"
                },
                {
                    "@id": "agriculture:CropInput"
                },
                {
                    "@id": "agriculture:CropProtectionTreatment"
                },
                {
                    "@id": "agriculture:CropResidue"
                },
                {
                    "@id": "agriculture:CropStage"
                },
                {
                    "@id": "agriculture:Event"
                },
                {
                    "@id": "agriculture:Issue"
                },
                {
                    "@id": "agriculture:Material"
                },
                {
                    "@id": "agriculture:Package"
                },
                {
                    "@id": "agriculture:Party"
                },
                {
                    "@id": "agriculture:Produce"
                },
                {
                    "@id": "agriculture:Product"
                },
                {
                    "@id": "agriculture:ProductionUnit"
                },
                {
                    "@id": "agriculture:Reason"
                },
                {
                    "@id": "agriculture:Scope"
                },
                {
                    "@id": "agriculture:SoilOccupation"
                },
                {
                    "@id": "agriculture:SoilSupplement"
                },
                {
                    "@id": "agriculture:SpeciesVariety"
                },
                {
                    "@id": "agriculture:TargetObject"
                },
                {
                    "@id": "agriculture:WorkItem"
                }
            ],
            "rdfs:comment": [
                "A code specifying a type of agricultural construction, such as a building, greenhouse, installation, storage.",
                "A code specifying a type of agricultural input material.",
                "A code specifying a type of agricultural production unit.",
                "A code specifying a type of complaint issue.",
                "A code specifying the type of this SPS party that is independent of its role.",
                "The code specifying the type of SPS package.",
                "The code specifying the type of agricultural area, such as crop surface area.",
                "The code specifying the type of agricultural certificate.",
                "The code specifying the type of agricultural characteristic.",
                "The code specifying the type of agricultural country sub-division.",
                "The code specifying the type of agricultural input product.",
                "The code specifying the type of agricultural process condition, such as weather condition or soil condition.",
                "The code specifying the type of agricultural process crop input.",
                "The code specifying the type of agricultural process crop stage.",
                "The code specifying the type of agricultural process for this crop production.",
                "The code specifying the type of agricultural process reason.",
                "The code specifying the type of agricultural process target object, such as pests, diseases or weeds.",
                "The code specifying the type of agricultural process work item.",
                "The code specifying the type of agricultural produce.",
                "The code specifying the type of agronomical observation target object, such as pests, diseases or weeds.",
                "The code specifying the type of animal certificate.",
                "The code specifying the type of animal holding event.",
                "The code specifying the type of chemical for this agricultural input.",
                "The code specifying the type of crop input chemical, such as magnesium, nitrogen or zinc.",
                "The code specifying the type of crop produce batch.",
                "The code specifying the type of crop produce.",
                "The code specifying the type of crop protection treatment.",
                "The code specifying the type of crop species variety.",
                "The code specifying the type of plot agricultural process.",
                "The code specifying the type of plot soil occupation, such as main crop or catch crop.",
                "The code specifying the type of product batch.",
                "The code specifying the type of soil occupation crop residue.",
                "The code specifying the type of specified soil supplement.",
                "The code specifying the type of this agronomical observation scope, such as leaves, whole plant, plant stem.",
                "The code specifying the type of this specified agricultural device.",
                "The code specifying the type of veterinarian event, such as a vaccination."
            ],
            "rdfs:label": "typeCode",
            "unece:cefactElementMetadata": [
                {
                    "@id": "cefact:Agricultural_Certificate.Type.Code",
                    "@type": "unece:BasicBIE",
                    "unece:cefactUNId": "UN01012282",
                    "unece:cefactBieDomainClass": "cefact:Agricultural_Certificate.Details",
                    "rdfs:comment": "The code specifying the type of agricultural certificate."
                },
                {
                    "@id": "cefact:Product_Batch.Type.Code",
                    "@type": "unece:BasicBIE",
                    "unece:cefactUNId": "UN01012350",
                    "unece:cefactBieDomainClass": "cefact:Product_Batch.Details",
                    "rdfs:comment": "The code specifying the type of product batch."
                },
                {
                    "@id": "cefact:Crop_Produce.Type.Code",
                    "@type": "unece:BasicBIE",
                    "unece:cefactUNId": "UN01012326",
                    "unece:cefactBieDomainClass": "cefact:Crop_Produce.Details",
                    "rdfs:comment": "The code specifying the type of crop produce."
                },
                {
                    "@id": "cefact:CropInput_Chemical.Type.Code",
                    "@type": "unece:BasicBIE",
                    "unece:cefactUNId": "UN01002747",
                    "unece:cefactBieDomainClass": "cefact:CropInput_Chemical.Details",
                    "rdfs:comment": "The code specifying the type of crop input chemical, such as magnesium, nitrogen or zinc."
                },
                {
                    "@id": "cefact:CropProduce_Batch.Type.Code",
                    "@type": "unece:BasicBIE",
                    "unece:cefactUNId": "UN01012336",
                    "unece:cefactBieDomainClass": "cefact:CropProduce_Batch.Details",
                    "rdfs:comment": "The code specifying the type of crop produce batch."
                },
                {
                    "@id": "cefact:Veterinarian_Event.Type.Code",
                    "@type": "unece:BasicBIE",
                    "unece:TDED": "9171",
                    "unece:cefactUNId": "UN01007632",
                    "unece:cefactBieDomainClass": "cefact:Veterinarian_Event.Details",
                    "rdfs:comment": "The code specifying the type of veterinarian event, such as a vaccination."
                },
                {
                    "@id": "cefact:AgriculturalProcess_WorkItem.Type.Code",
                    "@type": "unece:BasicBIE",
                    "unece:cefactUNId": "UN01002805",
                    "unece:cefactBieDomainClass": "cefact:AgriculturalProcess_WorkItem.Details",
                    "rdfs:comment": "The code specifying the type of agricultural process work item."
                },
                {
                    "@id": "cefact:Plot_AgriculturalProcess.Type.Code",
                    "@type": "unece:BasicBIE",
                    "unece:cefactUNId": "UN01002784",
                    "unece:cefactBieDomainClass": "cefact:Plot_AgriculturalProcess.Details",
                    "rdfs:comment": "The code specifying the type of plot agricultural process."
                },
                {
                    "@id": "cefact:AgriculturalProcess_CropInput.Type.Code",
                    "@type": "unece:BasicBIE",
                    "unece:cefactUNId": "UN01002725",
                    "unece:cefactBieDomainClass": "cefact:AgriculturalProcess_CropInput.Details",
                    "rdfs:comment": "The code specifying the type of agricultural process crop input."
                },
                {
                    "@id": "cefact:Complaint_Issue.Type.Code",
                    "@type": "unece:BasicBIE",
                    "unece:cefactUNId": "UN01012268",
                    "unece:cefactBieDomainClass": "cefact:Complaint_Issue.Details",
                    "rdfs:comment": "A code specifying a type of complaint issue."
                },
                {
                    "@id": "cefact:SPS_Party.Type.Code",
                    "@type": "unece:BasicBIE",
                    "unece:cefactUNId": "UN03000115",
                    "unece:cefactBieDomainClass": "cefact:SPS_Party.Details",
                    "rdfs:comment": "A code specifying the type of this SPS party that is independent of its role."
                },
                {
                    "@id": "cefact:AgronomicalObservation_TargetObject.Type.Code",
                    "@type": "unece:BasicBIE",
                    "unece:cefactUNId": "UN01009319",
                    "unece:cefactBieDomainClass": "cefact:AgronomicalObservation_TargetObject.Details",
                    "rdfs:comment": "The code specifying the type of agronomical observation target object, such as pests, diseases or weeds."
                },
                {
                    "@id": "cefact:Agricultural_Construction.Type.Code",
                    "@type": "unece:BasicBIE",
                    "unece:cefactUNId": "UN01012229",
                    "unece:cefactBieDomainClass": "cefact:Agricultural_Construction.Details",
                    "rdfs:comment": "A code specifying a type of agricultural construction, such as a building, greenhouse, installation, storage."
                },
                {
                    "@id": "cefact:AgriculturalProcess_CropStage.Type.Code",
                    "@type": "unece:BasicBIE",
                    "unece:cefactUNId": "UN01002696",
                    "unece:cefactBieDomainClass": "cefact:AgriculturalProcess_CropStage.Details",
                    "rdfs:comment": "The code specifying the type of agricultural process crop stage."
                },
                {
                    "@id": "cefact:SoilOccupation_CropResidue.Type.Code",
                    "@type": "unece:BasicBIE",
                    "unece:cefactUNId": "UN01002693",
                    "unece:cefactBieDomainClass": "cefact:SoilOccupation_CropResidue.Details",
                    "rdfs:comment": "The code specifying the type of soil occupation crop residue."
                },
                {
                    "@id": "cefact:Plot_SoilOccupation.Type.Code",
                    "@type": "unece:BasicBIE",
                    "unece:cefactUNId": "UN01002750",
                    "unece:cefactBieDomainClass": "cefact:Plot_SoilOccupation.Details",
                    "rdfs:comment": "The code specifying the type of plot soil occupation, such as main crop or catch crop."
                },
                {
                    "@id": "cefact:AgriculturalInput_Product.Type.Code",
                    "@type": "unece:BasicBIE",
                    "unece:cefactUNId": "UN01012377",
                    "unece:cefactBieDomainClass": "cefact:AgriculturalInput_Product.Details",
                    "rdfs:comment": "The code specifying the type of agricultural input product."
                },
                {
                    "@id": "cefact:AnimalHolding_Event.Type.Code",
                    "@type": "unece:BasicBIE",
                    "unece:TDED": "9171",
                    "unece:cefactUNId": "UN01011240",
                    "unece:cefactBieDomainClass": "cefact:AnimalHolding_Event.Details",
                    "rdfs:comment": "The code specifying the type of animal holding event."
                },
                {
                    "@id": "cefact:SPS_Package.Type.Code",
                    "@type": "unece:BasicBIE",
                    "unece:TDED": "7065",
                    "unece:cefactUNId": "UN03000106",
                    "unece:cefactBieDomainClass": "cefact:SPS_Package.Details",
                    "rdfs:comment": "The code specifying the type of SPS package."
                },
                {
                    "@id": "cefact:CropProduction_AgriculturalProcess.Type.Code",
                    "@type": "unece:BasicBIE",
                    "unece:cefactUNId": "UN01012409",
                    "unece:cefactBieDomainClass": "cefact:CropProduction_AgriculturalProcess.Details",
                    "rdfs:comment": "The code specifying the type of agricultural process for this crop production."
                },
                {
                    "@id": "cefact:AgronomicalObservation_Scope.Type.Code",
                    "@type": "unece:BasicBIE",
                    "unece:cefactUNId": "UN01009326",
                    "unece:cefactBieDomainClass": "cefact:AgronomicalObservation_Scope.Details",
                    "rdfs:comment": "The code specifying the type of this agronomical observation scope, such as leaves, whole plant, plant stem."
                },
                {
                    "@id": "cefact:AgriculturalInput_Material.Type.Code",
                    "@type": "unece:BasicBIE",
                    "unece:cefactUNId": "UN01012388",
                    "unece:cefactBieDomainClass": "cefact:AgriculturalInput_Material.Details",
                    "rdfs:comment": "A code specifying a type of agricultural input material."
                },
                {
                    "@id": "cefact:Specified_SoilSupplement.Type.Code",
                    "@type": "unece:BasicBIE",
                    "unece:cefactUNId": "UN01002719",
                    "unece:cefactBieDomainClass": "cefact:Specified_SoilSupplement.Details",
                    "rdfs:comment": "The code specifying the type of specified soil supplement."
                },
                {
                    "@id": "cefact:Agricultural_ProductionUnit.Type.Code",
                    "@type": "unece:BasicBIE",
                    "unece:cefactUNId": "UN01012246",
                    "unece:cefactBieDomainClass": "cefact:Agricultural_ProductionUnit.Details",
                    "rdfs:comment": "A code specifying a type of agricultural production unit."
                },
                {
                    "@id": "cefact:Agricultural_Characteristic.Type.Code",
                    "@type": "unece:BasicBIE",
                    "unece:cefactUNId": "UN01012361",
                    "unece:cefactBieDomainClass": "cefact:Agricultural_Characteristic.Details",
                    "rdfs:comment": "The code specifying the type of agricultural characteristic."
                },
                {
                    "@id": "cefact:Agricultural_CountrySub-Division.Type.Code",
                    "@type": "unece:BasicBIE",
                    "unece:cefactUNId": "UN01002778",
                    "unece:cefactBieDomainClass": "cefact:Agricultural_CountrySubDivision.Details",
                    "rdfs:comment": "The code specifying the type of agricultural country sub-division."
                },
                {
                    "@id": "cefact:Crop_SpeciesVariety.Type.Code",
                    "@type": "unece:BasicBIE",
                    "unece:cefactUNId": "UN01002775",
                    "unece:cefactBieDomainClass": "cefact:Crop_SpeciesVariety.Details",
                    "rdfs:comment": "The code specifying the type of crop species variety."
                },
                {
                    "@id": "cefact:Animal_Certificate.Type.Code",
                    "@type": "unece:BasicBIE",
                    "unece:cefactUNId": "UN01011239",
                    "unece:cefactBieDomainClass": "cefact:Animal_Certificate.Details",
                    "rdfs:comment": "The code specifying the type of animal certificate."
                },
                {
                    "@id": "cefact:Agricultural_Area.Type.Code",
                    "@type": "unece:BasicBIE",
                    "unece:cefactUNId": "UN01002672",
                    "unece:cefactBieDomainClass": "cefact:Agricultural_Area.Details",
                    "rdfs:comment": "The code specifying the type of agricultural area, such as crop surface area."
                },
                {
                    "@id": "cefact:Specified_CropProtectionTreatment.Type.Code",
                    "@type": "unece:BasicBIE",
                    "unece:cefactUNId": "UN01014287",
                    "unece:cefactBieDomainClass": "cefact:Specified_CropProtectionTreatment.Details",
                    "rdfs:comment": "The code specifying the type of crop protection treatment."
                },
                {
                    "@id": "cefact:AgriculturalProcess_TargetObject.Type.Code",
                    "@type": "unece:BasicBIE",
                    "unece:cefactUNId": "UN01002771",
                    "unece:cefactBieDomainClass": "cefact:AgriculturalProcess_TargetObject.Details",
                    "rdfs:comment": "The code specifying the type of agricultural process target object, such as pests, diseases or weeds."
                },
                {
                    "@id": "cefact:AgriculturalProcess_Condition.Type.Code",
                    "@type": "unece:BasicBIE",
                    "unece:cefactUNId": "UN01002682",
                    "unece:cefactBieDomainClass": "cefact:AgriculturalProcess_Condition.Details",
                    "rdfs:comment": "The code specifying the type of agricultural process condition, such as weather condition or soil condition."
                },
                {
                    "@id": "cefact:AgriculturalProcess_Reason.Type.Code",
                    "@type": "unece:BasicBIE",
                    "unece:cefactUNId": "UN01002742",
                    "unece:cefactBieDomainClass": "cefact:AgriculturalProcess_Reason.Details",
                    "rdfs:comment": "The code specifying the type of agricultural process reason."
                },
                {
                    "@id": "cefact:Agricultural_Produce.Type.Code",
                    "@type": "unece:BasicBIE",
                    "unece:cefactUNId": "UN01002700",
                    "unece:cefactBieDomainClass": "cefact:Agricultural_Produce.Details",
                    "rdfs:comment": "The code specifying the type of agricultural produce."
                },
                {
                    "@id": "cefact:Specified_AgriculturalDevice.Type.Code",
                    "@type": "unece:BasicBIE",
                    "unece:cefactUNId": "UN01002738",
                    "unece:cefactBieDomainClass": "cefact:Specified_AgriculturalDevice.Details",
                    "rdfs:comment": "The code specifying the type of this specified agricultural device."
                },
                {
                    "@id": "cefact:AgriculturalInput_Chemical.Type.Code",
                    "@type": "unece:BasicBIE",
                    "unece:cefactUNId": "UN01012405",
                    "unece:cefactBieDomainClass": "cefact:AgriculturalInput_Chemical.Details",
                    "rdfs:comment": "The code specifying the type of chemical for this agricultural input."
                }
            ]
        },
        {
            "@id": "agriculture:typeName",
            "@type": "rdf:Property",
            "schema:rangeIncludes": {
                "@id": "xsd:string"
            },
            "schema:domainIncludes": [
                {
                    "@id": "agriculture:Sample"
                },
                {
                    "@id": "agriculture:SampledObject"
                }
            ],
            "rdfs:comment": [
                "The name, expressed as text, for the type of this sampled agricultural object.",
                "The name, expressed as text, of this agricultural sample."
            ],
            "rdfs:label": "typeName",
            "unece:cefactElementMetadata": [
                {
                    "@id": "cefact:Agricultural_Sample.TypeName.Text",
                    "@type": "unece:BasicBIE",
                    "unece:cefactUNId": "UN01009594",
                    "unece:cefactBieDomainClass": "cefact:Agricultural_Sample.Details",
                    "rdfs:comment": "The name, expressed as text, of this agricultural sample."
                },
                {
                    "@id": "cefact:Agricultural_SampledObject.TypeName.Text",
                    "@type": "unece:BasicBIE",
                    "unece:cefactUNId": "UN01009614",
                    "unece:cefactBieDomainClass": "cefact:Agricultural_SampledObject.Details",
                    "rdfs:comment": "The name, expressed as text, for the type of this sampled agricultural object."
                }
            ]
        },
        {
            "@id": "agriculture:uOMLabelList",
            "@type": "rdf:Property",
            "schema:rangeIncludes": {
                "@id": "xsd:string"
            },
            "schema:domainIncludes": {
                "@id": "agriculture:DirectPositionList"
            },
            "rdfs:comment": "An ordered list of Unit Of Measure (UOM) labels, expressed as text, for this specified direct position list.",
            "rdfs:label": "uOMLabelList",
            "unece:cefactElementMetadata": [
                {
                    "@id": "cefact:Specified_DirectPositionList.UOM_LabelList.Text",
                    "@type": "unece:BasicBIE",
                    "unece:cefactUNId": "UN01012476",
                    "unece:cefactBieDomainClass": "cefact:Specified_DirectPositionList.Details",
                    "rdfs:comment": "An ordered list of Unit Of Measure (UOM) labels, expressed as text, for this specified direct position list."
                }
            ]
        },
        {
            "@id": "agriculture:uRICommunication",
            "@type": "rdf:Property",
            "schema:rangeIncludes": {
                "@id": "agriculture:Communication"
            },
            "schema:domainIncludes": {
                "@id": "agriculture:Party"
            },
            "rdfs:comment": "Uniform Resource Identifier (URI) communication information, such as a web or email address, specified for this party.",
            "rdfs:label": "uRICommunication",
            "unece:cefactElementMetadata": [
                {
                    "@id": "cefact:Specified_Party.URI.Specified_Communication",
                    "@type": "unece:AssociationBIE",
                    "unece:cefactUNId": "UN01012461",
                    "unece:cefactBieDomainClass": "cefact:Specified_Party.Details",
                    "rdfs:comment": "Uniform Resource Identifier (URI) communication information, such as a web or email address, specified for this party."
                }
            ]
        },
        {
            "@id": "agriculture:unifiedAppearanceApplicableClassification",
            "@type": "rdf:Property",
            "schema:rangeIncludes": {
                "@id": "agriculture:Classification"
            },
            "schema:domainIncludes": {
                "@id": "agriculture:Animal"
            },
            "rdfs:comment": "The unified appearance classification applicable to this livestock animal.",
            "rdfs:label": "unifiedAppearanceApplicableClassification",
            "unece:cefactElementMetadata": [
                {
                    "@id": "cefact:Livestock_Animal.UnifiedAppearance_Applicable.Specified_Classification",
                    "@type": "unece:AssociationBIE",
                    "unece:cefactUNId": "UN01007651",
                    "unece:cefactBieDomainClass": "cefact:Livestock_Animal.Details",
                    "rdfs:comment": "The unified appearance classification applicable to this livestock animal."
                }
            ]
        },
        {
            "@id": "agriculture:unifiedApplicableClassification",
            "@type": "rdf:Property",
            "schema:rangeIncludes": {
                "@id": "agriculture:Classification"
            },
            "schema:domainIncludes": {
                "@id": "agriculture:Event"
            },
            "rdfs:comment": "The unified classification applicable to this animal movement event.",
            "rdfs:label": "unifiedApplicableClassification",
            "unece:cefactElementMetadata": [
                {
                    "@id": "cefact:AnimalMovement_Event.Unified_Applicable.Specified_Classification",
                    "@type": "unece:AssociationBIE",
                    "unece:cefactUNId": "UN01007641",
                    "unece:cefactBieDomainClass": "cefact:AnimalMovement_Event.Details",
                    "rdfs:comment": "The unified classification applicable to this animal movement event."
                }
            ]
        },
        {
            "@id": "agriculture:unifiedColourApplicableClassification",
            "@type": "rdf:Property",
            "schema:rangeIncludes": {
                "@id": "agriculture:Classification"
            },
            "schema:domainIncludes": {
                "@id": "agriculture:Animal"
            },
            "rdfs:comment": "The unified colour or pattern classification applicable to this livestock animal.",
            "rdfs:label": "unifiedColourApplicableClassification",
            "unece:cefactElementMetadata": [
                {
                    "@id": "cefact:Livestock_Animal.UnifiedColour_Applicable.Specified_Classification",
                    "@type": "unece:AssociationBIE",
                    "unece:cefactUNId": "UN01007653",
                    "unece:cefactBieDomainClass": "cefact:Livestock_Animal.Details",
                    "rdfs:comment": "The unified colour or pattern classification applicable to this livestock animal."
                }
            ]
        },
        {
            "@id": "agriculture:unitQuantity",
            "@type": "rdf:Property",
            "schema:rangeIncludes": {
                "@id": "xsd:decimal"
            },
            "schema:domainIncludes": {
                "@id": "agriculture:Batch"
            },
            "rdfs:comment": [
                "The number of units, expressed as a quantity, for this animal batch.",
                "The number of units, expressed as a quantity, for this crop produce batch.",
                "The number of units, expressed as a quantity, for this product batch."
            ],
            "rdfs:label": "unitQuantity",
            "unece:cefactElementMetadata": [
                {
                    "@id": "cefact:CropProduce_Batch.Unit.Quantity",
                    "@type": "unece:BasicBIE",
                    "unece:cefactUNId": "UN01012338",
                    "unece:cefactBieDomainClass": "cefact:CropProduce_Batch.Details",
                    "rdfs:comment": "The number of units, expressed as a quantity, for this crop produce batch."
                },
                {
                    "@id": "cefact:Product_Batch.Unit.Quantity",
                    "@type": "unece:BasicBIE",
                    "unece:cefactUNId": "UN01012353",
                    "unece:cefactBieDomainClass": "cefact:Product_Batch.Details",
                    "rdfs:comment": "The number of units, expressed as a quantity, for this product batch."
                },
                {
                    "@id": "cefact:Animal_Batch.Unit.Quantity",
                    "@type": "unece:BasicBIE",
                    "unece:cefactUNId": "UN01011253",
                    "unece:cefactBieDomainClass": "cefact:Animal_Batch.Details",
                    "rdfs:comment": "The number of units, expressed as a quantity, for this animal batch."
                }
            ]
        },
        {
            "@id": "agriculture:unloadingBaseportLocation",
            "@type": "rdf:Property",
            "schema:rangeIncludes": {
                "@id": "agriculture:Location"
            },
            "schema:domainIncludes": {
                "@id": "agriculture:Consignment"
            },
            "rdfs:comment": "The baseport location at which this SPS consignment is to be unloaded from a means of transport according to the transport contract.",
            "rdfs:label": "unloadingBaseportLocation",
            "unece:cefactElementMetadata": [
                {
                    "@id": "cefact:SPS_Consignment.UnloadingBaseport.SPS_Location",
                    "@type": "unece:AssociationBIE",
                    "unece:cefactUNId": "UN03000068",
                    "unece:cefactBieDomainClass": "cefact:SPS_Consignment.Details",
                    "rdfs:comment": "The baseport location at which this SPS consignment is to be unloaded from a means of transport according to the transport contract."
                }
            ]
        },
        {
            "@id": "agriculture:use",
            "@type": "rdf:Property",
            "schema:rangeIncludes": {
                "@id": "xsd:string"
            },
            "schema:domainIncludes": {
                "@id": "agriculture:Product"
            },
            "rdfs:comment": "The use, expressed as text, for this agricultural input product.",
            "rdfs:label": "use",
            "unece:cefactElementMetadata": [
                {
                    "@id": "cefact:AgriculturalInput_Product.Use.Text",
                    "@type": "unece:BasicBIE",
                    "unece:cefactUNId": "UN01012378",
                    "unece:cefactBieDomainClass": "cefact:AgriculturalInput_Product.Details",
                    "rdfs:comment": "The use, expressed as text, for this agricultural input product."
                }
            ]
        },
        {
            "@id": "agriculture:useCode",
            "@type": "rdf:Property",
            "schema:rangeIncludes": {
                "@id": "xsd:token"
            },
            "schema:domainIncludes": {
                "@id": "agriculture:Produce"
            },
            "rdfs:comment": "The code specifying the use for this agricultural produce, such as for human consumption.",
            "rdfs:label": "useCode",
            "unece:cefactElementMetadata": [
                {
                    "@id": "cefact:Agricultural_Produce.Use.Code",
                    "@type": "unece:BasicBIE",
                    "unece:cefactUNId": "UN01002704",
                    "unece:cefactBieDomainClass": "cefact:Agricultural_Produce.Details",
                    "rdfs:comment": "The code specifying the use for this agricultural produce, such as for human consumption."
                }
            ]
        },
        {
            "@id": "agriculture:usedAgriculturalDevice",
            "@type": "rdf:Property",
            "schema:rangeIncludes": {
                "@id": "agriculture:AgriculturalDevice"
            },
            "schema:domainIncludes": {
                "@id": "agriculture:AgriculturalProcess"
            },
            "rdfs:comment": [
                "A specified agricultural device used in this plot agricultural process.",
                "An agricultural device used for the crop production agricultural process."
            ],
            "rdfs:label": "usedAgriculturalDevice",
            "unece:cefactElementMetadata": [
                {
                    "@id": "cefact:CropProduction_AgriculturalProcess.Used.Specified_AgriculturalDevice",
                    "@type": "unece:AssociationBIE",
                    "unece:cefactUNId": "UN01012418",
                    "unece:cefactBieDomainClass": "cefact:CropProduction_AgriculturalProcess.Details",
                    "rdfs:comment": "An agricultural device used for the crop production agricultural process."
                },
                {
                    "@id": "cefact:Plot_AgriculturalProcess.Used.Specified_AgriculturalDevice",
                    "@type": "unece:AssociationBIE",
                    "unece:cefactUNId": "UN01002792",
                    "unece:cefactBieDomainClass": "cefact:Plot_AgriculturalProcess.Details",
                    "rdfs:comment": "A specified agricultural device used in this plot agricultural process."
                }
            ]
        },
        {
            "@id": "agriculture:usedArea",
            "@type": "rdf:Property",
            "schema:rangeIncludes": {
                "@id": "agriculture:Area"
            },
            "schema:domainIncludes": [
                {
                    "@id": "agriculture:CropProductionCycle"
                },
                {
                    "@id": "agriculture:SoilOccupation"
                }
            ],
            "rdfs:comment": [
                "An agricultural area used for this agricultural crop production cycle.",
                "An agricultural area used for this plot soil occupation."
            ],
            "rdfs:label": "usedArea",
            "unece:cefactElementMetadata": [
                {
                    "@id": "cefact:Agricultural_CropProductionCycle.Used.Agricultural_Area",
                    "@type": "unece:AssociationBIE",
                    "unece:cefactUNId": "UN01002769",
                    "unece:cefactBieDomainClass": "cefact:Agricultural_CropProductionCycle.Details",
                    "rdfs:comment": "An agricultural area used for this agricultural crop production cycle."
                },
                {
                    "@id": "cefact:Plot_SoilOccupation.Used.Agricultural_Area",
                    "@type": "unece:AssociationBIE",
                    "unece:cefactUNId": "UN01002759",
                    "unece:cefactBieDomainClass": "cefact:Plot_SoilOccupation.Details",
                    "rdfs:comment": "An agricultural area used for this plot soil occupation."
                }
            ]
        },
        {
            "@id": "agriculture:usedCropInput",
            "@type": "rdf:Property",
            "schema:rangeIncludes": {
                "@id": "agriculture:CropInput"
            },
            "schema:domainIncludes": {
                "@id": "agriculture:AgriculturalProcess"
            },
            "rdfs:comment": "An agricultural process crop input used in this plot agricultural process.",
            "rdfs:label": "usedCropInput",
            "unece:cefactElementMetadata": [
                {
                    "@id": "cefact:Plot_AgriculturalProcess.Used.AgriculturalProcess_CropInput",
                    "@type": "unece:AssociationBIE",
                    "unece:cefactUNId": "UN01002794",
                    "unece:cefactBieDomainClass": "cefact:Plot_AgriculturalProcess.Details",
                    "rdfs:comment": "An agricultural process crop input used in this plot agricultural process."
                }
            ]
        },
        {
            "@id": "agriculture:usedMaterial",
            "@type": "rdf:Property",
            "schema:rangeIncludes": {
                "@id": "agriculture:Material"
            },
            "schema:domainIncludes": {
                "@id": "agriculture:CropProtectionTreatment"
            },
            "rdfs:comment": "Material used for this specified crop protection treatment.",
            "rdfs:label": "usedMaterial",
            "unece:cefactElementMetadata": [
                {
                    "@id": "cefact:Specified_CropProtectionTreatment.Used.Specified_Material",
                    "@type": "unece:AssociationBIE",
                    "unece:cefactUNId": "UN01014289",
                    "unece:cefactBieDomainClass": "cefact:Specified_CropProtectionTreatment.Details",
                    "rdfs:comment": "Material used for this specified crop protection treatment."
                }
            ]
        },
        {
            "@id": "agriculture:usedProcess",
            "@type": "rdf:Property",
            "schema:rangeIncludes": {
                "@id": "agriculture:Process"
            },
            "schema:domainIncludes": {
                "@id": "agriculture:TargetObject"
            },
            "rdfs:comment": "The observation process used in relation to this agronomical observation target object.",
            "rdfs:label": "usedProcess",
            "unece:cefactElementMetadata": [
                {
                    "@id": "cefact:AgronomicalObservation_TargetObject.Used.Observation_Process",
                    "@type": "unece:AssociationBIE",
                    "unece:cefactUNId": "UN01009324",
                    "unece:cefactBieDomainClass": "cefact:AgronomicalObservation_TargetObject.Details",
                    "rdfs:comment": "The observation process used in relation to this agronomical observation target object."
                }
            ]
        },
        {
            "@id": "agriculture:usedSoftware",
            "@type": "rdf:Property",
            "schema:rangeIncludes": {
                "@id": "agriculture:Software"
            },
            "schema:domainIncludes": {
                "@id": "agriculture:Party"
            },
            "rdfs:comment": "The production software used by this agronomical observation party.",
            "rdfs:label": "usedSoftware",
            "unece:cefactElementMetadata": [
                {
                    "@id": "cefact:AgronomicalObservation_Party.Used.Production_Software",
                    "@type": "unece:AssociationBIE",
                    "unece:cefactUNId": "UN01009307",
                    "unece:cefactBieDomainClass": "cefact:AgronomicalObservation_Party.Details",
                    "rdfs:comment": "The production software used by this agronomical observation party."
                }
            ]
        },
        {
            "@id": "agriculture:usedTransportMeans",
            "@type": "rdf:Property",
            "schema:rangeIncludes": {
                "@id": "agriculture:TransportMeans"
            },
            "schema:domainIncludes": [
                {
                    "@id": "agriculture:SampledObject"
                },
                {
                    "@id": "agriculture:TransportMovement"
                }
            ],
            "rdfs:comment": [
                "A referenced means of transport used for this agricultural sampled object.",
                "The means of transport used for this SPS transport movement."
            ],
            "rdfs:label": "usedTransportMeans",
            "unece:cefactElementMetadata": [
                {
                    "@id": "cefact:SPS_TransportMovement.Used.SPS_TransportMeans",
                    "@type": "unece:AssociationBIE",
                    "unece:cefactUNId": "UN03000175",
                    "unece:cefactBieDomainClass": "cefact:SPS_TransportMovement.Details",
                    "rdfs:comment": "The means of transport used for this SPS transport movement."
                },
                {
                    "@id": "cefact:Agricultural_SampledObject.Used.Referenced_TransportMeans",
                    "@type": "unece:AssociationBIE",
                    "unece:cefactUNId": "UN01012466",
                    "unece:cefactBieDomainClass": "cefact:Agricultural_SampledObject.Details",
                    "rdfs:comment": "A referenced means of transport used for this agricultural sampled object."
                }
            ]
        },
        {
            "@id": "agriculture:utilizedTransportEquipment",
            "@type": "rdf:Property",
            "schema:rangeIncludes": {
                "@id": "agriculture:TransportEquipment"
            },
            "schema:domainIncludes": {
                "@id": "agriculture:Consignment"
            },
            "rdfs:comment": "Transport equipment utilized for this SPS consignment.",
            "rdfs:label": "utilizedTransportEquipment",
            "unece:cefactElementMetadata": [
                {
                    "@id": "cefact:SPS_Consignment.Utilized.SPS_TransportEquipment",
                    "@type": "unece:AssociationBIE",
                    "unece:cefactUNId": "UN03000075",
                    "unece:cefactBieDomainClass": "cefact:SPS_Consignment.Details",
                    "rdfs:comment": "Transport equipment utilized for this SPS consignment."
                }
            ]
        },
        {
            "@id": "agriculture:value",
            "@type": "rdf:Property",
            "schema:rangeIncludes": {
                "@id": "xsd:string"
            },
            "schema:domainIncludes": {
                "@id": "agriculture:Characteristic"
            },
            "rdfs:comment": "The value, expressed as text, for this agricultural characteristic.",
            "rdfs:label": "value",
            "unece:cefactElementMetadata": [
                {
                    "@id": "cefact:Agricultural_Characteristic.Value.Text",
                    "@type": "unece:BasicBIE",
                    "unece:TDED": "7110",
                    "unece:cefactUNId": "UN01012364",
                    "unece:cefactBieDomainClass": "cefact:Agricultural_Characteristic.Details",
                    "rdfs:comment": "The value, expressed as text, for this agricultural characteristic."
                }
            ]
        },
        {
            "@id": "agriculture:valueAmount",
            "@type": "rdf:Property",
            "schema:rangeIncludes": {
                "@id": "xsd:decimal"
            },
            "schema:domainIncludes": {
                "@id": "agriculture:Characteristic"
            },
            "rdfs:comment": "The value, expressed as an amount, for this agricultural characteristic.",
            "rdfs:label": "valueAmount",
            "unece:cefactElementMetadata": [
                {
                    "@id": "cefact:Agricultural_Characteristic.Value.Amount",
                    "@type": "unece:BasicBIE",
                    "unece:cefactUNId": "UN01013711",
                    "unece:cefactBieDomainClass": "cefact:Agricultural_Characteristic.Details",
                    "rdfs:comment": "The value, expressed as an amount, for this agricultural characteristic."
                }
            ]
        },
        {
            "@id": "agriculture:valueDateTime",
            "@type": "rdf:Property",
            "schema:rangeIncludes": {
                "@id": "xsd:dateTime"
            },
            "schema:domainIncludes": {
                "@id": "agriculture:Characteristic"
            },
            "rdfs:comment": "The value, expressed as a date, time, date time, or other date time value, of this agricultural characteristic.",
            "rdfs:label": "valueDateTime",
            "unece:cefactElementMetadata": [
                {
                    "@id": "cefact:Agricultural_Characteristic.Value.DateTime",
                    "@type": "unece:BasicBIE",
                    "unece:cefactUNId": "UN01012366",
                    "unece:cefactBieDomainClass": "cefact:Agricultural_Characteristic.Details",
                    "rdfs:comment": "The value, expressed as a date, time, date time, or other date time value, of this agricultural characteristic."
                }
            ]
        },
        {
            "@id": "agriculture:valueIndicator",
            "@type": "rdf:Property",
            "schema:rangeIncludes": {
                "@id": "xsd:boolean"
            },
            "schema:domainIncludes": {
                "@id": "agriculture:Characteristic"
            },
            "rdfs:comment": "The value, expressed as an indicator, for this agricultural characteristic.",
            "rdfs:label": "valueIndicator",
            "unece:cefactElementMetadata": [
                {
                    "@id": "cefact:Agricultural_Characteristic.Value.Indicator",
                    "@type": "unece:BasicBIE",
                    "unece:cefactUNId": "UN01012367",
                    "unece:cefactBieDomainClass": "cefact:Agricultural_Characteristic.Details",
                    "rdfs:comment": "The value, expressed as an indicator, for this agricultural characteristic."
                }
            ]
        },
        {
            "@id": "agriculture:valueMeasure",
            "@type": "rdf:Property",
            "schema:rangeIncludes": {
                "@id": "xsd:decimal"
            },
            "schema:domainIncludes": [
                {
                    "@id": "agriculture:Characteristic"
                },
                {
                    "@id": "agriculture:Condition"
                },
                {
                    "@id": "agriculture:Temperature"
                }
            ],
            "rdfs:comment": [
                "The measure of a value for this SPS process characteristic.",
                "The measure of a value for this agricultural characteristic.",
                "The measure of a value for this agricultural process condition.",
                "The measure of the value of this SPS temperature, such as a temperature value of ten degrees Celsius."
            ],
            "rdfs:label": "valueMeasure",
            "unece:cefactElementMetadata": [
                {
                    "@id": "cefact:Agricultural_Characteristic.Value.Measure",
                    "@type": "unece:BasicBIE",
                    "unece:cefactUNId": "UN01012363",
                    "unece:cefactBieDomainClass": "cefact:Agricultural_Characteristic.Details",
                    "rdfs:comment": "The measure of a value for this agricultural characteristic."
                },
                {
                    "@id": "cefact:AgriculturalProcess_Condition.Value.Measure",
                    "@type": "unece:BasicBIE",
                    "unece:cefactUNId": "UN01002684",
                    "unece:cefactBieDomainClass": "cefact:AgriculturalProcess_Condition.Details",
                    "rdfs:comment": "The measure of a value for this agricultural process condition."
                },
                {
                    "@id": "cefact:SPSProcess_Characteristic.Value.Measure",
                    "@type": "unece:BasicBIE",
                    "unece:TDED": "6314",
                    "unece:cefactUNId": "UN03000180",
                    "unece:cefactBieDomainClass": "cefact:SPSProcess_Characteristic.Details",
                    "rdfs:comment": "The measure of a value for this SPS process characteristic."
                },
                {
                    "@id": "cefact:SPS_Temperature.Value.Measure",
                    "@type": "unece:BasicBIE",
                    "unece:TDED": "6246",
                    "unece:cefactUNId": "UN03000142",
                    "unece:cefactBieDomainClass": "cefact:SPS_Temperature.Details",
                    "rdfs:comment": "The measure of the value of this SPS temperature, such as a temperature value of ten degrees Celsius."
                }
            ]
        },
        {
            "@id": "agriculture:valueMethod",
            "@type": "rdf:Property",
            "schema:rangeIncludes": {
                "@id": "agriculture:Method"
            },
            "schema:domainIncludes": {
                "@id": "agriculture:Characteristic"
            },
            "rdfs:comment": "A method specified for the value of this agricultural characteristic.",
            "rdfs:label": "valueMethod",
            "unece:cefactElementMetadata": [
                {
                    "@id": "cefact:Agricultural_Characteristic.Value.Specified_Method",
                    "@type": "unece:AssociationBIE",
                    "unece:cefactUNId": "UN01013712",
                    "unece:cefactBieDomainClass": "cefact:Agricultural_Characteristic.Details",
                    "rdfs:comment": "A method specified for the value of this agricultural characteristic."
                }
            ]
        },
        {
            "@id": "agriculture:valueNumeric",
            "@type": "rdf:Property",
            "schema:rangeIncludes": {
                "@id": "xsd:decimal"
            },
            "schema:domainIncludes": {
                "@id": "agriculture:Characteristic"
            },
            "rdfs:comment": "The value, expressed as a number, for this agricultural characteristic.",
            "rdfs:label": "valueNumeric",
            "unece:cefactElementMetadata": [
                {
                    "@id": "cefact:Agricultural_Characteristic.Value.Numeric",
                    "@type": "unece:BasicBIE",
                    "unece:cefactUNId": "UN01013710",
                    "unece:cefactBieDomainClass": "cefact:Agricultural_Characteristic.Details",
                    "rdfs:comment": "The value, expressed as a number, for this agricultural characteristic."
                }
            ]
        },
        {
            "@id": "agriculture:valueParameter",
            "@type": "rdf:Property",
            "schema:rangeIncludes": {
                "@id": "agriculture:Parameter"
            },
            "schema:domainIncludes": {
                "@id": "agriculture:Characteristic"
            },
            "rdfs:comment": "A parameter specified for the value of this agricultural characteristic.",
            "rdfs:label": "valueParameter",
            "unece:cefactElementMetadata": [
                {
                    "@id": "cefact:Agricultural_Characteristic.Value.Specified_Parameter",
                    "@type": "unece:AssociationBIE",
                    "unece:cefactUNId": "UN01013713",
                    "unece:cefactBieDomainClass": "cefact:Agricultural_Characteristic.Details",
                    "rdfs:comment": "A parameter specified for the value of this agricultural characteristic."
                }
            ]
        },
        {
            "@id": "agriculture:valueRange",
            "@type": "rdf:Property",
            "schema:rangeIncludes": {
                "@id": "agriculture:Range"
            },
            "schema:domainIncludes": {
                "@id": "agriculture:Characteristic"
            },
            "rdfs:comment": "A range specified for the value of this agricultural characteristic.",
            "rdfs:label": "valueRange",
            "unece:cefactElementMetadata": [
                {
                    "@id": "cefact:Agricultural_Characteristic.Value.Specified_Range",
                    "@type": "unece:AssociationBIE",
                    "unece:cefactUNId": "UN01013714",
                    "unece:cefactBieDomainClass": "cefact:Agricultural_Characteristic.Details",
                    "rdfs:comment": "A range specified for the value of this agricultural characteristic."
                }
            ]
        },
        {
            "@id": "agriculture:valueTolerance",
            "@type": "rdf:Property",
            "schema:rangeIncludes": {
                "@id": "agriculture:Tolerance"
            },
            "schema:domainIncludes": {
                "@id": "agriculture:Characteristic"
            },
            "rdfs:comment": "A tolerance specified for the value of this agricultural characteristic.",
            "rdfs:label": "valueTolerance",
            "unece:cefactElementMetadata": [
                {
                    "@id": "cefact:Agricultural_Characteristic.Value.Specified_Tolerance",
                    "@type": "unece:AssociationBIE",
                    "unece:cefactUNId": "UN01013715",
                    "unece:cefactBieDomainClass": "cefact:Agricultural_Characteristic.Details",
                    "rdfs:comment": "A tolerance specified for the value of this agricultural characteristic."
                }
            ]
        },
        {
            "@id": "agriculture:versionId",
            "@type": "rdf:Property",
            "schema:rangeIncludes": {
                "@id": "xsd:token"
            },
            "schema:domainIncludes": [
                {
                    "@id": "agriculture:Document"
                },
                {
                    "@id": "agriculture:Identity"
                }
            ],
            "rdfs:comment": [
                "The identifier for the version of this animal passport document.",
                "The identifier of the version of this animal identity."
            ],
            "rdfs:label": "versionId",
            "unece:cefactElementMetadata": [
                {
                    "@id": "cefact:Animal_Identity.Version.Identifier",
                    "@type": "unece:BasicBIE",
                    "unece:cefactUNId": "UN01007628",
                    "unece:cefactBieDomainClass": "cefact:Animal_Identity.Details",
                    "rdfs:comment": "The identifier of the version of this animal identity."
                },
                {
                    "@id": "cefact:AnimalPassport_Document.Version_Identification.Identifier",
                    "@type": "unece:BasicBIE",
                    "unece:TDED": "1004",
                    "unece:cefactUNId": "UN01007673",
                    "unece:cefactBieDomainClass": "cefact:AnimalPassport_Document.Details",
                    "rdfs:comment": "The identifier for the version of this animal passport document."
                }
            ]
        },
        {
            "@id": "agriculture:volumeMeasure",
            "@type": "rdf:Property",
            "schema:rangeIncludes": {
                "@id": "xsd:decimal"
            },
            "schema:domainIncludes": [
                {
                    "@id": "agriculture:CropInput"
                },
                {
                    "@id": "agriculture:Material"
                }
            ],
            "rdfs:comment": [
                "The measure of the volume of this agricultural input material.",
                "The measure of the volume of this agricultural process crop input."
            ],
            "rdfs:label": "volumeMeasure",
            "unece:cefactElementMetadata": [
                {
                    "@id": "cefact:AgriculturalProcess_CropInput.Volume.Measure",
                    "@type": "unece:BasicBIE",
                    "unece:cefactUNId": "UN01002729",
                    "unece:cefactBieDomainClass": "cefact:AgriculturalProcess_CropInput.Details",
                    "rdfs:comment": "The measure of the volume of this agricultural process crop input."
                },
                {
                    "@id": "cefact:AgriculturalInput_Material.Volume.Measure",
                    "@type": "unece:BasicBIE",
                    "unece:cefactUNId": "UN01012392",
                    "unece:cefactBieDomainClass": "cefact:AgriculturalInput_Material.Details",
                    "rdfs:comment": "The measure of the volume of this agricultural input material."
                }
            ]
        },
        {
            "@id": "agriculture:volumeRatioMeasure",
            "@type": "rdf:Property",
            "schema:rangeIncludes": {
                "@id": "xsd:decimal"
            },
            "schema:domainIncludes": {
                "@id": "agriculture:Material"
            },
            "rdfs:comment": "The volume measure of this agricultural input material expressed as a ratio to another volume, such as the total volume.",
            "rdfs:label": "volumeRatioMeasure",
            "unece:cefactElementMetadata": [
                {
                    "@id": "cefact:AgriculturalInput_Material.VolumeRatio.Measure",
                    "@type": "unece:BasicBIE",
                    "unece:cefactUNId": "UN01012393",
                    "unece:cefactBieDomainClass": "cefact:AgriculturalInput_Material.Details",
                    "rdfs:comment": "The volume measure of this agricultural input material expressed as a ratio to another volume, such as the total volume."
                }
            ]
        },
        {
            "@id": "agriculture:weightMeasure",
            "@type": "rdf:Property",
            "schema:rangeIncludes": {
                "@id": "xsd:decimal"
            },
            "schema:domainIncludes": [
                {
                    "@id": "agriculture:Batch"
                },
                {
                    "@id": "agriculture:Chemical"
                },
                {
                    "@id": "agriculture:CropInput"
                },
                {
                    "@id": "agriculture:CropResidue"
                },
                {
                    "@id": "agriculture:Produce"
                },
                {
                    "@id": "agriculture:SoilSupplement"
                }
            ],
            "rdfs:comment": [
                "The measure of the weight (mass) of this agricultural process crop input.",
                "The measure of the weight (mass) of this agricultural produce.",
                "The measure of the weight (mass) of this crop input batch.",
                "The measure of the weight (mass) of this soil occupation crop residue.",
                "The measure of the weight (mass) of this specified soil supplement.",
                "The weight, expressed as a measure, for this agricultural input chemical.",
                "The weight, expressed as a measure, for this animal batch.",
                "The weight, expressed as a measure, for this product batch."
            ],
            "rdfs:label": "weightMeasure",
            "unece:cefactElementMetadata": [
                {
                    "@id": "cefact:Agricultural_Produce.Weight.Measure",
                    "@type": "unece:BasicBIE",
                    "unece:cefactUNId": "UN01002703",
                    "unece:cefactBieDomainClass": "cefact:Agricultural_Produce.Details",
                    "rdfs:comment": "The measure of the weight (mass) of this agricultural produce."
                },
                {
                    "@id": "cefact:Product_Batch.Weight.Measure",
                    "@type": "unece:BasicBIE",
                    "unece:cefactUNId": "UN01012352",
                    "unece:cefactBieDomainClass": "cefact:Product_Batch.Details",
                    "rdfs:comment": "The weight, expressed as a measure, for this product batch."
                },
                {
                    "@id": "cefact:Specified_SoilSupplement.Weight.Measure",
                    "@type": "unece:BasicBIE",
                    "unece:cefactUNId": "UN01002721",
                    "unece:cefactBieDomainClass": "cefact:Specified_SoilSupplement.Details",
                    "rdfs:comment": "The measure of the weight (mass) of this specified soil supplement."
                },
                {
                    "@id": "cefact:AgriculturalProcess_CropInput.Weight.Measure",
                    "@type": "unece:BasicBIE",
                    "unece:cefactUNId": "UN01002728",
                    "unece:cefactBieDomainClass": "cefact:AgriculturalProcess_CropInput.Details",
                    "rdfs:comment": "The measure of the weight (mass) of this agricultural process crop input."
                },
                {
                    "@id": "cefact:Animal_Batch.Weight.Measure",
                    "@type": "unece:BasicBIE",
                    "unece:cefactUNId": "UN01011254",
                    "unece:cefactBieDomainClass": "cefact:Animal_Batch.Details",
                    "rdfs:comment": "The weight, expressed as a measure, for this animal batch."
                },
                {
                    "@id": "cefact:AgriculturalInput_Chemical.Weight.Measure",
                    "@type": "unece:BasicBIE",
                    "unece:cefactUNId": "UN01012404",
                    "unece:cefactBieDomainClass": "cefact:AgriculturalInput_Chemical.Details",
                    "rdfs:comment": "The weight, expressed as a measure, for this agricultural input chemical."
                },
                {
                    "@id": "cefact:CropInput_Batch.Weight.Measure",
                    "@type": "unece:BasicBIE",
                    "unece:cefactUNId": "UN01002711",
                    "unece:cefactBieDomainClass": "cefact:CropInput_Batch.Details",
                    "rdfs:comment": "The measure of the weight (mass) of this crop input batch."
                },
                {
                    "@id": "cefact:SoilOccupation_CropResidue.Weight.Measure",
                    "@type": "unece:BasicBIE",
                    "unece:cefactUNId": "UN01002694",
                    "unece:cefactBieDomainClass": "cefact:SoilOccupation_CropResidue.Details",
                    "rdfs:comment": "The measure of the weight (mass) of this soil occupation crop residue."
                }
            ]
        }
    ]
}